<?xml version="1.0" encoding="UTF-8"?>
<!DOCTYPE rdf:RDF [
	<!ENTITY cmns-adr "https://www.omg.org/spec/Commons/Addresses/">
	<!ENTITY cmns-av "https://www.omg.org/spec/Commons/AnnotationVocabulary/">
	<!ENTITY cmns-cds "https://www.omg.org/spec/Commons/CodesAndCodeSets/">
	<!ENTITY cmns-cls "https://www.omg.org/spec/Commons/Classifiers/">
	<!ENTITY cmns-col "https://www.omg.org/spec/Commons/Collections/">
	<!ENTITY cmns-cxtdsg "https://www.omg.org/spec/Commons/ContextualDesignators/">
	<!ENTITY cmns-cxtid "https://www.omg.org/spec/Commons/ContextualIdentifiers/">
	<!ENTITY cmns-doc "https://www.omg.org/spec/Commons/Documents/">
	<!ENTITY cmns-dsg "https://www.omg.org/spec/Commons/Designators/">
	<!ENTITY cmns-id "https://www.omg.org/spec/Commons/Identifiers/">
	<!ENTITY cmns-loc "https://www.omg.org/spec/Commons/Locations/">
	<!ENTITY cmns-qtu "https://www.omg.org/spec/Commons/QuantitiesAndUnits/">
	<!ENTITY cmns-txt "https://www.omg.org/spec/Commons/TextDatatype/">
	<!ENTITY dct "http://purl.org/dc/terms/">
	<!ENTITY owl "http://www.w3.org/2002/07/owl#">
	<!ENTITY rdf "http://www.w3.org/1999/02/22-rdf-syntax-ns#">
	<!ENTITY rdfs "http://www.w3.org/2000/01/rdf-schema#">
	<!ENTITY skos "http://www.w3.org/2004/02/skos/core#">
	<!ENTITY xsd "http://www.w3.org/2001/XMLSchema#">
]>
<rdf:RDF xml:base="https://www.omg.org/spec/Commons/Addresses/"
	xmlns:cmns-adr="https://www.omg.org/spec/Commons/Addresses/"
	xmlns:cmns-av="https://www.omg.org/spec/Commons/AnnotationVocabulary/"
	xmlns:cmns-cds="https://www.omg.org/spec/Commons/CodesAndCodeSets/"
	xmlns:cmns-cls="https://www.omg.org/spec/Commons/Classifiers/"
	xmlns:cmns-col="https://www.omg.org/spec/Commons/Collections/"
	xmlns:cmns-cxtdsg="https://www.omg.org/spec/Commons/ContextualDesignators/"
	xmlns:cmns-cxtid="https://www.omg.org/spec/Commons/ContextualIdentifiers/"
	xmlns:cmns-doc="https://www.omg.org/spec/Commons/Documents/"
	xmlns:cmns-dsg="https://www.omg.org/spec/Commons/Designators/"
	xmlns:cmns-id="https://www.omg.org/spec/Commons/Identifiers/"
	xmlns:cmns-loc="https://www.omg.org/spec/Commons/Locations/"
	xmlns:cmns-qtu="https://www.omg.org/spec/Commons/QuantitiesAndUnits/"
	xmlns:cmns-txt="https://www.omg.org/spec/Commons/TextDatatype/"
	xmlns:dct="http://purl.org/dc/terms/"
	xmlns:owl="http://www.w3.org/2002/07/owl#"
	xmlns:rdf="http://www.w3.org/1999/02/22-rdf-syntax-ns#"
	xmlns:rdfs="http://www.w3.org/2000/01/rdf-schema#"
	xmlns:skos="http://www.w3.org/2004/02/skos/core#"
	xmlns:xsd="http://www.w3.org/2001/XMLSchema#">
	
	<owl:Ontology rdf:about="https://www.omg.org/spec/Commons/Addresses/">
		<rdfs:label>Addresses Ontology</rdfs:label>
		<dct:abstract>This ontology provides high level definitions for addresses and address components including elements that are common to addressing standards. It was derived from a combination of the ISO 19160 Addressing International Standard (ISO 19160-1:2015, ISO 19160-2:2023, ISO 19160-3:2020 and ISO 19160-4:2023) and the United States Postal Service (USPS) Publication 28, which is used by many of the international shipping services.</dct:abstract>
		<dct:license>Copyright (c) 2013-2025 EDM Council, Inc.
Copyright (c) 2013-2025 Object Management Group, Inc.

Permission is hereby granted, free of charge, to any person obtaining a copy of this software and associated documentation files (the &apos;Software&apos;), to deal in the Software without restriction, including without limitation the rights to use, copy, modify, merge, publish, distribute, sublicense, and/or sell copies of the Software, and to permit persons to whom the Software is furnished to do so, subject to the following conditions:

The above copyright notice and this permission notice shall be included in all copies or substantial portions of the Software.

THE SOFTWARE IS PROVIDED &apos;AS IS&apos;, WITHOUT WARRANTY OF ANY KIND, EXPRESS OR IMPLIED, INCLUDING BUT NOT LIMITED TO THE WARRANTIES OF MERCHANTABILITY, FITNESS FOR A PARTICULAR PURPOSE AND NONINFRINGEMENT. IN NO EVENT SHALL THE AUTHORS OR COPYRIGHT HOLDERS BE LIABLE FOR ANY CLAIM, DAMAGES OR OTHER LIABILITY, WHETHER IN AN ACTION OF CONTRACT, TORT OR OTHERWISE, ARISING FROM, OUT OF OR IN CONNECTION WITH THE SOFTWARE OR THE USE OR OTHER DEALINGS IN THE SOFTWARE.
		
See https://opensource.org/licenses/MIT.</dct:license>
		<owl:imports rdf:resource="https://www.omg.org/spec/Commons/AnnotationVocabulary/"/>
		<owl:imports rdf:resource="https://www.omg.org/spec/Commons/Classifiers/"/>
		<owl:imports rdf:resource="https://www.omg.org/spec/Commons/CodesAndCodeSets/"/>
		<owl:imports rdf:resource="https://www.omg.org/spec/Commons/Collections/"/>
		<owl:imports rdf:resource="https://www.omg.org/spec/Commons/ContextualDesignators/"/>
		<owl:imports rdf:resource="https://www.omg.org/spec/Commons/ContextualIdentifiers/"/>
		<owl:imports rdf:resource="https://www.omg.org/spec/Commons/Designators/"/>
		<owl:imports rdf:resource="https://www.omg.org/spec/Commons/Documents/"/>
		<owl:imports rdf:resource="https://www.omg.org/spec/Commons/Identifiers/"/>
		<owl:imports rdf:resource="https://www.omg.org/spec/Commons/Locations/"/>
		<owl:imports rdf:resource="https://www.omg.org/spec/Commons/QuantitiesAndUnits/"/>
		<owl:imports rdf:resource="https://www.omg.org/spec/Commons/TextDatatype/"/>
		<owl:versionIRI rdf:resource="https://www.omg.org/spec/Commons/20250201/Addresses/"/>
		<skos:scopeNote>This ontology was originally designed for use in the Financial Industry Business Ontology (FIBO) for representing addresses for people and organizations. It has been extended to reflect some of the recent revisions to the high-level elements of the conceptual model specified in ISO 19160. The initial version of the ontology is focused primarily on delivery addresses rather than on extensions including, for example, bar codes, and other details of business addresses. Note too that representation of address lineage, provenance, and data governance is deferred until the OMG Pedigree and Provenance Notation (PPMN) ontology is available.</skos:scopeNote>
		<cmns-av:copyright>Copyright (c) 2013-2025 EDM Council, Inc.</cmns-av:copyright>
		<cmns-av:copyright>Copyright (c) 2013-2025 Object Management Group, Inc.</cmns-av:copyright>
	</owl:Ontology>
	
	<owl:Class rdf:about="&cmns-adr;Address">
		<rdfs:subClassOf rdf:resource="&cmns-cxtdsg;Context"/>
		<rdfs:subClassOf>
			<owl:Restriction>
				<owl:onProperty rdf:resource="&cmns-adr;hasAddressPreferenceLevel"/>
				<owl:minCardinality rdf:datatype="&xsd;nonNegativeInteger">0</owl:minCardinality>
			</owl:Restriction>
		</rdfs:subClassOf>
		<rdfs:subClassOf>
			<owl:Restriction>
				<owl:onProperty rdf:resource="&cmns-adr;hasAddressAlias"/>
				<owl:onClass rdf:resource="&cmns-adr;Address"/>
				<owl:minQualifiedCardinality rdf:datatype="&xsd;nonNegativeInteger">0</owl:minQualifiedCardinality>
			</owl:Restriction>
		</rdfs:subClassOf>
		<rdfs:subClassOf>
			<owl:Restriction>
				<owl:onProperty rdf:resource="&cmns-qtu;specializes"/>
				<owl:onClass rdf:resource="&cmns-adr;Address"/>
				<owl:minQualifiedCardinality rdf:datatype="&xsd;nonNegativeInteger">0</owl:minQualifiedCardinality>
			</owl:Restriction>
		</rdfs:subClassOf>
		<rdfs:subClassOf>
			<owl:Restriction>
				<owl:onProperty rdf:resource="&cmns-col;comprises"/>
				<owl:onClass rdf:resource="&cmns-adr;AddressComponent"/>
				<owl:minQualifiedCardinality rdf:datatype="&xsd;nonNegativeInteger">0</owl:minQualifiedCardinality>
			</owl:Restriction>
		</rdfs:subClassOf>
		<rdfs:subClassOf>
			<owl:Restriction>
				<owl:onProperty rdf:resource="&cmns-id;isIdentifiedBy"/>
				<owl:onClass rdf:resource="&cmns-adr;AddressIdentifier"/>
				<owl:minQualifiedCardinality rdf:datatype="&xsd;nonNegativeInteger">0</owl:minQualifiedCardinality>
			</owl:Restriction>
		</rdfs:subClassOf>
		<rdfs:subClassOf>
			<owl:Restriction>
				<owl:onProperty rdf:resource="&cmns-doc;isSpecifiedIn"/>
				<owl:onClass rdf:resource="&cmns-adr;AddressSpecification"/>
				<owl:minQualifiedCardinality rdf:datatype="&xsd;nonNegativeInteger">0</owl:minQualifiedCardinality>
			</owl:Restriction>
		</rdfs:subClassOf>
		<rdfs:subClassOf>
			<owl:Restriction>
				<owl:onProperty rdf:resource="&cmns-doc;refersTo"/>
				<owl:onClass rdf:resource="&cmns-loc;Location"/>
				<owl:qualifiedCardinality rdf:datatype="&xsd;nonNegativeInteger">1</owl:qualifiedCardinality>
			</owl:Restriction>
		</rdfs:subClassOf>
		<rdfs:label xml:lang="en">address</rdfs:label>
		<skos:definition>frame of reference that facilitates the unambiguous determination of something for purposes of identification and location and to which communications may be delivered</skos:definition>
		<skos:example>Address where the [identified] object is a building: Lombardy House, 809 Lombardy Street, The Hills, 0039, South Africa.</skos:example>
		<skos:example>Address where the [identified] object is a business: 611 Fifth Avenue, New York NY 10022.</skos:example>
		<skos:example>Address where the [identified] object is a land parcel for a building: San 4–5, Munjae-ro, Songpa-gu, Seoul, 13144, South Korea.</skos:example>
		<skos:example>Address where the object is a building group, such as a school or large apartment area: 228-dong 404-ho, 26 Kyunghee-daero, Dongdaemun-gu, Seoul 130–701, South Korea.</skos:example>
		<cmns-av:adaptedFrom>ISO 19160-1:2015 Addressing - Part 1: Conceptual model, First edition, 2015-12-15, clause 4.1 and 6.3.2, Figures 1-4</cmns-av:adaptedFrom>
		<cmns-av:explanatoryNote>Note that the ISO specification rules out virtual and electronic addresses in a note, which this ontology does not.</cmns-av:explanatoryNote>
		<cmns-av:usageNote>The concept of &apos;child address&apos;, i.e., one that is defined relative to a &apos;parent address&apos; is represented using the specializes relation in this ontology. Examples include an address for an apartment within an apartment building, if the building itself has an independent address; in Japan, a jukyo bango (residence number) within a gaiku (block); and a building within a complex of buildings. In Korea, a dong (wing or section of a building) within a group of buildings may be considered a &apos;child address&apos;.</cmns-av:usageNote>
		<cmns-av:usageNote>The concept of an address classifier (AddressClass code set in ISO 19160), which is used to differentiate structural distinctions in the ISO standard, is explicitly omitted. Such distinctions are represented as subclasses of address using this ontology (e.g., conventional street address, post office box address).</cmns-av:usageNote>
	</owl:Class>
	
	<owl:Class rdf:about="&cmns-adr;AddressComponent">
		<rdfs:subClassOf rdf:resource="&cmns-col;Constituent"/>
		<rdfs:subClassOf>
			<owl:Restriction>
				<owl:onProperty rdf:resource="&cmns-col;isIncludedIn"/>
				<owl:someValuesFrom rdf:resource="&cmns-adr;Address"/>
			</owl:Restriction>
		</rdfs:subClassOf>
		<rdfs:subClassOf>
			<owl:Restriction>
				<owl:onProperty rdf:resource="&cmns-cxtdsg;isApplicableIn"/>
				<owl:someValuesFrom rdf:resource="&cmns-adr;AddressComponent"/>
			</owl:Restriction>
		</rdfs:subClassOf>
		<rdfs:label>address component</rdfs:label>
		<skos:definition>constituent part of an address</skos:definition>
		<skos:note>An address component may have one or more alternative values, e.g. alternatives in different languages or abbreviated alternatives.</skos:note>
		<skos:note>An address component may reference another object such as a spatial object (e.g. an administrative boundary or a land parcel) or a non-spatial object (e.g. an organization or a person).</skos:note>
		<cmns-av:adaptedFrom>ISO 19160-1:2015 Addressing - Part 1: Conceptual model, First edition, 2015-12-15, clause 4.5 and 6.3.3, Figures 1-4</cmns-av:adaptedFrom>
	</owl:Class>
	
	<owl:Class rdf:about="&cmns-adr;AddressIdentifier">
		<rdfs:subClassOf rdf:resource="&cmns-cxtid;ContextualIdentifier"/>
		<rdfs:subClassOf>
			<owl:Restriction>
				<owl:onProperty rdf:resource="&cmns-col;isMemberOf"/>
				<owl:onClass rdf:resource="&cmns-adr;AddressSpecification"/>
				<owl:minQualifiedCardinality rdf:datatype="&xsd;nonNegativeInteger">0</owl:minQualifiedCardinality>
			</owl:Restriction>
		</rdfs:subClassOf>
		<rdfs:subClassOf>
			<owl:Restriction>
				<owl:onProperty rdf:resource="&cmns-id;identifies"/>
				<owl:someValuesFrom rdf:resource="&cmns-adr;Address"/>
			</owl:Restriction>
		</rdfs:subClassOf>
		<rdfs:subClassOf>
			<owl:Restriction>
				<owl:onProperty rdf:resource="&cmns-txt;hasTextValue"/>
				<owl:someValuesFrom rdf:resource="&xsd;string"/>
			</owl:Restriction>
		</rdfs:subClassOf>
		<rdfs:label>address identifier</rdfs:label>
		<skos:definition>unique, context-specific identifier for the address</skos:definition>
		<cmns-av:adaptedFrom>ISO 19160-1:2015 Addressing - Part 1: Conceptual model, First edition, 2015-12-15, clause 6.3.2 and Figure 4</cmns-av:adaptedFrom>
	</owl:Class>
	
	<owl:Class rdf:about="&cmns-adr;AddressSpecification">
		<rdfs:subClassOf rdf:resource="&cmns-col;Arrangement"/>
		<rdfs:subClassOf rdf:resource="&cmns-doc;Specification"/>
		<rdfs:subClassOf>
			<owl:Restriction>
				<owl:onProperty rdf:resource="&cmns-doc;specifies"/>
				<owl:onClass rdf:resource="&cmns-adr;Address"/>
				<owl:minQualifiedCardinality rdf:datatype="&xsd;nonNegativeInteger">0</owl:minQualifiedCardinality>
			</owl:Restriction>
		</rdfs:subClassOf>
		<rdfs:label>address specification</rdfs:label>
		<skos:definition>system for allocating addresses to objects</skos:definition>
		<skos:note>An address specification includes a defined set of address components and the rules for their combination into addresses.</skos:note>
		<cmns-av:adaptedFrom>ISO 19160-1:2015 Addressing - Part 1: Conceptual model, First edition, 2015-12-15, clauses 4.8, 6.3.6, Figures 2-4</cmns-av:adaptedFrom>
		<cmns-av:synonym>address reference system</cmns-av:synonym>
		<cmns-av:synonym>addressing scheme</cmns-av:synonym>
	</owl:Class>
	
	<owl:NamedIndividual rdf:about="&cmns-adr;Apartment">
		<rdf:type rdf:resource="&cmns-adr;SecondaryUnitDesignator"/>
		<rdfs:label xml:lang="en">apartment</rdfs:label>
		<skos:definition>room or a group of related rooms, among similar sets in one building, designed for use as a dwelling</skos:definition>
		<cmns-adr:requiresSecondaryUnitRange rdf:datatype="&xsd;boolean">true</cmns-adr:requiresSecondaryUnitRange>
	</owl:NamedIndividual>
	
	<owl:NamedIndividual rdf:about="&cmns-adr;Basement">
		<rdf:type rdf:resource="&cmns-adr;SecondaryUnitDesignator"/>
		<rdfs:label xml:lang="en">basement</rdfs:label>
		<skos:definition>part of a building consisting of rooms that are partly or entirely below ground</skos:definition>
		<cmns-adr:requiresSecondaryUnitRange rdf:datatype="&xsd;boolean">false</cmns-adr:requiresSecondaryUnitRange>
	</owl:NamedIndividual>
	
	<owl:NamedIndividual rdf:about="&cmns-adr;Building">
		<rdf:type rdf:resource="&cmns-adr;SecondaryUnitDesignator"/>
		<rdfs:label xml:lang="en">building</rdfs:label>
		<skos:definition>relatively permanent enclosed structure, that has a roof and walls and stands more or less permanently in one place</skos:definition>
		<cmns-adr:requiresSecondaryUnitRange rdf:datatype="&xsd;boolean">true</cmns-adr:requiresSecondaryUnitRange>
	</owl:NamedIndividual>
	
	<owl:Class rdf:about="&cmns-adr;ConventionalStreetAddress">
		<rdfs:subClassOf rdf:resource="&cmns-adr;PhysicalAddress"/>
		<rdfs:subClassOf>
			<owl:Restriction>
				<owl:onProperty rdf:resource="&cmns-adr;hasStreetAddress"/>
				<owl:onClass rdf:resource="&cmns-adr;StreetAddress"/>
				<owl:maxQualifiedCardinality rdf:datatype="&xsd;nonNegativeInteger">1</owl:maxQualifiedCardinality>
			</owl:Restriction>
		</rdfs:subClassOf>
		<rdfs:subClassOf>
			<owl:Restriction>
				<owl:onProperty rdf:resource="&cmns-adr;hasAddressLine1"/>
				<owl:maxQualifiedCardinality rdf:datatype="&xsd;nonNegativeInteger">1</owl:maxQualifiedCardinality>
				<owl:onDataRange rdf:resource="&rdfs;Literal"/>
			</owl:Restriction>
		</rdfs:subClassOf>
		<rdfs:subClassOf>
			<owl:Restriction>
				<owl:onProperty rdf:resource="&cmns-adr;hasAddressLine2"/>
				<owl:maxQualifiedCardinality rdf:datatype="&xsd;nonNegativeInteger">1</owl:maxQualifiedCardinality>
				<owl:onDataRange rdf:resource="&rdfs;Literal"/>
			</owl:Restriction>
		</rdfs:subClassOf>
		<rdfs:subClassOf>
			<owl:Restriction>
				<owl:onProperty rdf:resource="&cmns-adr;hasAddressLine3"/>
				<owl:maxQualifiedCardinality rdf:datatype="&xsd;nonNegativeInteger">1</owl:maxQualifiedCardinality>
				<owl:onDataRange rdf:resource="&rdfs;Literal"/>
			</owl:Restriction>
		</rdfs:subClassOf>
		<rdfs:label>conventional street address</rdfs:label>
		<skos:definition>physical address that identifies a location on a street to which communications may be delivered</skos:definition>
		<cmns-av:explanatoryNote>Other unconventional addresses may include rural and highway route addresses, general delivery addresses, post office box addresses, private mail center addresses, and so forth.</cmns-av:explanatoryNote>
	</owl:Class>
	
	<owl:NamedIndividual rdf:about="&cmns-adr;Department">
		<rdf:type rdf:resource="&cmns-adr;SecondaryUnitDesignator"/>
		<rdfs:label xml:lang="en">department</rdfs:label>
		<skos:definition>division of a large organization such as a government, university, business, or shop, dealing with a specific subject, commodity, or area of activity</skos:definition>
		<cmns-adr:requiresSecondaryUnitRange rdf:datatype="&xsd;boolean">true</cmns-adr:requiresSecondaryUnitRange>
	</owl:NamedIndividual>
	
	<owl:NamedIndividual rdf:about="&cmns-adr;Floor">
		<rdf:type rdf:resource="&cmns-adr;SecondaryUnitDesignator"/>
		<rdfs:label xml:lang="en">floor</rdfs:label>
		<skos:definition>all of the rooms or areas on the same level of a building; a story</skos:definition>
		<cmns-adr:requiresSecondaryUnitRange rdf:datatype="&xsd;boolean">true</cmns-adr:requiresSecondaryUnitRange>
		<cmns-av:explanatoryNote>Labeling systems for floors vary from country to country, and may be specific to the building, for example, whether or not a 13th floor is identified as such tends to be on a case-by-case basis.</cmns-av:explanatoryNote>
	</owl:NamedIndividual>
	
	<owl:NamedIndividual rdf:about="&cmns-adr;Front">
		<rdf:type rdf:resource="&cmns-adr;SecondaryUnitDesignator"/>
		<rdfs:label xml:lang="en">front</rdfs:label>
		<skos:definition>side or part of a building that presents itself to view first, that faces the street; the most forward part of a building</skos:definition>
		<cmns-adr:requiresSecondaryUnitRange rdf:datatype="&xsd;boolean">false</cmns-adr:requiresSecondaryUnitRange>
	</owl:NamedIndividual>
	
	<owl:Class rdf:about="&cmns-adr;GeographicDirectionalSymbol">
		<rdfs:subClassOf rdf:resource="&cmns-adr;AddressComponent"/>
		<rdfs:subClassOf rdf:resource="&cmns-cds;CodeElement"/>
		<rdfs:subClassOf>
			<owl:Restriction>
				<owl:onProperty rdf:resource="&cmns-txt;hasTextValue"/>
				<owl:someValuesFrom rdf:resource="&xsd;string"/>
			</owl:Restriction>
		</rdfs:subClassOf>
		<rdfs:label>geographic directional symbol</rdfs:label>
		<skos:definition>code element that gives directional information for postal delivery</skos:definition>
		<skos:example>In the United States, these include N, S, E, W, NE, NW, SE, SW.</skos:example>
	</owl:Class>
	
	<owl:NamedIndividual rdf:about="&cmns-adr;Hangar">
		<rdf:type rdf:resource="&cmns-adr;SecondaryUnitDesignator"/>
		<rdfs:label xml:lang="en">hanger</rdfs:label>
		<skos:definition>shed or shelter; any relatively wide structure used for housing airplanes or airships</skos:definition>
		<cmns-adr:requiresSecondaryUnitRange rdf:datatype="&xsd;boolean">true</cmns-adr:requiresSecondaryUnitRange>
	</owl:NamedIndividual>
	
	<owl:NamedIndividual rdf:about="&cmns-adr;Key">
		<rdf:type rdf:resource="&cmns-adr;SecondaryUnitDesignator"/>
		<rdfs:label xml:lang="en">key</rdfs:label>
		<skos:definition>usually metal instrument by which the bolt of a lock is turned</skos:definition>
		<cmns-adr:requiresSecondaryUnitRange rdf:datatype="&xsd;boolean">true</cmns-adr:requiresSecondaryUnitRange>
	</owl:NamedIndividual>
	
	<owl:NamedIndividual rdf:about="&cmns-adr;Lobby">
		<rdf:type rdf:resource="&cmns-adr;SecondaryUnitDesignator"/>
		<rdfs:label xml:lang="en">lobby</rdfs:label>
		<skos:definition>entrance hall, corridor, or vestibule, as in a public building, often serving as an anteroom; foyer</skos:definition>
		<cmns-adr:requiresSecondaryUnitRange rdf:datatype="&xsd;boolean">false</cmns-adr:requiresSecondaryUnitRange>
	</owl:NamedIndividual>
	
	<owl:NamedIndividual rdf:about="&cmns-adr;Lot">
		<rdf:type rdf:resource="&cmns-adr;SecondaryUnitDesignator"/>
		<rdfs:label xml:lang="en">lot</rdfs:label>
		<skos:definition>measured parcel of land having fixed boundaries and designated on a plot or survey</skos:definition>
		<cmns-adr:requiresSecondaryUnitRange rdf:datatype="&xsd;boolean">true</cmns-adr:requiresSecondaryUnitRange>
	</owl:NamedIndividual>
	
	<owl:NamedIndividual rdf:about="&cmns-adr;Lower">
		<rdf:type rdf:resource="&cmns-adr;SecondaryUnitDesignator"/>
		<rdfs:label xml:lang="en">lower</rdfs:label>
		<skos:definition>floor of a building in a multistory structure that is closer to ground level</skos:definition>
		<cmns-adr:requiresSecondaryUnitRange rdf:datatype="&xsd;boolean">false</cmns-adr:requiresSecondaryUnitRange>
	</owl:NamedIndividual>
	
	<owl:NamedIndividual rdf:about="&cmns-adr;Office">
		<rdf:type rdf:resource="&cmns-adr;SecondaryUnitDesignator"/>
		<rdfs:label xml:lang="en">office</rdfs:label>
		<skos:definition>place where a particular kind of business is transacted or a service is supplied</skos:definition>
		<cmns-adr:requiresSecondaryUnitRange rdf:datatype="&xsd;boolean">false</cmns-adr:requiresSecondaryUnitRange>
	</owl:NamedIndividual>
	
	<owl:NamedIndividual rdf:about="&cmns-adr;Penthouse">
		<rdf:type rdf:resource="&cmns-adr;SecondaryUnitDesignator"/>
		<rdfs:label xml:lang="en">penthouse</rdfs:label>
		<skos:definition>structure or dwelling on the roof or top floor of a building</skos:definition>
		<cmns-adr:requiresSecondaryUnitRange rdf:datatype="&xsd;boolean">false</cmns-adr:requiresSecondaryUnitRange>
	</owl:NamedIndividual>
	
	<owl:Class rdf:about="&cmns-adr;PhysicalAddress">
		<rdfs:subClassOf rdf:resource="&cmns-adr;Address"/>
		<rdfs:subClassOf>
			<owl:Restriction>
				<owl:onProperty rdf:resource="&cmns-adr;hasIndividualPostcode"/>
				<owl:onClass rdf:resource="&cmns-adr;Postcode"/>
				<owl:maxQualifiedCardinality rdf:datatype="&xsd;nonNegativeInteger">1</owl:maxQualifiedCardinality>
			</owl:Restriction>
		</rdfs:subClassOf>
		<rdfs:subClassOf>
			<owl:Restriction>
				<owl:onProperty rdf:resource="&cmns-loc;hasCountry"/>
				<owl:onClass rdf:resource="&cmns-loc;Country"/>
				<owl:maxQualifiedCardinality rdf:datatype="&xsd;nonNegativeInteger">1</owl:maxQualifiedCardinality>
			</owl:Restriction>
		</rdfs:subClassOf>
		<rdfs:subClassOf>
			<owl:Restriction>
				<owl:onProperty rdf:resource="&cmns-loc;hasMunicipality"/>
				<owl:onClass rdf:resource="&cmns-loc;Municipality"/>
				<owl:maxQualifiedCardinality rdf:datatype="&xsd;nonNegativeInteger">1</owl:maxQualifiedCardinality>
			</owl:Restriction>
		</rdfs:subClassOf>
		<rdfs:subClassOf>
			<owl:Restriction>
				<owl:onProperty rdf:resource="&cmns-adr;hasPostalCode"/>
				<owl:maxQualifiedCardinality rdf:datatype="&xsd;nonNegativeInteger">1</owl:maxQualifiedCardinality>
				<owl:onDataRange rdf:resource="&rdfs;Literal"/>
			</owl:Restriction>
		</rdfs:subClassOf>
		<rdfs:subClassOf>
			<owl:Restriction>
				<owl:onProperty rdf:resource="&cmns-loc;hasCityName"/>
				<owl:maxQualifiedCardinality rdf:datatype="&xsd;nonNegativeInteger">1</owl:maxQualifiedCardinality>
				<owl:onDataRange rdf:resource="&rdfs;Literal"/>
			</owl:Restriction>
		</rdfs:subClassOf>
		<rdfs:subClassOf>
			<owl:Restriction>
				<owl:onProperty rdf:resource="&cmns-doc;refersTo"/>
				<owl:onClass rdf:resource="&cmns-loc;PhysicalLocation"/>
				<owl:minQualifiedCardinality rdf:datatype="&xsd;nonNegativeInteger">0</owl:minQualifiedCardinality>
			</owl:Restriction>
		</rdfs:subClassOf>
		<rdfs:subClassOf>
			<owl:Restriction>
				<owl:onProperty rdf:resource="&cmns-col;comprises"/>
				<owl:someValuesFrom rdf:resource="&cmns-adr;AddressComponent"/>
			</owl:Restriction>
		</rdfs:subClassOf>
		<rdfs:subClassOf>
			<owl:Restriction>
				<owl:onProperty rdf:resource="&cmns-loc;hasSubdivision"/>
				<owl:someValuesFrom rdf:resource="&cmns-loc;CountrySubdivision"/>
			</owl:Restriction>
		</rdfs:subClassOf>
		<rdfs:label xml:lang="en">physical address</rdfs:label>
		<skos:definition>physical address where communications can be addressed, papers served or representatives located for any kind of organization or person</skos:definition>
		<skos:scopeNote>An address may be used as an index to the location of a building, apartment, office within an office block, or other structure or parcel of land, often using political boundaries and street names as references, along with other information such as house or building numbers or names. Some addresses also contain secondary elements such as apartment or building numbers, or special codes to aid routing of mail and packages.</skos:scopeNote>
		<cmns-av:usageNote>Typically, addresses will have only one postcode expressed either as a string value or individual, and only a municipality (individual) or city (string value).</cmns-av:usageNote>
	</owl:Class>
	
	<owl:Class rdf:about="&cmns-adr;PhysicalAddressIdentifier">
		<rdfs:subClassOf rdf:resource="&cmns-cds;CodeElement"/>
		<rdfs:subClassOf rdf:resource="&cmns-id;Identifier"/>
		<rdfs:subClassOf>
			<owl:Restriction>
				<owl:onProperty rdf:resource="&cmns-id;identifies"/>
				<owl:onClass rdf:resource="&cmns-adr;PhysicalAddress"/>
				<owl:qualifiedCardinality rdf:datatype="&xsd;nonNegativeInteger">1</owl:qualifiedCardinality>
			</owl:Restriction>
		</rdfs:subClassOf>
		<rdfs:subClassOf>
			<owl:Restriction>
				<owl:onProperty rdf:resource="&cmns-col;isMemberOf"/>
				<owl:onClass rdf:resource="&cmns-adr;PhysicalAddressingScheme"/>
				<owl:qualifiedCardinality rdf:datatype="&xsd;nonNegativeInteger">1</owl:qualifiedCardinality>
			</owl:Restriction>
		</rdfs:subClassOf>
		<rdfs:label>physical address identifier</rdfs:label>
		<skos:definition>unique identifier for a physical address</skos:definition>
		<skos:example>Physical address identifiers may include bar codes, QCR codes, and +codes in a number of countries.</skos:example>
	</owl:Class>
	
	<owl:Class rdf:about="&cmns-adr;PhysicalAddressingScheme">
		<rdfs:subClassOf rdf:resource="&cmns-adr;AddressSpecification"/>
		<rdfs:subClassOf>
			<owl:Class>
				<owl:unionOf rdf:parseType="Collection">
					<owl:Restriction>
						<owl:onProperty rdf:resource="&cmns-dsg;defines"/>
						<owl:onClass rdf:resource="&cmns-adr;PhysicalAddressIdentifier"/>
						<owl:minQualifiedCardinality rdf:datatype="&xsd;nonNegativeInteger">0</owl:minQualifiedCardinality>
					</owl:Restriction>
					<owl:Restriction>
						<owl:onProperty rdf:resource="&cmns-dsg;defines"/>
						<owl:onClass rdf:resource="&cmns-adr;PhysicalAddress"/>
						<owl:minQualifiedCardinality rdf:datatype="&xsd;nonNegativeInteger">0</owl:minQualifiedCardinality>
					</owl:Restriction>
				</owl:unionOf>
			</owl:Class>
		</rdfs:subClassOf>
		<rdfs:label>physical addressing scheme</rdfs:label>
		<rdfs:seeAlso rdf:resource="https://pe.usps.com/cpim/ftp/pubs/Pub28/pub28.pdf"/>
		<skos:definition>scheme for specifying physical addresses according to a country specific standard</skos:definition>
	</owl:Class>
	
	<owl:NamedIndividual rdf:about="&cmns-adr;Pier">
		<rdf:type rdf:resource="&cmns-adr;SecondaryUnitDesignator"/>
		<rdfs:label xml:lang="en">pier</rdfs:label>
		<skos:definition>structure extending into navigable water for use as a landing place or promenade</skos:definition>
		<cmns-adr:requiresSecondaryUnitRange rdf:datatype="&xsd;boolean">true</cmns-adr:requiresSecondaryUnitRange>
	</owl:NamedIndividual>
	
	<owl:Class rdf:about="&cmns-adr;PostCodeArea">
		<rdfs:subClassOf rdf:resource="&cmns-loc;GeographicRegion"/>
		<rdfs:label xml:lang="en">post code area</rdfs:label>
		<skos:definition>physical area uniquely identified by some postal code</skos:definition>
	</owl:Class>
	
	<owl:Class rdf:about="&cmns-adr;PostOfficeBox">
		<rdfs:subClassOf rdf:resource="&cmns-adr;SupplementalAddressComponent"/>
		<rdfs:subClassOf>
			<owl:Restriction>
				<owl:onProperty rdf:resource="&cmns-col;comprises"/>
				<owl:onClass rdf:resource="&cmns-adr;PostOfficeBoxDesignator"/>
				<owl:qualifiedCardinality rdf:datatype="&xsd;nonNegativeInteger">1</owl:qualifiedCardinality>
			</owl:Restriction>
		</rdfs:subClassOf>
		<rdfs:label>post office box</rdfs:label>
		<skos:definition>post office box associated with an address</skos:definition>
		<cmns-av:explanatoryNote>Post office box identifiers are only unique to a given jurisdiction, which may be a post office, town, or other region.</cmns-av:explanatoryNote>
	</owl:Class>
	
	<owl:Class rdf:about="&cmns-adr;PostOfficeBoxAddress">
		<rdfs:subClassOf rdf:resource="&cmns-adr;PhysicalAddress"/>
		<rdfs:subClassOf>
			<owl:Restriction>
				<owl:onProperty rdf:resource="&cmns-col;comprises"/>
				<owl:onClass rdf:resource="&cmns-adr;PostOfficeBox"/>
				<owl:qualifiedCardinality rdf:datatype="&xsd;nonNegativeInteger">1</owl:qualifiedCardinality>
			</owl:Restriction>
		</rdfs:subClassOf>
		<rdfs:label>post office box address</rdfs:label>
		<skos:definition>physical address used to deliver communications to a designated container at a local post office or the local equivalent for the jurisdiction, where mail is held until the recipient collects it, rather than to a given house, building, or other location</skos:definition>
	</owl:Class>
	
	<owl:Class rdf:about="&cmns-adr;PostOfficeBoxDesignator">
		<rdfs:subClassOf rdf:resource="&cmns-adr;SupplementalAddressDesignator"/>
		<rdfs:label xml:lang="en">post office box designator</rdfs:label>
		<skos:definition>designator used, together with an identifier, for a post office box</skos:definition>
		<skos:example>In the U.S., the preferred designator is &apos;PO BOX&apos;.</skos:example>
	</owl:Class>
	
	<owl:Class rdf:about="&cmns-adr;Postcode">
		<rdfs:subClassOf rdf:resource="&cmns-adr;AddressComponent"/>
		<rdfs:subClassOf rdf:resource="&cmns-cds;CodeElement"/>
		<rdfs:subClassOf rdf:resource="&cmns-loc;GeographicRegionIdentifier"/>
		<rdfs:subClassOf>
			<owl:Restriction>
				<owl:onProperty rdf:resource="&cmns-id;identifies"/>
				<owl:onClass rdf:resource="&cmns-adr;PostCodeArea"/>
				<owl:qualifiedCardinality rdf:datatype="&xsd;nonNegativeInteger">1</owl:qualifiedCardinality>
			</owl:Restriction>
		</rdfs:subClassOf>
		<rdfs:label xml:lang="en">postcode</rdfs:label>
		<skos:definition>sequence of characters used to assist in the sorting of mail</skos:definition>
		<cmns-av:synonym>postal code</cmns-av:synonym>
	</owl:Class>
	
	<owl:Class rdf:about="&cmns-adr;PostdirectionalSymbol">
		<rdfs:subClassOf rdf:resource="&cmns-adr;GeographicDirectionalSymbol"/>
		<rdfs:label>postdirectional symbol</rdfs:label>
		<skos:definition>geographic directional symbol that follows the street name and street suffix in a street address</skos:definition>
	</owl:Class>
	
	<owl:Class rdf:about="&cmns-adr;PredirectionalSymbol">
		<rdfs:subClassOf rdf:resource="&cmns-adr;GeographicDirectionalSymbol"/>
		<rdfs:label>predirectional symbol</rdfs:label>
		<skos:definition>geographic directional symbol that occurs after the primary street number but before the street name in a street address</skos:definition>
	</owl:Class>
	
	<owl:Class rdf:about="&cmns-adr;PrimaryAddressNumber">
		<rdfs:subClassOf rdf:resource="&cmns-adr;AddressComponent"/>
		<rdfs:subClassOf>
			<owl:Restriction>
				<owl:onProperty rdf:resource="&cmns-txt;hasTextValue"/>
				<owl:onDataRange rdf:resource="&xsd;string"/>
				<owl:qualifiedCardinality rdf:datatype="&xsd;nonNegativeInteger">1</owl:qualifiedCardinality>
			</owl:Restriction>
		</rdfs:subClassOf>
		<rdfs:label>primary address number</rdfs:label>
		<skos:definition>address component that identifies a location with respect to a given street</skos:definition>
		<cmns-av:explanatoryNote>Although traditionally called a &apos;number&apos;, the street number may consist of alphanumeric characters, for example, &apos;221B&apos;.</cmns-av:explanatoryNote>
		<cmns-av:synonym>street number</cmns-av:synonym>
	</owl:Class>
	
	<owl:NamedIndividual rdf:about="&cmns-adr;Rear">
		<rdf:type rdf:resource="&cmns-adr;SecondaryUnitDesignator"/>
		<rdfs:label xml:lang="en">rear</rdfs:label>
		<skos:definition>side or part of a building at the back, located opposite its front</skos:definition>
		<cmns-adr:requiresSecondaryUnitRange rdf:datatype="&xsd;boolean">false</cmns-adr:requiresSecondaryUnitRange>
	</owl:NamedIndividual>
	
	<owl:Class rdf:about="&cmns-adr;RegionSpecificIdentifier">
		<rdfs:subClassOf rdf:resource="&cmns-loc;GeographicRegionIdentifier"/>
		<rdfs:subClassOf>
			<owl:Restriction>
				<owl:onProperty rdf:resource="&cmns-cxtdsg;isUsedBy"/>
				<owl:someValuesFrom rdf:resource="&cmns-loc;GeopoliticalEntity"/>
			</owl:Restriction>
		</rdfs:subClassOf>
		<rdfs:label>region-specific identifier</rdfs:label>
		<skos:definition>geographic region or subdivision identifier used internally by a country or other region</skos:definition>
	</owl:Class>
	
	<owl:NamedIndividual rdf:about="&cmns-adr;Room">
		<rdf:type rdf:resource="&cmns-adr;SecondaryUnitDesignator"/>
		<rdfs:label xml:lang="en">room</rdfs:label>
		<skos:definition>partitioned part of the inside of a building</skos:definition>
		<cmns-adr:requiresSecondaryUnitRange rdf:datatype="&xsd;boolean">true</cmns-adr:requiresSecondaryUnitRange>
	</owl:NamedIndividual>
	
	<owl:Class rdf:about="&cmns-adr;SecondaryUnit">
		<rdfs:subClassOf rdf:resource="&cmns-adr;AddressComponent"/>
		<rdfs:subClassOf>
			<owl:Restriction>
				<owl:onProperty rdf:resource="&cmns-col;comprises"/>
				<owl:onClass rdf:resource="&cmns-adr;SecondaryUnitIndicator"/>
				<owl:minQualifiedCardinality rdf:datatype="&xsd;nonNegativeInteger">0</owl:minQualifiedCardinality>
			</owl:Restriction>
		</rdfs:subClassOf>
		<rdfs:subClassOf>
			<owl:Restriction>
				<owl:onProperty rdf:resource="&cmns-col;comprises"/>
				<owl:onClass rdf:resource="&cmns-adr;SecondaryUnitDesignator"/>
				<owl:qualifiedCardinality rdf:datatype="&xsd;nonNegativeInteger">1</owl:qualifiedCardinality>
			</owl:Restriction>
		</rdfs:subClassOf>
		<rdfs:label>secondary unit</rdfs:label>
		<skos:definition>address component that identifies an individual unit within a larger structure, such as an apartment, office, hangar, slip, mailbox, and so forth, at a given street address</skos:definition>
	</owl:Class>
	
	<owl:Class rdf:about="&cmns-adr;SecondaryUnitDesignator">
		<rdfs:subClassOf rdf:resource="&cmns-cls;Classifier"/>
		<rdfs:subClassOf>
			<owl:Restriction>
				<owl:onProperty rdf:resource="&cmns-adr;requiresSecondaryUnitRange"/>
				<owl:onDataRange rdf:resource="&xsd;boolean"/>
				<owl:qualifiedCardinality rdf:datatype="&xsd;nonNegativeInteger">1</owl:qualifiedCardinality>
			</owl:Restriction>
		</rdfs:subClassOf>
		<rdfs:label>secondary unit designator</rdfs:label>
		<skos:definition>classifier for a smaller structure or component within a larger facility, such as an apartment, office, mail stop, or other similar designation</skos:definition>
		<cmns-av:explanatoryNote>Note that only certain secondary units require a secondary range, such as an apartment number, to complete a delivery point.</cmns-av:explanatoryNote>
	</owl:Class>
	
	<owl:Class rdf:about="&cmns-adr;SecondaryUnitIndicator">
		<rdfs:subClassOf rdf:resource="&cmns-adr;AddressComponent"/>
		<rdfs:subClassOf>
			<owl:Restriction>
				<owl:onProperty rdf:resource="&cmns-txt;hasTextValue"/>
				<owl:onDataRange rdf:resource="&xsd;string"/>
				<owl:qualifiedCardinality rdf:datatype="&xsd;nonNegativeInteger">1</owl:qualifiedCardinality>
			</owl:Restriction>
		</rdfs:subClassOf>
		<rdfs:label>secondary unit indicator</rdfs:label>
		<skos:definition>index to the specific unit within a secondary unit, such as a building or apartment, at a particular street address</skos:definition>
	</owl:Class>
	
	<owl:NamedIndividual rdf:about="&cmns-adr;Side">
		<rdf:type rdf:resource="&cmns-adr;SecondaryUnitDesignator"/>
		<rdfs:label xml:lang="en">side</rdfs:label>
		<skos:definition>place, space, or direction with respect to a center or to a line of division</skos:definition>
		<cmns-adr:requiresSecondaryUnitRange rdf:datatype="&xsd;boolean">false</cmns-adr:requiresSecondaryUnitRange>
	</owl:NamedIndividual>
	
	<owl:NamedIndividual rdf:about="&cmns-adr;Slip">
		<rdf:type rdf:resource="&cmns-adr;SecondaryUnitDesignator"/>
		<rdfs:label xml:lang="en">slip</rdfs:label>
		<skos:definition>sloping ramp extending out into the water to serve as a place for landing or repairing ships; ship&apos;s or boat&apos;s berth between two piers</skos:definition>
		<cmns-adr:requiresSecondaryUnitRange rdf:datatype="&xsd;boolean">true</cmns-adr:requiresSecondaryUnitRange>
	</owl:NamedIndividual>
	
	<owl:NamedIndividual rdf:about="&cmns-adr;Space">
		<rdf:type rdf:resource="&cmns-adr;SecondaryUnitDesignator"/>
		<rdfs:label xml:lang="en">space</rdfs:label>
		<skos:definition>extent set apart or available, such as a parking or storage space</skos:definition>
		<cmns-adr:requiresSecondaryUnitRange rdf:datatype="&xsd;boolean">true</cmns-adr:requiresSecondaryUnitRange>
	</owl:NamedIndividual>
	
	<owl:NamedIndividual rdf:about="&cmns-adr;Stop">
		<rdf:type rdf:resource="&cmns-adr;SecondaryUnitDesignator"/>
		<rdfs:label xml:lang="en">stop</rdfs:label>
		<skos:definition>stopping place, such as a bus or mail stop</skos:definition>
		<cmns-adr:requiresSecondaryUnitRange rdf:datatype="&xsd;boolean">true</cmns-adr:requiresSecondaryUnitRange>
	</owl:NamedIndividual>
	
	<owl:Class rdf:about="&cmns-adr;StreetAddress">
		<rdfs:subClassOf rdf:resource="&cmns-adr;AddressComponent"/>
		<rdfs:subClassOf>
			<owl:Restriction>
				<owl:onProperty rdf:resource="&cmns-adr;hasPrimaryAddressNumber"/>
				<owl:onClass rdf:resource="&cmns-adr;PrimaryAddressNumber"/>
				<owl:maxQualifiedCardinality rdf:datatype="&xsd;nonNegativeInteger">1</owl:maxQualifiedCardinality>
			</owl:Restriction>
		</rdfs:subClassOf>
		<rdfs:subClassOf>
			<owl:Restriction>
				<owl:onProperty rdf:resource="&cmns-adr;hasPostdirectionalSymbol"/>
				<owl:onClass rdf:resource="&cmns-adr;PostdirectionalSymbol"/>
				<owl:minQualifiedCardinality rdf:datatype="&xsd;nonNegativeInteger">0</owl:minQualifiedCardinality>
			</owl:Restriction>
		</rdfs:subClassOf>
		<rdfs:subClassOf>
			<owl:Restriction>
				<owl:onProperty rdf:resource="&cmns-adr;hasPredirectionalSymbol"/>
				<owl:onClass rdf:resource="&cmns-adr;PredirectionalSymbol"/>
				<owl:minQualifiedCardinality rdf:datatype="&xsd;nonNegativeInteger">0</owl:minQualifiedCardinality>
			</owl:Restriction>
		</rdfs:subClassOf>
		<rdfs:subClassOf>
			<owl:Restriction>
				<owl:onProperty rdf:resource="&cmns-adr;hasSecondaryUnit"/>
				<owl:onClass rdf:resource="&cmns-adr;SecondaryUnit"/>
				<owl:minQualifiedCardinality rdf:datatype="&xsd;nonNegativeInteger">0</owl:minQualifiedCardinality>
			</owl:Restriction>
		</rdfs:subClassOf>
		<rdfs:subClassOf>
			<owl:Restriction>
				<owl:onProperty rdf:resource="&cmns-adr;hasStreetSuffix"/>
				<owl:onClass rdf:resource="&cmns-adr;StreetSuffix"/>
				<owl:minQualifiedCardinality rdf:datatype="&xsd;nonNegativeInteger">0</owl:minQualifiedCardinality>
			</owl:Restriction>
		</rdfs:subClassOf>
		<rdfs:subClassOf>
			<owl:Restriction>
				<owl:onProperty rdf:resource="&cmns-adr;hasStreetName"/>
				<owl:someValuesFrom rdf:resource="&cmns-adr;StreetName"/>
			</owl:Restriction>
		</rdfs:subClassOf>
		<rdfs:label>street address</rdfs:label>
		<skos:definition>index to a location that consists of a primary address number, predirectional, street name, suffix, postdirectional, and an optional secondary unit</skos:definition>
	</owl:Class>
	
	<owl:Class rdf:about="&cmns-adr;StreetName">
		<rdfs:subClassOf rdf:resource="&cmns-adr;AddressComponent"/>
		<rdfs:subClassOf rdf:resource="&cmns-dsg;Name"/>
		<rdfs:subClassOf>
			<owl:Restriction>
				<owl:onProperty rdf:resource="&cmns-txt;hasTextValue"/>
				<owl:onDataRange rdf:resource="&xsd;string"/>
				<owl:qualifiedCardinality rdf:datatype="&xsd;nonNegativeInteger">1</owl:qualifiedCardinality>
			</owl:Restriction>
		</rdfs:subClassOf>
		<rdfs:label>street name</rdfs:label>
		<skos:definition>identifier for a street in some context (e.g., city, municipality, geographic region)</skos:definition>
	</owl:Class>
	
	<owl:Class rdf:about="&cmns-adr;StreetSuffix">
		<rdfs:subClassOf rdf:resource="&cmns-adr;AddressComponent"/>
		<rdfs:subClassOf rdf:resource="&cmns-cls;Classifier"/>
		<rdfs:label>street suffix</rdfs:label>
		<skos:definition>classifier for a street or other delivery location, such as a dwelling located along a waterway</skos:definition>
		<cmns-av:explanatoryNote>The suffix may provide some insight into the size or length of the street, though not necessarily consistently. In some cities, the suffix differentiates the street from another in the same context, such as 19th Street vs. 19th Avenue in San Francisco.</cmns-av:explanatoryNote>
	</owl:Class>
	
	<owl:Class rdf:about="&cmns-adr;StructureName">
		<rdfs:subClassOf rdf:resource="&cmns-adr;AddressComponent"/>
		<rdfs:subClassOf rdf:resource="&cmns-dsg;Name"/>
		<rdfs:subClassOf>
			<owl:Restriction>
				<owl:onProperty rdf:resource="&cmns-txt;hasTextValue"/>
				<owl:onDataRange rdf:resource="&xsd;string"/>
				<owl:qualifiedCardinality rdf:datatype="&xsd;nonNegativeInteger">1</owl:qualifiedCardinality>
			</owl:Restriction>
		</rdfs:subClassOf>
		<rdfs:label>structure name</rdfs:label>
		<skos:definition>name for a building, house, office complex, shopping center, or other structure or group of structures</skos:definition>
		<skos:example>Examples include &apos;McCoy Center&apos;, which is the name of the office complex where JPMorgan Chase&apos;s Polaris facility is located, &apos;Apple Park&apos;, which is the name of the corporate headquarters of Apple, Inc., and &apos;Howells Bridge Cottage&apos;, which is the name of a very old cottage in Cornwall.</skos:example>
	</owl:Class>
	
	<owl:NamedIndividual rdf:about="&cmns-adr;Suite">
		<rdf:type rdf:resource="&cmns-adr;SecondaryUnitDesignator"/>
		<rdfs:label xml:lang="en">suite</rdfs:label>
		<skos:definition>group of rooms occupied as a unit</skos:definition>
		<cmns-adr:requiresSecondaryUnitRange rdf:datatype="&xsd;boolean">true</cmns-adr:requiresSecondaryUnitRange>
	</owl:NamedIndividual>
	
	<owl:Class rdf:about="&cmns-adr;SupplementalAddressComponent">
		<rdfs:subClassOf rdf:resource="&cmns-adr;AddressComponent"/>
		<rdfs:subClassOf>
			<owl:Restriction>
				<owl:onProperty rdf:resource="&cmns-col;comprises"/>
				<owl:onClass rdf:resource="&cmns-adr;SupplementalAddressUnit"/>
				<owl:minQualifiedCardinality rdf:datatype="&xsd;nonNegativeInteger">0</owl:minQualifiedCardinality>
			</owl:Restriction>
		</rdfs:subClassOf>
		<rdfs:subClassOf>
			<owl:Restriction>
				<owl:onProperty rdf:resource="&cmns-txt;hasTextValue"/>
				<owl:minQualifiedCardinality rdf:datatype="&xsd;nonNegativeInteger">0</owl:minQualifiedCardinality>
				<owl:onDataRange rdf:resource="&rdfs;Literal"/>
			</owl:Restriction>
		</rdfs:subClassOf>
		<rdfs:subClassOf>
			<owl:Restriction>
				<owl:onProperty rdf:resource="&cmns-col;comprises"/>
				<owl:onClass rdf:resource="&cmns-adr;SupplementalAddressDesignator"/>
				<owl:qualifiedCardinality rdf:datatype="&xsd;nonNegativeInteger">1</owl:qualifiedCardinality>
			</owl:Restriction>
		</rdfs:subClassOf>
		<rdfs:label>supplemental address component</rdfs:label>
		<skos:definition>address component that provides additional information that is important to ensuring proper delivery of communications</skos:definition>
		<cmns-av:explanatoryNote>Supplemental components include post office box information, rural route and highway contract route information, private mailboxes, and so forth, that are not part of a conventional street address.</cmns-av:explanatoryNote>
	</owl:Class>
	
	<owl:Class rdf:about="&cmns-adr;SupplementalAddressDesignator">
		<rdfs:subClassOf rdf:resource="&cmns-cls;Classifier"/>
		<rdfs:subClassOf>
			<owl:Restriction>
				<owl:onProperty rdf:resource="&cmns-cls;classifies"/>
				<owl:someValuesFrom rdf:resource="&cmns-adr;SupplementalAddressComponent"/>
			</owl:Restriction>
		</rdfs:subClassOf>
		<rdfs:label>supplemental address designator</rdfs:label>
		<skos:definition>classifier for supplemental address information, such as a highway contract route, rural route, building complex, shopping center, condominium complex, mail box, or other similar designation</skos:definition>
	</owl:Class>
	
	<owl:Class rdf:about="&cmns-adr;SupplementalAddressUnit">
		<rdfs:subClassOf rdf:resource="&cmns-adr;AddressComponent"/>
		<rdfs:subClassOf>
			<owl:Restriction>
				<owl:onProperty rdf:resource="&cmns-txt;hasTextValue"/>
				<owl:onDataRange rdf:resource="&xsd;string"/>
				<owl:qualifiedCardinality rdf:datatype="&xsd;nonNegativeInteger">1</owl:qualifiedCardinality>
			</owl:Restriction>
		</rdfs:subClassOf>
		<rdfs:label>supplemental address unit</rdfs:label>
		<skos:definition>address component that includes a specific route, box, apartment, condominium or other indicator or unit associated with a specific address</skos:definition>
	</owl:Class>
	
	<owl:NamedIndividual rdf:about="&cmns-adr;Trailer">
		<rdf:type rdf:resource="&cmns-adr;SecondaryUnitDesignator"/>
		<rdfs:label xml:lang="en">trailer</rdfs:label>
		<skos:definition>vehicle designed to serve wherever parked as a temporary dwelling or place of business</skos:definition>
		<cmns-adr:requiresSecondaryUnitRange rdf:datatype="&xsd;boolean">true</cmns-adr:requiresSecondaryUnitRange>
	</owl:NamedIndividual>
	
	<owl:NamedIndividual rdf:about="&cmns-adr;Unit">
		<rdf:type rdf:resource="&cmns-adr;SecondaryUnitDesignator"/>
		<rdfs:label xml:lang="en">unit</rdfs:label>
		<skos:definition>area in a facility, such as a medical facility or hospital that is specially staffed and equipped to provide a particular service or type of care</skos:definition>
		<cmns-adr:requiresSecondaryUnitRange rdf:datatype="&xsd;boolean">true</cmns-adr:requiresSecondaryUnitRange>
	</owl:NamedIndividual>
	
	<owl:NamedIndividual rdf:about="&cmns-adr;Upper">
		<rdf:type rdf:resource="&cmns-adr;SecondaryUnitDesignator"/>
		<rdfs:label xml:lang="en">upper</rdfs:label>
		<skos:definition>floor of a building in a multistory structure that is farther away from the ground level</skos:definition>
		<cmns-adr:requiresSecondaryUnitRange rdf:datatype="&xsd;boolean">false</cmns-adr:requiresSecondaryUnitRange>
	</owl:NamedIndividual>
	
	<owl:Class rdf:about="&cmns-adr;VirtualAddress">
		<rdfs:subClassOf rdf:resource="&cmns-adr;Address"/>
		<rdfs:subClassOf rdf:resource="&cmns-cxtid;StructuredIdentifier"/>
		<rdfs:subClassOf>
			<owl:Restriction>
				<owl:onProperty rdf:resource="&cmns-txt;hasTextValue"/>
				<owl:onDataRange rdf:resource="&xsd;string"/>
				<owl:qualifiedCardinality rdf:datatype="&xsd;nonNegativeInteger">1</owl:qualifiedCardinality>
			</owl:Restriction>
		</rdfs:subClassOf>
		<rdfs:label>virtual address</rdfs:label>
		<owl:disjointWith rdf:resource="&cmns-adr;PhysicalAddress"/>
		<skos:definition>address identifying a virtual, i.e. non-physical, location</skos:definition>
	</owl:Class>
	
	<owl:ObjectProperty rdf:about="&cmns-adr;hasAddress">
		<rdfs:subPropertyOf rdf:resource="&cmns-cls;isCharacterizedBy"/>
		<rdfs:label>has address</rdfs:label>
		<rdfs:range rdf:resource="&cmns-adr;Address"/>
		<skos:definition>indicates a means by which something (in the case of a network address) or some entity may be located or contacted or may receive correspondence</skos:definition>
	</owl:ObjectProperty>
	
	<owl:ObjectProperty rdf:about="&cmns-adr;hasAddressAlias">
		<rdf:type rdf:resource="&owl;SymmetricProperty"/>
		<rdfs:subPropertyOf rdf:resource="&cmns-adr;hasAddress"/>
		<rdfs:label>has address alias</rdfs:label>
		<dct:source>ISO 19160-1:2015 Addressing - Part 1: Conceptual model, First edition, 2015-12-15, clause 4.3</dct:source>
		<rdfs:domain rdf:resource="&cmns-adr;Address"/>
		<rdfs:range rdf:resource="&cmns-adr;Address"/>
		<skos:definition>indicates one of a set of addresses unambiguously determining the same addressable object</skos:definition>
	</owl:ObjectProperty>
	
	<owl:DatatypeProperty rdf:about="&cmns-adr;hasAddressLine1">
		<rdfs:subPropertyOf rdf:resource="&cmns-txt;hasTextValue"/>
		<rdfs:label>has address line 1</rdfs:label>
		<rdfs:domain rdf:resource="&cmns-adr;PhysicalAddress"/>
		<skos:definition>the first line of the street address</skos:definition>
		<cmns-av:adaptedFrom rdf:datatype="&xsd;anyURI">https://www.gleif.org/en/about-lei/common-data-file-format/lei-cdf-format/lei-cdf-format-version-2-1</cmns-av:adaptedFrom>
	</owl:DatatypeProperty>
	
	<owl:DatatypeProperty rdf:about="&cmns-adr;hasAddressLine2">
		<rdfs:subPropertyOf rdf:resource="&cmns-txt;hasTextValue"/>
		<rdfs:label>has address line 2</rdfs:label>
		<rdfs:domain rdf:resource="&cmns-adr;PhysicalAddress"/>
		<skos:definition>the second line of the street address</skos:definition>
		<cmns-av:adaptedFrom rdf:datatype="&xsd;anyURI">https://www.gleif.org/en/about-lei/common-data-file-format/lei-cdf-format/lei-cdf-format-version-2-1</cmns-av:adaptedFrom>
	</owl:DatatypeProperty>
	
	<owl:DatatypeProperty rdf:about="&cmns-adr;hasAddressLine3">
		<rdfs:subPropertyOf rdf:resource="&cmns-txt;hasTextValue"/>
		<rdfs:label>has address line 3</rdfs:label>
		<rdfs:domain rdf:resource="&cmns-adr;PhysicalAddress"/>
		<skos:definition>the third line of the street address</skos:definition>
		<cmns-av:adaptedFrom rdf:datatype="&xsd;anyURI">https://www.gleif.org/en/about-lei/common-data-file-format/lei-cdf-format/lei-cdf-format-version-2-1</cmns-av:adaptedFrom>
		<cmns-av:usageNote>This element SHALL be omitted if address line 2 is omitted.</cmns-av:usageNote>
	</owl:DatatypeProperty>
	
	<owl:ObjectProperty rdf:about="&cmns-adr;hasAddressPreferenceLevel">
		<rdfs:subPropertyOf rdf:resource="&cmns-cls;isCharacterizedBy"/>
		<rdfs:label>has address preference level</rdfs:label>
		<rdfs:domain rdf:resource="&cmns-adr;Address"/>
		<skos:definition>indicates the ranking or preferred nature of the address in a set of address aliases</skos:definition>
		<cmns-av:adaptedFrom>ISO 19160-1:2015 Addressing - Part 1: Conceptual model, First edition, 2015-12-15, clause 6.3.2</cmns-av:adaptedFrom>
		<cmns-av:usageNote>The preference level could be a numeric ranking, as suggested in the ISO standard, or may reference a controlled vocabulary, thus the range of this property is left to the user.</cmns-av:usageNote>
	</owl:ObjectProperty>
	
	<owl:DatatypeProperty rdf:about="&cmns-adr;hasAttentionLine">
		<rdfs:subPropertyOf rdf:resource="&cmns-txt;hasTextValue"/>
		<rdfs:label>has attention line</rdfs:label>
		<rdfs:domain rdf:resource="&cmns-adr;PhysicalAddress"/>
		<skos:definition>an optional, free text address line denoting the intended recipient</skos:definition>
	</owl:DatatypeProperty>
	
	<owl:ObjectProperty rdf:about="&cmns-adr;hasIndividualPostcode">
		<rdfs:subPropertyOf rdf:resource="&cmns-col;comprises"/>
		<rdfs:label>has individual postcode</rdfs:label>
		<rdfs:domain rdf:resource="&cmns-adr;PhysicalAddress"/>
		<rdfs:range rdf:resource="&cmns-adr;Postcode"/>
		<skos:definition>indicates the local or international postcode element of a delivery address as specified by the local postal service</skos:definition>
		<cmns-av:adaptedFrom rdf:datatype="&xsd;anyURI">https://www.gleif.org/en/about-lei/common-data-file-format/lei-cdf-format/lei-cdf-format-version-2-1</cmns-av:adaptedFrom>
	</owl:ObjectProperty>
	
	<owl:DatatypeProperty rdf:about="&cmns-adr;hasMailRouting">
		<rdfs:subPropertyOf rdf:resource="&cmns-txt;hasTextValue"/>
		<rdfs:label>has mail routing</rdfs:label>
		<rdfs:domain rdf:resource="&cmns-adr;PhysicalAddress"/>
		<skos:definition>an optional, free text address line containing explicit routing information (this elements&apos;s presence indicates that this address is a routing / &apos;care of&apos; address)</skos:definition>
		<cmns-av:adaptedFrom rdf:datatype="&xsd;anyURI">https://www.gleif.org/en/about-lei/common-data-file-format/lei-cdf-format/lei-cdf-format-version-2-1</cmns-av:adaptedFrom>
	</owl:DatatypeProperty>
	
	<owl:DatatypeProperty rdf:about="&cmns-adr;hasPostalCode">
		<rdfs:subPropertyOf rdf:resource="&cmns-txt;hasTextValue"/>
		<rdfs:label>has postal code</rdfs:label>
		<rdfs:domain rdf:resource="&cmns-adr;PhysicalAddress"/>
		<skos:definition>the postal code of this address as specified by the local postal service</skos:definition>
		<cmns-av:adaptedFrom rdf:datatype="&xsd;anyURI">https://www.gleif.org/en/about-lei/common-data-file-format/lei-cdf-format/lei-cdf-format-version-2-1</cmns-av:adaptedFrom>
	</owl:DatatypeProperty>
	
	<owl:ObjectProperty rdf:about="&cmns-adr;hasPostdirectionalSymbol">
		<rdfs:subPropertyOf rdf:resource="&cmns-col;comprises"/>
		<rdfs:label>has postdirectional symbol</rdfs:label>
		<rdfs:domain rdf:resource="&cmns-adr;StreetAddress"/>
		<rdfs:range rdf:resource="&cmns-adr;PostdirectionalSymbol"/>
		<skos:definition>specifies a geographic directional symbol that follows the street name and street suffix in a street address</skos:definition>
	</owl:ObjectProperty>
	
	<owl:ObjectProperty rdf:about="&cmns-adr;hasPredirectionalSymbol">
		<rdfs:subPropertyOf rdf:resource="&cmns-col;comprises"/>
		<rdfs:label>has predirectional symbol</rdfs:label>
		<rdfs:domain rdf:resource="&cmns-adr;StreetAddress"/>
		<rdfs:range rdf:resource="&cmns-adr;PredirectionalSymbol"/>
		<skos:definition>specifies a geographic directional symbol that occurs after the primary street number but before the street name in a street address</skos:definition>
	</owl:ObjectProperty>
	
	<owl:ObjectProperty rdf:about="&cmns-adr;hasPrimaryAddressNumber">
		<rdfs:subPropertyOf rdf:resource="&cmns-col;comprises"/>
		<rdfs:label>has primary address number</rdfs:label>
		<rdfs:domain rdf:resource="&cmns-adr;StreetAddress"/>
		<rdfs:range rdf:resource="&cmns-adr;PrimaryAddressNumber"/>
		<skos:definition>specifies a a location with respect to a given street</skos:definition>
	</owl:ObjectProperty>
	
	<owl:ObjectProperty rdf:about="&cmns-adr;hasSecondaryUnit">
		<rdfs:subPropertyOf rdf:resource="&cmns-col;comprises"/>
		<rdfs:label>has secondary unit</rdfs:label>
		<rdfs:domain rdf:resource="&cmns-adr;StreetAddress"/>
		<rdfs:range rdf:resource="&cmns-adr;SecondaryUnit"/>
		<skos:definition>specifies an individual unit within a larger structure, such as an apartment, office, hangar, slip, mailbox, and so forth, at a given street address</skos:definition>
	</owl:ObjectProperty>
	
	<owl:ObjectProperty rdf:about="&cmns-adr;hasStreetAddress">
		<rdfs:subPropertyOf rdf:resource="&cmns-col;comprises"/>
		<rdfs:label>has street address</rdfs:label>
		<rdfs:domain rdf:resource="&cmns-adr;ConventionalStreetAddress"/>
		<rdfs:range rdf:resource="&cmns-adr;StreetAddress"/>
		<skos:definition>indicates a fully-specified address component that consists of a primary address number, predirectional, street name, suffix, postdirectional, and an optional secondary unit</skos:definition>
	</owl:ObjectProperty>
	
	<owl:ObjectProperty rdf:about="&cmns-adr;hasStreetName">
		<rdfs:subPropertyOf rdf:resource="&cmns-col;comprises"/>
		<rdfs:label>has street name</rdfs:label>
		<rdfs:domain rdf:resource="&cmns-adr;StreetAddress"/>
		<rdfs:range rdf:resource="&cmns-adr;StreetName"/>
		<skos:definition>specifies an identifier for a street in some context (e.g., &apos;Baker&apos;, &apos;First&apos;, &apos;Main&apos;)</skos:definition>
	</owl:ObjectProperty>
	
	<owl:ObjectProperty rdf:about="&cmns-adr;hasStreetSuffix">
		<rdfs:subPropertyOf rdf:resource="&cmns-col;comprises"/>
		<rdfs:label>has street suffix</rdfs:label>
		<rdfs:domain rdf:resource="&cmns-adr;StreetAddress"/>
		<rdfs:range rdf:resource="&cmns-adr;StreetSuffix"/>
		<skos:definition>specifies an additional qualifier for a street or other delivery location, such as a dwelling located along a waterway</skos:definition>
	</owl:ObjectProperty>
	
	<owl:ObjectProperty rdf:about="&cmns-adr;hasStructureName">
		<rdfs:subPropertyOf rdf:resource="&cmns-col;comprises"/>
		<rdfs:label>has structure name</rdfs:label>
		<rdfs:domain rdf:resource="&cmns-adr;PhysicalAddress"/>
		<rdfs:range rdf:resource="&cmns-adr;StructureName"/>
		<skos:definition>specifies an identifier for a building, house, office complex, shopping center, or other structure or group of structures</skos:definition>
	</owl:ObjectProperty>
	
	<owl:ObjectProperty rdf:about="&cmns-adr;hasTransliteratedAddress">
		<rdfs:subPropertyOf rdf:resource="&cmns-adr;hasAddress"/>
		<rdfs:label>has transliterated address</rdfs:label>
		<rdfs:range rdf:resource="&cmns-adr;Address"/>
		<skos:definition>identifies a transliterated (i.e., in Latin or Romanized ASCII) address for the registered entity</skos:definition>
		<cmns-av:adaptedFrom rdf:datatype="&xsd;anyURI">https://www.gleif.org/en/about-lei/common-data-file-format/lei-cdf-format/lei-cdf-format-version-2-1</cmns-av:adaptedFrom>
	</owl:ObjectProperty>
	
	<owl:DatatypeProperty rdf:about="&cmns-adr;requiresSecondaryUnitRange">
		<rdfs:subPropertyOf rdf:resource="&cmns-txt;hasTextValue"/>
		<rdfs:label>requires secondary unit range</rdfs:label>
		<rdfs:range rdf:resource="&xsd;boolean"/>
		<rdfs:seeAlso rdf:resource="https://pe.usps.com/cpim/ftp/pubs/Pub28/pub28.pdf"/>
		<skos:definition>if true, indicates that an additional qualifier is needed to complete the delivery point description, such as an apartment number</skos:definition>
		<cmns-av:explanatoryNote>Note that in some cases, such as for lobby or office, if there are multiple secondary units then a range may be needed to differentiate between them, even if the range is not always required.</cmns-av:explanatoryNote>
	</owl:DatatypeProperty>
	
	<owl:Class rdf:about="&cmns-loc;Location">
		<rdfs:subClassOf>
			<owl:Restriction>
				<owl:onProperty rdf:resource="&cmns-doc;isReferredToBy"/>
				<owl:onClass rdf:resource="&cmns-adr;Address"/>
				<owl:minQualifiedCardinality rdf:datatype="&xsd;nonNegativeInteger">0</owl:minQualifiedCardinality>
			</owl:Restriction>
		</rdfs:subClassOf>
	</owl:Class>
	
	<owl:Class rdf:about="&cmns-loc;PhysicalLocation">
		<rdfs:subClassOf>
			<owl:Restriction>
				<owl:onProperty rdf:resource="&cmns-doc;isReferredToBy"/>
				<owl:onClass rdf:resource="&cmns-adr;PhysicalAddress"/>
				<owl:minQualifiedCardinality rdf:datatype="&xsd;nonNegativeInteger">0</owl:minQualifiedCardinality>
			</owl:Restriction>
		</rdfs:subClassOf>
	</owl:Class>
	
	<owl:Class rdf:about="&cmns-loc;VirtualLocation">
		<rdfs:subClassOf>
			<owl:Restriction>
				<owl:onProperty rdf:resource="&cmns-doc;isReferredToBy"/>
				<owl:onClass rdf:resource="&cmns-adr;VirtualAddress"/>
				<owl:minQualifiedCardinality rdf:datatype="&xsd;nonNegativeInteger">0</owl:minQualifiedCardinality>
			</owl:Restriction>
		</rdfs:subClassOf>
	</owl:Class>

</rdf:RDF>