<?xml version="1.0" encoding="UTF-8"?>
<!DOCTYPE rdf:RDF [
	<!ENTITY cmns-av "https://www.omg.org/spec/Commons/AnnotationVocabulary/">
	<!ENTITY cmns-col "https://www.omg.org/spec/Commons/Collections/">
	<!ENTITY cmns-doc "https://www.omg.org/spec/Commons/Documents/">
	<!ENTITY cmns-dt "https://www.omg.org/spec/Commons/DatesAndTimes/">
	<!ENTITY dct "http://purl.org/dc/terms/">
	<!ENTITY owl "http://www.w3.org/2002/07/owl#">
	<!ENTITY rdf "http://www.w3.org/1999/02/22-rdf-syntax-ns#">
	<!ENTITY rdfs "http://www.w3.org/2000/01/rdf-schema#">
	<!ENTITY skos "http://www.w3.org/2004/02/skos/core#">
	<!ENTITY xsd "http://www.w3.org/2001/XMLSchema#">
]>
<rdf:RDF xml:base="https://www.omg.org/spec/Commons/Documents/"
	xmlns:cmns-av="https://www.omg.org/spec/Commons/AnnotationVocabulary/"
	xmlns:cmns-col="https://www.omg.org/spec/Commons/Collections/"
	xmlns:cmns-doc="https://www.omg.org/spec/Commons/Documents/"
	xmlns:cmns-dt="https://www.omg.org/spec/Commons/DatesAndTimes/"
	xmlns:dct="http://purl.org/dc/terms/"
	xmlns:owl="http://www.w3.org/2002/07/owl#"
	xmlns:rdf="http://www.w3.org/1999/02/22-rdf-syntax-ns#"
	xmlns:rdfs="http://www.w3.org/2000/01/rdf-schema#"
	xmlns:skos="http://www.w3.org/2004/02/skos/core#"
	xmlns:xsd="http://www.w3.org/2001/XMLSchema#">
	
	<owl:Ontology rdf:about="https://www.omg.org/spec/Commons/Documents/">
		<rdfs:label>Commons Documents Ontology</rdfs:label>
		<dct:abstract>This ontology defines high-level concepts for representation of documents, including legal documents and any kind of record, such as a transaction record, purchase history, and payment history.</dct:abstract>
		<dct:license rdf:datatype="&xsd;anyURI">http://opensource.org/licenses/MIT</dct:license>
		<owl:imports rdf:resource="https://www.omg.org/spec/Commons/AnnotationVocabulary/"/>
		<owl:imports rdf:resource="https://www.omg.org/spec/Commons/Collections/"/>
		<owl:imports rdf:resource="https://www.omg.org/spec/Commons/DatesAndTimes/"/>
		<owl:versionIRI rdf:resource="https://www.omg.org/spec/Commons/20220501/Documents/"/>
		<cmns-av:copyright>Copyright (c) 2014-2022 EDM Council, Inc.</cmns-av:copyright>
		<cmns-av:copyright>Copyright (c) 2014-2022 Object Management Group, Inc.</cmns-av:copyright>
	</owl:Ontology>
	
	<owl:Class rdf:about="&cmns-doc;Certificate">
		<rdfs:subClassOf rdf:resource="&cmns-doc;Document"/>
		<rdfs:label>certificate</rdfs:label>
		<skos:definition>document attesting to the truth of some fact or set of facts</skos:definition>
	</owl:Class>
	
	<owl:Class rdf:about="&cmns-doc;Document">
		<rdfs:subClassOf>
			<owl:Restriction>
				<owl:onProperty rdf:resource="&cmns-doc;isAbout"/>
				<owl:someValuesFrom rdf:resource="&owl;Thing"/>
			</owl:Restriction>
		</rdfs:subClassOf>
		<rdfs:label>document</rdfs:label>
		<skos:definition>something tangible that records something, such as a recording or a photograph, or a writing that can be used to furnish evidence or information</skos:definition>
		<skos:note>A document, especially a legal document, may serve to establish one or several facts, and can be relied upon as a proof thereof.</skos:note>
	</owl:Class>
	
	<owl:Class rdf:about="&cmns-doc;LegalDocument">
		<rdfs:subClassOf rdf:resource="&cmns-doc;Document"/>
		<rdfs:label>legal document</rdfs:label>
		<skos:definition>document that bears the original, official, or legal form of something, that can be fully attributed to its author, that records and formally expresses a legally enforceable act, process, or contractual duty, obligation, or right and that can be used to furnish decisive evidence for that act, process, or agreement</skos:definition>
		<skos:example>Examples include some certificates, deeds, bonds, business documents (such as articles of incorporation, bylaws, partnership agreements), contracts, certain identity documents, wills, trusts, legislative acts, notarial acts, court writs or processes (such as related complaints and pleadings in the context of litigation as well as other documents relevant to some legal issue), and any law passed by a competent legislative body in municipal (domestic) or international law.</skos:example>
		<skos:note>In order for a document to be legal, it must conform to the laws of the jurisdiction where it will be enforced. Typically, such a document should also be properly signed, witnessed and filed to be considered legal.</skos:note>
	</owl:Class>
	
	<owl:Class rdf:about="&cmns-doc;Notice">
		<rdfs:subClassOf rdf:resource="&cmns-doc;Document"/>
		<rdfs:label>notice</rdfs:label>
		<skos:definition>announcement, intimation, or advance warning of something, especially to allow preparations to be made</skos:definition>
		<skos:note>Although many notices are delivered electronically, certain legal notices must be given given in writing, often by regular mail or hand delivery, with the sender retaining sufficient proof of having given such notice (e.g., through a certificate of service).</skos:note>
	</owl:Class>
	
	<owl:Class rdf:about="&cmns-doc;Record">
		<rdfs:subClassOf rdf:resource="&cmns-col;Collection"/>
		<rdfs:label>record</rdfs:label>
		<skos:definition>memorialization and objective evidence of activities performed, events occurred, results achieved, or statements made, regardless of its characteristics, media, physical form, or the manner in which it is recorded or stored</skos:definition>
		<skos:example>Records include accounts, agreements, books, drawings, letters, magnetic/optical disks, memos, micrographics, etc.</skos:example>
		<skos:note>Records are created or received by an organization in routine transaction of its business or in pursuance of its legal obligations.</skos:note>
	</owl:Class>
	
	<owl:Class rdf:about="&cmns-doc;ReferenceDocument">
		<rdfs:subClassOf rdf:resource="&cmns-doc;Document"/>
		<rdfs:label>reference document</rdfs:label>
		<dct:source>ISO/IEC 11179-3 Information technology - Metadata registries (MDR) - Part 3: Registry metamodel and basic attributes, Third edition, 2013-02-15</dct:source>
		<skos:definition>document that provides pertinent details for consultation about a subject</skos:definition>
	</owl:Class>
	
	<owl:ObjectProperty rdf:about="&cmns-doc;hasDataSource">
		<rdfs:subPropertyOf rdf:resource="&cmns-doc;refersTo"/>
		<rdfs:label>has data source</rdfs:label>
		<skos:definition>relates something, such as an agreement, contract, document, record, report, or process, to a source of data used to analyze, develop, explain, produce, or otherwise create it</skos:definition>
		<skos:note>Although in many cases an annotation property, such as dct:source, is sufficient for this purpose, there are occasions when a more complete description of a source is required, for which this property may be used.</skos:note>
	</owl:ObjectProperty>
	
	<owl:ObjectProperty rdf:about="&cmns-doc;hasDateOfIssuance">
		<rdf:type rdf:resource="&owl;FunctionalProperty"/>
		<rdfs:subPropertyOf rdf:resource="&cmns-dt;hasStartDate"/>
		<rdfs:label>has date of issuance</rdfs:label>
		<rdfs:range rdf:resource="&cmns-dt;Date"/>
		<skos:definition>links something, typically an agreement, contract, or report, with the date it was produced or published</skos:definition>
	</owl:ObjectProperty>
	
	<owl:ObjectProperty rdf:about="&cmns-doc;hasExpirationDate">
		<rdfs:subPropertyOf rdf:resource="&cmns-dt;hasEndDate"/>
		<rdfs:label>has expiration date</rdfs:label>
		<rdfs:range rdf:resource="&cmns-dt;Date"/>
		<skos:definition>links something, such as an agreement, contract, report, other document, or perishable item, with a date beyond which it is no longer valid</skos:definition>
	</owl:ObjectProperty>
	
	<owl:ObjectProperty rdf:about="&cmns-doc;hasRecord">
		<rdfs:subPropertyOf rdf:resource="&cmns-col;comprises"/>
		<rdfs:label>has record</rdfs:label>
		<rdfs:range rdf:resource="&cmns-doc;Record"/>
		<skos:definition>links something to a record that pertains to it</skos:definition>
	</owl:ObjectProperty>
	
	<owl:ObjectProperty rdf:about="&cmns-doc;hasReportingPeriod">
		<rdfs:subPropertyOf rdf:resource="&cmns-dt;hasDatePeriod"/>
		<rdfs:label>has reporting period</rdfs:label>
		<rdfs:range rdf:resource="&cmns-dt;ExplicitDatePeriod"/>
		<skos:definition>specifies the period for which a report, document, statistical measure or something else, applies</skos:definition>
	</owl:ObjectProperty>
	
	<owl:ObjectProperty rdf:about="&cmns-doc;hasTerminationDate">
		<rdfs:subPropertyOf rdf:resource="&cmns-dt;hasEndDate"/>
		<rdfs:label>has termination date</rdfs:label>
		<rdfs:range rdf:resource="&cmns-dt;Date"/>
		<skos:definition>links something, typically an agreement, contract, document, or process, with a date on which it was or will be terminated</skos:definition>
	</owl:ObjectProperty>
	
	<owl:ObjectProperty rdf:about="&cmns-doc;isAbout">
		<rdfs:label>is about</rdfs:label>
		<skos:definition>indicates the subject or topic of something, such as a document</skos:definition>
	</owl:ObjectProperty>
	
	<owl:ObjectProperty rdf:about="&cmns-doc;records">
		<rdfs:label>records</rdfs:label>
		<skos:definition>documents for later reference</skos:definition>
	</owl:ObjectProperty>
	
	<owl:ObjectProperty rdf:about="&cmns-doc;refersTo">
		<rdfs:label>refers to</rdfs:label>
		<skos:definition>makes reference to as a source for information or explanation</skos:definition>
	</owl:ObjectProperty>

</rdf:RDF>