<?xml version="1.0" encoding="UTF-8"?>
<!DOCTYPE rdf:RDF [
	<!ENTITY cmns-av "https://www.omg.org/spec/Commons/AnnotationVocabulary/">
	<!ENTITY cmns-cds "https://www.omg.org/spec/Commons/CodesAndCodeSets/">
	<!ENTITY cmns-cls "https://www.omg.org/spec/Commons/Classifiers/">
	<!ENTITY cmns-col "https://www.omg.org/spec/Commons/Collections/">
	<!ENTITY cmns-dsg "https://www.omg.org/spec/Commons/Designators/">
	<!ENTITY cmns-id "https://www.omg.org/spec/Commons/Identifiers/">
	<!ENTITY cmns-loc "https://www.omg.org/spec/Commons/Locations/">
	<!ENTITY cmns-qtu "https://www.omg.org/spec/Commons/QuantitiesAndUnits/">
	<!ENTITY cmns-txt "https://www.omg.org/spec/Commons/TextDatatype/">
	<!ENTITY dct "http://purl.org/dc/terms/">
	<!ENTITY owl "http://www.w3.org/2002/07/owl#">
	<!ENTITY rdf "http://www.w3.org/1999/02/22-rdf-syntax-ns#">
	<!ENTITY rdfs "http://www.w3.org/2000/01/rdf-schema#">
	<!ENTITY skos "http://www.w3.org/2004/02/skos/core#">
	<!ENTITY xsd "http://www.w3.org/2001/XMLSchema#">
]>
<rdf:RDF xml:base="https://www.omg.org/spec/Commons/Locations/"
	xmlns:cmns-av="https://www.omg.org/spec/Commons/AnnotationVocabulary/"
	xmlns:cmns-cds="https://www.omg.org/spec/Commons/CodesAndCodeSets/"
	xmlns:cmns-cls="https://www.omg.org/spec/Commons/Classifiers/"
	xmlns:cmns-col="https://www.omg.org/spec/Commons/Collections/"
	xmlns:cmns-dsg="https://www.omg.org/spec/Commons/Designators/"
	xmlns:cmns-id="https://www.omg.org/spec/Commons/Identifiers/"
	xmlns:cmns-loc="https://www.omg.org/spec/Commons/Locations/"
	xmlns:cmns-qtu="https://www.omg.org/spec/Commons/QuantitiesAndUnits/"
	xmlns:cmns-txt="https://www.omg.org/spec/Commons/TextDatatype/"
	xmlns:dct="http://purl.org/dc/terms/"
	xmlns:owl="http://www.w3.org/2002/07/owl#"
	xmlns:rdf="http://www.w3.org/1999/02/22-rdf-syntax-ns#"
	xmlns:rdfs="http://www.w3.org/2000/01/rdf-schema#"
	xmlns:skos="http://www.w3.org/2004/02/skos/core#"
	xmlns:xsd="http://www.w3.org/2001/XMLSchema#">
	
	<owl:Ontology rdf:about="https://www.omg.org/spec/Commons/Locations/">
		<rdfs:label>Commons Locations Ontology</rdfs:label>
		<dct:abstract>This ontology provides a very high level definition of geographic region and geopolitical entity related concepts, including, but not limited to, countries, sub-country regions such as states and provinces, and municipalities. The representation was derived from a combination of ISO 3166, the UN M49 Region codes, Geonames, the SWIFT registry, the UN FAO and CIA World Factbook, and other sources. It aims to provide a systematic description of the vocabulary used for country and geopolitical entity representation, useful for mapping among the various names and codes for countries and their subdivisions used world-wide, including but not limited to FIPA and International Olympics codes for countries, (based strictly on requirements for business applications, not broader geographic or political uses).The terms defined herein terms are reused by the OMG&apos;s LCC controlled vocabulary representing ISO 3166 country and country subdivision codes, and may be mapped to other standards and de facto standards such as those mentioned.</dct:abstract>
		<dct:contributor>Elisa Kendall, Thematix Partners LLC</dct:contributor>
		<dct:contributor>Evan Wallace, U.S. National Institute of Standards and Technology (NIST)</dct:contributor>
		<dct:contributor>Pete Rivett, Federated Knowledge, LLC</dct:contributor>
		<dct:contributor>Roy Bell, Thematix Partners LLC</dct:contributor>
		<dct:license>Copyright (c) 2015-2024 Adaptive, Inc.
		Copyright (c) 2015-2024 EDM Council, Inc.
		Copyright (c) 2015-2024 Object Management Group, Inc.
		Copyright (c) 2015-2024 Thematix Partners LLC
		Copyright (c) 2015-2017 Unisys
		Copyright (c) 2019-2024 agnos.ai UK Ltd.
		Copyright (c) 2021-2024 Federated Knowledge, LLC	
		
		Permission is hereby granted, free of charge, to any person obtaining a copy of this software and associated documentation files (the &apos;Software&apos;), to deal in the Software without restriction, including without limitation the rights to use, copy, modify, merge, publish, distribute, sublicense, and/or sell copies of the Software, and to permit persons to whom the Software is furnished to do so, subject to the following conditions:

The above copyright notice and this permission notice shall be included in all copies or substantial portions of the Software.

THE SOFTWARE IS PROVIDED &apos;AS IS&apos;, WITHOUT WARRANTY OF ANY KIND, EXPRESS OR IMPLIED, INCLUDING BUT NOT LIMITED TO THE WARRANTIES OF MERCHANTABILITY, FITNESS FOR A PARTICULAR PURPOSE AND NONINFRINGEMENT. IN NO EVENT SHALL THE AUTHORS OR COPYRIGHT HOLDERS BE LIABLE FOR ANY CLAIM, DAMAGES OR OTHER LIABILITY, WHETHER IN AN ACTION OF CONTRACT, TORT OR OTHERWISE, ARISING FROM, OUT OF OR IN CONNECTION WITH THE SOFTWARE OR THE USE OR OTHER DEALINGS IN THE SOFTWARE.
		
		See https://opensource.org/licenses/MIT.</dct:license>
		<owl:imports rdf:resource="https://www.omg.org/spec/Commons/AnnotationVocabulary/"/>
		<owl:imports rdf:resource="https://www.omg.org/spec/Commons/Classifiers/"/>
		<owl:imports rdf:resource="https://www.omg.org/spec/Commons/CodesAndCodeSets/"/>
		<owl:imports rdf:resource="https://www.omg.org/spec/Commons/Collections/"/>
		<owl:imports rdf:resource="https://www.omg.org/spec/Commons/Designators/"/>
		<owl:imports rdf:resource="https://www.omg.org/spec/Commons/Identifiers/"/>
		<owl:imports rdf:resource="https://www.omg.org/spec/Commons/QuantitiesAndUnits/"/>
		<owl:imports rdf:resource="https://www.omg.org/spec/Commons/TextDatatype/"/>
		<owl:versionIRI rdf:resource="https://www.omg.org/spec/Commons/20240801/Locations/"/>
		<skos:note>This ontology is largely derived from the Object Management Group&apos;s Languages, Countries and Codes (LCC) standard (to provide a more general ontology on which LCC can depend) and the Financial Industry Business Ontology (FIBO) Locations and Virtual Locations ontologies.</skos:note>
		<cmns-av:copyright>Copyright (c) 2015-2017 Unisys</cmns-av:copyright>
		<cmns-av:copyright>Copyright (c) 2015-2024 Adaptive, Inc.</cmns-av:copyright>
		<cmns-av:copyright>Copyright (c) 2015-2024 EDM Council, Inc.</cmns-av:copyright>
		<cmns-av:copyright>Copyright (c) 2015-2024 Object Management Group, Inc.</cmns-av:copyright>
		<cmns-av:copyright>Copyright (c) 2015-2024 Thematix Partners LLC</cmns-av:copyright>
		<cmns-av:copyright>Copyright (c) 2019-2024 agnos.ai UK Ltd.</cmns-av:copyright>
		<cmns-av:copyright>Copyright (c) 2021-2024 Federated Knowledge, LLC</cmns-av:copyright>
	</owl:Ontology>
	
	<owl:Class rdf:about="&cmns-loc;BusinessCenter">
		<rdfs:subClassOf rdf:resource="&cmns-loc;Municipality"/>
		<rdfs:label>business center</rdfs:label>
		<skos:definition>municipality where business is conducted, especially one that is considered a financial center</skos:definition>
		<cmns-av:adaptedFrom>FpML Business Center and related codes, see http://www.fpml.org/coding-scheme/business-center-7-14.xml</cmns-av:adaptedFrom>
	</owl:Class>
	
	<owl:Class rdf:about="&cmns-loc;Country">
		<rdfs:subClassOf rdf:resource="&cmns-loc;GeopoliticalEntity"/>
		<rdfs:subClassOf>
			<owl:Restriction>
				<owl:onProperty rdf:resource="&cmns-loc;isIndependent"/>
				<owl:onDataRange rdf:resource="&xsd;boolean"/>
				<owl:qualifiedCardinality rdf:datatype="&xsd;nonNegativeInteger">1</owl:qualifiedCardinality>
			</owl:Restriction>
		</rdfs:subClassOf>
		<rdfs:label>country</rdfs:label>
		<rdfs:seeAlso rdf:resource="https://datahelpdesk.worldbank.org/knowledgebase/articles/906519"/>
		<rdfs:seeAlso rdf:resource="https://www.un.org/development/desa/dpad/wp-content/uploads/sites/45/2017wesp_annex_en.pdf"/>
		<skos:definition>geopolitical entity representing a distinct territorial body or political entity or dependent territory</skos:definition>
		<cmns-av:explanatoryNote>It may be an independent sovereign state or part of a larger state, as a non-sovereign or formerly sovereign political division, a physical territory with a government, or a geographic region associated with sets of previously independent or differently associated peoples with distinct political characteristics.</cmns-av:explanatoryNote>
	</owl:Class>
	
	<owl:Class rdf:about="&cmns-loc;CountrySubdivision">
		<rdfs:subClassOf rdf:resource="&cmns-loc;GeopoliticalEntity"/>
		<rdfs:subClassOf>
			<owl:Restriction>
				<owl:onProperty rdf:resource="&cmns-cls;isClassifiedBy"/>
				<owl:someValuesFrom rdf:resource="&cmns-loc;GeographicRegionKind"/>
			</owl:Restriction>
		</rdfs:subClassOf>
		<rdfs:label>country subdivision</rdfs:label>
		<rdfs:seeAlso rdf:resource="https://www.census.gov/programs-surveys/popest/guidance-geographies/terms-and-definitions.html"/>
		<skos:definition>geopolitical entity that is a legal division of a country, dependency, or other area of special geopolitical interest related to a country or other geopolitical entity</skos:definition>
		<cmns-av:explanatoryNote>In the US, the US Census Bureau and other federal agencies may group some number of other subdivisions for statistical analysis and reporting purposes, ranging from multiple states to minor civil divisions.</cmns-av:explanatoryNote>
	</owl:Class>
	
	<owl:Class rdf:about="&cmns-loc;County">
		<rdfs:subClassOf rdf:resource="&cmns-loc;CountrySubdivision"/>
		<rdfs:label>county</rdfs:label>
		<skos:definition>political and administrative division of a country, state or province, providing certain local governmental services</skos:definition>
	</owl:Class>
	
	<owl:Class rdf:about="&cmns-loc;FederalCapitalArea">
		<rdfs:subClassOf rdf:resource="&cmns-loc;CountrySubdivision"/>
		<rdfs:label>federal capital area</rdfs:label>
		<skos:definition>country subdivision that is or includes the municipality or capital city that acts as the seat of the federal government</skos:definition>
		<skos:example>Examples include the District of Columbia in the US, and the Canberra area in Australia.</skos:example>
		<cmns-av:explanatoryNote>The capital administrative region of some federations includes those for which the capital is situated other than within one of the states or provinces which make up the country as a whole.</cmns-av:explanatoryNote>
	</owl:Class>
	
	<owl:Class rdf:about="&cmns-loc;FederalState">
		<rdfs:subClassOf rdf:resource="&cmns-loc;CountrySubdivision"/>
		<rdfs:label>federal state</rdfs:label>
		<skos:definition>self-governing geopolitical unit which forms part of a wider geopolitical unit that is recognized as a country</skos:definition>
		<cmns-av:explanatoryNote>This type of entity, variously referred to as a state, province or canton, has a level of self government including its own legal system and court jurisdiction, but cedes a level of autonomy to the federation of which it forms a part.</cmns-av:explanatoryNote>
		<cmns-av:synonym>canton</cmns-av:synonym>
		<cmns-av:synonym>province</cmns-av:synonym>
		<cmns-av:synonym>state</cmns-av:synonym>
	</owl:Class>
	
	<owl:Class rdf:about="&cmns-loc;GeodeticCoordinateSystem">
		<rdfs:subClassOf rdf:resource="&cmns-col;Arrangement"/>
		<rdfs:label>geodetic coordinate system</rdfs:label>
		<dct:source rdf:resource="http://edndoc.esri.com/arcsde/9.1/general_topics/what_coord_sys.htm"/>
		<dct:source rdf:resource="https://pubs.usgs.gov/circ/1983/0878b/report.pdf"/>
		<skos:definition>three-dimensional reference system that is a global frame of reference for precisely representing the position of locations on Earth or other planetary bodies by means of geodetic coordinates</skos:definition>
		<skos:example>The three most widely used systems for indicating point locations in the United States are (1) latitude and longitude [and optionally elevation], (2) Universal Transverse Mercator (UTM) system, and (3) State Plane Coordinate Systems (SPCS).</skos:example>
		<skos:note>The unit of measure is usually decimal degrees. A point has two coordinate values, latitude and longitude. Latitude and longitude measure angles.</skos:note>
		<cmns-av:explanatoryNote>Geodetic coordinates are crucial to any technology or technique based on spatial location, including geodesy, navigation, surveying, geographic information systems, remote sensing, and cartography.</cmns-av:explanatoryNote>
	</owl:Class>
	
	<owl:Class rdf:about="&cmns-loc;GeographicRegion">
		<rdfs:subClassOf rdf:resource="&cmns-loc;Region"/>
		<rdfs:subClassOf>
			<owl:Restriction>
				<owl:onProperty rdf:resource="&cmns-dsg;hasTextualName"/>
				<owl:minCardinality rdf:datatype="&xsd;nonNegativeInteger">0</owl:minCardinality>
			</owl:Restriction>
		</rdfs:subClassOf>
		<rdfs:subClassOf>
			<owl:Restriction>
				<owl:onProperty rdf:resource="&cmns-dsg;hasName"/>
				<owl:onClass rdf:resource="&cmns-dsg;Name"/>
				<owl:minQualifiedCardinality rdf:datatype="&xsd;nonNegativeInteger">0</owl:minQualifiedCardinality>
			</owl:Restriction>
		</rdfs:subClassOf>
		<rdfs:label>geographic region</rdfs:label>
		<dct:source rdf:resource="https://www.nationalgeographic.org/encyclopedia/region/"/>
		<skos:definition>area of land that has common features</skos:definition>
		<cmns-av:explanatoryNote>A region may be defined by natural or artificial features, and may be described as part of a country or the world having definable characteristics but not always fixed boundaries.</cmns-av:explanatoryNote>
		<cmns-av:usageNote>Many cases in which a geographic region, or subclass thereof, is mapped to certain applications or a relational store, or where codes are used to identify the region, require a class to represent the name of the region. In such situations, attributes of the name, such as the dates when a particular name was in use, or was valid under certain circumstances, may be important. For other applications, such as for addressing, a text value may be required. Thus, both options are provided here, with a preference for use of the full class option, depending on the use case.</cmns-av:usageNote>
	</owl:Class>
	
	<owl:Class rdf:about="&cmns-loc;GeographicRegionIdentificationScheme">
		<rdfs:subClassOf rdf:resource="&cmns-id;IdentificationScheme"/>
		<rdfs:label>geographic region identification scheme</rdfs:label>
		<skos:definition>identification scheme dedicated to the unique identification of geographic regions</skos:definition>
	</owl:Class>
	
	<owl:Class rdf:about="&cmns-loc;GeographicRegionIdentifier">
		<rdfs:subClassOf rdf:resource="&cmns-cds;CodeElement"/>
		<rdfs:subClassOf rdf:resource="&cmns-id;Identifier"/>
		<rdfs:subClassOf>
			<owl:Restriction>
				<owl:onProperty rdf:resource="&cmns-col;isMemberOf"/>
				<owl:onClass rdf:resource="&cmns-loc;GeographicRegionIdentificationScheme"/>
				<owl:qualifiedCardinality rdf:datatype="&xsd;nonNegativeInteger">1</owl:qualifiedCardinality>
			</owl:Restriction>
		</rdfs:subClassOf>
		<rdfs:subClassOf>
			<owl:Restriction>
				<owl:onProperty rdf:resource="&cmns-id;identifies"/>
				<owl:someValuesFrom rdf:resource="&cmns-loc;GeographicRegion"/>
			</owl:Restriction>
		</rdfs:subClassOf>
		<rdfs:subClassOf>
			<owl:Restriction>
				<owl:onProperty rdf:resource="&cmns-txt;hasTextValue"/>
				<owl:someValuesFrom rdf:resource="&xsd;string"/>
			</owl:Restriction>
		</rdfs:subClassOf>
		<rdfs:label>geographic region identifier</rdfs:label>
		<skos:definition>string of letters that indicates a code or other identifier for geographical region, assigned for the purpose of uniquely identifying it within some context</skos:definition>
	</owl:Class>
	
	<owl:Class rdf:about="&cmns-loc;GeographicRegionKind">
		<rdfs:subClassOf rdf:resource="&cmns-cls;Classifier"/>
		<rdfs:subClassOf>
			<owl:Restriction>
				<owl:onProperty rdf:resource="&cmns-cls;classifies"/>
				<owl:allValuesFrom rdf:resource="&cmns-loc;GeographicRegion"/>
			</owl:Restriction>
		</rdfs:subClassOf>
		<rdfs:label>geographic region kind</rdfs:label>
		<skos:definition>classifier for a geographic region, including but not limited to a subdivision of a geopolitical entity, (noting that there may be more than one kind for a given country or other entity)</skos:definition>
	</owl:Class>
	
	<owl:Class rdf:about="&cmns-loc;GeopoliticalEntity">
		<rdfs:subClassOf rdf:resource="&cmns-loc;GeographicRegion"/>
		<rdfs:label>geopolitical entity</rdfs:label>
		<skos:definition>geographic area that represents a geophysical location associated with some form of political structure</skos:definition>
		<skos:example>A geopolitical entity may be any country, federal province, city or other administrative unit that represents a geophysical location</skos:example>
	</owl:Class>
	
	<owl:Class rdf:about="&cmns-loc;Location">
		<rdfs:label>location</rdfs:label>
		<skos:definition>place or position in time and/or space, including a virtual place</skos:definition>
	</owl:Class>
	
	<owl:Class rdf:about="&cmns-loc;Municipality">
		<rdfs:subClassOf rdf:resource="&cmns-loc;CountrySubdivision"/>
		<rdfs:label>municipality</rdfs:label>
		<skos:definition>urban administrative division having corporate status and usually powers of self-government or jurisdiction</skos:definition>
		<skos:example>A municipality can be any political jurisdiction from a sovereign state, such as the Principality of Monaco, or a small village, such as West Hampton Dunes, New York.</skos:example>
		<skos:scopeNote>The territory over which a municipality has jurisdiction may encompass:
- only one populated place such as a city, town, or village
- several of such places (e.g., early jurisdictions in the state of New Jersey (1798-1899) as townships governing several villages, Municipalities of Mexico)
- only parts of such places, sometimes boroughs of a city such as the 34 municipalities of Santiago, Chile.</skos:scopeNote>
		<cmns-av:explanatoryNote>A municipality is a general-purpose administrative subdivision, as opposed to a special-purpose district.</cmns-av:explanatoryNote>
	</owl:Class>
	
	<owl:Class rdf:about="&cmns-loc;PhysicalLocation">
		<rdfs:subClassOf rdf:resource="&cmns-loc;Location"/>
		<rdfs:label>physical location</rdfs:label>
		<skos:definition>location in physical space</skos:definition>
	</owl:Class>
	
	<owl:Class rdf:about="&cmns-loc;Region">
		<rdfs:label>region</rdfs:label>
		<skos:definition>area that is a continuous part of a surface, space, or body</skos:definition>
	</owl:Class>
	
	<owl:Class rdf:about="&cmns-loc;Territory">
		<rdfs:subClassOf rdf:resource="&cmns-loc;GeographicRegion"/>
		<rdfs:label>territory</rdfs:label>
		<skos:definition>geographic area, typically considered an area of special geopolitical interest, subject to the sovereignty, control, or jurisdiction of a state or other entity</skos:definition>
		<skos:note>Certain territories are included in the ISO 3166-2 code set without an alpha 2 or alpha 3 code. In these cases, the numeric code for the subregion may have more than 3 characters in their corresponding numeric region codes.</skos:note>
	</owl:Class>
	
	<owl:Class rdf:about="&cmns-loc;VirtualLocation">
		<rdfs:subClassOf rdf:resource="&cmns-loc;Location"/>
		<rdfs:label>virtual location</rdfs:label>
		<owl:disjointWith rdf:resource="&cmns-loc;PhysicalLocation"/>
		<skos:definition>place that does not exist in any single physical location</skos:definition>
		<skos:example>a network-based location without geographic boundaries</skos:example>
	</owl:Class>
	
	<owl:ObjectProperty rdf:about="&cmns-loc;hasBusinessCenter">
		<rdfs:subPropertyOf rdf:resource="&cmns-loc;hasMunicipality"/>
		<rdfs:label>has business center</rdfs:label>
		<rdfs:range rdf:resource="&cmns-loc;BusinessCenter"/>
		<skos:definition>identifies a location where business is conducted, and hence the business calendar used to adjust dates</skos:definition>
	</owl:ObjectProperty>
	
	<owl:DatatypeProperty rdf:about="&cmns-loc;hasCityName">
		<rdfs:subPropertyOf rdf:resource="&cmns-dsg;hasTextualName"/>
		<rdfs:label>has city name</rdfs:label>
		<skos:definition>indicates the name of a typically large, permanent, and densely settled place</skos:definition>
		<cmns-av:adaptedFrom rdf:datatype="&xsd;anyURI">https://en.wikipedia.org/wiki/City</cmns-av:adaptedFrom>
		<cmns-av:adaptedFrom rdf:datatype="&xsd;anyURI">https://www.gleif.org/en/about-lei/common-data-file-format/current-versions/level-1-data-lei-cdf-3-1-format</cmns-av:adaptedFrom>
		<cmns-av:explanatoryNote>Typical working definitions for small-city populations start at around 100,000 people. Common population definitions for an urban area (city or town) range between 1,500 and 50,000 people, with most U.S states using a minimum between 1,500 and 5,000 inhabitants. Some jurisdictions set no such minima.</cmns-av:explanatoryNote>
		<cmns-av:usageNote>This property should be used in cases where a formal individual for the business center or municipality is not available. Note that Geonames could be used as a source in cases where an individual is desired. Use the property cmns-loc;hasMunicipality in cases where an individual is available. Also note that with respect to an address, this property may stand in for any village, town, or city of any size.</cmns-av:usageNote>
	</owl:DatatypeProperty>
	
	<owl:ObjectProperty rdf:about="&cmns-loc;hasCountry">
		<rdfs:subPropertyOf rdf:resource="&cmns-loc;hasRegion"/>
		<rdfs:label>has country</rdfs:label>
		<rdfs:range rdf:resource="&cmns-loc;Country"/>
		<skos:definition>indicates a country, such as one that is recognized by the United Nations</skos:definition>
		<cmns-av:adaptedFrom rdf:datatype="&xsd;anyURI">https://www.gleif.org/en/about-lei/common-data-file-format/current-versions/level-1-data-lei-cdf-3-1-format</cmns-av:adaptedFrom>
	</owl:ObjectProperty>
	
	<owl:ObjectProperty rdf:about="&cmns-loc;hasCounty">
		<rdfs:subPropertyOf rdf:resource="&cmns-loc;hasSubdivision"/>
		<rdfs:label>has county</rdfs:label>
		<rdfs:range rdf:resource="&cmns-loc;County"/>
		<skos:definition>indicates a country subdivision providing certain local governmental services</skos:definition>
	</owl:ObjectProperty>
	
	<owl:ObjectProperty rdf:about="&cmns-loc;hasCoverageArea">
		<rdfs:subPropertyOf rdf:resource="&cmns-loc;hasRegion"/>
		<rdfs:label>has coverage area</rdfs:label>
		<rdfs:range rdf:resource="&cmns-loc;GeographicRegion"/>
		<skos:definition>indicates a geographic region in which some service is provided, or to which some policy applies, or in which something is available</skos:definition>
	</owl:ObjectProperty>
	
	<owl:DatatypeProperty rdf:about="&cmns-loc;hasLatitude">
		<rdfs:subPropertyOf rdf:resource="&cmns-qtu;hasNumericValue"/>
		<rdfs:label>has latitude</rdfs:label>
		<dct:source rdf:resource="http://edndoc.esri.com/arcsde/9.1/general_topics/what_coord_sys.htm"/>
		<rdfs:range>
			<rdfs:Datatype>
				<owl:onDatatype rdf:resource="&xsd;decimal"/>
				<owl:withRestrictions rdf:parseType="Collection">
					<rdf:Description>
						<xsd:maxInclusive rdf:datatype="&xsd;decimal">90</xsd:maxInclusive>
					</rdf:Description>
					<rdf:Description>
						<xsd:minInclusive rdf:datatype="&xsd;decimal">-90</xsd:minInclusive>
					</rdf:Description>
				</owl:withRestrictions>
			</rdfs:Datatype>
		</rdfs:range>
		<skos:definition>the angle formed by the intersection of a line perpendicular to the Earth&apos;s (or other celestial body&apos;s) surface at a point and the plane of the Equator</skos:definition>
		<skos:note>Points north of the Equator have positive latitude values, while points south have negative values. Latitude values range from minus 90 to plus 90 degrees. Lines of latitude are also called parallels because a particular value of latitude forms a circle parallel to the Equator.</skos:note>
	</owl:DatatypeProperty>
	
	<owl:ObjectProperty rdf:about="&cmns-loc;hasLocation">
		<rdfs:label>has location</rdfs:label>
		<rdfs:range rdf:resource="&cmns-loc;Location"/>
		<skos:definition>relates something to a location, which might be physical or virtual</skos:definition>
	</owl:ObjectProperty>
	
	<owl:DatatypeProperty rdf:about="&cmns-loc;hasLongitude">
		<rdfs:subPropertyOf rdf:resource="&cmns-qtu;hasNumericValue"/>
		<rdfs:label>has longitude</rdfs:label>
		<dct:source rdf:resource="http://edndoc.esri.com/arcsde/9.1/general_topics/what_coord_sys.htm"/>
		<rdfs:range>
			<rdfs:Datatype>
				<owl:onDatatype rdf:resource="&xsd;decimal"/>
				<owl:withRestrictions rdf:parseType="Collection">
					<rdf:Description>
						<xsd:maxInclusive rdf:datatype="&xsd;decimal">180</xsd:maxInclusive>
					</rdf:Description>
					<rdf:Description>
						<xsd:minInclusive rdf:datatype="&xsd;decimal">-180</xsd:minInclusive>
					</rdf:Description>
				</owl:withRestrictions>
			</rdfs:Datatype>
		</rdfs:range>
		<skos:definition>the angle between a plane that passes through the point and the North and South poles, and a reference plane</skos:definition>
		<skos:note>The reference plane is known as the prime meridian. The most common prime meridian passes through Greenwich, United Kingdom. Other examples of prime meridians in use pass through Paris and Bogota. Longitude values range from minus 180 to plus 180 degrees.</skos:note>
	</owl:DatatypeProperty>
	
	<owl:DatatypeProperty rdf:about="&cmns-loc;hasMaximumLatitude">
		<rdfs:subPropertyOf rdf:resource="&cmns-loc;hasLatitude"/>
		<rdfs:label>has maximum latitude</rdfs:label>
		<rdfs:range rdf:resource="&xsd;decimal"/>
		<skos:definition>indicates the highest value / maximum for latitude with respect to a range</skos:definition>
	</owl:DatatypeProperty>
	
	<owl:DatatypeProperty rdf:about="&cmns-loc;hasMaximumLongitude">
		<rdfs:subPropertyOf rdf:resource="&cmns-loc;hasLongitude"/>
		<rdfs:label>has maximum longitude</rdfs:label>
		<rdfs:range rdf:resource="&xsd;decimal"/>
		<skos:definition>indicates the highest value / maximum for longitude with respect to a range</skos:definition>
	</owl:DatatypeProperty>
	
	<owl:DatatypeProperty rdf:about="&cmns-loc;hasMinimumLatitude">
		<rdfs:subPropertyOf rdf:resource="&cmns-loc;hasLatitude"/>
		<rdfs:label>has minimum latitude</rdfs:label>
		<rdfs:range rdf:resource="&xsd;decimal"/>
		<skos:definition>indicates the lowest value / latitude with respect to a range</skos:definition>
	</owl:DatatypeProperty>
	
	<owl:DatatypeProperty rdf:about="&cmns-loc;hasMinimumLongitude">
		<rdfs:subPropertyOf rdf:resource="&cmns-loc;hasLongitude"/>
		<rdfs:label>has minimum longitude</rdfs:label>
		<rdfs:range rdf:resource="&xsd;decimal"/>
		<skos:definition>indicates the lowest value / longitude with respect to a range</skos:definition>
	</owl:DatatypeProperty>
	
	<owl:ObjectProperty rdf:about="&cmns-loc;hasMunicipality">
		<rdfs:subPropertyOf rdf:resource="&cmns-loc;hasRegion"/>
		<rdfs:label>has municipality</rdfs:label>
		<rdfs:range rdf:resource="&cmns-loc;Municipality"/>
		<skos:definition>indicates a business center, city, or municipality</skos:definition>
		<cmns-av:usageNote>Note that certain greater metropolitan areas span multiple counties or states (e.g., the greater Washington, D.C. area, which includes parts of Maryland and Virginia, and divided/disputed cities such as Jerusalem), thus hasMunicipality is a subproperty of hasRegion rather than hasSubdivision.</cmns-av:usageNote>
	</owl:ObjectProperty>
	
	<owl:ObjectProperty rdf:about="&cmns-loc;hasRegion">
		<rdfs:label>has region</rdfs:label>
		<rdfs:range rdf:resource="&cmns-loc;GeographicRegion"/>
		<skos:definition>indicates a demarcated area on the surface of the Earth</skos:definition>
	</owl:ObjectProperty>
	
	<owl:ObjectProperty rdf:about="&cmns-loc;hasSubdivision">
		<rdfs:subPropertyOf rdf:resource="&cmns-loc;hasRegion"/>
		<rdfs:label>has subdivision</rdfs:label>
		<rdfs:range rdf:resource="&cmns-loc;CountrySubdivision"/>
		<skos:definition>identifies a country subdivision (state, province, region, etc.)</skos:definition>
		<cmns-av:adaptedFrom rdf:datatype="&xsd;anyURI">https://www.gleif.org/en/about-lei/common-data-file-format/current-versions/level-1-data-lei-cdf-3-1-format</cmns-av:adaptedFrom>
	</owl:ObjectProperty>
	
	<owl:ObjectProperty rdf:about="&cmns-loc;hasSubregion">
		<rdfs:subPropertyOf rdf:resource="&cmns-col;hasPart"/>
		<rdfs:subPropertyOf rdf:resource="&cmns-loc;hasRegion"/>
		<rdfs:label>has subregion</rdfs:label>
		<rdfs:domain rdf:resource="&cmns-loc;GeographicRegion"/>
		<rdfs:range rdf:resource="&cmns-loc;GeographicRegion"/>
		<skos:definition>relates a geographic region to another geographic region that is a designated subregion of it</skos:definition>
	</owl:ObjectProperty>
	
	<owl:DatatypeProperty rdf:about="&cmns-loc;isIndependent">
		<rdfs:label>is independent</rdfs:label>
		<rdfs:domain rdf:resource="&cmns-loc;GeopoliticalEntity"/>
		<rdfs:range rdf:resource="&xsd;boolean"/>
		<skos:definition>indicates whether a geopolitical entity stands alone or is considered part of another geopolitical entity (e.g., a country)</skos:definition>
	</owl:DatatypeProperty>
	
	<owl:ObjectProperty rdf:about="&cmns-loc;isSubregionOf">
		<rdfs:subPropertyOf rdf:resource="&cmns-col;isPartOf"/>
		<rdfs:label>is subregion of</rdfs:label>
		<rdfs:domain rdf:resource="&cmns-loc;GeographicRegion"/>
		<rdfs:range rdf:resource="&cmns-loc;GeographicRegion"/>
		<owl:inverseOf rdf:resource="&cmns-loc;hasSubregion"/>
		<skos:definition>relates a geographic region to another geographic region that it is a part of</skos:definition>
	</owl:ObjectProperty>

</rdf:RDF>