<?xml version="1.0" encoding="UTF-8"?>
<!DOCTYPE rdf:RDF [
	<!ENTITY cmns-av "https://www.omg.org/spec/Commons/AnnotationVocabulary/">
	<!ENTITY cmns-cmp "https://www.omg.org/spec/Commons/Composites/">
	<!ENTITY cmns-col "https://www.omg.org/spec/Commons/Collections/">
	<!ENTITY cmns-cxtdsg "https://www.omg.org/spec/Commons/ContextualDesignators/">
	<!ENTITY cmns-dsg "https://www.omg.org/spec/Commons/Designators/">
	<!ENTITY cmns-id "https://www.omg.org/spec/Commons/Identifiers/">
	<!ENTITY cmns-org "https://www.omg.org/spec/Commons/Organizations/">
	<!ENTITY cmns-pts "https://www.omg.org/spec/Commons/PartiesAndSituations/">
	<!ENTITY dct "http://purl.org/dc/terms/">
	<!ENTITY lcc-cr "https://www.omg.org/spec/LCC/Countries/CountryRepresentation/">
	<!ENTITY owl "http://www.w3.org/2002/07/owl#">
	<!ENTITY rdf "http://www.w3.org/1999/02/22-rdf-syntax-ns#">
	<!ENTITY rdfs "http://www.w3.org/2000/01/rdf-schema#">
	<!ENTITY skos "http://www.w3.org/2004/02/skos/core#">
	<!ENTITY xsd "http://www.w3.org/2001/XMLSchema#">
]>
<rdf:RDF xml:base="https://www.omg.org/spec/Commons/Organizations/"
	xmlns:cmns-av="https://www.omg.org/spec/Commons/AnnotationVocabulary/"
	xmlns:cmns-cmp="https://www.omg.org/spec/Commons/Composites/"
	xmlns:cmns-col="https://www.omg.org/spec/Commons/Collections/"
	xmlns:cmns-cxtdsg="https://www.omg.org/spec/Commons/ContextualDesignators/"
	xmlns:cmns-dsg="https://www.omg.org/spec/Commons/Designators/"
	xmlns:cmns-id="https://www.omg.org/spec/Commons/Identifiers/"
	xmlns:cmns-org="https://www.omg.org/spec/Commons/Organizations/"
	xmlns:cmns-pts="https://www.omg.org/spec/Commons/PartiesAndSituations/"
	xmlns:dct="http://purl.org/dc/terms/"
	xmlns:lcc-cr="https://www.omg.org/spec/LCC/Countries/CountryRepresentation/"
	xmlns:owl="http://www.w3.org/2002/07/owl#"
	xmlns:rdf="http://www.w3.org/1999/02/22-rdf-syntax-ns#"
	xmlns:rdfs="http://www.w3.org/2000/01/rdf-schema#"
	xmlns:skos="http://www.w3.org/2004/02/skos/core#"
	xmlns:xsd="http://www.w3.org/2001/XMLSchema#">
	
	<owl:Ontology rdf:about="https://www.omg.org/spec/Commons/Organizations/">
		<rdfs:label>Commons Organizations Ontology</rdfs:label>
		<dct:abstract>This ontology defines high-level concepts for organizations and related terms. It is purposefully underspecified to facilitate mapping to specific organization ontologies, such as the emerging W3C organization ontology, organization from a BMM or BPMN perspective, organization from a records management (RMS) perspective, and so forth.</dct:abstract>
		<dct:license rdf:datatype="&xsd;anyURI">https://opensource.org/licenses/MIT</dct:license>
		<owl:imports rdf:resource="https://www.omg.org/spec/Commons/AnnotationVocabulary/"/>
		<owl:imports rdf:resource="https://www.omg.org/spec/Commons/Collections/"/>
		<owl:imports rdf:resource="https://www.omg.org/spec/Commons/Composites/"/>
		<owl:imports rdf:resource="https://www.omg.org/spec/Commons/ContextualDesignators/"/>
		<owl:imports rdf:resource="https://www.omg.org/spec/Commons/Designators/"/>
		<owl:imports rdf:resource="https://www.omg.org/spec/Commons/PartiesAndSituations/"/>
		<owl:imports rdf:resource="https://www.omg.org/spec/LCC/Countries/CountryRepresentation/"/>
		<owl:versionIRI rdf:resource="https://www.omg.org/spec/Commons/20230801/Organizations/"/>
		<skos:note>This ontology is derived from the Financial Industry Business Ontology (FIBO) Organizations, Formal Organizations, and Legal Persons ontologies.</skos:note>
		<cmns-av:copyright>Copyright (c) 2013-2023 EDM Council, Inc.</cmns-av:copyright>
		<cmns-av:copyright>Copyright (c) 2013-2023 Object Management Group, Inc.</cmns-av:copyright>
	</owl:Ontology>
	
	<owl:Class rdf:about="&cmns-org;FormalOrganization">
		<rdfs:subClassOf rdf:resource="&cmns-org;Organization"/>
		<rdfs:subClassOf>
			<owl:Restriction>
				<owl:onProperty rdf:resource="&cmns-org;isDomiciledIn"/>
				<owl:onClass rdf:resource="&lcc-cr;GeopoliticalEntity"/>
				<owl:minQualifiedCardinality rdf:datatype="&xsd;nonNegativeInteger">0</owl:minQualifiedCardinality>
			</owl:Restriction>
		</rdfs:subClassOf>
		<rdfs:label>formal organization</rdfs:label>
		<owl:disjointWith rdf:resource="&cmns-org;InformalOrganization"/>
		<skos:definition>organization that is recognized in some legal jurisdiction, with associated rights and responsibilities</skos:definition>
		<skos:example>Examples include a corporation, charity, government or church.</skos:example>
		<cmns-av:adaptedFrom rdf:datatype="&xsd;anyURI">https://www.w3.org/TR/vocab-org/#class-formalorganization</cmns-av:adaptedFrom>
	</owl:Class>
	
	<owl:Class rdf:about="&cmns-org;Group">
		<rdfs:subClassOf rdf:resource="&cmns-col;Collection"/>
		<rdfs:subClassOf>
			<owl:Restriction>
				<owl:onProperty rdf:resource="&cmns-col;hasMember"/>
				<owl:allValuesFrom rdf:resource="&cmns-pts;Agent"/>
			</owl:Restriction>
		</rdfs:subClassOf>
		<rdfs:label>group</rdfs:label>
		<skos:definition>collection of agents (people, organizations, software agents, etc.) that are considered as a unit</skos:definition>
	</owl:Class>
	
	<owl:Class rdf:about="&cmns-org;InformalOrganization">
		<rdfs:subClassOf rdf:resource="&cmns-org;Organization"/>
		<rdfs:label>informal organization</rdfs:label>
		<skos:definition>organization that is not formally constituted in some way</skos:definition>
	</owl:Class>
	
	<owl:Class rdf:about="&cmns-org;LegalEntity">
		<rdfs:subClassOf rdf:resource="&cmns-org;FormalOrganization"/>
		<rdfs:subClassOf rdf:resource="&cmns-org;LegalPerson"/>
		<rdfs:label>legal entity</rdfs:label>
		<skos:definition>legal person that is a partnership, corporation, or other organization having the capacity to negotiate contracts, assume financial obligations, and pay off debts, organized under the laws of some jurisdiction</skos:definition>
		<skos:scopeNote>The term &apos;legal entities&apos; includes, but is not limited to, unique parties that are legally or financially responsible for the performance of financial transactions or have the legal right in their jurisdiction to enter independently into legal contracts, regardless of whether they are incorporated or constituted in some other way (e.g. trust, partnership, contractual). It excludes natural persons, but includes governmental organizations and supranationals.</skos:scopeNote>
		<cmns-av:adaptedFrom>ISO 17442, Financial services - Legal Entity Identifier (LEI), first edition, 2012-06-01, section 3.1</cmns-av:adaptedFrom>
		<cmns-av:synonym>artificial person</cmns-av:synonym>
		<cmns-av:synonym>juridical entity</cmns-av:synonym>
		<cmns-av:synonym>juridical person</cmns-av:synonym>
		<cmns-av:synonym>juristic person</cmns-av:synonym>
	</owl:Class>
	
	<owl:Class rdf:about="&cmns-org;LegalPerson">
		<rdfs:subClassOf rdf:resource="&cmns-pts;Party"/>
		<rdfs:label xml:lang="en">legal person</rdfs:label>
		<skos:definition>party that is recognized as having rights and obligations under the law, including but not limited to the right to sue and be sued, enter into contracts, own property, and incur financial and other obligations</skos:definition>
		<cmns-av:explanatoryNote>To have legal personality means to be capable of having legal rights and duties within a certain legal system, such as to enter into contracts, sue, and be sued. Legal personality is a prerequisite to legal capacity, the ability of any legal person to amend (enter into, transfer, etc.) rights and obligations.</cmns-av:explanatoryNote>
	</owl:Class>
	
	<owl:Class rdf:about="&cmns-org;MemberBearingOrganization">
		<rdfs:subClassOf rdf:resource="&cmns-pts;PartyRole"/>
		<rdfs:subClassOf>
			<owl:Restriction>
				<owl:onProperty rdf:resource="&cmns-cmp;isPlayedBy"/>
				<owl:someValuesFrom>
					<owl:Restriction>
						<owl:onProperty rdf:resource="&cmns-col;hasMember"/>
						<owl:someValuesFrom rdf:resource="&cmns-pts;Party"/>
					</owl:Restriction>
				</owl:someValuesFrom>
			</owl:Restriction>
		</rdfs:subClassOf>
		<rdfs:label>member-bearing organization</rdfs:label>
		<skos:definition>role of a group or organization that has members that are people or other organizations</skos:definition>
	</owl:Class>
	
	<owl:Class rdf:about="&cmns-org;Membership">
		<rdfs:subClassOf rdf:resource="&cmns-pts;Situation"/>
		<rdfs:subClassOf>
			<owl:Restriction>
				<owl:onProperty rdf:resource="&cmns-org;hasMembership"/>
				<owl:someValuesFrom rdf:resource="&cmns-org;MemberBearingOrganization"/>
			</owl:Restriction>
		</rdfs:subClassOf>
		<rdfs:subClassOf>
			<owl:Restriction>
				<owl:onProperty rdf:resource="&cmns-org;hasOrganizationMember"/>
				<owl:someValuesFrom rdf:resource="&cmns-org;OrganizationMember"/>
			</owl:Restriction>
		</rdfs:subClassOf>
		<rdfs:label xml:lang="en">membership</rdfs:label>
		<rdfs:seeAlso rdf:resource="https://www.w3.org/TR/vocab-org/#class-membership"/>
		<skos:definition>situation, corresponding to an n-ary relation, in which some group or organization has at least one member (person or organization) for some period of time</skos:definition>
	</owl:Class>
	
	<owl:Class rdf:about="&cmns-org;Organization">
		<rdfs:subClassOf rdf:resource="&cmns-pts;Party"/>
		<rdfs:subClassOf>
			<owl:Restriction>
				<owl:onProperty rdf:resource="&cmns-col;hasPart"/>
				<owl:allValuesFrom rdf:resource="&cmns-org;Organization"/>
			</owl:Restriction>
		</rdfs:subClassOf>
		<rdfs:subClassOf>
			<owl:Restriction>
				<owl:onProperty rdf:resource="&cmns-col;hasMember"/>
				<owl:allValuesFrom rdf:resource="&cmns-pts;Party"/>
			</owl:Restriction>
		</rdfs:subClassOf>
		<rdfs:subClassOf>
			<owl:Restriction>
				<owl:onProperty rdf:resource="&cmns-dsg;hasName"/>
				<owl:onClass rdf:resource="&cmns-org;OrganizationName"/>
				<owl:minQualifiedCardinality rdf:datatype="&xsd;nonNegativeInteger">0</owl:minQualifiedCardinality>
			</owl:Restriction>
		</rdfs:subClassOf>
		<rdfs:label xml:lang="en">organization</rdfs:label>
		<rdfs:seeAlso rdf:resource="https://www.w3.org/TR/vocab-org/#org:Organization"/>
		<skos:definition>collection of one or more people, or groups of people formed together into a community or other social, commercial or political structure to act, or that is designated to act, towards some purpose, such as to meet a need or pursue collective goals on a continuing basis</skos:definition>
		<skos:example>This may be a business entity, government, international organization, not-for-profit, academic institution, or other unincorporated and/or informal social organization.</skos:example>
		<cmns-av:adaptedFrom>ISO/IEC 6523-1:1998 Information technology — Structure for the identification of organizations and organization parts — Part 1: Identification of organization identification schemes, https://www.iso.org/obp/ui/#iso:std:iso-iec:6523:-1:ed-1:v1:en</cmns-av:adaptedFrom>
	</owl:Class>
	
	<owl:Class rdf:about="&cmns-org;OrganizationIdentificationScheme">
		<rdfs:subClassOf rdf:resource="&cmns-id;IdentificationScheme"/>
		<rdfs:label>organization identification scheme</rdfs:label>
		<skos:definition>identification scheme dedicated to the unique identification of organizations</skos:definition>
		<cmns-av:adaptedFrom>ISO/IEC 6523-1:1998 Information technology — Structure for the identification of organizations and organization parts — Part 1: Identification of organization identification schemes, https://www.iso.org/obp/ui/#iso:std:iso-iec:6523:-1:ed-1:v1:en</cmns-av:adaptedFrom>
	</owl:Class>
	
	<owl:Class rdf:about="&cmns-org;OrganizationIdentifier">
		<rdfs:subClassOf rdf:resource="&cmns-id;Identifier"/>
		<rdfs:subClassOf>
			<owl:Restriction>
				<owl:onProperty rdf:resource="&cmns-col;isMemberOf"/>
				<owl:onClass rdf:resource="&cmns-org;OrganizationIdentificationScheme"/>
				<owl:qualifiedCardinality rdf:datatype="&xsd;nonNegativeInteger">1</owl:qualifiedCardinality>
			</owl:Restriction>
		</rdfs:subClassOf>
		<rdfs:subClassOf>
			<owl:Restriction>
				<owl:onProperty rdf:resource="&cmns-id;identifies"/>
				<owl:someValuesFrom rdf:resource="&cmns-org;Organization"/>
			</owl:Restriction>
		</rdfs:subClassOf>
		<rdfs:label>organization identifier</rdfs:label>
		<skos:definition>identifier assigned to an organization within an organization identification scheme, and unique within that scheme</skos:definition>
		<cmns-av:adaptedFrom>ISO/IEC 6523-1:1998 Information technology — Structure for the identification of organizations and organization parts — Part 1: Identification of organization identification schemes, https://www.iso.org/obp/ui/#iso:std:iso-iec:6523:-1:ed-1:v1:en</cmns-av:adaptedFrom>
	</owl:Class>
	
	<owl:Class rdf:about="&cmns-org;OrganizationMember">
		<rdfs:subClassOf rdf:resource="&cmns-pts;PartyRole"/>
		<rdfs:subClassOf>
			<owl:Restriction>
				<owl:onProperty rdf:resource="&cmns-cmp;isPlayedBy"/>
				<owl:someValuesFrom>
					<owl:Restriction>
						<owl:onProperty rdf:resource="&cmns-col;isMemberOf"/>
						<owl:allValuesFrom rdf:resource="&cmns-org;Organization"/>
					</owl:Restriction>
				</owl:someValuesFrom>
			</owl:Restriction>
		</rdfs:subClassOf>
		<rdfs:label>organization member</rdfs:label>
		<rdfs:seeAlso rdf:resource="https://www.w3.org/TR/vocab-org/#org:Role"/>
		<skos:definition>party (person or organization) that has a membership role with respect to some organization</skos:definition>
	</owl:Class>
	
	<owl:Class rdf:about="&cmns-org;OrganizationName">
		<rdfs:subClassOf rdf:resource="&cmns-cxtdsg;ContextualName"/>
		<rdfs:subClassOf>
			<owl:Restriction>
				<owl:onProperty rdf:resource="&cmns-dsg;isNameOf"/>
				<owl:onClass rdf:resource="&cmns-org;Organization"/>
				<owl:minQualifiedCardinality rdf:datatype="&xsd;nonNegativeInteger">0</owl:minQualifiedCardinality>
			</owl:Restriction>
		</rdfs:subClassOf>
		<rdfs:label>organization name</rdfs:label>
		<skos:definition>designation by which some organization is known in some context</skos:definition>
	</owl:Class>
	
	<owl:Class rdf:about="&cmns-org;OrganizationPartIdentifier">
		<rdfs:subClassOf rdf:resource="&cmns-id;Identifier"/>
		<rdfs:subClassOf>
			<owl:Restriction>
				<owl:onProperty rdf:resource="&cmns-id;identifies"/>
				<owl:someValuesFrom rdf:resource="&cmns-org;OrganizationalSubUnit"/>
			</owl:Restriction>
		</rdfs:subClassOf>
		<rdfs:label>organization part identifier</rdfs:label>
		<skos:definition>identifier allocated to a particular organizational sub-unit</skos:definition>
		<cmns-av:abbreviation>OPI</cmns-av:abbreviation>
		<cmns-av:adaptedFrom>ISO/IEC 6523-1:1998 Information technology — Structure for the identification of organizations and organization parts — Part 1: Identification of organization identification schemes, https://www.iso.org/obp/ui/#iso:std:iso-iec:6523:-1:ed-1:v1:en</cmns-av:adaptedFrom>
		<cmns-av:synonym>organization sub-unit identifier</cmns-av:synonym>
	</owl:Class>
	
	<owl:Class rdf:about="&cmns-org;OrganizationalSubUnit">
		<rdfs:subClassOf rdf:resource="&cmns-org;Organization"/>
		<rdfs:subClassOf>
			<owl:Restriction>
				<owl:onProperty rdf:resource="&cmns-col;isPartOf"/>
				<owl:allValuesFrom rdf:resource="&cmns-org;Organization"/>
			</owl:Restriction>
		</rdfs:subClassOf>
		<rdfs:label>organizational sub-unit</rdfs:label>
		<rdfs:seeAlso rdf:resource="https://www.w3.org/TR/vocab-org/#org:OrganizationalUnit"/>
		<skos:definition>any department, service, and other entity within a larger organization that only has full recognition within the context of that organization, but requires identification for some purpose</skos:definition>
		<cmns-av:adaptedFrom>ISO/IEC 6523-1:1998 Information technology — Structure for the identification of organizations and organization parts — Part 1: Identification of organization identification schemes, https://www.iso.org/obp/ui/#iso:std:iso-iec:6523:-1:ed-1:v1:en</cmns-av:adaptedFrom>
		<cmns-av:explanatoryNote>In other words, it is not a legal entity in its own right.</cmns-av:explanatoryNote>
		<cmns-av:synonym>organization part</cmns-av:synonym>
	</owl:Class>
	
	<owl:ObjectProperty rdf:about="&cmns-org;hasMembership">
		<rdfs:subPropertyOf rdf:resource="&cmns-pts;hasActor"/>
		<rdfs:label>has membership</rdfs:label>
		<rdfs:domain rdf:resource="&cmns-org;Membership"/>
		<rdfs:range rdf:resource="&cmns-org;MemberBearingOrganization"/>
		<rdfs:seeAlso rdf:resource="https://www.w3.org/TR/vocab-org/#org:organization"/>
		<owl:inverseOf rdf:resource="&cmns-org;isMembershipPartyIn"/>
		<skos:definition>identifies the organization acting in the role of having members in an organizational membership situation</skos:definition>
	</owl:ObjectProperty>
	
	<owl:ObjectProperty rdf:about="&cmns-org;hasOrganizationMember">
		<rdfs:subPropertyOf rdf:resource="&cmns-pts;hasUndergoer"/>
		<rdfs:label>has organization member</rdfs:label>
		<rdfs:domain rdf:resource="&cmns-org;Membership"/>
		<rdfs:range rdf:resource="&cmns-org;OrganizationMember"/>
		<rdfs:seeAlso rdf:resource="https://www.w3.org/TR/vocab-org/#org:member"/>
		<owl:inverseOf rdf:resource="&cmns-org;isOrganizationMember"/>
		<skos:definition>indicates the party that is the member in an organizational membership situation</skos:definition>
	</owl:ObjectProperty>
	
	<owl:ObjectProperty rdf:about="&cmns-org;hasSubUnit">
		<rdfs:subPropertyOf rdf:resource="&cmns-col;hasPart"/>
		<rdfs:label>has sub-unit</rdfs:label>
		<rdfs:domain rdf:resource="&cmns-org;Organization"/>
		<rdfs:range rdf:resource="&cmns-org;OrganizationalSubUnit"/>
		<rdfs:seeAlso rdf:resource="https://www.w3.org/TR/vocab-org/#org:hasSubOrganization"/>
		<owl:inverseOf rdf:resource="&cmns-org;isSubUnitOf"/>
		<skos:definition>relates an organization to a part of that organization</skos:definition>
	</owl:ObjectProperty>
	
	<owl:ObjectProperty rdf:about="&cmns-org;isDomiciledIn">
		<rdfs:label>is domiciled in</rdfs:label>
		<rdfs:domain rdf:resource="&cmns-org;FormalOrganization"/>
		<rdfs:range rdf:resource="&lcc-cr;GeopoliticalEntity"/>
		<skos:definition>indicates the principal place where an entity conducts business within some country, such as where its headquarters is located</skos:definition>
		<cmns-av:explanatoryNote>Corporate domicile refers to a place where a company&apos;s affairs are discharged. It is also typically the legal home of a corporation within a country because the place is considered by law as the center of corporate affairs. In cases where a business has incorporated in one location for convenience, such as for taxation, legal, or regulatory purposes, but operates primarily in one or more other locations, domicile refers to the operational location(s) rather than legal location. Many companies in the US have incorporated in the State of Delaware, for example, but do not have operational facilities in Delaware (or only have small offices there).</cmns-av:explanatoryNote>
	</owl:ObjectProperty>
	
	<owl:ObjectProperty rdf:about="&cmns-org;isMembershipPartyIn">
		<rdfs:subPropertyOf rdf:resource="&cmns-pts;actsIn"/>
		<rdfs:label>is membership party in</rdfs:label>
		<rdfs:domain rdf:resource="&cmns-org;MemberBearingOrganization"/>
		<rdfs:range rdf:resource="&cmns-org;Membership"/>
		<skos:definition>indicates the context of membership in which the party plays the role of having members</skos:definition>
	</owl:ObjectProperty>
	
	<owl:ObjectProperty rdf:about="&cmns-org;isOrganizationMember">
		<rdfs:subPropertyOf rdf:resource="&cmns-pts;undergoes"/>
		<rdfs:label>is organization member</rdfs:label>
		<rdfs:domain rdf:resource="&cmns-org;OrganizationMember"/>
		<rdfs:range rdf:resource="&cmns-org;Membership"/>
		<rdfs:seeAlso rdf:resource="https://www.w3.org/TR/vocab-org/#org:role"/>
		<skos:definition>indicates the context of membership in which some party is an organization member</skos:definition>
	</owl:ObjectProperty>
	
	<owl:ObjectProperty rdf:about="&cmns-org;isSubUnitOf">
		<rdfs:subPropertyOf rdf:resource="&cmns-col;isPartOf"/>
		<rdfs:label>is sub-unit of</rdfs:label>
		<rdfs:domain rdf:resource="&cmns-org;OrganizationalSubUnit"/>
		<rdfs:range rdf:resource="&cmns-org;Organization"/>
		<rdfs:seeAlso rdf:resource="https://www.w3.org/TR/vocab-org/#org:subOrganizationOf"/>
		<skos:definition>relates a part of an organization to the larger entity</skos:definition>
	</owl:ObjectProperty>

</rdf:RDF>