<?xml version="1.0" encoding="UTF-8"?>
<!DOCTYPE rdf:RDF [
	<!ENTITY cmns-av "https://www.omg.org/spec/Commons/AnnotationVocabulary/">
	<!ENTITY cmns-col "https://www.omg.org/spec/Commons/Collections/">
	<!ENTITY cmns-cxtdsg "https://www.omg.org/spec/Commons/ContextualDesignators/">
	<!ENTITY cmns-dsg "https://www.omg.org/spec/Commons/Designators/">
	<!ENTITY cmns-dt "https://www.omg.org/spec/Commons/DatesAndTimes/">
	<!ENTITY cmns-pts "https://www.omg.org/spec/Commons/PartiesAndSituations/">
	<!ENTITY dct "http://purl.org/dc/terms/">
	<!ENTITY owl "http://www.w3.org/2002/07/owl#">
	<!ENTITY rdf "http://www.w3.org/1999/02/22-rdf-syntax-ns#">
	<!ENTITY rdfs "http://www.w3.org/2000/01/rdf-schema#">
	<!ENTITY skos "http://www.w3.org/2004/02/skos/core#">
	<!ENTITY xsd "http://www.w3.org/2001/XMLSchema#">
]>
<rdf:RDF xml:base="https://www.omg.org/spec/Commons/PartiesAndSituations/"
	xmlns:cmns-av="https://www.omg.org/spec/Commons/AnnotationVocabulary/"
	xmlns:cmns-col="https://www.omg.org/spec/Commons/Collections/"
	xmlns:cmns-cxtdsg="https://www.omg.org/spec/Commons/ContextualDesignators/"
	xmlns:cmns-dsg="https://www.omg.org/spec/Commons/Designators/"
	xmlns:cmns-dt="https://www.omg.org/spec/Commons/DatesAndTimes/"
	xmlns:cmns-pts="https://www.omg.org/spec/Commons/PartiesAndSituations/"
	xmlns:dct="http://purl.org/dc/terms/"
	xmlns:owl="http://www.w3.org/2002/07/owl#"
	xmlns:rdf="http://www.w3.org/1999/02/22-rdf-syntax-ns#"
	xmlns:rdfs="http://www.w3.org/2000/01/rdf-schema#"
	xmlns:skos="http://www.w3.org/2004/02/skos/core#"
	xmlns:xsd="http://www.w3.org/2001/XMLSchema#">
	
	<owl:Ontology rdf:about="https://www.omg.org/spec/Commons/PartiesAndSituations/">
		<rdfs:label>Commons Parties and Situations Ontology</rdfs:label>
		<dct:abstract>This ontology defines the high-level concepts of parties and the roles they play in various situations.</dct:abstract>
		<dct:contributor>Dean Allemang, Working Ontologist</dct:contributor>
		<dct:contributor>Elisa Kendall, Thematix Partners LLC</dct:contributor>
		<dct:license rdf:datatype="&xsd;anyURI">http://opensource.org/licenses/MIT</dct:license>
		<owl:imports rdf:resource="https://www.omg.org/spec/Commons/AnnotationVocabulary/"/>
		<owl:imports rdf:resource="https://www.omg.org/spec/Commons/Collections/"/>
		<owl:imports rdf:resource="https://www.omg.org/spec/Commons/ContextualDesignators/"/>
		<owl:imports rdf:resource="https://www.omg.org/spec/Commons/DatesAndTimes/"/>
		<owl:imports rdf:resource="https://www.omg.org/spec/Commons/Designators/"/>
		<owl:versionIRI rdf:resource="https://www.omg.org/spec/Commons/20220901/PartiesAndSituations/"/>
		<skos:note>This ontology was originally designed for use in the Financial Industry Business Ontology (FIBO) for representing complex relationships between parties, such as employment, ownership and control.</skos:note>
		<cmns-av:copyright>Copyright (c) 2020-2022 EDM Council, Inc.</cmns-av:copyright>
		<cmns-av:copyright>Copyright (c) 2020-2022 Thematix Partners LLC</cmns-av:copyright>
		<cmns-av:copyright>Copyright (c) 2020-2022 Working Ontologist LLC</cmns-av:copyright>
		<cmns-av:copyright>Copyright (c) 2022 Object Management Group, Inc.</cmns-av:copyright>
	</owl:Ontology>
	
	<owl:Class rdf:about="&cmns-pts;Actor">
		<rdfs:subClassOf rdf:resource="&cmns-pts;PartyRole"/>
		<rdfs:label>actor</rdfs:label>
		<skos:definition>party that is the primary performer in a relationship between parties, i.e., the party that does something, causes something to happen, or otherwise plays an agentive role in the relationship</skos:definition>
		<skos:example>Examples include owner, controlling party, beneficiary, guarantor, partner in a partnership, shareholder, etc.</skos:example>
	</owl:Class>
	
	<owl:Class rdf:about="&cmns-pts;Agent">
		<rdfs:subClassOf>
			<owl:Restriction>
				<owl:onProperty rdf:resource="&cmns-dsg;hasName"/>
				<owl:onClass rdf:resource="&cmns-cxtdsg;ContextualName"/>
				<owl:minQualifiedCardinality rdf:datatype="&xsd;nonNegativeInteger">0</owl:minQualifiedCardinality>
			</owl:Restriction>
		</rdfs:subClassOf>
		<rdfs:label>agent</rdfs:label>
		<rdfs:seeAlso rdf:datatype="&xsd;anyURI">http://www.jamesodell.com/WhatIsAnAgent.pdf</rdfs:seeAlso>
		<rdfs:seeAlso rdf:datatype="&xsd;anyURI">http://www.jamesodell.com/WhyShouldWeCareAboutAgents.pdf</rdfs:seeAlso>
		<skos:definition>something autonomous that can adapt to and interact with its environment</skos:definition>
		<skos:note>Agents can be human beings, organizations, software agents, robots and living things other than plants. They are defined as having the following three important properties: autonomy, interactive behavior, and adaptability. (1) Autonomy - an agent is capable of acting without direct external intervention. This includes software or other agents that have some degree of control over their internal state and can act based on their own experiences. They can also possess their own set of internal responsibilities and capabilities that enable them to act without any external choreography. This definition excludes agents that act on on behalf of (or as a proxy for) some person or thing (see AgentRole). (2) Interactive behavior - they are capable of exchanging communicating with other things in their environment. This includes, in the case of software agents, messages that can support requests for services and other kinds of resources, as well as event detection and notification. They can be synchronous or asynchronous in nature. The interaction can also be conversational in nature, such as negotiating contracts, marketplace-style bidding, or simply making a query. (3) Adaptability - an agent is capable of responding to other agents and/or its environment. Agents can react to communications and events and then respond appropriately. Software agents can be designed to make difficult decisions and even modify their behavior based on their experiences. In other words, they can learn and evolve.</skos:note>
		<skos:note>Note that this does not necessarily imply that an agent is free to act as it sees fit, without constraint. Rather, an agent in the sense meant here is something which may or may not be subject to controls and constraints but is self-actualizing in its behavior in response to any such constraints.</skos:note>
		<cmns-av:directSource rdf:datatype="&xsd;anyURI">http://www.omg.org/techprocess/meetings/schedule/AMP.html</cmns-av:directSource>
	</owl:Class>
	
	<owl:Class rdf:about="&cmns-pts;AgentRole">
		<rdfs:subClassOf rdf:resource="&cmns-pts;Role"/>
		<rdfs:subClassOf>
			<owl:Restriction>
				<owl:onProperty rdf:resource="&cmns-pts;isPlayedBy"/>
				<owl:onClass rdf:resource="&cmns-pts;Agent"/>
				<owl:minQualifiedCardinality rdf:datatype="&xsd;nonNegativeInteger">0</owl:minQualifiedCardinality>
			</owl:Restriction>
		</rdfs:subClassOf>
		<rdfs:label>agent role</rdfs:label>
		<skos:definition>role that is played by an agent</skos:definition>
	</owl:Class>
	
	<owl:Class rdf:about="&cmns-pts;Constituency">
		<rdfs:subClassOf>
			<owl:Restriction>
				<owl:onProperty rdf:resource="&cmns-dsg;defines"/>
				<owl:allValuesFrom rdf:resource="&owl;Thing"/>
			</owl:Restriction>
		</rdfs:subClassOf>
		<rdfs:subClassOf>
			<owl:Restriction>
				<owl:onProperty rdf:resource="&cmns-col;hasConstituent"/>
				<owl:allValuesFrom rdf:resource="&cmns-col;Constituent"/>
			</owl:Restriction>
		</rdfs:subClassOf>
		<rdfs:subClassOf>
			<owl:Restriction>
				<owl:onProperty rdf:resource="&cmns-pts;hasRole"/>
				<owl:allValuesFrom rdf:resource="&cmns-pts;Role"/>
			</owl:Restriction>
		</rdfs:subClassOf>
		<rdfs:subClassOf>
			<owl:Restriction>
				<owl:onProperty rdf:resource="&cmns-cxtdsg;isApplicableIn"/>
				<owl:onClass rdf:resource="&cmns-cxtdsg;Context"/>
				<owl:minQualifiedCardinality rdf:datatype="&xsd;nonNegativeInteger">0</owl:minQualifiedCardinality>
			</owl:Restriction>
		</rdfs:subClassOf>
		<rdfs:label>constituency</rdfs:label>
		<skos:definition>relationship that defines something based on its constituent(s) and/or constituent roles that may be context-specific</skos:definition>
	</owl:Class>
	
	<owl:Class rdf:about="&cmns-pts;FunctionalRole">
		<rdfs:subClassOf rdf:resource="&cmns-pts;Role"/>
		<rdfs:label>functional role</rdfs:label>
		<skos:definition>role specifying one or more activities, capabilities, purposes, skills or combination thereof</skos:definition>
		<skos:note>A functional role may be played by an agent involved in a process or business activity, or by material or equipment that is produced by, consumed by, or participates in some process, for example.</skos:note>
	</owl:Class>
	
	<owl:Class rdf:about="&cmns-pts;Party">
		<rdfs:subClassOf rdf:resource="&cmns-pts;Agent"/>
		<rdfs:label>party</rdfs:label>
		<owl:disjointWith rdf:resource="&cmns-pts;Role"/>
		<skos:definition>person or organization</skos:definition>
	</owl:Class>
	
	<owl:Class rdf:about="&cmns-pts;PartyRole">
		<rdfs:subClassOf rdf:resource="&cmns-pts;AgentRole"/>
		<rdfs:subClassOf>
			<owl:Restriction>
				<owl:onProperty rdf:resource="&cmns-cxtdsg;hasApplicablePeriod"/>
				<owl:onClass rdf:resource="&cmns-dt;DatePeriod"/>
				<owl:minQualifiedCardinality rdf:datatype="&xsd;nonNegativeInteger">0</owl:minQualifiedCardinality>
			</owl:Restriction>
		</rdfs:subClassOf>
		<rdfs:subClassOf>
			<owl:Restriction>
				<owl:onProperty rdf:resource="&cmns-pts;isPlayedBy"/>
				<owl:onClass rdf:resource="&cmns-pts;Party"/>
				<owl:minQualifiedCardinality rdf:datatype="&xsd;nonNegativeInteger">0</owl:minQualifiedCardinality>
			</owl:Restriction>
		</rdfs:subClassOf>
		<rdfs:label>party role</rdfs:label>
		<skos:definition>agent role that is played by person or organization, that typically holds for some period of time</skos:definition>
		<skos:example>Examples include organization member, employee, issuer, owner, partner in a partnership, shareholder, and so forth.</skos:example>
		<skos:note>Note that there may be cases whre the identity of the party playing the role is not known, as well as cases where in some situation, such as ownership, there may be more than one party playing the role of owner.</skos:note>
		<skos:scopeNote>The concept of a party role is used in contexts in which one would call someone a &apos;party to something&apos;, such as party to a contract or to a transaction, a supplier, buyer, customer, student, employee, and so forth. More specific roles such as those that are performed in the context of some activity or process are actors in that situation.</skos:scopeNote>
	</owl:Class>
	
	<owl:Class rdf:about="&cmns-pts;Role">
		<rdfs:subClassOf>
			<owl:Restriction>
				<owl:onProperty rdf:resource="&cmns-pts;isPlayedBy"/>
				<owl:minCardinality rdf:datatype="&xsd;nonNegativeInteger">0</owl:minCardinality>
			</owl:Restriction>
		</rdfs:subClassOf>
		<rdfs:label>role</rdfs:label>
		<skos:definition>relative concept that ties a part to something or someone that fills it</skos:definition>
	</owl:Class>
	
	<owl:Class rdf:about="&cmns-pts;Situation">
		<rdfs:subClassOf>
			<owl:Restriction>
				<owl:onProperty rdf:resource="&cmns-pts;holdsDuring"/>
				<owl:onClass rdf:resource="&cmns-dt;DatePeriod"/>
				<owl:minQualifiedCardinality rdf:datatype="&xsd;nonNegativeInteger">0</owl:minQualifiedCardinality>
			</owl:Restriction>
		</rdfs:subClassOf>
		<rdfs:subClassOf>
			<owl:Restriction>
				<owl:onProperty rdf:resource="&cmns-pts;hasObjectRole"/>
				<owl:onClass rdf:resource="&cmns-pts;Role"/>
				<owl:minQualifiedCardinality rdf:datatype="&xsd;nonNegativeInteger">0</owl:minQualifiedCardinality>
			</owl:Restriction>
		</rdfs:subClassOf>
		<rdfs:subClassOf>
			<owl:Restriction>
				<owl:onProperty rdf:resource="&cmns-pts;hasSubjectRole"/>
				<owl:someValuesFrom rdf:resource="&cmns-pts;Role"/>
			</owl:Restriction>
		</rdfs:subClassOf>
		<rdfs:label>situation</rdfs:label>
		<skos:definition>setting, state of being, or relationship that is relatively stable for some period of time</skos:definition>
		<skos:example>Examples include ownership, control, possession, affiliation, beneficial ownership, employment, and other similar situations.</skos:example>
		<skos:note>From a usage perspective, situations are essentially reified relations, sometimes called mediating relationships.</skos:note>
	</owl:Class>
	
	<owl:Class rdf:about="&cmns-pts;Undergoer">
		<rdfs:subClassOf rdf:resource="&cmns-pts;Role"/>
		<rdfs:label>undergoer</rdfs:label>
		<skos:definition>something that plays the role of the object or recipient in a situation, i.e., the thing (or party) that the situation impacts, affects, or that otherwise plays a passive recipient / patient or thematic role</skos:definition>
		<skos:example>Examples include something that is owned or controlled.</skos:example>
	</owl:Class>
	
	<owl:ObjectProperty rdf:about="&cmns-pts;actsIn">
		<rdfs:subPropertyOf rdf:resource="&cmns-pts;isSubjectRoleIn"/>
		<rdfs:label>acts in</rdfs:label>
		<rdfs:domain rdf:resource="&cmns-pts;Actor"/>
		<rdfs:range rdf:resource="&cmns-pts;Situation"/>
		<owl:inverseOf rdf:resource="&cmns-pts;hasActor"/>
		<skos:definition>indicates a situation in which the actor plays a primary role</skos:definition>
	</owl:ObjectProperty>
	
	<owl:ObjectProperty rdf:about="&cmns-pts;actsOn">
		<rdfs:label>acts on</rdfs:label>
		<owl:propertyChainAxiom rdf:parseType="Collection">
			<rdf:Description rdf:about="&cmns-pts;actsIn">
			</rdf:Description>
			<rdf:Description rdf:about="&cmns-pts;hasUndergoer">
			</rdf:Description>
		</owl:propertyChainAxiom>
		<skos:definition>relates an actor in a given situation to the undergoer that they affect under the circumstances</skos:definition>
	</owl:ObjectProperty>
	
	<owl:ObjectProperty rdf:about="&cmns-pts;directlyAffects">
		<rdfs:label>directly affects</rdfs:label>
		<owl:inverseOf rdf:resource="&cmns-pts;experiencesWith"/>
		<owl:propertyChainAxiom rdf:parseType="Collection">
			<rdf:Description rdf:about="&cmns-pts;actsIn">
			</rdf:Description>
			<rdf:Description rdf:about="&cmns-pts;hasUndergoer">
			</rdf:Description>
			<rdf:Description rdf:about="&cmns-pts;isPlayedBy">
			</rdf:Description>
		</owl:propertyChainAxiom>
		<skos:definition>relates an actor in a given situation to the thing (or party) that they impact under the circumstances</skos:definition>
	</owl:ObjectProperty>
	
	<owl:ObjectProperty rdf:about="&cmns-pts;experiences">
		<rdfs:label>experiences</rdfs:label>
		<owl:propertyChainAxiom rdf:parseType="Collection">
			<rdf:Description rdf:about="&cmns-pts;playsRole">
			</rdf:Description>
			<rdf:Description rdf:about="&cmns-pts;undergoes">
			</rdf:Description>
		</owl:propertyChainAxiom>
		<skos:definition>relates something to a situation that affects them in some way</skos:definition>
	</owl:ObjectProperty>
	
	<owl:ObjectProperty rdf:about="&cmns-pts;experiencesDirectly">
		<rdfs:label>experiences directly</rdfs:label>
		<owl:propertyChainAxiom rdf:parseType="Collection">
			<rdf:Description rdf:about="&cmns-pts;playsRole">
			</rdf:Description>
			<rdf:Description rdf:about="&cmns-pts;undergoes">
			</rdf:Description>
			<rdf:Description rdf:about="&cmns-pts;hasActor">
			</rdf:Description>
			<rdf:Description rdf:about="&cmns-pts;isPlayedBy">
			</rdf:Description>
		</owl:propertyChainAxiom>
		<skos:definition>relates something directly to a party that drives a situation involving it</skos:definition>
	</owl:ObjectProperty>
	
	<owl:ObjectProperty rdf:about="&cmns-pts;experiencesWith">
		<rdfs:label>experiences with</rdfs:label>
		<owl:propertyChainAxiom rdf:parseType="Collection">
			<rdf:Description rdf:about="&cmns-pts;playsRole">
			</rdf:Description>
			<rdf:Description rdf:about="&cmns-pts;undergoes">
			</rdf:Description>
			<rdf:Description rdf:about="&cmns-pts;hasActor">
			</rdf:Description>
		</owl:propertyChainAxiom>
		<skos:definition>relates something to an actor that drives a situation involving it</skos:definition>
	</owl:ObjectProperty>
	
	<owl:ObjectProperty rdf:about="&cmns-pts;hasActiveParty">
		<rdfs:label>has active party</rdfs:label>
		<owl:inverseOf rdf:resource="&cmns-pts;playsActivePartyIn"/>
		<owl:propertyChainAxiom rdf:parseType="Collection">
			<rdf:Description rdf:about="&cmns-pts;hasActor">
			</rdf:Description>
			<rdf:Description rdf:about="&cmns-pts;isPlayedBy">
			</rdf:Description>
		</owl:propertyChainAxiom>
		<skos:definition>relates a situation to the person or organization acting in a primary (agentive) role</skos:definition>
	</owl:ObjectProperty>
	
	<owl:ObjectProperty rdf:about="&cmns-pts;hasActiveRole">
		<rdfs:label>has active role</rdfs:label>
		<owl:inverseOf rdf:resource="&cmns-pts;playsActiveRoleIn"/>
		<owl:propertyChainAxiom rdf:parseType="Collection">
			<rdf:Description rdf:about="&cmns-pts;hasSubjectRole">
			</rdf:Description>
			<rdf:Description rdf:about="&cmns-pts;isPlayedBy">
			</rdf:Description>
		</owl:propertyChainAxiom>
		<skos:definition>relates a situation to something that is acting in a primary (agentive) role</skos:definition>
	</owl:ObjectProperty>
	
	<owl:ObjectProperty rdf:about="&cmns-pts;hasActor">
		<rdfs:subPropertyOf rdf:resource="&cmns-pts;hasPartyRole"/>
		<rdfs:subPropertyOf rdf:resource="&cmns-pts;hasSubjectRole"/>
		<rdfs:label>has actor</rdfs:label>
		<rdfs:domain rdf:resource="&cmns-pts;Situation"/>
		<rdfs:range rdf:resource="&cmns-pts;Actor"/>
		<skos:definition>identifies the primary party acting in a specific role with respect to a given situation</skos:definition>
	</owl:ObjectProperty>
	
	<owl:ObjectProperty rdf:about="&cmns-pts;hasObjectRole">
		<rdfs:subPropertyOf rdf:resource="&cmns-pts;hasRole"/>
		<rdfs:label>has object role</rdfs:label>
		<rdfs:domain>
			<owl:Class>
				<owl:unionOf rdf:parseType="Collection">
					<rdf:Description rdf:about="&cmns-pts;Constituency">
					</rdf:Description>
					<rdf:Description rdf:about="&cmns-pts;Situation">
					</rdf:Description>
				</owl:unionOf>
			</owl:Class>
		</rdfs:domain>
		<rdfs:range rdf:resource="&cmns-pts;Role"/>
		<skos:definition>identifies a person or thing that is affected by, or is a secondary argument in a specific role with respect to a given relation or situation</skos:definition>
	</owl:ObjectProperty>
	
	<owl:ObjectProperty rdf:about="&cmns-pts;hasParty">
		<rdfs:label>has party</rdfs:label>
		<rdfs:range rdf:resource="&cmns-pts;Party"/>
		<skos:definition>identifies an independent party associated with an agreement, contract, policy, regulation, or other arrangement</skos:definition>
	</owl:ObjectProperty>
	
	<owl:ObjectProperty rdf:about="&cmns-pts;hasPartyRole">
		<rdfs:subPropertyOf rdf:resource="&cmns-pts;hasRole"/>
		<rdfs:label>has party role</rdfs:label>
		<rdfs:range rdf:resource="&cmns-pts;PartyRole"/>
		<skos:definition>identifies a specific role played by some person or organization as related to a situation, agreement, contract, policy, regulation, activity or other relationship</skos:definition>
	</owl:ObjectProperty>
	
	<owl:ObjectProperty rdf:about="&cmns-pts;hasRelatedPartyRole">
		<rdfs:subPropertyOf rdf:resource="&cmns-pts;hasRole"/>
		<rdfs:label>has related party role</rdfs:label>
		<rdfs:domain rdf:resource="&cmns-pts;PartyRole"/>
		<rdfs:range rdf:resource="&cmns-pts;PartyRole"/>
		<skos:definition>relates a party acting in a specific role directly to another party acting in the same or another role</skos:definition>
		<skos:note>This property is intended as an abstract property, whose subproperties may or may not be symmetric, but could be inverses of one another.</skos:note>
	</owl:ObjectProperty>
	
	<owl:ObjectProperty rdf:about="&cmns-pts;hasRole">
		<rdfs:label>has role</rdfs:label>
		<rdfs:range rdf:resource="&cmns-pts;Role"/>
		<skos:definition>identifies something acting in a recipient or target role as related to the particular agreement, contract, policy, regulation, situation, or other arrangement</skos:definition>
	</owl:ObjectProperty>
	
	<owl:ObjectProperty rdf:about="&cmns-pts;hasSubjectRole">
		<rdfs:subPropertyOf rdf:resource="&cmns-pts;hasRole"/>
		<rdfs:label>has subject role</rdfs:label>
		<rdfs:domain rdf:resource="&cmns-pts;Situation"/>
		<rdfs:range rdf:resource="&cmns-pts;Role"/>
		<skos:definition>identifies the person or thing that is being discussed, described, dealt with, or is the main topic in a specific role with respect to a given situation</skos:definition>
	</owl:ObjectProperty>
	
	<owl:ObjectProperty rdf:about="&cmns-pts;hasUndergoer">
		<rdfs:subPropertyOf rdf:resource="&cmns-pts;hasObjectRole"/>
		<rdfs:label>has undergoer</rdfs:label>
		<rdfs:domain rdf:resource="&cmns-pts;Situation"/>
		<rdfs:range rdf:resource="&cmns-pts;Undergoer"/>
		<skos:definition>identifies an experiencer / passive or other object role in a given situation</skos:definition>
	</owl:ObjectProperty>
	
	<owl:ObjectProperty rdf:about="&cmns-pts;holdsDuring">
		<rdfs:subPropertyOf rdf:resource="&cmns-cxtdsg;hasApplicablePeriod"/>
		<rdfs:label>holds during</rdfs:label>
		<rdfs:range rdf:resource="&cmns-dt;DatePeriod"/>
		<skos:definition>indicates a date period during which something is true</skos:definition>
	</owl:ObjectProperty>
	
	<owl:ObjectProperty rdf:about="&cmns-pts;isAPartyTo">
		<rdfs:label>is a party to</rdfs:label>
		<rdfs:domain rdf:resource="&cmns-pts;Party"/>
		<owl:inverseOf rdf:resource="&cmns-pts;hasParty"/>
		<skos:definition>identifies an agreement, contract, policy, regulation, or other arrangement that an independent party is associated with</skos:definition>
	</owl:ObjectProperty>
	
	<owl:ObjectProperty rdf:about="&cmns-pts;isAffectedBy">
		<rdfs:label>is affected by</rdfs:label>
		<owl:propertyChainAxiom rdf:parseType="Collection">
			<rdf:Description rdf:about="&cmns-pts;undergoes">
			</rdf:Description>
			<rdf:Description rdf:about="&cmns-pts;hasActor">
			</rdf:Description>
		</owl:propertyChainAxiom>
		<skos:definition>relates an undergoer in a given situation to the actor that has an impact on them under the circumstances</skos:definition>
	</owl:ObjectProperty>
	
	<owl:ObjectProperty rdf:about="&cmns-pts;isDirectlyAffectedBy">
		<rdfs:label>is directly affected by</rdfs:label>
		<owl:propertyChainAxiom rdf:parseType="Collection">
			<rdf:Description rdf:about="&cmns-pts;undergoes">
			</rdf:Description>
			<rdf:Description rdf:about="&cmns-pts;hasActor">
			</rdf:Description>
			<rdf:Description rdf:about="&cmns-pts;isPlayedBy">
			</rdf:Description>
		</owl:propertyChainAxiom>
		<skos:definition>relates an undergoer in a given situation to the person or organization that has an impact on them under the circumstances</skos:definition>
	</owl:ObjectProperty>
	
	<owl:ObjectProperty rdf:about="&cmns-pts;isExperiencedBy">
		<rdfs:label>is experienced by</rdfs:label>
		<owl:inverseOf rdf:resource="&cmns-pts;experiences"/>
		<owl:propertyChainAxiom rdf:parseType="Collection">
			<rdf:Description rdf:about="&cmns-pts;hasUndergoer">
			</rdf:Description>
			<rdf:Description rdf:about="&cmns-pts;isPlayedBy">
			</rdf:Description>
		</owl:propertyChainAxiom>
		<skos:definition>relates a situation to something that is directly involved in or affected by it</skos:definition>
	</owl:ObjectProperty>
	
	<owl:ObjectProperty rdf:about="&cmns-pts;isManifestedIn">
		<rdfs:label>is manifested in</rdfs:label>
		<rdfs:domain rdf:resource="&cmns-pts;Role"/>
		<owl:inverseOf rdf:resource="&cmns-pts;manifests"/>
		<skos:definition>indicates something in which the role is realized, appears, or occurs</skos:definition>
	</owl:ObjectProperty>
	
	<owl:ObjectProperty rdf:about="&cmns-pts;isObjectRoleIn">
		<rdfs:subPropertyOf rdf:resource="&cmns-pts;isRoleIn"/>
		<rdfs:label>is object role in</rdfs:label>
		<rdfs:domain rdf:resource="&cmns-pts;Role"/>
		<rdfs:range>
			<owl:Class>
				<owl:unionOf rdf:parseType="Collection">
					<rdf:Description rdf:about="&cmns-pts;Constituency">
					</rdf:Description>
					<rdf:Description rdf:about="&cmns-pts;Situation">
					</rdf:Description>
				</owl:unionOf>
			</owl:Class>
		</rdfs:range>
		<owl:inverseOf rdf:resource="&cmns-pts;hasObjectRole"/>
		<skos:definition>indicates a situation in which the role is secondary, such as an experiencer or passive participant</skos:definition>
	</owl:ObjectProperty>
	
	<owl:ObjectProperty rdf:about="&cmns-pts;isPlayedBy">
		<rdf:type rdf:resource="&owl;FunctionalProperty"/>
		<rdfs:label>is played by</rdfs:label>
		<rdfs:domain rdf:resource="&cmns-pts;Role"/>
		<owl:inverseOf rdf:resource="&cmns-pts;playsRole"/>
		<skos:definition>indicates the independent thing, such as a person, organization, or asset, filling a role</skos:definition>
		<skos:example>A party, counterparty, or third party to a contract is played by an organization or person; an issuer of a financial instrument is typically played by an organization.</skos:example>
	</owl:ObjectProperty>
	
	<owl:ObjectProperty rdf:about="&cmns-pts;isRealizedIn">
		<rdfs:label>is realized in</rdfs:label>
		<owl:inverseOf rdf:resource="&cmns-pts;realizes"/>
		<owl:propertyChainAxiom rdf:parseType="Collection">
			<rdf:Description rdf:about="&cmns-pts;hasObjectRole">
			</rdf:Description>
			<rdf:Description rdf:about="&cmns-pts;isPlayedBy">
			</rdf:Description>
		</owl:propertyChainAxiom>
		<skos:definition>relates a situation or constituency to something that is affected by, or is a secondary argument to in a specific role with respect to a given relation or situation</skos:definition>
	</owl:ObjectProperty>
	
	<owl:ObjectProperty rdf:about="&cmns-pts;isRoleIn">
		<rdfs:label>is role in</rdfs:label>
		<rdfs:domain rdf:resource="&cmns-pts;Role"/>
		<owl:inverseOf rdf:resource="&cmns-pts;hasRole"/>
		<skos:definition>identifies an agreement, policy, regulation, situation, constituency or other arrangementinvolving the role</skos:definition>
	</owl:ObjectProperty>
	
	<owl:ObjectProperty rdf:about="&cmns-pts;isSubjectRoleIn">
		<rdfs:subPropertyOf rdf:resource="&cmns-pts;isRoleIn"/>
		<rdfs:label>is subject role in</rdfs:label>
		<rdfs:domain rdf:resource="&cmns-pts;Role"/>
		<rdfs:range rdf:resource="&cmns-pts;Situation"/>
		<owl:inverseOf rdf:resource="&cmns-pts;hasSubjectRole"/>
		<skos:definition>indicates a situation in which the role is the primary topic</skos:definition>
	</owl:ObjectProperty>
	
	<owl:ObjectProperty rdf:about="&cmns-pts;manifests">
		<rdfs:label>manifests</rdfs:label>
		<rdfs:range rdf:resource="&cmns-pts;Role"/>
		<skos:definition>indicates a role that realizes, displays, or shows something, typically in some context</skos:definition>
	</owl:ObjectProperty>
	
	<owl:ObjectProperty rdf:about="&cmns-pts;playsActivePartyIn">
		<rdfs:label>plays active party in</rdfs:label>
		<owl:propertyChainAxiom rdf:parseType="Collection">
			<rdf:Description rdf:about="&cmns-pts;playsRole">
			</rdf:Description>
			<rdf:Description rdf:about="&cmns-pts;actsIn">
			</rdf:Description>
		</owl:propertyChainAxiom>
		<skos:definition>relates a person or organization to a situation that they are directly involved in</skos:definition>
	</owl:ObjectProperty>
	
	<owl:ObjectProperty rdf:about="&cmns-pts;playsActiveRoleIn">
		<rdfs:label>plays active role in</rdfs:label>
		<owl:propertyChainAxiom rdf:parseType="Collection">
			<rdf:Description rdf:about="&cmns-pts;playsRole">
			</rdf:Description>
			<rdf:Description rdf:about="&cmns-pts;isSubjectRoleIn">
			</rdf:Description>
		</owl:propertyChainAxiom>
		<skos:definition>relates something to a situation that it is directly involved in</skos:definition>
	</owl:ObjectProperty>
	
	<owl:ObjectProperty rdf:about="&cmns-pts;playsActiveRoleThatAffects">
		<rdfs:label>plays active role that affects</rdfs:label>
		<owl:inverseOf rdf:resource="&cmns-pts;isDirectlyAffectedBy"/>
		<owl:propertyChainAxiom rdf:parseType="Collection">
			<rdf:Description rdf:about="&cmns-pts;playsRole">
			</rdf:Description>
			<rdf:Description rdf:about="&cmns-pts;actsIn">
			</rdf:Description>
			<rdf:Description rdf:about="&cmns-pts;hasUndergoer">
			</rdf:Description>
		</owl:propertyChainAxiom>
		<skos:definition>relates a person or organization to an undergoer they have an impact on under the circumstances</skos:definition>
	</owl:ObjectProperty>
	
	<owl:ObjectProperty rdf:about="&cmns-pts;playsActiveRoleThatDirectlyAffects">
		<rdfs:label>plays active role that directly affects</rdfs:label>
		<owl:inverseOf rdf:resource="&cmns-pts;experiencesDirectly"/>
		<owl:propertyChainAxiom rdf:parseType="Collection">
			<rdf:Description rdf:about="&cmns-pts;playsRole">
			</rdf:Description>
			<rdf:Description rdf:about="&cmns-pts;actsIn">
			</rdf:Description>
			<rdf:Description rdf:about="&cmns-pts;hasUndergoer">
			</rdf:Description>
			<rdf:Description rdf:about="&cmns-pts;isPlayedBy">
			</rdf:Description>
		</owl:propertyChainAxiom>
		<skos:definition>relates a person or organization to something they have a direct impact on under the circumstances</skos:definition>
	</owl:ObjectProperty>
	
	<owl:ObjectProperty rdf:about="&cmns-pts;playsRole">
		<rdfs:label>plays role</rdfs:label>
		<rdfs:range rdf:resource="&cmns-pts;Role"/>
		<skos:definition>indicates a part that someone or something plays under some circumstance</skos:definition>
		<skos:example>an organization may play the role of employer, issuer, regulatory agency, bank, custodian, manufacturer, vendor, etc.; a person may play the role of employee, examiner, banker, seller, buyer, etc.</skos:example>
	</owl:ObjectProperty>
	
	<owl:ObjectProperty rdf:about="&cmns-pts;realizes">
		<rdfs:label>realizes</rdfs:label>
		<owl:propertyChainAxiom rdf:parseType="Collection">
			<rdf:Description rdf:about="&cmns-pts;playsRole">
			</rdf:Description>
			<rdf:Description rdf:about="&cmns-pts;isObjectRoleIn">
			</rdf:Description>
		</owl:propertyChainAxiom>
		<skos:definition>relates something to a situation or constituency in which the role they play is secondary, such as an experiencer or passive participant</skos:definition>
	</owl:ObjectProperty>
	
	<owl:ObjectProperty rdf:about="&cmns-pts;undergoes">
		<rdfs:subPropertyOf rdf:resource="&cmns-pts;isObjectRoleIn"/>
		<rdfs:label>undergoes</rdfs:label>
		<rdfs:domain rdf:resource="&cmns-pts;Undergoer"/>
		<rdfs:range rdf:resource="&cmns-pts;Situation"/>
		<owl:inverseOf rdf:resource="&cmns-pts;hasUndergoer"/>
		<skos:definition>indicates a situation that the undergoer experiences</skos:definition>
	</owl:ObjectProperty>

</rdf:RDF>