<?xml version="1.0" encoding="UTF-8"?>
<!DOCTYPE rdf:RDF [
	<!ENTITY authority "http://publications.europa.eu/ontology/authority/">
	<!ENTITY idmp "https://purl.iso.org/idmp/">
	<!ENTITY ns1 "http://www.novartis.com/data_governance/knowledgefeed#">
	<!ENTITY nvs "https://data-qa.novartis.net/r1/informationtechnology/architecture/iserver/v1/object/">
	<!ENTITY nvsdoc "https://data-qa.novartis.net/r1/informationtechnology/architecture/iserver/v1/document/">
	<!ENTITY owl "http://www.w3.org/2002/07/owl#">
	<!ENTITY rdf "http://www.w3.org/1999/02/22-rdf-syntax-ns#">
	<!ENTITY rdfs "http://www.w3.org/2000/01/rdf-schema#">
	<!ENTITY skos "http://www.w3.org/2004/02/skos/core#">
	<!ENTITY skos-xl "http://www.w3.org/2008/05/skos-xl#">
	<!ENTITY terms "http://purl.org/dc/terms/">
	<!ENTITY upper "https://data-qa.novartis.net/r1/enterprise/datastrategy/upperontology/v1/">
	<!ENTITY xsd "http://www.w3.org/2001/XMLSchema#">
]>
<rdf:RDF xml:base="https://purl.iso.org/idmp/core"
	xmlns="https://purl.iso.org/idmp/core#"
	xmlns:authority="http://publications.europa.eu/ontology/authority/"
	xmlns:idmp="https://purl.iso.org/idmp/"
	xmlns:ns1="http://www.novartis.com/data_governance/knowledgefeed#"
	xmlns:nvs="https://data-qa.novartis.net/r1/informationtechnology/architecture/iserver/v1/object/"
	xmlns:nvsdoc="https://data-qa.novartis.net/r1/informationtechnology/architecture/iserver/v1/document/"
	xmlns:owl="http://www.w3.org/2002/07/owl#"
	xmlns:rdf="http://www.w3.org/1999/02/22-rdf-syntax-ns#"
	xmlns:rdfs="http://www.w3.org/2000/01/rdf-schema#"
	xmlns:skos="http://www.w3.org/2004/02/skos/core#"
	xmlns:skos-xl="http://www.w3.org/2008/05/skos-xl#"
	xmlns:terms="http://purl.org/dc/terms/"
	xmlns:upper="https://data-qa.novartis.net/r1/enterprise/datastrategy/upperontology/v1/"
	xmlns:xsd="http://www.w3.org/2001/XMLSchema#">
	
	<owl:Ontology rdf:about="&idmp;core">
		<rdfs:label>Core Ontology of Identification of Medicinal Products (IDMP)</rdfs:label>
		<rdfs:label>Core Ontology of identification of medicinal products (IDMP)</rdfs:label>
		<rdfs:comment>This artifact represents the core vocabulary of IDMP based on ISO standards:
		ISO_11238_2018(en) Substance,
		ISO_11239_2012(en) Dose form, unit, route of administration,
		ISO_11240_2012(en) Unit details,
		ISO_11615_2017(en) Medicinal product,
		ISO_11616_2017(en) Pharmaceutical product,
		ISO/TS 19844 E Implementation guideline for 11238,
		ISO/TS 20443 E Implementation guideline for 11615,
		ISO/TS 20451 E Implementation guideline for 11616,

		Representation of information in agreement of IDMP requires application of further ISO standards:
		ISO 639-1 Codes for names of languages (part 1: Alpha-2 code),
		ISO 3166-1:2013 Codes for names of countries (part 1: Country codes),
		ISO 8601 Data elements and interchange formats</rdfs:comment>
		<rdfs:comment>This ontology contains entities that are shared between different modules of IDMP ontology. The core ontology imports codelists that are shared between modules of the IDMP ontology.</rdfs:comment>
		<terms:creator rdf:resource="https://accurids.com"/>
		<terms:issued rdf:datatype="&xsd;dateTime">2020-11-05T12:00:00Z</terms:issued>
		<terms:license>These files are shared Intellectual Property of OSTHUS and ACCURIDS and may be used only through explicit written permission through OSTHUS or ACCURIDS. In particular further distribution and copy of parts are prohibited.</terms:license>
		<terms:modified rdf:datatype="&xsd;date">2022-01-31</terms:modified>
		<terms:rightsHolder rdf:resource="https://accurids.com"/>
		<terms:rightsHolder rdf:resource="https://osthus.com"/>
		<terms:title>Core Ontology of Identification of Medicinal Products (IDMP)</terms:title>
		<terms:title>Core Ontology of identification of medicinal products (IDMP)</terms:title>
		<owl:imports rdf:resource="http://www.w3.org/2004/02/skos/core"/>
		<owl:imports rdf:resource="https://purl.iso.org/datatypes"/>
		<owl:versionIRI rdf:resource="https://purl.iso.org/idmp/core/0.1"/>
	</owl:Ontology>
	
	<owl:Class rdf:about="http://purl.org/dc/dcmitype/Text">
	</owl:Class>
	
	<owl:AnnotationProperty rdf:about="&terms;identifer">
	</owl:AnnotationProperty>
	
	<owl:AnnotationProperty rdf:about="&terms;publisher">
	</owl:AnnotationProperty>
	
	<owl:AnnotationProperty rdf:about="&terms;source">
	</owl:AnnotationProperty>
	
	<owl:NamedIndividual rdf:about="&idmp;ChangeMade">
		<rdf:type rdf:resource="&owl;Class"/>
		<rdfs:subClassOf rdf:resource="&skos;Concept"/>
		<terms:source>ISO/TS 19844:2018(E) page 67</terms:source>
		<skos:definition>The description of the updates or changes of the substance should be specified. The field will be left empty when first insert of substance.</skos:definition>
		<skos:example>Update to previous version to include additional translations.</skos:example>
		<skos:prefLabel>change made</skos:prefLabel>
		<idmp:conformance rdf:resource="&idmp;MandatoryInformation"/>
	</owl:NamedIndividual>
	
	<owl:NamedIndividual rdf:about="&idmp;EffectiveDate">
		<rdf:type rdf:resource="&owl;Class"/>
		<rdfs:subClassOf rdf:resource="&skos;Concept"/>
		<terms:source>ISO/TS 19844:2018(E) page 67</terms:source>
		<skos:definition>The date when the substance was effective should be provided in line with the ISO 8601 date format. This shall be defined when the substance is generated or modified.</skos:definition>
		<skos:example>20110219</skos:example>
		<skos:prefLabel>effective date</skos:prefLabel>
		<idmp:businessRules>The value may be implicitly derived.</idmp:businessRules>
		<idmp:conformance rdf:resource="&idmp;MandatoryInformation"/>
	</owl:NamedIndividual>
	
	<owl:NamedIndividual rdf:about="&idmp;MandatoryInformation">
	</owl:NamedIndividual>
	
	<owl:NamedIndividual rdf:about="&idmp;Version">
		<rdf:type rdf:resource="&owl;Class"/>
		<rdfs:subClassOf rdf:resource="&skos;Concept"/>
		<terms:source>ISO/TS 19844:2018(E) page 66</terms:source>
		<skos:definition>This subclause shall provide information on the version of the substance. Where no “Version Number” and “Effective Date” have been assigned by an authority source, the version number shall be set as 0 with the date set as the date of initial submission of the substance. Any changes or updates to a given substance will result in a new version. This could include changes in the definition of the substance or the addition of names or codes. The version of substances should be tracked. Submitters should also indicate if it is a new version of a previous submission.</skos:definition>
		<skos:narrower rdf:resource="&idmp;ChangeMade"/>
		<skos:narrower rdf:resource="&idmp;EffectiveDate"/>
		<skos:narrower rdf:resource="&idmp;VersionNumber"/>
		<skos:prefLabel>version</skos:prefLabel>
		<idmp:conformance rdf:resource="&idmp;MandatoryInformation"/>
	</owl:NamedIndividual>
	
	<owl:NamedIndividual rdf:about="&idmp;VersionNumber">
		<rdf:type rdf:resource="&owl;Class"/>
		<rdfs:subClassOf rdf:resource="&skos;Concept"/>
		<terms:source>ISO/TS 19844:2018(E) page 67</terms:source>
		<skos:definition>The number of the version of the substance shall be provided.</skos:definition>
		<skos:example>1, 2, 3, 99</skos:example>
		<skos:prefLabel>version number</skos:prefLabel>
		<idmp:businessRules>If same document set exists, version shall be greater than the last submitted version.
For maintainance purpose, the version number shall be updated after the effective date.</idmp:businessRules>
		<idmp:conformance rdf:resource="&idmp;MandatoryInformation"/>
	</owl:NamedIndividual>
	
	<owl:AnnotationProperty rdf:about="&idmp;allowedValues">
		<rdfs:comment>Capture defined allowed values according to the ISO standard. This is preliminary and likely to be replaced by a different pattern with controlled lists.</rdfs:comment>
		<skos:prefLabel>allowed values</skos:prefLabel>
	</owl:AnnotationProperty>
	
	<owl:AnnotationProperty rdf:about="&idmp;businessRules">
		<rdfs:comment>Capture defined business rules according to the ISO standard.</rdfs:comment>
		<skos:prefLabel>business rules</skos:prefLabel>
	</owl:AnnotationProperty>
	
	<owl:AnnotationProperty rdf:about="&idmp;conformance">
		<rdfs:comment>Capture defined conformance information according to the ISO standard.</rdfs:comment>
		<skos:prefLabel>conformance</skos:prefLabel>
	</owl:AnnotationProperty>
	
	<owl:ObjectProperty rdf:about="&idmp;hasUMLAttribute">
		<rdfs:comment>This property is used to link UML objects with corresponding &apos;attributes&apos; according to the ISO specification. Its use is preliminary and is assumed to change to a different modelling pattern.</rdfs:comment>
		<owl:inverseOf rdf:resource="&idmp;isUMLAttributeOf"/>
		<skos:prefLabel>has UML attribute</skos:prefLabel>
	</owl:ObjectProperty>
	
	<owl:ObjectProperty rdf:about="&idmp;isUMLAttributeOf">
		<rdfs:comment>This property is used to link &apos;attributes&apos; with corresponding UML objects according to the ISO specification. Its use is preliminary and is assumed to change to a different modelling pattern.</rdfs:comment>
		<skos:prefLabel>is UML attribute of</skos:prefLabel>
	</owl:ObjectProperty>
	
	<owl:NamedIndividual rdf:about="https://purl.iso.org/idmp/iso-11238/2018E">
		<rdf:type rdf:resource="http://purl.org/dc/dcmitype/Text"/>
		<rdf:type rdf:resource="https://www.wikidata.org/wiki/Q1334738"/>
		<terms:identifer>ISO 11238:2018(E)</terms:identifer>
		<terms:publisher rdf:resource="https://www.wikidata.org/wiki/Q15028"/>
		<terms:rightsHolder rdf:resource="https://www.wikidata.org/wiki/Q15028"/>
		<terms:title>Health Informatics — Identification of medicinal products — Data elements and structures for the unique identification and exchange of regulated information on substances</terms:title>
		<skos:exactMatch rdf:resource="https://www.wikidata.org/wiki/Q17575887"/>
		<skos:prefLabel>ISO IDMP 11238 second edition 2018-07</skos:prefLabel>
	</owl:NamedIndividual>
	
	<owl:NamedIndividual rdf:about="https://purl.iso.org/idmp/iso-11239/2012E">
		<rdf:type rdf:resource="http://purl.org/dc/dcmitype/Text"/>
		<rdf:type rdf:resource="https://www.wikidata.org/wiki/Q1334738"/>
		<terms:identifer>ISO 11239:2012(E)</terms:identifer>
		<terms:publisher rdf:resource="https://www.wikidata.org/wiki/Q15028"/>
		<terms:rightsHolder rdf:resource="https://www.wikidata.org/wiki/Q15028"/>
		<terms:title>Health informatics — Identification of medicinal products — Data elements and structures for the unique identification and exchange of regulated information on pharmaceutical dose forms, units of presentation, routes of administration and packaging</terms:title>
		<skos:exactMatch rdf:resource="https://www.wikidata.org/wiki/Q17575890"/>
		<skos:prefLabel>ISO IDMP 11239 first edition 2012-11</skos:prefLabel>
	</owl:NamedIndividual>
	
	<owl:NamedIndividual rdf:about="https://purl.iso.org/idmp/iso-11240/2012E">
		<rdf:type rdf:resource="http://purl.org/dc/dcmitype/Text"/>
		<rdf:type rdf:resource="https://www.wikidata.org/wiki/Q1334738"/>
		<terms:identifer>ISO 11240:2012(E)</terms:identifer>
		<terms:publisher rdf:resource="https://www.wikidata.org/wiki/Q15028"/>
		<terms:rightsHolder rdf:resource="https://www.wikidata.org/wiki/Q15028"/>
		<terms:title>Health informatics — Identification of medicinal products — Data elements and structures for the unique identification and exchange of units of measurement</terms:title>
		<skos:exactMatch rdf:resource="https://www.wikidata.org/wiki/Q18021000"/>
		<skos:prefLabel>ISO IDMP 11240 first edition 2012-11</skos:prefLabel>
	</owl:NamedIndividual>
	
	<owl:NamedIndividual rdf:about="https://purl.iso.org/idmp/iso-11615/2017E">
		<rdf:type rdf:resource="http://purl.org/dc/dcmitype/Text"/>
		<rdf:type rdf:resource="https://www.wikidata.org/wiki/Q1334738"/>
		<terms:identifer>ISO 11615:2017(E)</terms:identifer>
		<terms:publisher rdf:resource="https://www.wikidata.org/wiki/Q15028"/>
		<terms:rightsHolder rdf:resource="https://www.wikidata.org/wiki/Q15028"/>
		<terms:title>Health informatics — Identification of medicinal products — Data elements and structures for the unique identification and exchange of regulated medicinal product information</terms:title>
		<skos:exactMatch rdf:resource="https://www.wikidata.org/wiki/Q17575893"/>
		<skos:prefLabel>ISO IDMP 11615 second edition 2017-10</skos:prefLabel>
	</owl:NamedIndividual>
	
	<owl:NamedIndividual rdf:about="https://purl.iso.org/idmp/iso-11616/2017E">
		<rdf:type rdf:resource="http://purl.org/dc/dcmitype/Text"/>
		<rdf:type rdf:resource="https://www.wikidata.org/wiki/Q1334738"/>
		<terms:identifer>ISO 11616:2017(E)</terms:identifer>
		<terms:publisher rdf:resource="https://www.wikidata.org/wiki/Q15028"/>
		<terms:rightsHolder rdf:resource="https://www.wikidata.org/wiki/Q15028"/>
		<terms:title>Health informatics — Identification of medicinal products — Data elements and structures for unique identification and exchange of regulated pharmaceutical product information</terms:title>
		<skos:exactMatch rdf:resource="https://www.wikidata.org/wiki/Q17575895"/>
		<skos:prefLabel>ISO IDMP 11616 second edition 2017-10</skos:prefLabel>
	</owl:NamedIndividual>
	
	<owl:NamedIndividual rdf:about="https://purl.iso.org/idmp/iso-ts-19844/2018E">
		<rdf:type rdf:resource="http://purl.org/dc/dcmitype/Text"/>
		<rdf:type rdf:resource="https://www.wikidata.org/wiki/Q1334738"/>
		<terms:identifer>ISO 19844:2018(E)</terms:identifer>
		<terms:publisher rdf:resource="https://www.wikidata.org/wiki/Q15028"/>
		<terms:rightsHolder rdf:resource="https://www.wikidata.org/wiki/Q15028"/>
		<terms:title>Health informatics — Identification of medicinal products (IDMP) — Implementation guidelines for ISO 11238 for data elements and structures for the unique identification and exchange of regulated information on substances</terms:title>
		<skos:prefLabel>ISO IDMP Technical Specificatoin 19844 third edition 2018-07</skos:prefLabel>
	</owl:NamedIndividual>
	
	<owl:Class rdf:about="https://www.wikidata.org/wiki/Q1334738">
	</owl:Class>
	
	<owl:NamedIndividual rdf:about="https://www.wikidata.org/wiki/Q17575887">
	</owl:NamedIndividual>
	
	<owl:NamedIndividual rdf:about="https://www.wikidata.org/wiki/Q17575890">
	</owl:NamedIndividual>
	
	<owl:NamedIndividual rdf:about="https://www.wikidata.org/wiki/Q17575893">
	</owl:NamedIndividual>
	
	<owl:NamedIndividual rdf:about="https://www.wikidata.org/wiki/Q17575895">
	</owl:NamedIndividual>
	
	<owl:NamedIndividual rdf:about="https://www.wikidata.org/wiki/Q18021000">
	</owl:NamedIndividual>

</rdf:RDF>