<?xml version="1.0" encoding="UTF-8"?>
<!DOCTYPE rdf:RDF [
	<!ENTITY cmns-av "https://www.omg.org/spec/Commons/AnnotationVocabulary/">
	<!ENTITY cmns-cls "https://www.omg.org/spec/Commons/Classifiers/">
	<!ENTITY dct "http://purl.org/dc/terms/">
	<!ENTITY idmp-chg "https://spec.pistoiaalliance.org/idmp/ontology/META/ChangeManagement/">
	<!ENTITY owl "http://www.w3.org/2002/07/owl#">
	<!ENTITY rdf "http://www.w3.org/1999/02/22-rdf-syntax-ns#">
	<!ENTITY rdfs "http://www.w3.org/2000/01/rdf-schema#">
	<!ENTITY skos "http://www.w3.org/2004/02/skos/core#">
	<!ENTITY xsd "http://www.w3.org/2001/XMLSchema#">
]>
<rdf:RDF xml:base="https://spec.pistoiaalliance.org/idmp/ontology/META/ChangeManagement/"
	xmlns:cmns-av="https://www.omg.org/spec/Commons/AnnotationVocabulary/"
	xmlns:cmns-cls="https://www.omg.org/spec/Commons/Classifiers/"
	xmlns:dct="http://purl.org/dc/terms/"
	xmlns:idmp-chg="https://spec.pistoiaalliance.org/idmp/ontology/META/ChangeManagement/"
	xmlns:owl="http://www.w3.org/2002/07/owl#"
	xmlns:rdf="http://www.w3.org/1999/02/22-rdf-syntax-ns#"
	xmlns:rdfs="http://www.w3.org/2000/01/rdf-schema#"
	xmlns:skos="http://www.w3.org/2004/02/skos/core#"
	xmlns:xsd="http://www.w3.org/2001/XMLSchema#">
	
	<owl:Ontology rdf:about="https://spec.pistoiaalliance.org/idmp/ontology/META/ChangeManagement/">
		<rdfs:label>Change Management Ontology</rdfs:label>
		<dct:abstract>The IDMP Change Management ontology provides metadata for data management and governance of the IDMP ontologies.</dct:abstract>
		<dct:license rdf:datatype="&xsd;anyURI">http://opensource.org/licenses/MIT</dct:license>
		<dct:references rdf:resource="http://purl.org/dc/terms/"/>
		<owl:imports rdf:resource="https://www.omg.org/spec/Commons/AnnotationVocabulary/"/>
		<owl:imports rdf:resource="https://www.omg.org/spec/Commons/Classifiers/"/>
		<owl:versionIRI rdf:resource="https://spec.pistoiaalliance.org/idmp/ontology/META/20221001/ChangeManagement/"/>
		<idmp-chg:hasMaturityLevel rdf:resource="&idmp-chg;Release"/>
		<cmns-av:copyright>Copyright (c) 2022 EDM Council, Inc.</cmns-av:copyright>
		<cmns-av:copyright>Copyright (c) 2022 Pistoia Alliance, Inc.</cmns-av:copyright>
	</owl:Ontology>
	
	<owl:NamedIndividual rdf:about="&idmp-chg;Informative">
		<rdf:type rdf:resource="&idmp-chg;MaturityLevel"/>
		<rdfs:label>informative</rdfs:label>
		<skos:definition xml:lang="en">entity that demonstrates how to use some elements of the ontology</skos:definition>
		<cmns-av:explanatoryNote xml:lang="en">Informative content includes examples that are useful but should not be incorporated in any application. They have been created to support testing and provide guidance to users with respect to how to implement certain constructs.</cmns-av:explanatoryNote>
	</owl:NamedIndividual>
	
	<owl:Class rdf:about="&idmp-chg;MaturityLevel">
		<rdfs:subClassOf rdf:resource="&cmns-cls;Classifier"/>
		<rdfs:label>maturity level</rdfs:label>
		<skos:definition>classifier used to indicate the state of an artifact with respect to the IDMP data management and governance lifecycle</skos:definition>
	</owl:Class>
	
	<owl:Class rdf:about="&idmp-chg;Module">
		<rdfs:subClassOf rdf:resource="&cmns-cls;Classifier"/>
		<rdfs:label>module</rdfs:label>
		<skos:definition xml:lang="en">separable component of something else, organized by topic or functional area</skos:definition>
		<skos:note xml:lang="en">Modularization of any engineering model, including a large ontology, involves principles of the model driven architecture methodology (MDA), such as separation of concerns, coherence, and establishing clear logical boundaries in order to increase reusability and maintainability.

A module should be designed to reflect these principles, including a small number of models that have well-defined relationships with one another, that form a coherent and cohesive whole for some purpose, and that have clear boundaries or interfaces to other external modules.</skos:note>
	</owl:Class>
	
	<owl:NamedIndividual rdf:about="&idmp-chg;Preliminary">
		<rdf:type rdf:resource="&idmp-chg;MaturityLevel"/>
		<rdfs:label>preliminary</rdfs:label>
		<skos:definition xml:lang="en">entity that is considered to be in early stages of development</skos:definition>
		<cmns-av:explanatoryNote xml:lang="en">Preliminary content is subject to significant change, and may be renamed or moved to another ontology prior to achieving provisional status. Users should be aware that it is not dependable, but could be used for reference and as the basis for further work.</cmns-av:explanatoryNote>
	</owl:NamedIndividual>
	
	<owl:NamedIndividual rdf:about="&idmp-chg;Provisional">
		<rdf:type rdf:resource="&idmp-chg;MaturityLevel"/>
		<rdfs:label>provisional</rdfs:label>
		<skos:definition xml:lang="en">entity that is considered to be in later stages of development</skos:definition>
		<cmns-av:explanatoryNote xml:lang="en">Provisional content may change prior to release but is more stable and reliable than preliminary content.</cmns-av:explanatoryNote>
	</owl:NamedIndividual>
	
	<owl:NamedIndividual rdf:about="&idmp-chg;Release">
		<rdf:type rdf:resource="&idmp-chg;MaturityLevel"/>
		<rdfs:label>release</rdfs:label>
		<skos:definition xml:lang="en">entity that is considered to be stable and mature from a development perspective</skos:definition>
		<cmns-av:explanatoryNote xml:lang="en">Release notes will be provided for any changes with respect to released content, and any revisions will be backwards compatible with the prior version to the degree possible.</cmns-av:explanatoryNote>
	</owl:NamedIndividual>
	
	<owl:Class rdf:about="&idmp-chg;Specification">
		<rdfs:subClassOf rdf:resource="&cmns-cls;Classifier"/>
		<rdfs:label>specification</rdfs:label>
		<skos:definition xml:lang="en">explicit set of requirements to be satisfied by a material, model, product, or service</skos:definition>
		<cmns-av:abbreviation xml:lang="en">spec</cmns-av:abbreviation>
	</owl:Class>
	
	<owl:AnnotationProperty rdf:about="&idmp-chg;hasMaturityLevel">
		<rdfs:label>has maturity level</rdfs:label>
		<skos:definition>links something to its state with respect to a development lifecycle</skos:definition>
	</owl:AnnotationProperty>

</rdf:RDF>