<?xml version="1.0" encoding="UTF-8"?>
<!DOCTYPE rdf:RDF [
	<!ENTITY cmns-av "https://www.omg.org/spec/Commons/AnnotationVocabulary/">
	<!ENTITY dct "http://purl.org/dc/terms/">
	<!ENTITY owl "http://www.w3.org/2002/07/owl#">
	<!ENTITY rdf "http://www.w3.org/1999/02/22-rdf-syntax-ns#">
	<!ENTITY rdfs "http://www.w3.org/2000/01/rdf-schema#">
	<!ENTITY skos "http://www.w3.org/2004/02/skos/core#">
	<!ENTITY xsd "http://www.w3.org/2001/XMLSchema#">
]>
<rdf:RDF xml:base="https://www.omg.org/spec/Commons/AnnotationVocabulary/"
	xmlns:cmns-av="https://www.omg.org/spec/Commons/AnnotationVocabulary/"
	xmlns:dct="http://purl.org/dc/terms/"
	xmlns:owl="http://www.w3.org/2002/07/owl#"
	xmlns:rdf="http://www.w3.org/1999/02/22-rdf-syntax-ns#"
	xmlns:rdfs="http://www.w3.org/2000/01/rdf-schema#"
	xmlns:skos="http://www.w3.org/2004/02/skos/core#"
	xmlns:xsd="http://www.w3.org/2001/XMLSchema#">
	
	<owl:Ontology rdf:about="https://www.omg.org/spec/Commons/AnnotationVocabulary/">
		<rdfs:label>Annotation Vocabulary</rdfs:label>
		<dct:abstract>The Annotation Vocabulary provides a set of OWL annotation properties for documenting content with metadata to facilitate user and ontology developer understanding.

Note that any of the original properties provided in Dublin Core and SKOS can be used in addition to the terms provided herein.  However, any Dublin Core terms that are not explicitly defined as OWL annotation properties in this ontology or in any of its imports must be so declared in the ontologies that use them.</dct:abstract>
		<dct:license rdf:datatype="&xsd;anyURI">http://opensource.org/licenses/MIT</dct:license>
		<dct:references rdf:resource="http://purl.org/dc/terms/"/>
		<dct:references rdf:resource="http://www.w3.org/2004/02/skos/core#"/>
		<dct:title>Commons Annotation Vocabulary</dct:title>
		<owl:versionIRI rdf:resource="https://www.omg.org/spec/Commons/20220101/AnnotationVocabulary/"/>
		<skos:note>The annotation properties defined herein are derived from similar annotation vocabularies used in (1) all ontology specifications published by the Object Management Group (OMG) - see http://www.omg.org/techprocess/ab/SpecificationMetadata/, (2) additional annotations used in the Financial Industry Business Ontology (FIBO) - see https://spec.edmcouncil.org/fibo/ontology/FND/Utilities/AnnotationVocabulary/, and (3) refinement of these two ontologies for use by other task forces.  They have been further refined to support the requirements of the Commons ontologies.</skos:note>
		<cmns-av:copyright>Copyright (c) 2022 EDM Council, Inc.</cmns-av:copyright>
		<cmns-av:copyright>Copyright (c) 2022 Object Management Group, Inc.</cmns-av:copyright>
	</owl:Ontology>
	
	<owl:AnnotationProperty rdf:about="&dct;abstract">
		<rdfs:subPropertyOf rdf:resource="&dct;description"/>
		<rdfs:label>abstract</rdfs:label>
		<rdfs:isDefinedBy rdf:resource="&dct;abstract"/>
		<skos:definition>summary of the resource</skos:definition>
		<cmns-av:usageNote>This annotation is used to describe an artifact such as a controlled vocabulary, ontology, or ontology module.</cmns-av:usageNote>
	</owl:AnnotationProperty>
	
	<owl:AnnotationProperty rdf:about="&dct;contributor">
		<rdfs:label>contributor</rdfs:label>
		<rdfs:isDefinedBy rdf:resource="&dct;contributor"/>
		<skos:definition>party that has made contributions to the resource</skos:definition>
	</owl:AnnotationProperty>
	
	<owl:AnnotationProperty rdf:about="&dct;creator">
		<rdfs:subPropertyOf rdf:resource="&dct;contributor"/>
		<rdfs:label>creator</rdfs:label>
		<rdfs:isDefinedBy rdf:resource="&dct;creator"/>
		<skos:definition>party that originated the resource</skos:definition>
	</owl:AnnotationProperty>
	
	<owl:AnnotationProperty rdf:about="&dct;description">
		<rdfs:subPropertyOf rdf:resource="&skos;note"/>
		<rdfs:label>description</rdfs:label>
		<rdfs:isDefinedBy rdf:resource="&dct;description"/>
		<skos:definition>account of the resource</skos:definition>
	</owl:AnnotationProperty>
	
	<owl:AnnotationProperty rdf:about="&dct;issued">
		<rdfs:label>issued</rdfs:label>
		<rdfs:isDefinedBy rdf:resource="&dct;issued"/>
		<skos:definition>date of formal issuance of the resource</skos:definition>
		<cmns-av:usageNote>This annotation is used to describe an artifact such as a controlled vocabulary, ontology, or ontology module.</cmns-av:usageNote>
	</owl:AnnotationProperty>
	
	<owl:AnnotationProperty rdf:about="&dct;license">
		<rdfs:label>license</rdfs:label>
		<rdfs:isDefinedBy rdf:resource="&dct;license"/>
		<skos:definition>legal document giving official permission to do something with the resource</skos:definition>
		<cmns-av:usageNote>This annotation is used to describe an artifact such as a controlled vocabulary, ontology, or ontology module.</cmns-av:usageNote>
	</owl:AnnotationProperty>
	
	<owl:AnnotationProperty rdf:about="&dct;modified">
		<rdfs:label>modified</rdfs:label>
		<rdfs:isDefinedBy rdf:resource="&dct;modified"/>
		<skos:definition>date on which the resource was most recently revised</skos:definition>
	</owl:AnnotationProperty>
	
	<owl:AnnotationProperty rdf:about="&dct;publisher">
		<rdfs:label>publisher</rdfs:label>
		<rdfs:isDefinedBy rdf:resource="&dct;publisher"/>
		<skos:definition>primary party responsible for making the resource available</skos:definition>
		<cmns-av:usageNote>This annotation is used to describe an artifact such as a controlled vocabulary, ontology, or ontology module.</cmns-av:usageNote>
	</owl:AnnotationProperty>
	
	<owl:AnnotationProperty rdf:about="&dct;references">
		<rdfs:label>references</rdfs:label>
		<rdfs:isDefinedBy rdf:resource="&dct;references"/>
		<skos:definition>indicates a related resource that is referenced, cited, or otherwise pointed to by the described resource</skos:definition>
	</owl:AnnotationProperty>
	
	<owl:AnnotationProperty rdf:about="&dct;rights">
		<rdfs:label>rights</rdfs:label>
		<rdfs:isDefinedBy rdf:resource="&dct;rights"/>
		<skos:definition>provides nformation about rights held in and over the resource</skos:definition>
		<cmns-av:usageNote>This annotation is used to describe an artifact such as a controlled vocabulary, ontology, or ontology module.</cmns-av:usageNote>
	</owl:AnnotationProperty>
	
	<owl:AnnotationProperty rdf:about="&dct;source">
		<rdfs:label>source</rdfs:label>
		<rdfs:isDefinedBy rdf:resource="&dct;source"/>
		<skos:definition>related resource from which the described resource is derived</skos:definition>
		<cmns-av:explanatoryNote>The intent is to provide a user with a reference as to how the thing being annotated was derived or arrived at. The source can be a URL to a standard, common dictionary (e.g., Collins, Merriam-Webster, Oxford), a formal reference such as an ISO standard, or similar reference. Or it can be a short description of where the entity being annotated was derived from.</cmns-av:explanatoryNote>
	</owl:AnnotationProperty>
	
	<owl:AnnotationProperty rdf:about="&dct;title">
		<rdfs:label>title</rdfs:label>
		<rdfs:isDefinedBy rdf:resource="&dct;title"/>
		<skos:definition>formal name given to the resource (artifact, such as a controlled vocabulary or ontology)</skos:definition>
		<cmns-av:usageNote>This annotation is used to describe an artifact such as a controlled vocabulary, document, ontology, or ontology module.</cmns-av:usageNote>
	</owl:AnnotationProperty>
	
	<owl:AnnotationProperty rdf:about="&skos;altLabel">
		<rdfs:subPropertyOf rdf:resource="&rdfs;label"/>
		<rdfs:label>alternative label</rdfs:label>
		<rdfs:isDefinedBy rdf:resource="http://www.w3.org/2004/02/skos/core"/>
		<skos:definition>alternative lexical tag for a resource</skos:definition>
	</owl:AnnotationProperty>
	
	<owl:AnnotationProperty rdf:about="&skos;changeNote">
		<rdfs:subPropertyOf rdf:resource="&skos;note"/>
		<rdfs:label>change note</rdfs:label>
		<rdfs:isDefinedBy rdf:resource="http://www.w3.org/2004/02/skos/core"/>
		<skos:definition>note describing a modification to a resource</skos:definition>
	</owl:AnnotationProperty>
	
	<owl:AnnotationProperty rdf:about="&skos;definition">
		<rdfs:subPropertyOf rdf:resource="&skos;note"/>
		<rdfs:label>definition</rdfs:label>
		<rdfs:isDefinedBy rdf:resource="http://www.w3.org/2004/02/skos/core"/>
		<skos:definition>formal statement of the meaning of a resource</skos:definition>
	</owl:AnnotationProperty>
	
	<owl:AnnotationProperty rdf:about="&skos;editorialNote">
		<rdfs:subPropertyOf rdf:resource="&skos;note"/>
		<rdfs:label>editorial note</rdfs:label>
		<rdfs:isDefinedBy rdf:resource="http://www.w3.org/2004/02/skos/core"/>
		<skos:definition>note for an editor, translator, or maintainer of the controlled vocabulary or ontology</skos:definition>
	</owl:AnnotationProperty>
	
	<owl:AnnotationProperty rdf:about="&skos;example">
		<rdfs:subPropertyOf rdf:resource="&skos;note"/>
		<rdfs:label>example</rdfs:label>
		<rdfs:isDefinedBy rdf:resource="http://www.w3.org/2004/02/skos/core"/>
		<skos:definition>illustration of the use of some resource</skos:definition>
	</owl:AnnotationProperty>
	
	<owl:AnnotationProperty rdf:about="&skos;note">
		<rdfs:label>note</rdfs:label>
		<rdfs:isDefinedBy rdf:resource="http://www.w3.org/2004/02/skos/core"/>
		<skos:definition>general remark, for any purpose</skos:definition>
	</owl:AnnotationProperty>
	
	<owl:AnnotationProperty rdf:about="&skos;prefLabel">
		<rdfs:subPropertyOf rdf:resource="&rdfs;label"/>
		<rdfs:label>preferred label</rdfs:label>
		<rdfs:isDefinedBy rdf:resource="http://www.w3.org/2004/02/skos/core"/>
		<skos:definition>preferred lexical label for a resource, in a given language</skos:definition>
	</owl:AnnotationProperty>
	
	<owl:AnnotationProperty rdf:about="&skos;scopeNote">
		<rdfs:subPropertyOf rdf:resource="&skos;note"/>
		<rdfs:label>scope note</rdfs:label>
		<rdfs:isDefinedBy rdf:resource="http://www.w3.org/2004/02/skos/core"/>
		<skos:definition>note that helps to clarify the meaning of something within the overall context of the intended use of the ontology or controlled vocabulary</skos:definition>
	</owl:AnnotationProperty>
	
	<owl:AnnotationProperty rdf:about="&cmns-av;abbreviation">
		<rdfs:subPropertyOf rdf:resource="&cmns-av;synonym"/>
		<rdfs:label>abbreviation</rdfs:label>
		<skos:definition>designation formed by omitting parts from its full form and that denotes the same concept</skos:definition>
		<skos:example>Chemical Symbols: H, O, Mg; Units of Measure: Km, Kg, G</skos:example>
		<skos:note>Abbreviations can be created by removing individual words, or can be acronyms, initialisms, or clipped terms.</skos:note>
		<cmns-av:adaptedFrom>ISO 1087 Terminology work and terminology science - Vocabulary, Second edition, 2019-09</cmns-av:adaptedFrom>
		<cmns-av:adaptedFrom>ISO 31-0 Quantities and units - General principles</cmns-av:adaptedFrom>
		<cmns-av:explanatoryNote>The symbols for quantities are generally single letters of the Latin or Greek alphabet, sometimes with subscripts or other modifying signs. These letters, including those that are members of the Greek alphabet are not symbols for the purposes of this ontology, however, they are abbreviations. Expressions of chemical formulae may, however, include a combination of abbreviations and symbols, as needed to define a given quantity.</cmns-av:explanatoryNote>
	</owl:AnnotationProperty>
	
	<owl:AnnotationProperty rdf:about="&cmns-av;acronym">
		<rdfs:subPropertyOf rdf:resource="&cmns-av;abbreviation"/>
		<rdfs:label>acronym</rdfs:label>
		<skos:definition>abbreviation that is made up of the initial letters of the components of the full form of a term or proper name or from syllables of the full form</skos:definition>
		<skos:example>Examples of acronyms are: laser, ISO, GATT, UNESCO, UNICEF</skos:example>
		<skos:note>Acronyms are frequently pronounced syllabically.</skos:note>
		<cmns-av:adaptedFrom>ISO 1087 Terminology work and terminology science - Vocabulary, Second edition, 2019-09</cmns-av:adaptedFrom>
	</owl:AnnotationProperty>
	
	<owl:AnnotationProperty rdf:about="&cmns-av;adaptedFrom">
		<rdfs:subPropertyOf rdf:resource="&dct;source"/>
		<rdfs:label>adapted from</rdfs:label>
		<skos:definition>document or other source from which a given term (or its definition) was adapted (i.e., compatible with but not quoted); the range for this annotation can be a string, URI, or citation</skos:definition>
		<cmns-av:usageNote>This annotation should be used to indicate that a reference was used, for example, as input to the development of a definition or term but would not be considered infringing on a copyright.</cmns-av:usageNote>
	</owl:AnnotationProperty>
	
	<owl:AnnotationProperty rdf:about="&cmns-av;copyright">
		<rdfs:subPropertyOf rdf:resource="&dct;rights"/>
		<rdfs:label>copyright</rdfs:label>
		<skos:definition>exclusive legal right, given to an originator or an assignee to print, publish, perform, film, or record literary, artistic, or musical material, and to authorize others to do the same</skos:definition>
		<cmns-av:usageNote>This annotation is used to describe an artifact such as a controlled vocabulary, ontology, or ontology module.</cmns-av:usageNote>
	</owl:AnnotationProperty>
	
	<owl:AnnotationProperty rdf:about="&cmns-av;directSource">
		<rdfs:subPropertyOf rdf:resource="&dct;source"/>
		<rdfs:label>direct source</rdfs:label>
		<skos:definition>quoted reference for the subject resource; the range for this annotation can be a string, URI, or bibliographic citation</skos:definition>
	</owl:AnnotationProperty>
	
	<owl:AnnotationProperty rdf:about="&cmns-av;explanatoryNote">
		<rdfs:subPropertyOf rdf:resource="&skos;note"/>
		<rdfs:label>explanatory note</rdfs:label>
		<skos:definition>note that provides additional explanatory material for a resource</skos:definition>
	</owl:AnnotationProperty>
	
	<owl:AnnotationProperty rdf:about="&cmns-av;logicalDefinition">
		<rdfs:subPropertyOf rdf:resource="&skos;definition"/>
		<rdfs:label>logical definition</rdfs:label>
		<skos:definition>definition in the form of a formal expression, such as the mathematical or logic representation, for the resource</skos:definition>
	</owl:AnnotationProperty>
	
	<owl:AnnotationProperty rdf:about="&cmns-av;symbol">
		<rdfs:subPropertyOf rdf:resource="&cmns-av;synonym"/>
		<rdfs:label>symbol</rdfs:label>
		<skos:definition>abbreviation that is a design or mark, or other non-alpha-numeric character(s) used conventionally to represent something, such as a currency or mathematical sign or operator</skos:definition>
	</owl:AnnotationProperty>
	
	<owl:AnnotationProperty rdf:about="&cmns-av;synonym">
		<rdfs:subPropertyOf rdf:resource="&skos;altLabel"/>
		<rdfs:label>synonym</rdfs:label>
		<skos:definition>designation that can be substituted for the primary representation of something</skos:definition>
		<cmns-av:adaptedFrom>ISO 1087 Terminology work and terminology science - Vocabulary, Second edition, 2019-09</cmns-av:adaptedFrom>
	</owl:AnnotationProperty>
	
	<owl:AnnotationProperty rdf:about="&cmns-av;usageNote">
		<rdfs:subPropertyOf rdf:resource="&skos;note"/>
		<rdfs:label>usage note</rdfs:label>
		<skos:definition>note that provides information about how a given resource is used or may be extended</skos:definition>
	</owl:AnnotationProperty>

</rdf:RDF>