<?xml version="1.0" encoding="UTF-8"?>
<!DOCTYPE rdf:RDF [
	<!ENTITY cmns-av "https://www.omg.org/spec/Commons/AnnotationVocabulary/">
	<!ENTITY cmns-cds "https://www.omg.org/spec/Commons/CodesAndCodeSets/">
	<!ENTITY cmns-cls "https://www.omg.org/spec/Commons/Classifiers/">
	<!ENTITY cmns-cmp "https://www.omg.org/spec/Commons/Composites/">
	<!ENTITY cmns-col "https://www.omg.org/spec/Commons/Collections/">
	<!ENTITY cmns-cxtdsg "https://www.omg.org/spec/Commons/ContextualDesignators/">
	<!ENTITY cmns-dsg "https://www.omg.org/spec/Commons/Designators/">
	<!ENTITY cmns-ge "https://www.omg.org/spec/Commons/GovernmentEntities/">
	<!ENTITY cmns-ge-euj "https://www.omg.org/spec/Commons/EuropeanJurisdiction/EUGovernmentEntitiesAndJurisdictions/">
	<!ENTITY cmns-id "https://www.omg.org/spec/Commons/Identifiers/">
	<!ENTITY cmns-org "https://www.omg.org/spec/Commons/Organizations/">
	<!ENTITY cmns-prd "https://www.omg.org/spec/Commons/ProductsAndServices/">
	<!ENTITY cmns-pts "https://www.omg.org/spec/Commons/PartiesAndSituations/">
	<!ENTITY cmns-ra "https://www.omg.org/spec/Commons/RegistrationAuthorities/">
	<!ENTITY cmns-txt "https://www.omg.org/spec/Commons/TextDatatype/">
	<!ENTITY dct "http://purl.org/dc/terms/">
	<!ENTITY idmp-chg "https://spec.pistoiaalliance.org/idmp/ontology/META/ChangeManagement/">
	<!ENTITY idmp-eura "https://spec.pistoiaalliance.org/idmp/ontology/ISO/EuropeanJurisdiction/EuropeanRegistrationAuthorities/">
	<!ENTITY idmp-eurga "https://spec.pistoiaalliance.org/idmp/ontology/ISO/EuropeanJurisdiction/EuropeanRegulatoryAgencies/">
	<!ENTITY idmp-mprd "https://spec.pistoiaalliance.org/idmp/ontology/ISO/ISO11615-MedicinalProducts/">
	<!ENTITY idmp-sub "https://spec.pistoiaalliance.org/idmp/ontology/ISO/ISO11238-Substances/">
	<!ENTITY lcc-lr "https://www.omg.org/spec/LCC/Languages/LanguageRepresentation/">
	<!ENTITY owl "http://www.w3.org/2002/07/owl#">
	<!ENTITY rdf "http://www.w3.org/1999/02/22-rdf-syntax-ns#">
	<!ENTITY rdfs "http://www.w3.org/2000/01/rdf-schema#">
	<!ENTITY skos "http://www.w3.org/2004/02/skos/core#">
	<!ENTITY xsd "http://www.w3.org/2001/XMLSchema#">
]>
<rdf:RDF xml:base="https://spec.pistoiaalliance.org/idmp/ontology/ISO/EuropeanJurisdiction/EuropeanRegistrationAuthorities/"
	xmlns:cmns-av="https://www.omg.org/spec/Commons/AnnotationVocabulary/"
	xmlns:cmns-cds="https://www.omg.org/spec/Commons/CodesAndCodeSets/"
	xmlns:cmns-cls="https://www.omg.org/spec/Commons/Classifiers/"
	xmlns:cmns-cmp="https://www.omg.org/spec/Commons/Composites/"
	xmlns:cmns-col="https://www.omg.org/spec/Commons/Collections/"
	xmlns:cmns-cxtdsg="https://www.omg.org/spec/Commons/ContextualDesignators/"
	xmlns:cmns-dsg="https://www.omg.org/spec/Commons/Designators/"
	xmlns:cmns-ge="https://www.omg.org/spec/Commons/GovernmentEntities/"
	xmlns:cmns-ge-euj="https://www.omg.org/spec/Commons/EuropeanJurisdiction/EUGovernmentEntitiesAndJurisdictions/"
	xmlns:cmns-id="https://www.omg.org/spec/Commons/Identifiers/"
	xmlns:cmns-org="https://www.omg.org/spec/Commons/Organizations/"
	xmlns:cmns-prd="https://www.omg.org/spec/Commons/ProductsAndServices/"
	xmlns:cmns-pts="https://www.omg.org/spec/Commons/PartiesAndSituations/"
	xmlns:cmns-ra="https://www.omg.org/spec/Commons/RegistrationAuthorities/"
	xmlns:cmns-txt="https://www.omg.org/spec/Commons/TextDatatype/"
	xmlns:dct="http://purl.org/dc/terms/"
	xmlns:idmp-chg="https://spec.pistoiaalliance.org/idmp/ontology/META/ChangeManagement/"
	xmlns:idmp-eura="https://spec.pistoiaalliance.org/idmp/ontology/ISO/EuropeanJurisdiction/EuropeanRegistrationAuthorities/"
	xmlns:idmp-eurga="https://spec.pistoiaalliance.org/idmp/ontology/ISO/EuropeanJurisdiction/EuropeanRegulatoryAgencies/"
	xmlns:idmp-mprd="https://spec.pistoiaalliance.org/idmp/ontology/ISO/ISO11615-MedicinalProducts/"
	xmlns:idmp-sub="https://spec.pistoiaalliance.org/idmp/ontology/ISO/ISO11238-Substances/"
	xmlns:lcc-lr="https://www.omg.org/spec/LCC/Languages/LanguageRepresentation/"
	xmlns:owl="http://www.w3.org/2002/07/owl#"
	xmlns:rdf="http://www.w3.org/1999/02/22-rdf-syntax-ns#"
	xmlns:rdfs="http://www.w3.org/2000/01/rdf-schema#"
	xmlns:skos="http://www.w3.org/2004/02/skos/core#"
	xmlns:xsd="http://www.w3.org/2001/XMLSchema#">
	
	<owl:Ontology rdf:about="https://spec.pistoiaalliance.org/idmp/ontology/ISO/EuropeanJurisdiction/EuropeanRegistrationAuthorities/">
		<rdfs:label>European Registration Authorities Ontology</rdfs:label>
		<dct:abstract>The registration authorities ontology provides the registration authorities, registries and related codes that are specific to Europe and needed for identification of substances and medicinal products.</dct:abstract>
		<dct:license rdf:datatype="&xsd;anyURI">https://opensource.org/licenses/MIT</dct:license>
		<owl:imports rdf:resource="https://spec.pistoiaalliance.org/idmp/ontology/ISO/EuropeanJurisdiction/EuropeanRegulatoryAgencies/"/>
		<owl:imports rdf:resource="https://spec.pistoiaalliance.org/idmp/ontology/ISO/ISO11238-Substances/"/>
		<owl:imports rdf:resource="https://spec.pistoiaalliance.org/idmp/ontology/ISO/ISO11615-MedicinalProducts/"/>
		<owl:imports rdf:resource="https://spec.pistoiaalliance.org/idmp/ontology/META/ChangeManagement/"/>
		<owl:imports rdf:resource="https://www.omg.org/spec/Commons/AnnotationVocabulary/"/>
		<owl:imports rdf:resource="https://www.omg.org/spec/Commons/Classifiers/"/>
		<owl:imports rdf:resource="https://www.omg.org/spec/Commons/CodesAndCodeSets/"/>
		<owl:imports rdf:resource="https://www.omg.org/spec/Commons/Collections/"/>
		<owl:imports rdf:resource="https://www.omg.org/spec/Commons/Composites/"/>
		<owl:imports rdf:resource="https://www.omg.org/spec/Commons/ContextualDesignators/"/>
		<owl:imports rdf:resource="https://www.omg.org/spec/Commons/Designators/"/>
		<owl:imports rdf:resource="https://www.omg.org/spec/Commons/EuropeanJurisdiction/EUGovernmentEntitiesAndJurisdictions/"/>
		<owl:imports rdf:resource="https://www.omg.org/spec/Commons/GovernmentEntities/"/>
		<owl:imports rdf:resource="https://www.omg.org/spec/Commons/Identifiers/"/>
		<owl:imports rdf:resource="https://www.omg.org/spec/Commons/Organizations/"/>
		<owl:imports rdf:resource="https://www.omg.org/spec/Commons/PartiesAndSituations/"/>
		<owl:imports rdf:resource="https://www.omg.org/spec/Commons/ProductsAndServices/"/>
		<owl:imports rdf:resource="https://www.omg.org/spec/Commons/RegistrationAuthorities/"/>
		<owl:imports rdf:resource="https://www.omg.org/spec/Commons/TextDatatype/"/>
		<owl:imports rdf:resource="https://www.omg.org/spec/LCC/Languages/LanguageRepresentation/"/>
		<owl:versionIRI rdf:resource="https://spec.pistoiaalliance.org/idmp/ontology/ISO/20230801/EuropeanJurisdiction/EuropeanRegistrationAuthorities/"/>
		<idmp-chg:hasMaturityLevel rdf:resource="&idmp-chg;Provisional"/>
		<cmns-av:copyright>Copyright (c) 2022-2023 EDM Council, Inc.</cmns-av:copyright>
		<cmns-av:copyright>Copyright (c) 2022-2023 Pistoia Alliance, Inc.</cmns-av:copyright>
	</owl:Ontology>
	
	<owl:NamedIndividual rdf:about="&idmp-eura;BritishPharmacologicalSociety">
		<rdf:type rdf:resource="&cmns-org;FormalOrganization"/>
		<rdfs:label>British Pharmacological Society</rdfs:label>
		<rdfs:seeAlso rdf:resource="https://www.bps.ac.uk/"/>
		<skos:definition>not-for-profit organization with a mission to promote and advance the whole spectrum of pharmacology, with over 4,000 members from more than 60 countries worldwide</skos:definition>
		<cmns-av:abbreviation>BPS</cmns-av:abbreviation>
	</owl:NamedIndividual>
	
	<owl:NamedIndividual rdf:about="&idmp-eura;BritishPharmacologicalSocietyAsRegistrationAuthority">
		<rdf:type rdf:resource="&cmns-ra;RegistrationAuthority"/>
		<rdfs:label>British Pharmacological Society as registration authority</rdfs:label>
		<skos:definition>British Pharmacological Society in its role as a Registration Authority (RA)</skos:definition>
		<cmns-av:abbreviation>BPS RA</cmns-av:abbreviation>
		<cmns-cmp:isPlayedBy rdf:resource="&idmp-eura;BritishPharmacologicalSociety"/>
		<cmns-ra:manages rdf:resource="&idmp-eura;InternationalUnionOfBasicAndClinicalPharmacologyGuide"/>
	</owl:NamedIndividual>
	
	<owl:NamedIndividual rdf:about="&idmp-eura;ChemblDatabase">
		<rdf:type rdf:resource="&cmns-ra;Registry"/>
		<rdfs:label>ChEMBL database</rdfs:label>
		<skos:definition>manually curated database of bioactive molecules with drug-like properties</skos:definition>
		<cmns-av:abbreviation>ChEMBL</cmns-av:abbreviation>
		<cmns-av:directSource rdf:resource="https://www.ebi.ac.uk/chembl/"/>
		<cmns-ra:isManagedBy rdf:resource="&idmp-eura;EuropeanMolecularBiologyLaboratoryEuropeanBioinformaticsInstituteRegistrationAuthority"/>
		<lcc-lr:hasTextualName>ChEMBL database</lcc-lr:hasTextualName>
	</owl:NamedIndividual>
	
	<owl:NamedIndividual rdf:about="&idmp-eura;ChemicalEntitiesOfBiologicalInterest">
		<rdf:type rdf:resource="&cmns-ra;Registry"/>
		<rdfs:label>Chemical Entities of Biological Interest</rdfs:label>
		<skos:definition>freely available dictionary of molecular entities focused on &apos;small&apos; chemical compounds</skos:definition>
		<cmns-av:directSource rdf:resource="https://www.ebi.ac.uk/chebi/"/>
		<cmns-ra:isManagedBy rdf:resource="&idmp-eura;EuropeanMolecularBiologyLaboratoryEuropeanBioinformaticsInstituteRegistrationAuthority"/>
		<lcc-lr:hasTextualName>Chemical Entities of Biological Interest (ChEBI)</lcc-lr:hasTextualName>
	</owl:NamedIndividual>
	
	<owl:Class rdf:about="&idmp-eura;ChemicalEntitiesOfBiologicalInterestEntry">
		<rdfs:subClassOf rdf:resource="&cmns-ra;RegistryEntry"/>
		<rdfs:subClassOf>
			<owl:Restriction>
				<owl:onProperty rdf:resource="&cmns-col;isIncludedIn"/>
				<owl:hasValue rdf:resource="&idmp-eura;ChemicalEntitiesOfBiologicalInterest"/>
			</owl:Restriction>
		</rdfs:subClassOf>
		<rdfs:subClassOf>
			<owl:Restriction>
				<owl:onProperty rdf:resource="&cmns-col;comprises"/>
				<owl:someValuesFrom rdf:resource="&idmp-eura;ChemicalEntitiesOfBiologicalInterestIdentifier"/>
			</owl:Restriction>
		</rdfs:subClassOf>
		<rdfs:subClassOf>
			<owl:Restriction>
				<owl:onProperty rdf:resource="&cmns-cxtdsg;appliesTo"/>
				<owl:someValuesFrom rdf:resource="&idmp-sub;Substance"/>
			</owl:Restriction>
		</rdfs:subClassOf>
		<rdfs:label>Chemical Entities of Biological Interest registry entry</rdfs:label>
		<skos:definition>entry in the Chemical Entities of Biological Interest, that includes the Chemical Entities of Biological Interest Identifier used in electronic listing and other regulatory activities</skos:definition>
	</owl:Class>
	
	<owl:Class rdf:about="&idmp-eura;ChemicalEntitiesOfBiologicalInterestIdentifier">
		<rdfs:subClassOf rdf:resource="&idmp-sub;SubstanceCode"/>
		<rdfs:subClassOf>
			<owl:Restriction>
				<owl:onProperty rdf:resource="&cmns-ra;isRegisteredIn"/>
				<owl:hasValue rdf:resource="&idmp-eura;ChemicalEntitiesOfBiologicalInterest"/>
			</owl:Restriction>
		</rdfs:subClassOf>
		<rdfs:subClassOf>
			<owl:Restriction>
				<owl:onProperty rdf:resource="&cmns-ra;hasRegistrationAuthority"/>
				<owl:hasValue rdf:resource="&idmp-eura;EuropeanMolecularBiologyLaboratoryEuropeanBioinformaticsInstituteRegistrationAuthority"/>
			</owl:Restriction>
		</rdfs:subClassOf>
		<rdfs:subClassOf>
			<owl:Restriction>
				<owl:onProperty rdf:resource="&cmns-id;identifies"/>
				<owl:someValuesFrom rdf:resource="&idmp-sub;Substance"/>
			</owl:Restriction>
		</rdfs:subClassOf>
		<rdfs:label>Chemical Entities of Biological Interest identifer</rdfs:label>
		<skos:definition>numeric string that is used to identify records in the Chemical Entities of Biological Interest registry</skos:definition>
		<cmns-av:synonym>ChEBI ID</cmns-av:synonym>
	</owl:Class>
	
	<owl:Class rdf:about="&idmp-eura;EudraClinicalTrialsNumber">
		<rdfs:subClassOf rdf:resource="&idmp-mprd;ClinicalTrialIdentifier"/>
		<rdfs:subClassOf>
			<owl:Restriction>
				<owl:onProperty rdf:resource="&cmns-ra;hasRegistrationAuthority"/>
				<owl:hasValue rdf:resource="&idmp-eura;EuropeanMedicinesAgencyRegistrationAuthority"/>
			</owl:Restriction>
		</rdfs:subClassOf>
		<rdfs:subClassOf>
			<owl:Restriction>
				<owl:onProperty rdf:resource="&cmns-ra;isRegisteredIn"/>
				<owl:hasValue rdf:resource="&idmp-eura;EuropeanUnionClinicalTrialsRegister"/>
			</owl:Restriction>
		</rdfs:subClassOf>
		<rdfs:label>Eudra clinical trials number</rdfs:label>
		<skos:definition>unique code assigned to clinical trials in the EU Clinical Trials Register</skos:definition>
		<cmns-av:abbreviation>EudraCT Number</cmns-av:abbreviation>
	</owl:Class>
	
	<owl:Class rdf:about="&idmp-eura;EudraVigilanceCode">
		<rdfs:subClassOf rdf:resource="&idmp-sub;SubstanceCode"/>
		<rdfs:subClassOf>
			<owl:Restriction>
				<owl:onProperty rdf:resource="&cmns-ra;hasRegistrationAuthority"/>
				<owl:hasValue rdf:resource="&idmp-eura;EuropeanMedicinesAgencyRegistrationAuthority"/>
			</owl:Restriction>
		</rdfs:subClassOf>
		<rdfs:subClassOf>
			<owl:Restriction>
				<owl:onProperty rdf:resource="&cmns-ra;isRegisteredIn"/>
				<owl:hasValue rdf:resource="&idmp-eura;ExtendedEudraVigilanceMedicinalProductDictionary"/>
			</owl:Restriction>
		</rdfs:subClassOf>
		<rdfs:subClassOf>
			<owl:Restriction>
				<owl:onProperty rdf:resource="&cmns-id;identifies"/>
				<owl:someValuesFrom rdf:resource="&idmp-sub;Substance"/>
			</owl:Restriction>
		</rdfs:subClassOf>
		<rdfs:label>EudraVigilance code</rdfs:label>
		<skos:definition>unique code assigned to any substance entered in the eXtended EudraVigilance Medicinal Product Dictionary (XEVMPD)</skos:definition>
		<skos:note>An EV Code for a substance is generated after the substance has been inserted successfully in the XEVMPD via an eXtended EudraVigilance Product Report Message (XEVPRM).</skos:note>
		<skos:note>The XEVMPD is a format to electronically submit to the European Medicines Agency (EMA) information on substances, referentials and medicinal products for human use authorized in the European Union as referred into the Article 57 (2) of the regulation 726/2004. It was developed by the EMA in collaboration with the EudraVigilance implementation fora.</skos:note>
		<cmns-av:abbreviation>EV Code</cmns-av:abbreviation>
		<cmns-av:abbreviation>EVMPD Code</cmns-av:abbreviation>
		<cmns-av:abbreviation>XEVMPD Code</cmns-av:abbreviation>
		<cmns-av:directSource>ISO 11238:2018 Health informatics - Identification of medicinal products (IDMP) - Data elements and structures for the unique identification and exchange of regulated information on substances, clause A.1.7</cmns-av:directSource>
	</owl:Class>
	
	<owl:NamedIndividual rdf:about="&idmp-eura;EuropeanChemicalsAgencyRegistrationAuthority">
		<rdf:type rdf:resource="&cmns-ra;RegistrationAuthority"/>
		<rdfs:label>European Chemicals Agency registration authority</rdfs:label>
		<skos:definition>European Chemicals Agency in its role as a Registration Authority (RA)</skos:definition>
		<cmns-cmp:isPlayedBy rdf:resource="&idmp-eurga;EuropeanChemicalsAgency"/>
		<cmns-ra:manages rdf:resource="&idmp-eura;EuropeanInventoryOfExistingCommercialChemicalSubstances"/>
	</owl:NamedIndividual>
	
	<owl:NamedIndividual rdf:about="&idmp-eura;EuropeanCommissionFoodAdditivesDatabase">
		<rdf:type rdf:resource="&cmns-ra;Registry"/>
		<rdfs:label>European Commission Food Additives Database</rdfs:label>
		<skos:definition>database that informs about the food additives approved for use in food in the EU and their conditions of use</skos:definition>
		<cmns-av:directSource rdf:resource="https://ec.europa.eu/food/safety/food-improvement-agents/additives/database_en"/>
		<cmns-av:explanatoryNote>It is based on the Union list of food additives.</cmns-av:explanatoryNote>
		<cmns-ra:isManagedBy rdf:resource="&idmp-eura;EuropeanDirectorateForTheQualityOfMedicinesAndHealthcareRegistrationAuthority"/>
		<lcc-lr:hasTextualName>European Commission Food Additives Database</lcc-lr:hasTextualName>
	</owl:NamedIndividual>
	
	<owl:NamedIndividual rdf:about="&idmp-eura;EuropeanCommissionScientificCommitteeOnConsumerSafetyOpinions">
		<rdf:type rdf:resource="&cmns-ra;Registry"/>
		<rdfs:label>European Commission Scientific Committee on Consumer Safety Opinions</rdfs:label>
		<skos:definition>registry that provides opinions on health and safety risks (chemical, biological, mechanical and other physical risks) of non-food consumer products (e.g. cosmetic products and their ingredients, toys, textiles, clothing, personal care and household products) and services (e.g. tattooing, artificial sun tanning)</skos:definition>
		<cmns-av:directSource rdf:resource="https://ec.europa.eu/health/scientific-committees/scientific-committee-consumer-safety-sccs_en"/>
		<cmns-ra:isManagedBy rdf:resource="&idmp-eura;EuropeanCommissionScientificCommitteeOnConsumerSafetyRegistrationAuthority"/>
		<lcc-lr:hasTextualName>European Commission Scientific Committee on Consumer Safety Opinions</lcc-lr:hasTextualName>
	</owl:NamedIndividual>
	
	<owl:NamedIndividual rdf:about="&idmp-eura;EuropeanCommissionScientificCommitteeOnConsumerSafetyRegistrationAuthority">
		<rdf:type rdf:resource="&cmns-ra;RegistrationAuthority"/>
		<rdfs:label>European Commission Scientific Committee on Consumer Safety registration authority</rdfs:label>
		<skos:definition>European Commission Scientific Committee on Consumer Safety in its role as a Registration Authority (RA)</skos:definition>
		<cmns-cmp:isPlayedBy rdf:resource="&idmp-eurga;EuropeanCommissionScientificCommitteeOnConsumerSafety"/>
		<cmns-ra:manages rdf:resource="&idmp-eura;EuropeanCommissionScientificCommitteeOnConsumerSafetyOpinions"/>
	</owl:NamedIndividual>
	
	<owl:Class rdf:about="&idmp-eura;EuropeanCommunityNumber">
		<rdfs:subClassOf rdf:resource="&idmp-sub;SubstanceCode"/>
		<rdfs:subClassOf>
			<owl:Restriction>
				<owl:onProperty rdf:resource="&cmns-ra;hasRegistrationAuthority"/>
				<owl:hasValue rdf:resource="&idmp-eura;EuropeanChemicalsAgencyRegistrationAuthority"/>
			</owl:Restriction>
		</rdfs:subClassOf>
		<rdfs:subClassOf>
			<owl:Restriction>
				<owl:onProperty rdf:resource="&cmns-ra;isRegisteredIn"/>
				<owl:hasValue rdf:resource="&idmp-eura;EuropeanInventoryOfExistingCommercialChemicalSubstances"/>
			</owl:Restriction>
		</rdfs:subClassOf>
		<rdfs:subClassOf>
			<owl:Restriction>
				<owl:onProperty rdf:resource="&cmns-id;identifies"/>
				<owl:someValuesFrom rdf:resource="&idmp-sub;Substance"/>
			</owl:Restriction>
		</rdfs:subClassOf>
		<rdfs:label>European community number</rdfs:label>
		<skos:definition>unique seven digit identifer assigned to substances for regulatory purposes by the European Chemicals Agency</skos:definition>
		<cmns-av:synonym>EC number</cmns-av:synonym>
	</owl:Class>
	
	<owl:NamedIndividual rdf:about="&idmp-eura;EuropeanDirectorateForTheQualityOfMedicinesAndHealthcareKnowledgeDatabase">
		<rdf:type rdf:resource="&cmns-ra;Registry"/>
		<rdfs:label>European Directorate for the Quality of Medicines and Healthcare Knowledge Database</rdfs:label>
		<skos:definition>repository managed by the European Directorate for the Quality of Medicines and Healthcare that provides information on a given substance or general method of analysis</skos:definition>
		<cmns-av:directSource rdf:resource="https://www.edqm.eu/en/knowledge-database"/>
		<cmns-ra:isManagedBy rdf:resource="&idmp-eura;EuropeanDirectorateForTheQualityOfMedicinesAndHealthcareRegistrationAuthority"/>
		<lcc-lr:hasTextualName>European Directorate for the Quality of Medicines and Healthcare Knowledge Database</lcc-lr:hasTextualName>
	</owl:NamedIndividual>
	
	<owl:NamedIndividual rdf:about="&idmp-eura;EuropeanDirectorateForTheQualityOfMedicinesAndHealthcareRegistrationAuthority">
		<rdf:type rdf:resource="&cmns-ra;RegistrationAuthority"/>
		<rdfs:label>European Directorate for the Quality of Medicines and Healthcare registration authority</rdfs:label>
		<skos:definition>European Directorate for the Quality of Medicines and Healthcare in its role as a Registration Authority (RA)</skos:definition>
		<cmns-cmp:isPlayedBy rdf:resource="&idmp-eurga;EuropeanDirectorateForTheQualityOfMedicinesAndHealthcare"/>
		<cmns-ra:manages rdf:resource="&idmp-eura;EuropeanCommissionFoodAdditivesDatabase"/>
		<cmns-ra:manages rdf:resource="&idmp-eura;EuropeanDirectorateForTheQualityOfMedicinesAndHealthcareKnowledgeDatabase"/>
	</owl:NamedIndividual>
	
	<owl:NamedIndividual rdf:about="&idmp-eura;EuropeanInventoryOfExistingCommercialChemicalSubstances">
		<rdf:type rdf:resource="&cmns-ra;Registry"/>
		<rdfs:label>European inventory of existing commercial chemical substances</rdfs:label>
		<skos:definition>legacy repository consisting of an inventory of substances that were deemed to be available on the European Community market between 1 January 1971 and 18 September 1981</skos:definition>
		<cmns-av:abbreviation>EINECS</cmns-av:abbreviation>
		<cmns-av:directSource rdf:resource="https://echa.europa.eu/information-on-chemicals/ec-inventory"/>
		<cmns-ra:isManagedBy rdf:resource="&idmp-eura;EuropeanChemicalsAgencyRegistrationAuthority"/>
		<lcc-lr:hasTextualName>EINECS (European inventory of existing commercial chemical substances)</lcc-lr:hasTextualName>
	</owl:NamedIndividual>
	
	<owl:Class rdf:about="&idmp-eura;EuropeanInventoryOfExistingCommercialChemicalSubstancesEntry">
		<rdfs:subClassOf rdf:resource="&cmns-ra;RegistryEntry"/>
		<rdfs:subClassOf>
			<owl:Restriction>
				<owl:onProperty rdf:resource="&cmns-col;isIncludedIn"/>
				<owl:hasValue rdf:resource="&idmp-eura;EuropeanInventoryOfExistingCommercialChemicalSubstances"/>
			</owl:Restriction>
		</rdfs:subClassOf>
		<rdfs:subClassOf>
			<owl:Restriction>
				<owl:onProperty rdf:resource="&cmns-col;comprises"/>
				<owl:someValuesFrom rdf:resource="&idmp-eura;EuropeanCommunityNumber"/>
			</owl:Restriction>
		</rdfs:subClassOf>
		<rdfs:subClassOf>
			<owl:Restriction>
				<owl:onProperty rdf:resource="&cmns-cxtdsg;appliesTo"/>
				<owl:someValuesFrom rdf:resource="&idmp-sub;Substance"/>
			</owl:Restriction>
		</rdfs:subClassOf>
		<rdfs:label>European inventory of existing commercial chemical substances entry</rdfs:label>
		<skos:definition>entry in the European Inventory of Existing Commercial chemical Substances, that includes the European Community Number used in electronic listing and other regulatory activities</skos:definition>
		<cmns-av:abbreviation>EINECS entry</cmns-av:abbreviation>
	</owl:Class>
	
	<owl:NamedIndividual rdf:about="&idmp-eura;EuropeanMedicinesAgencyRegistrationAuthority">
		<rdf:type rdf:resource="&cmns-ra;RegistrationAuthority"/>
		<rdfs:label>European Medicines Agency Registration Authority</rdfs:label>
		<skos:definition>European Medicines Agency (EMA) in its role as a Registration Authority (RA), which is a function of the eXtended EudraVigilance Medicinal Product Dictionary (XEVMPD) for registration of substances</skos:definition>
		<cmns-av:abbreviation>EMA XEVMPD RA</cmns-av:abbreviation>
		<cmns-av:adaptedFrom>ISO 11238:2018 Health informatics - Identification of medicinal products (IDMP) - Data elements and structures for the unique identification and exchange of regulated information on substances, clause A.1.7</cmns-av:adaptedFrom>
		<cmns-cmp:isPlayedBy rdf:resource="&idmp-eurga;EuropeanMedicinesAgency"/>
		<cmns-ra:manages rdf:resource="&idmp-eura;EuropeanPublicAssessmentReports"/>
		<cmns-ra:manages rdf:resource="&idmp-eura;EuropeanUnionClinicalTrialsRegister"/>
		<cmns-ra:manages rdf:resource="&idmp-eura;ExtendedEudraVigilanceMedicinalProductDictionary"/>
		<cmns-ra:manages rdf:resource="&idmp-eura;SummaryOfProductCharacteristics"/>
	</owl:NamedIndividual>
	
	<owl:NamedIndividual rdf:about="&idmp-eura;EuropeanMolecularBiologyLaboratory">
		<rdf:type rdf:resource="&cmns-org;FormalOrganization"/>
		<rdfs:label>European Molecular Biology Laboratory</rdfs:label>
		<rdfs:seeAlso rdf:resource="https://www.embl.org/about/"/>
		<skos:definition>not-for-profit organization that is Europe&apos;s leading life sciences laboratory, operating six sites across Europe each with its own research units, services and facilities</skos:definition>
		<cmns-av:abbreviation>EMBL</cmns-av:abbreviation>
	</owl:NamedIndividual>
	
	<owl:NamedIndividual rdf:about="&idmp-eura;EuropeanMolecularBiologyLaboratoryEuropeanBioinformaticsInstitute">
		<rdf:type rdf:resource="&cmns-org;OrganizationalSubUnit"/>
		<rdfs:label>European Molecular Biology Laboratory, European Bioinformatics Institute</rdfs:label>
		<rdfs:seeAlso rdf:resource="https://www.ebi.ac.uk/"/>
		<skos:definition>institute that is part of the European Molecular Biology Laboratory that helps scientists realise the potential of big data in biology, exploiting complex information to make discoveries that benefit humankind</skos:definition>
		<cmns-av:abbreviation>EMBL-EBI</cmns-av:abbreviation>
		<cmns-col:isPartOf rdf:resource="&idmp-eura;EuropeanMolecularBiologyLaboratory"/>
	</owl:NamedIndividual>
	
	<owl:NamedIndividual rdf:about="&idmp-eura;EuropeanMolecularBiologyLaboratoryEuropeanBioinformaticsInstituteRegistrationAuthority">
		<rdf:type rdf:resource="&cmns-ra;RegistrationAuthority"/>
		<rdfs:label>European Molecular Biology Laboratory European Bioinformatics Institute registration authority</rdfs:label>
		<skos:definition>European Molecular Biology Laboratory European Bioinformatics Institute in its role as a Registration Authority (RA)</skos:definition>
		<cmns-av:abbreviation>EMBL-EBI RA</cmns-av:abbreviation>
		<cmns-cmp:isPlayedBy rdf:resource="&idmp-eura;EuropeanMolecularBiologyLaboratoryEuropeanBioinformaticsInstitute"/>
		<cmns-ra:manages rdf:resource="&idmp-eura;EuropeanInventoryOfExistingCommercialChemicalSubstances"/>
	</owl:NamedIndividual>
	
	<owl:NamedIndividual rdf:about="&idmp-eura;EuropeanPublicAssessmentReports">
		<rdf:type rdf:resource="&cmns-ra;Registry"/>
		<rdfs:label>european public assessment reports</rdfs:label>
		<cmns-av:directSource rdf:resource="https://www.ema.europa.eu/en/glossary/european-public-assessment-report"/>
		<cmns-ra:isManagedBy rdf:resource="&idmp-eura;EuropeanMedicinesAgencyRegistrationAuthority"/>
		<lcc-lr:hasTextualName>European public assessment reports</lcc-lr:hasTextualName>
	</owl:NamedIndividual>
	
	<owl:NamedIndividual rdf:about="&idmp-eura;EuropeanUnionClinicalTrialsRegister">
		<rdf:type rdf:resource="&cmns-ra;Registry"/>
		<rdfs:label>European Union Clinical Trials Register</rdfs:label>
		<skos:definition>register that contains information on interventional clinical trials on medicines conducted in the European Union (EU), or the European Economic Area (EEA) which started after 1 May 2004</skos:definition>
		<cmns-av:directSource rdf:resource="https://www.clinicaltrialsregister.eu/about.html"/>
		<cmns-ra:isManagedBy rdf:resource="&idmp-eura;EuropeanMedicinesAgencyRegistrationAuthority"/>
		<lcc-lr:hasTextualName>European Union Clinical Trials Register</lcc-lr:hasTextualName>
	</owl:NamedIndividual>
	
	<owl:NamedIndividual rdf:about="&idmp-eura;ExtendedEudraVigilanceMedicinalProductDictionary">
		<rdf:type rdf:resource="&cmns-ra;Registry"/>
		<rdfs:label>eXtended EudraVigilance Medicinal Product Dictionary</rdfs:label>
		<skos:definition>registry that was designed to support the collection, reporting, coding and evaluation of authorized and investigational medicinal product and substance information in a standardized and structured way</skos:definition>
		<cmns-av:abbreviation>XEVMPD</cmns-av:abbreviation>
		<cmns-av:adaptedFrom>ISO 11238:2018 Health informatics - Identification of medicinal products (IDMP) - Data elements and structures for the unique identification and exchange of regulated information on substances, clause A.1.7</cmns-av:adaptedFrom>
		<cmns-ra:isManagedBy rdf:resource="&idmp-eura;EuropeanMedicinesAgencyRegistrationAuthority"/>
		<lcc-lr:hasTextualName>eXtended EudraVigilance Medicinal Product Dictionary</lcc-lr:hasTextualName>
	</owl:NamedIndividual>
	
	<owl:Class rdf:about="&idmp-eura;ExtendedEudraVigilanceMedicinalProductDictionaryEntry">
		<rdfs:subClassOf rdf:resource="&cmns-ra;RegistryEntry"/>
		<rdfs:subClassOf>
			<owl:Restriction>
				<owl:onProperty rdf:resource="&cmns-col;isIncludedIn"/>
				<owl:hasValue rdf:resource="&idmp-eura;ExtendedEudraVigilanceMedicinalProductDictionary"/>
			</owl:Restriction>
		</rdfs:subClassOf>
		<rdfs:subClassOf>
			<owl:Restriction>
				<owl:onProperty rdf:resource="&cmns-col;comprises"/>
				<owl:someValuesFrom rdf:resource="&idmp-eura;EudraVigilanceCode"/>
			</owl:Restriction>
		</rdfs:subClassOf>
		<rdfs:subClassOf>
			<owl:Restriction>
				<owl:onProperty rdf:resource="&cmns-cxtdsg;appliesTo"/>
				<owl:someValuesFrom rdf:resource="&idmp-sub;Substance"/>
			</owl:Restriction>
		</rdfs:subClassOf>
		<rdfs:label>eXtended EudraVigilance Medicinal Product Dictionary registry entry</rdfs:label>
		<skos:definition>entry in the eXtended EudraVigilance Medicinal Product Dictionary (XEVMPD) registry, that includes the EudraVigilance codes (EV codes) used in the electronic product dictionary and for other regulatory activities</skos:definition>
		<cmns-av:adaptedFrom>ISO 11238:2018 Health informatics - Identification of medicinal products (IDMP) - Data elements and structures for the unique identification and exchange of regulated information on substances, clause A.1.7</cmns-av:adaptedFrom>
	</owl:Class>
	
	<owl:NamedIndividual rdf:about="&idmp-eura;ExtendedEudraVigilanceMedicinalProductDictionaryService">
		<rdf:type rdf:resource="&cmns-ra;RegistrationService"/>
		<rdfs:label>eXtended EudraVigilance Medicinal Product Dictionary service</rdfs:label>
		<skos:definition>service for the collection, reporting, coding and evaluation of authorized and investigational medicinal product and substance information in a standardized and structured way</skos:definition>
		<cmns-av:abbreviation>XEVMPD service</cmns-av:abbreviation>
		<cmns-av:adaptedFrom>ISO 11238:2018 Health informatics - Identification of medicinal products (IDMP) - Data elements and structures for the unique identification and exchange of regulated information on substances, clause A.1.7</cmns-av:adaptedFrom>
		<cmns-prd:isProvidedBy rdf:resource="&idmp-eura;EuropeanMedicinesAgencyRegistrationAuthority"/>
	</owl:NamedIndividual>
	
	<owl:NamedIndividual rdf:about="&idmp-eura;InternationalUnionOfBasicAndClinicalPharmacologyGuide">
		<rdf:type rdf:resource="&cmns-ra;Registry"/>
		<rdfs:label>International Union of Basic and Clinical Pharmacology Guide</rdfs:label>
		<skos:definition>expert-curated resource of ligand-activity-target relationships, the majority of which come from high-quality pharmacological and medicinal chemistry literature</skos:definition>
		<cmns-av:directSource rdf:resource="https://www.guidetopharmacology.org/"/>
		<cmns-ra:isManagedBy rdf:resource="&idmp-eura;BritishPharmacologicalSocietyAsRegistrationAuthority"/>
		<lcc-lr:hasTextualName>International Union of Basic and Clinical Pharmacology Guide</lcc-lr:hasTextualName>
	</owl:NamedIndividual>
	
	<owl:Class rdf:about="&idmp-eura;MedDRAIdentifier">
		<rdfs:subClassOf rdf:resource="&cmns-ra;RegisteredIdentifier"/>
		<rdfs:subClassOf>
			<owl:Restriction>
				<owl:onProperty rdf:resource="&cmns-ra;isRegisteredIn"/>
				<owl:hasValue rdf:resource="&idmp-eura;MedicalDictionaryForRegulatoryActivities"/>
			</owl:Restriction>
		</rdfs:subClassOf>
		<rdfs:subClassOf>
			<owl:Restriction>
				<owl:onProperty rdf:resource="&cmns-id;identifies"/>
				<owl:onClass rdf:resource="&idmp-eura;MedDRATerm"/>
				<owl:qualifiedCardinality rdf:datatype="&xsd;nonNegativeInteger">1</owl:qualifiedCardinality>
			</owl:Restriction>
		</rdfs:subClassOf>
		<rdfs:label>MedDRA identifier</rdfs:label>
		<skos:definition>identifier for terms defining medical condition that are registered in the Medical Dictionary for Regulatory Activities registry</skos:definition>
	</owl:Class>
	
	<owl:Class rdf:about="&idmp-eura;MedDRATerm">
		<rdfs:subClassOf rdf:resource="&cmns-dsg;Designation"/>
		<rdfs:subClassOf>
			<owl:Restriction>
				<owl:onProperty rdf:resource="&cmns-ra;isRegisteredIn"/>
				<owl:hasValue rdf:resource="&idmp-eura;MedicalDictionaryForRegulatoryActivities"/>
			</owl:Restriction>
		</rdfs:subClassOf>
		<rdfs:subClassOf>
			<owl:Restriction>
				<owl:onProperty rdf:resource="&cmns-cls;isClassifiedBy"/>
				<owl:onClass rdf:resource="&idmp-eura;MedDRATermClassifier"/>
				<owl:qualifiedCardinality rdf:datatype="&xsd;nonNegativeInteger">1</owl:qualifiedCardinality>
			</owl:Restriction>
		</rdfs:subClassOf>
		<rdfs:label>MedDRA term</rdfs:label>
		<skos:definition>designation (term) that is registered in the Medical Dictionary for Regulatory Activities registry</skos:definition>
	</owl:Class>
	
	<owl:Class rdf:about="&idmp-eura;MedDRATermClassifier">
		<rdfs:subClassOf rdf:resource="&cmns-cls;Classifier"/>
		<rdfs:subClassOf rdf:resource="&cmns-cds;CodeElement"/>
		<rdfs:subClassOf>
			<owl:Restriction>
				<owl:onProperty rdf:resource="&cmns-cls;classifies"/>
				<owl:someValuesFrom rdf:resource="&idmp-eura;MedDRATerm"/>
			</owl:Restriction>
		</rdfs:subClassOf>
		<rdfs:subClassOf>
			<owl:Restriction>
				<owl:onProperty rdf:resource="&cmns-dsg;denotes"/>
				<owl:someValuesFrom rdf:resource="&idmp-eura;MedDRATerm"/>
			</owl:Restriction>
		</rdfs:subClassOf>
		<rdfs:label>MedDRA term classifier</rdfs:label>
		<skos:definition>clasifier indicating that a term appears at a particular level in the hierarchy of terms in the Medical Dictionary for Regulatory Activities registry</skos:definition>
		<skos:note>Multiple MedDRA terms may be classified at the same level.</skos:note>
	</owl:Class>
	
	<owl:NamedIndividual rdf:about="&idmp-eura;MedDRATermClassifier-HighLevelGroupTerm">
		<rdf:type rdf:resource="&idmp-eura;MedDRATermClassifier"/>
		<rdf:type rdf:resource="&cmns-cds;CodeElement"/>
		<rdfs:label>MedDRA term classifier - high level group term</rdfs:label>
		<cmns-av:acronym>HLGT</cmns-av:acronym>
		<cmns-col:isMemberOf rdf:resource="&idmp-eura;MedicalDictionaryForRegulatoryActivities-ClassificationScheme"/>
		<cmns-dsg:isDefinedIn rdf:resource="&idmp-eura;MedicalDictionaryForRegulatoryActivities-ClassificationScheme"/>
		<cmns-txt:hasTextValue>HLGT</cmns-txt:hasTextValue>
	</owl:NamedIndividual>
	
	<owl:NamedIndividual rdf:about="&idmp-eura;MedDRATermClassifier-HighLevelTerm">
		<rdf:type rdf:resource="&idmp-eura;MedDRATermClassifier"/>
		<rdf:type rdf:resource="&cmns-cds;CodeElement"/>
		<rdfs:label>MedDRA term classifier - high level term</rdfs:label>
		<cmns-av:acronym>HLT</cmns-av:acronym>
		<cmns-col:isMemberOf rdf:resource="&idmp-eura;MedicalDictionaryForRegulatoryActivities-ClassificationScheme"/>
		<cmns-dsg:isDefinedIn rdf:resource="&idmp-eura;MedicalDictionaryForRegulatoryActivities-ClassificationScheme"/>
		<cmns-txt:hasTextValue>HLT</cmns-txt:hasTextValue>
	</owl:NamedIndividual>
	
	<owl:NamedIndividual rdf:about="&idmp-eura;MedDRATermClassifier-LowestLevelTerm">
		<rdf:type rdf:resource="&idmp-eura;MedDRATermClassifier"/>
		<rdf:type rdf:resource="&cmns-cds;CodeElement"/>
		<rdfs:label>MedDRA term classifier - lowest level term</rdfs:label>
		<cmns-av:acronym>LLT</cmns-av:acronym>
		<cmns-col:isMemberOf rdf:resource="&idmp-eura;MedicalDictionaryForRegulatoryActivities-ClassificationScheme"/>
		<cmns-dsg:isDefinedIn rdf:resource="&idmp-eura;MedicalDictionaryForRegulatoryActivities-ClassificationScheme"/>
		<cmns-txt:hasTextValue>LLT</cmns-txt:hasTextValue>
	</owl:NamedIndividual>
	
	<owl:NamedIndividual rdf:about="&idmp-eura;MedDRATermClassifier-PreferredTerm">
		<rdf:type rdf:resource="&idmp-eura;MedDRATermClassifier"/>
		<rdf:type rdf:resource="&cmns-cds;CodeElement"/>
		<rdfs:label>MedDRA term classifier - preferred term</rdfs:label>
		<cmns-av:acronym>PT</cmns-av:acronym>
		<cmns-col:isMemberOf rdf:resource="&idmp-eura;MedicalDictionaryForRegulatoryActivities-ClassificationScheme"/>
		<cmns-dsg:isDefinedIn rdf:resource="&idmp-eura;MedicalDictionaryForRegulatoryActivities-ClassificationScheme"/>
		<cmns-txt:hasTextValue>PT</cmns-txt:hasTextValue>
	</owl:NamedIndividual>
	
	<owl:NamedIndividual rdf:about="&idmp-eura;MedDRATermClassifier-SystemOrganClass">
		<rdf:type rdf:resource="&idmp-eura;MedDRATermClassifier"/>
		<rdf:type rdf:resource="&cmns-cds;CodeElement"/>
		<rdfs:label>MedDRA term classifier - system organ class</rdfs:label>
		<cmns-av:acronym>SOC</cmns-av:acronym>
		<cmns-col:isMemberOf rdf:resource="&idmp-eura;MedicalDictionaryForRegulatoryActivities-ClassificationScheme"/>
		<cmns-dsg:isDefinedIn rdf:resource="&idmp-eura;MedicalDictionaryForRegulatoryActivities-ClassificationScheme"/>
		<cmns-txt:hasTextValue>SOC</cmns-txt:hasTextValue>
	</owl:NamedIndividual>
	
	<owl:NamedIndividual rdf:about="&idmp-eura;MedicalDictionaryForRegulatoryActivities">
		<rdf:type rdf:resource="&cmns-ra;Registry"/>
		<rdfs:label>Medical Dictionary for Regulatory Activities</rdfs:label>
		<dct:source rdf:resource="https://www.meddra.org/"/>
		<skos:definition>The International Council for Harmonisation of Technical Requirements for Pharmaceuticals for Human Use (ICH) developed MedDRA, a rich and highly specific standardised medical terminology to facilitate sharing of regulatory information internationally for medical products used by humans.</skos:definition>
		<cmns-av:abbreviation>MedDRA</cmns-av:abbreviation>
	</owl:NamedIndividual>
	
	<owl:NamedIndividual rdf:about="&idmp-eura;MedicalDictionaryForRegulatoryActivities-ClassificationScheme">
		<rdf:type rdf:resource="&cmns-cls;ClassificationScheme"/>
		<rdf:type rdf:resource="&cmns-cds;CodeSet"/>
		<rdfs:label>Medical Dictionary for Regulatory Activities classification scheme</rdfs:label>
		<dct:source rdf:resource="https://www.meddra.org/"/>
		<skos:definition>system for classifying medical terminology that is directly specified in the Medical Dictionary for Regulatory Activities</skos:definition>
	</owl:NamedIndividual>
	
	<owl:Class rdf:about="&idmp-eura;SPOR-OrganisationManagementSystemIdentifier">
		<rdfs:subClassOf rdf:resource="&cmns-ra;RegisteredIdentifier"/>
		<rdfs:subClassOf>
			<owl:Restriction>
				<owl:onProperty rdf:resource="&cmns-ra;isRegisteredIn"/>
				<owl:hasValue rdf:resource="&idmp-eura;SPOROrganisationManagementSystem"/>
			</owl:Restriction>
		</rdfs:subClassOf>
		<rdfs:subClassOf>
			<owl:Restriction>
				<owl:onProperty rdf:resource="&cmns-id;identifies"/>
				<owl:onClass rdf:resource="&idmp-eura;SPOR-OrganisationManagementSystemTerm"/>
				<owl:qualifiedCardinality rdf:datatype="&xsd;nonNegativeInteger">1</owl:qualifiedCardinality>
			</owl:Restriction>
		</rdfs:subClassOf>
		<rdfs:label>SPOR organisation management service identifier</rdfs:label>
		<skos:definition>identifier for terms defining organisations that are registered in the SPOR organisation management services registry</skos:definition>
	</owl:Class>
	
	<owl:Class rdf:about="&idmp-eura;SPOR-OrganisationManagementSystemTerm">
		<rdfs:subClassOf rdf:resource="&cmns-dsg;Designation"/>
		<rdfs:subClassOf>
			<owl:Restriction>
				<owl:onProperty rdf:resource="&cmns-ra;isRegisteredIn"/>
				<owl:hasValue rdf:resource="&idmp-eura;SPOROrganisationManagementSystem"/>
			</owl:Restriction>
		</rdfs:subClassOf>
		<rdfs:label>SPOR organisation management system term</rdfs:label>
		<skos:definition>designation (term) that is registered in the SPOR organisation management services registry</skos:definition>
	</owl:Class>
	
	<owl:Class rdf:about="&idmp-eura;SPOR-ProductManagementSystemIdentifier">
		<rdfs:subClassOf rdf:resource="&cmns-ra;RegisteredIdentifier"/>
		<rdfs:subClassOf>
			<owl:Restriction>
				<owl:onProperty rdf:resource="&cmns-ra;isRegisteredIn"/>
				<owl:hasValue rdf:resource="&idmp-eura;SPORProductManagementSystem"/>
			</owl:Restriction>
		</rdfs:subClassOf>
		<rdfs:subClassOf>
			<owl:Restriction>
				<owl:onProperty rdf:resource="&cmns-id;identifies"/>
				<owl:onClass rdf:resource="&idmp-eura;SPOR-ProductManagementSystemTerm"/>
				<owl:qualifiedCardinality rdf:datatype="&xsd;nonNegativeInteger">1</owl:qualifiedCardinality>
			</owl:Restriction>
		</rdfs:subClassOf>
		<rdfs:label>SPOR product management service identifier</rdfs:label>
		<skos:definition>identifier for terms defining products that are registered in the SPOR product management services registry</skos:definition>
	</owl:Class>
	
	<owl:Class rdf:about="&idmp-eura;SPOR-ProductManagementSystemTerm">
		<rdfs:subClassOf rdf:resource="&cmns-dsg;Designation"/>
		<rdfs:subClassOf>
			<owl:Restriction>
				<owl:onProperty rdf:resource="&cmns-ra;isRegisteredIn"/>
				<owl:hasValue rdf:resource="&idmp-eura;SPORProductManagementSystem"/>
			</owl:Restriction>
		</rdfs:subClassOf>
		<rdfs:label>SPOR product management system term</rdfs:label>
		<skos:definition>designation (term) that is registered in the SPOR product management services registry</skos:definition>
	</owl:Class>
	
	<owl:Class rdf:about="&idmp-eura;SPOR-ReferentialsManagementSystemIdentifier">
		<rdfs:subClassOf rdf:resource="&cmns-ra;RegisteredIdentifier"/>
		<rdfs:subClassOf>
			<owl:Restriction>
				<owl:onProperty rdf:resource="&cmns-ra;isRegisteredIn"/>
				<owl:hasValue rdf:resource="&idmp-eura;SPORReferentialsManagementSystem"/>
			</owl:Restriction>
		</rdfs:subClassOf>
		<rdfs:subClassOf>
			<owl:Restriction>
				<owl:onProperty rdf:resource="&cmns-id;identifies"/>
				<owl:onClass rdf:resource="&idmp-eura;SPOR-OrganisationManagementSystemTerm"/>
				<owl:qualifiedCardinality rdf:datatype="&xsd;nonNegativeInteger">1</owl:qualifiedCardinality>
			</owl:Restriction>
		</rdfs:subClassOf>
		<rdfs:label>SPOR referentials management service identifier</rdfs:label>
		<skos:definition>identifier for terms defining referentials that are registered in the SPOR referentials management services registry</skos:definition>
	</owl:Class>
	
	<owl:Class rdf:about="&idmp-eura;SPOR-ReferentialsManagementSystemTerm">
		<rdfs:subClassOf rdf:resource="&cmns-dsg;Designation"/>
		<rdfs:subClassOf>
			<owl:Restriction>
				<owl:onProperty rdf:resource="&cmns-ra;isRegisteredIn"/>
				<owl:hasValue rdf:resource="&idmp-eura;SPORReferentialsManagementSystem"/>
			</owl:Restriction>
		</rdfs:subClassOf>
		<rdfs:label>SPOR referentials management system term</rdfs:label>
		<skos:definition>designation (term) that is registered in the SPOR referentials management services registry</skos:definition>
	</owl:Class>
	
	<owl:Class rdf:about="&idmp-eura;SPOR-SubstanceManagementSystemIdentifier">
		<rdfs:subClassOf rdf:resource="&cmns-ra;RegisteredIdentifier"/>
		<rdfs:subClassOf>
			<owl:Restriction>
				<owl:onProperty rdf:resource="&cmns-ra;isRegisteredIn"/>
				<owl:hasValue rdf:resource="&idmp-eura;SPORSubstanceManagementSystem"/>
			</owl:Restriction>
		</rdfs:subClassOf>
		<rdfs:subClassOf>
			<owl:Restriction>
				<owl:onProperty rdf:resource="&cmns-id;identifies"/>
				<owl:onClass rdf:resource="&idmp-eura;SPOR-SubstanceManagementSystemTerm"/>
				<owl:qualifiedCardinality rdf:datatype="&xsd;nonNegativeInteger">1</owl:qualifiedCardinality>
			</owl:Restriction>
		</rdfs:subClassOf>
		<rdfs:label>SPOR substance management service identifier</rdfs:label>
		<skos:definition>identifier for terms defining substances that are registered in the SPOR substance management services registry</skos:definition>
	</owl:Class>
	
	<owl:Class rdf:about="&idmp-eura;SPOR-SubstanceManagementSystemTerm">
		<rdfs:subClassOf rdf:resource="&cmns-dsg;Designation"/>
		<rdfs:subClassOf>
			<owl:Restriction>
				<owl:onProperty rdf:resource="&cmns-ra;isRegisteredIn"/>
				<owl:hasValue rdf:resource="&idmp-eura;SPORSubstanceManagementSystem"/>
			</owl:Restriction>
		</rdfs:subClassOf>
		<rdfs:label>SPOR substance management system term</rdfs:label>
		<skos:definition>designation (term) that is registered in the SPOR substance management services registry</skos:definition>
	</owl:Class>
	
	<owl:NamedIndividual rdf:about="&idmp-eura;SPOROrganisationManagementSystem">
		<rdf:type rdf:resource="&cmns-ra;Registry"/>
		<rdfs:label>SPOR Organisation Management Services</rdfs:label>
		<dct:source rdf:resource="https://spor.ema.europa.eu/omswi/#/"/>
		<skos:definition>SPOR Organisation Management Services (OMS) provides a central dictionary of organisation data in multiple languages.</skos:definition>
		<cmns-av:abbreviation>SPOR-OMS</cmns-av:abbreviation>
		<cmns-col:isConstituentOf rdf:resource="&idmp-eura;SubstanceProductOrganisationReferentialDataServices"/>
	</owl:NamedIndividual>
	
	<owl:NamedIndividual rdf:about="&idmp-eura;SPORProductManagementSystem">
		<rdf:type rdf:resource="&cmns-ra;Registry"/>
		<rdfs:label>SPOR Product Management Services</rdfs:label>
		<cmns-av:abbreviation>SPOR-PMS</cmns-av:abbreviation>
		<cmns-col:isConstituentOf rdf:resource="&idmp-eura;SubstanceProductOrganisationReferentialDataServices"/>
	</owl:NamedIndividual>
	
	<owl:NamedIndividual rdf:about="&idmp-eura;SPORReferentialsManagementSystem">
		<rdf:type rdf:resource="&cmns-ra;Registry"/>
		<rdfs:label>SPOR Referentials Management Services</rdfs:label>
		<dct:source rdf:resource="https://spor.ema.europa.eu/rmswi/#/"/>
		<skos:definition>SPOR Referentials Management Services (RMS) provides referentials lists and terms (such as routes of administration, dosage forms) in multiple languages. RMS supports the continuous exchange of data between information systems across the European medicines regulatory network and the pharmaceutical industry.</skos:definition>
		<cmns-av:abbreviation>SPOR-RMS</cmns-av:abbreviation>
		<cmns-col:isConstituentOf rdf:resource="&idmp-eura;SubstanceProductOrganisationReferentialDataServices"/>
	</owl:NamedIndividual>
	
	<owl:NamedIndividual rdf:about="&idmp-eura;SPORSubstanceManagementSystem">
		<rdf:type rdf:resource="&cmns-ra;Registry"/>
		<rdfs:label>SPOR Substance Management Services</rdfs:label>
		<dct:source rdf:resource="https://spor.ema.europa.eu/smswi/#/"/>
		<skos:definition>SPOR Substance Management Services (SMS) provides a central dictionary of substance data in multiple languages. SMS supports the continuous exchange of data between information systems across the European medicines regulatory network and across the pharmaceutical industry.</skos:definition>
		<cmns-av:abbreviation>SPOR-SMS</cmns-av:abbreviation>
		<cmns-col:isConstituentOf rdf:resource="&idmp-eura;SubstanceProductOrganisationReferentialDataServices"/>
	</owl:NamedIndividual>
	
	<owl:NamedIndividual rdf:about="&idmp-eura;SubstanceProductOrganisationReferentialDataServices">
		<rdf:type rdf:resource="&cmns-ra;Registry"/>
		<rdfs:label>Substance, product, organisation and referential data services</rdfs:label>
		<dct:source rdf:resource="https://spor.ema.europa.eu/"/>
		<skos:definition>Substance, product, organisation and referential data services provide data services on substances, products, organisations and referentials to power EU regulatory activities.</skos:definition>
		<cmns-av:abbreviation>SPOR</cmns-av:abbreviation>
	</owl:NamedIndividual>
	
	<owl:NamedIndividual rdf:about="&idmp-eura;SummaryOfProductCharacteristics">
		<rdf:type rdf:resource="&cmns-ra;Registry"/>
		<rdfs:label>Summary of Product Characteristics</rdfs:label>
		<skos:definition>registry that contains documents describing the properties and the officially approved conditions of use of a medicine</skos:definition>
		<skos:note>Summaries of product characteristics form the basis of information for healthcare professionals on how to use the medicine safely and effectively.</skos:note>
		<cmns-av:abbreviation>SmPC</cmns-av:abbreviation>
		<cmns-av:directSource rdf:resource="https://www.ema.europa.eu/en/glossary/summary-product-characteristics"/>
		<cmns-ra:isManagedBy rdf:resource="&idmp-eura;EuropeanMedicinesAgencyRegistrationAuthority"/>
		<lcc-lr:hasTextualName>Summary of Product Characteristics</lcc-lr:hasTextualName>
	</owl:NamedIndividual>
	
	<owl:NamedIndividual rdf:about="&idmp-eura;UniProt">
		<rdf:type rdf:resource="&cmns-ra;Registry"/>
		<rdfs:label>UniProt</rdfs:label>
		<skos:definition>registry that provides the scientific community with a comprehensive, high-quality and freely accessible resource of protein sequence and functional information</skos:definition>
		<cmns-av:directSource rdf:resource="https://www.uniprot.org/"/>
		<lcc-lr:hasTextualName>UniProt</lcc-lr:hasTextualName>
	</owl:NamedIndividual>

</rdf:RDF>