<?xml version="1.0" encoding="UTF-8"?>
<!DOCTYPE rdf:RDF [
	<!ENTITY cmns-av "https://www.omg.org/spec/Commons/AnnotationVocabulary/">
	<!ENTITY cmns-cds "https://www.omg.org/spec/Commons/CodesAndCodeSets/">
	<!ENTITY cmns-cls "https://www.omg.org/spec/Commons/Classifiers/">
	<!ENTITY cmns-col "https://www.omg.org/spec/Commons/Collections/">
	<!ENTITY cmns-cxtdsg "https://www.omg.org/spec/Commons/ContextualDesignators/">
	<!ENTITY cmns-dsg "https://www.omg.org/spec/Commons/Designators/">
	<!ENTITY cmns-id "https://www.omg.org/spec/Commons/Identifiers/">
	<!ENTITY cmns-prd "https://www.omg.org/spec/Commons/ProductsAndServices/">
	<!ENTITY cmns-ra "https://www.omg.org/spec/Commons/RegistrationAuthorities/">
	<!ENTITY cmns-txt "https://www.omg.org/spec/Commons/TextDatatype/">
	<!ENTITY dct "http://purl.org/dc/terms/">
	<!ENTITY idmp-chg "https://spec.pistoiaalliance.org/idmp/ontology/META/ChangeManagement/">
	<!ENTITY idmp-dtp "https://spec.pistoiaalliance.org/idmp/ontology/ISO/ISO21090-HarmonizedDatatypes/">
	<!ENTITY idmp-eura "https://spec.pistoiaalliance.org/idmp/ontology/ISO/EuropeanJurisdiction/EuropeanRegistrationAuthorities/">
	<!ENTITY idmp-eurga "https://spec.pistoiaalliance.org/idmp/ontology/ISO/EuropeanJurisdiction/EuropeanRegulatoryAgencies/">
	<!ENTITY idmp-mprd "https://spec.pistoiaalliance.org/idmp/ontology/ISO/ISO11615-MedicinalProducts/">
	<!ENTITY idmp-spor "https://spec.pistoiaalliance.org/idmp/ontology/ISO/EuropeanJurisdiction/SubstancesProductsOrganisationsReferentials/">
	<!ENTITY idmp-sub "https://spec.pistoiaalliance.org/idmp/ontology/ISO/ISO11238-Substances/">
	<!ENTITY lcc-639-1 "https://www.omg.org/spec/LCC/Languages/ISO639-1-LanguageCodes/">
	<!ENTITY lcc-lr "https://www.omg.org/spec/LCC/Languages/LanguageRepresentation/">
	<!ENTITY mvf "https://www.omg.org/spec/MVF/MultipleVocabularyFacility/">
	<!ENTITY mvf-trm "https://www.omg.org/spec/MVF/ISO1087-VocabularyForTermsAndDefinitions/">
	<!ENTITY owl "http://www.w3.org/2002/07/owl#">
	<!ENTITY rdf "http://www.w3.org/1999/02/22-rdf-syntax-ns#">
	<!ENTITY rdfs "http://www.w3.org/2000/01/rdf-schema#">
	<!ENTITY skos "http://www.w3.org/2004/02/skos/core#">
	<!ENTITY xsd "http://www.w3.org/2001/XMLSchema#">
]>
<rdf:RDF xml:base="https://spec.pistoiaalliance.org/idmp/ontology/ISO/EuropeanJurisdiction/SubstancesProductsOrganisationsReferentials/"
	xmlns:cmns-av="https://www.omg.org/spec/Commons/AnnotationVocabulary/"
	xmlns:cmns-cds="https://www.omg.org/spec/Commons/CodesAndCodeSets/"
	xmlns:cmns-cls="https://www.omg.org/spec/Commons/Classifiers/"
	xmlns:cmns-col="https://www.omg.org/spec/Commons/Collections/"
	xmlns:cmns-cxtdsg="https://www.omg.org/spec/Commons/ContextualDesignators/"
	xmlns:cmns-dsg="https://www.omg.org/spec/Commons/Designators/"
	xmlns:cmns-id="https://www.omg.org/spec/Commons/Identifiers/"
	xmlns:cmns-prd="https://www.omg.org/spec/Commons/ProductsAndServices/"
	xmlns:cmns-ra="https://www.omg.org/spec/Commons/RegistrationAuthorities/"
	xmlns:cmns-txt="https://www.omg.org/spec/Commons/TextDatatype/"
	xmlns:dct="http://purl.org/dc/terms/"
	xmlns:idmp-chg="https://spec.pistoiaalliance.org/idmp/ontology/META/ChangeManagement/"
	xmlns:idmp-dtp="https://spec.pistoiaalliance.org/idmp/ontology/ISO/ISO21090-HarmonizedDatatypes/"
	xmlns:idmp-eura="https://spec.pistoiaalliance.org/idmp/ontology/ISO/EuropeanJurisdiction/EuropeanRegistrationAuthorities/"
	xmlns:idmp-eurga="https://spec.pistoiaalliance.org/idmp/ontology/ISO/EuropeanJurisdiction/EuropeanRegulatoryAgencies/"
	xmlns:idmp-mprd="https://spec.pistoiaalliance.org/idmp/ontology/ISO/ISO11615-MedicinalProducts/"
	xmlns:idmp-spor="https://spec.pistoiaalliance.org/idmp/ontology/ISO/EuropeanJurisdiction/SubstancesProductsOrganisationsReferentials/"
	xmlns:idmp-sub="https://spec.pistoiaalliance.org/idmp/ontology/ISO/ISO11238-Substances/"
	xmlns:lcc-639-1="https://www.omg.org/spec/LCC/Languages/ISO639-1-LanguageCodes/"
	xmlns:lcc-lr="https://www.omg.org/spec/LCC/Languages/LanguageRepresentation/"
	xmlns:mvf="https://www.omg.org/spec/MVF/MultipleVocabularyFacility/"
	xmlns:mvf-trm="https://www.omg.org/spec/MVF/ISO1087-VocabularyForTermsAndDefinitions/"
	xmlns:owl="http://www.w3.org/2002/07/owl#"
	xmlns:rdf="http://www.w3.org/1999/02/22-rdf-syntax-ns#"
	xmlns:rdfs="http://www.w3.org/2000/01/rdf-schema#"
	xmlns:skos="http://www.w3.org/2004/02/skos/core#"
	xmlns:xsd="http://www.w3.org/2001/XMLSchema#">
	
	<owl:Ontology rdf:about="https://spec.pistoiaalliance.org/idmp/ontology/ISO/EuropeanJurisdiction/SubstancesProductsOrganisationsReferentials/">
		<rdfs:label>Substances, Products, Organisations and Referentials (SPOR) Ontology</rdfs:label>
		<dct:abstract>The Substances, Products, Organisations and Referentials (SPOR) ontology extends the core IDMP ontologies to define additional content required to support alignment with the European Medicines Agency data management services for substances, products, organisations and referentials.</dct:abstract>
		<dct:license rdf:datatype="&xsd;anyURI">https://opensource.org/licenses/MIT</dct:license>
		<owl:imports rdf:resource="https://spec.pistoiaalliance.org/idmp/ontology/ISO/EuropeanJurisdiction/EuropeanRegistrationAuthorities/"/>
		<owl:imports rdf:resource="https://spec.pistoiaalliance.org/idmp/ontology/ISO/EuropeanJurisdiction/EuropeanRegulatoryAgencies/"/>
		<owl:imports rdf:resource="https://spec.pistoiaalliance.org/idmp/ontology/ISO/ISO11238-Substances/"/>
		<owl:imports rdf:resource="https://spec.pistoiaalliance.org/idmp/ontology/ISO/ISO11615-MedicinalProducts/"/>
		<owl:imports rdf:resource="https://spec.pistoiaalliance.org/idmp/ontology/ISO/ISO21090-HarmonizedDatatypes/"/>
		<owl:imports rdf:resource="https://spec.pistoiaalliance.org/idmp/ontology/META/ChangeManagement/"/>
		<owl:imports rdf:resource="https://www.omg.org/spec/Commons/AnnotationVocabulary/"/>
		<owl:imports rdf:resource="https://www.omg.org/spec/Commons/Classifiers/"/>
		<owl:imports rdf:resource="https://www.omg.org/spec/Commons/CodesAndCodeSets/"/>
		<owl:imports rdf:resource="https://www.omg.org/spec/Commons/Collections/"/>
		<owl:imports rdf:resource="https://www.omg.org/spec/Commons/ContextualDesignators/"/>
		<owl:imports rdf:resource="https://www.omg.org/spec/Commons/Designators/"/>
		<owl:imports rdf:resource="https://www.omg.org/spec/Commons/Identifiers/"/>
		<owl:imports rdf:resource="https://www.omg.org/spec/Commons/ProductsAndServices/"/>
		<owl:imports rdf:resource="https://www.omg.org/spec/Commons/RegistrationAuthorities/"/>
		<owl:imports rdf:resource="https://www.omg.org/spec/Commons/TextDatatype/"/>
		<owl:imports rdf:resource="https://www.omg.org/spec/LCC/Languages/ISO639-1-LanguageCodes/"/>
		<owl:imports rdf:resource="https://www.omg.org/spec/LCC/Languages/LanguageRepresentation/"/>
		<owl:imports rdf:resource="https://www.omg.org/spec/MVF/ISO1087-VocabularyForTermsAndDefinitions/"/>
		<owl:imports rdf:resource="https://www.omg.org/spec/MVF/MultipleVocabularyFacility/"/>
		<owl:versionIRI rdf:resource="https://spec.pistoiaalliance.org/idmp/ontology/ISO/20240701/EuropeanJurisdiction/SubstancesProductsOrganisationsReferentials/"/>
		<skos:changeNote>The https://spec.pistoiaalliance.org/idmp/ontology/ISO/20230801/EuropeanJurisdiction/SubstancesProductsOrganisationsReferentials.rdf version of this ontology was modified to eliminate EMA SPOR terms that will be generated rather than hand crafted (IDMP-674).</skos:changeNote>
		<skos:changeNote>The https://spec.pistoiaalliance.org/idmp/ontology/ISO/20231001/EuropeanJurisdiction/SubstancesProductsOrganisationsReferentials.rdf version of this ontology was modified to finalize names of certain elements for release (IDMP-616).</skos:changeNote>
		<idmp-chg:hasMaturityLevel rdf:resource="&idmp-chg;Provisional"/>
		<cmns-av:copyright>Copyright (c) 2022-2024 EDM Council, Inc.</cmns-av:copyright>
		<cmns-av:copyright>Copyright (c) 2022-2024 Pistoia Alliance, Inc.</cmns-av:copyright>
		<cmns-av:usageNote>Note that the copyright and licensing terms for contents of this ontology that are taken from the EMA SPOR repository(ies), including but not limited to the definitions and descriptions of specific lists (controlled vocabularies) managed therein, are also subject to the following copyright and license: &apos;The content of this list and associated intellectual property rights were developed under projects funded by the EMA therefore becoming the property of the EMA. Reproduction is authorised provided the source is acknowledged.&apos; Not all lists referenced in the SPOR repositories are covered under these terms if, for example, they came from other sources. The default case assumes that the EMA license and copyright applies, such as for Shelf Life Type. In cases used herein where different terms apply, additional annotations will be included on a per list (controlled vocabulary) basis.</cmns-av:usageNote>
	</owl:Ontology>
	
	<owl:NamedIndividual rdf:about="&idmp-eura;EuropeanMedicinesAgencyRegistrationAuthority">
		<cmns-ra:manages rdf:resource="&idmp-spor;OrganisationManagementServices"/>
		<cmns-ra:manages rdf:resource="&idmp-spor;ProductManagementServices"/>
		<cmns-ra:manages rdf:resource="&idmp-spor;ReferentialsManagementServicesRegistry"/>
		<cmns-ra:manages rdf:resource="&idmp-spor;SubstancesManagementServicesRegistry"/>
	</owl:NamedIndividual>
	
	<owl:NamedIndividual rdf:about="&idmp-spor;OrganisationManagementServices">
		<rdf:type rdf:resource="&cmns-ra;RegistrationService"/>
		<rdfs:label>Organisation Management Services (OMS)</rdfs:label>
		<skos:definition>services supporting a central dictionary of organisation data in multiple languages</skos:definition>
		<cmns-av:abbreviation>OMS services</cmns-av:abbreviation>
		<cmns-av:directSource rdf:resource="https://spor.ema.europa.eu/"/>
		<cmns-col:isPartOf rdf:resource="&idmp-spor;SubstancesProductsOrganisationsReferentialsDataManagementServices"/>
		<cmns-prd:isProvidedBy rdf:resource="&idmp-eura;EuropeanMedicinesAgencyRegistrationAuthority"/>
	</owl:NamedIndividual>
	
	<owl:NamedIndividual rdf:about="&idmp-spor;ProductManagementServices">
		<rdf:type rdf:resource="&cmns-ra;RegistrationService"/>
		<rdfs:label>Product Management Services (PMS)</rdfs:label>
		<skos:definition>services supporting a central dictionary of product data in multiple languages</skos:definition>
		<cmns-av:abbreviation>PMS service</cmns-av:abbreviation>
		<cmns-av:adaptedFrom>https://spor.ema.europa.eu/sporwi/</cmns-av:adaptedFrom>
		<cmns-col:isPartOf rdf:resource="&idmp-spor;SubstancesProductsOrganisationsReferentialsDataManagementServices"/>
		<cmns-prd:isProvidedBy rdf:resource="&idmp-eura;EuropeanMedicinesAgencyRegistrationAuthority"/>
	</owl:NamedIndividual>
	
	<owl:Class rdf:about="&idmp-spor;ProductManagementServicesIdentifier">
		<rdfs:subClassOf rdf:resource="&cmns-ra;RegisteredIdentifier"/>
		<rdfs:subClassOf>
			<owl:Restriction>
				<owl:onProperty rdf:resource="&cmns-col;compliesWith"/>
				<owl:hasValue rdf:resource="&idmp-spor;ProductManagementServicesRegistrationScheme"/>
			</owl:Restriction>
		</rdfs:subClassOf>
		<rdfs:subClassOf>
			<owl:Restriction>
				<owl:onProperty rdf:resource="&cmns-ra;isRegisteredIn"/>
				<owl:hasValue rdf:resource="&idmp-spor;ProductManagementServicesRegistry"/>
			</owl:Restriction>
		</rdfs:subClassOf>
		<rdfs:label>Product Management Services identifier</rdfs:label>
		<skos:definition>contextual identifier for medicinal product data that is registered in the Substances Products Organisations Referentials (SPOR) Product Management Services (PMS) registry</skos:definition>
		<cmns-av:abbreviation>PMS ID</cmns-av:abbreviation>
	</owl:Class>
	
	<owl:NamedIndividual rdf:about="&idmp-spor;ProductManagementServicesRegistrationScheme">
		<rdf:type rdf:resource="&cmns-ra;RegistrationScheme"/>
		<rdfs:label>Product Management Services (PMS) registration scheme</rdfs:label>
		<skos:definition>scheme for organizing information in the Substances Products Organisations Referentials (SPOR) Product Management Services (PMS) registry and allocating identifiers to registered items</skos:definition>
	</owl:NamedIndividual>
	
	<owl:NamedIndividual rdf:about="&idmp-spor;ProductManagementServicesRegistry">
		<rdf:type rdf:resource="&cmns-ra;Registry"/>
		<rdfs:label>Product Management Services (PMS) registry</rdfs:label>
		<skos:definition>central dictionary of product data in multiple languages available through the Substances Products Organisations Referentials (SPOR) Product Management Services (PMS)</skos:definition>
		<cmns-av:abbreviation>SPOR PMS</cmns-av:abbreviation>
		<cmns-av:abbreviation>SPOR-PMS</cmns-av:abbreviation>
		<cmns-av:directSource rdf:resource="https://spor.ema.europa.eu/"/>
		<cmns-ra:isManagedBy rdf:resource="&idmp-eura;EuropeanMedicinesAgencyRegistrationAuthority"/>
	</owl:NamedIndividual>
	
	<owl:NamedIndividual rdf:about="&idmp-spor;ReferentialsManagementServices">
		<rdf:type rdf:resource="&cmns-ra;RegistrationService"/>
		<rdfs:label>Referentials Management Services (RMS)</rdfs:label>
		<skos:definition>services supporting a central dictionary of referentials data in multiple languages</skos:definition>
		<cmns-av:abbreviation>RMS service</cmns-av:abbreviation>
		<cmns-av:directSource rdf:resource="https://spor.ema.europa.eu/"/>
		<cmns-col:isPartOf rdf:resource="&idmp-spor;SubstancesProductsOrganisationsReferentialsDataManagementServices"/>
		<cmns-prd:isProvidedBy rdf:resource="&idmp-eura;EuropeanMedicinesAgencyRegistrationAuthority"/>
	</owl:NamedIndividual>
	
	<owl:NamedIndividual rdf:about="&idmp-spor;ReferentialsManagementServicesRegistrationScheme">
		<rdf:type rdf:resource="&cmns-ra;RegistrationScheme"/>
		<rdfs:label>Referentials Management Services (RMS) registration scheme</rdfs:label>
		<skos:definition>scheme for organizing information in the Substances Products Organisations Referentials (SPOR) Referentials Management Services (RMS) registry and allocating identifiers to registered items</skos:definition>
	</owl:NamedIndividual>
	
	<owl:NamedIndividual rdf:about="&idmp-spor;ReferentialsManagementServicesRegistry">
		<rdf:type rdf:resource="&cmns-ra;Registry"/>
		<rdfs:label>Referentials Management Services (RMS) registry</rdfs:label>
		<skos:definition>central dictionary of referentials data in multiple languages available through the Substances Products Organisations Referentials (SPOR) Referentials Management Services (RMS)</skos:definition>
		<cmns-av:abbreviation>SPOR RMS</cmns-av:abbreviation>
		<cmns-av:abbreviation>SPOR-RMS</cmns-av:abbreviation>
		<cmns-av:directSource rdf:resource="https://spor.ema.europa.eu/"/>
		<cmns-ra:isManagedBy rdf:resource="&idmp-eura;EuropeanMedicinesAgencyRegistrationAuthority"/>
	</owl:NamedIndividual>
	
	<owl:Class rdf:about="&idmp-spor;SPOR-DataClassification">
		<rdfs:subClassOf rdf:resource="&idmp-spor;SPORControlledVocabularyTerm"/>
		<rdfs:label>SPOR data classification</rdfs:label>
		<skos:definition>classifier and code element that describes the nature of any data element in terms of accessibility from a Substances Products Organisations Referentials (SPOR) perspective</skos:definition>
		<cmns-av:directSource rdf:resource="https://spor.ema.europa.eu/v1/lists/200000004983"/>
	</owl:Class>
	
	<owl:NamedIndividual rdf:about="&idmp-spor;SPOR-DataClassification-Confidential">
		<rdf:type rdf:resource="&idmp-spor;SPOR-DataClassification"/>
		<owl:sameAs rdf:resource="https://spor.ema.europa.eu/v1/lists/200000004983/terms/200000004984"/>
		<rdfs:label>SPOR data classification - confidential</rdfs:label>
		<skos:definition>classifier and code element describes the nature of any data element that is confidential in terms of accessibility from a Substances Products Organisations Referentials (SPOR) perspective</skos:definition>
		<idmp-spor:hasSPORDomain rdf:resource="&idmp-spor;SPOR-Domain-HumanAndVeterinaryUse"/>
		<idmp-spor:hasSPORStatus rdf:resource="&idmp-spor;SPOR-RecordStatus-Current"/>
		<idmp-spor:hasSPORTermName rdf:resource="&idmp-spor;SPOR-DataClassificationVocabulary-Confidential-TermName-English"/>
		<idmp-spor:hasSPORVisibility rdf:resource="&idmp-spor;SPOR-DataClassification-Public"/>
		<cmns-col:isIncludedIn rdf:resource="&idmp-spor;SPOR-DataClassificationVocabulary"/>
		<cmns-id:isIdentifiedBy rdf:resource="&idmp-spor;SPOR-TermIdentifier-200000004983-200000004984"/>
	</owl:NamedIndividual>
	
	<owl:NamedIndividual rdf:about="&idmp-spor;SPOR-DataClassification-Public">
		<rdf:type rdf:resource="&idmp-spor;SPOR-DataClassification"/>
		<owl:sameAs rdf:resource="https://spor.ema.europa.eu/v1/lists/200000004983/terms/200000004985"/>
		<rdfs:label>SPOR data classification - public</rdfs:label>
		<skos:definition>classifier and code element describes the nature of any data element that is public in terms of accessibility from a Substances Products Organisations Referentials (SPOR) perspective</skos:definition>
		<idmp-spor:hasSPORDomain rdf:resource="&idmp-spor;SPOR-Domain-HumanAndVeterinaryUse"/>
		<idmp-spor:hasSPORStatus rdf:resource="&idmp-spor;SPOR-RecordStatus-Current"/>
		<idmp-spor:hasSPORTermName rdf:resource="&idmp-spor;SPOR-DataClassificationVocabulary-Public-TermName-English"/>
		<idmp-spor:hasSPORVisibility rdf:resource="&idmp-spor;SPOR-DataClassification-Public"/>
		<cmns-col:isIncludedIn rdf:resource="&idmp-spor;SPOR-DataClassificationVocabulary"/>
		<cmns-id:isIdentifiedBy rdf:resource="&idmp-spor;SPOR-TermIdentifier-200000004983-200000004985"/>
	</owl:NamedIndividual>
	
	<owl:NamedIndividual rdf:about="&idmp-spor;SPOR-DataClassification-Restricted">
		<rdf:type rdf:resource="&idmp-spor;SPOR-DataClassification"/>
		<owl:sameAs rdf:resource="https://spor.ema.europa.eu/v1/lists/200000004983/terms/200000004986"/>
		<rdfs:label>SPOR data classification - restricted</rdfs:label>
		<skos:definition>classifier and code element describes the nature of any data element that is restricted in terms of accessibility from a Substances Products Organisations Referentials (SPOR) perspective</skos:definition>
		<idmp-spor:hasSPORDomain rdf:resource="&idmp-spor;SPOR-Domain-HumanAndVeterinaryUse"/>
		<idmp-spor:hasSPORStatus rdf:resource="&idmp-spor;SPOR-RecordStatus-Current"/>
		<idmp-spor:hasSPORTermName rdf:resource="&idmp-spor;SPOR-DataClassificationVocabulary-Restricted-TermName-English"/>
		<idmp-spor:hasSPORVisibility rdf:resource="&idmp-spor;SPOR-DataClassification-Public"/>
		<cmns-col:isIncludedIn rdf:resource="&idmp-spor;SPOR-DataClassificationVocabulary"/>
		<cmns-id:isIdentifiedBy rdf:resource="&idmp-spor;SPOR-TermIdentifier-200000004983-200000004986"/>
	</owl:NamedIndividual>
	
	<owl:NamedIndividual rdf:about="&idmp-spor;SPOR-DataClassificationVocabulary">
		<rdf:type rdf:resource="&idmp-spor;SPORControlledVocabulary"/>
		<owl:sameAs rdf:resource="https://spor.ema.europa.eu/v1/lists/200000004983"/>
		<rdfs:label>SPOR Data Classification vocabulary</rdfs:label>
		<skos:definition>controlled vocabulary used to classify the nature of any data element in terms of accessibility from a Substances Products Organisations Referentials (SPOR) perspective</skos:definition>
		<cmns-av:synonym>SPOR RMS data classification list</cmns-av:synonym>
		<cmns-dsg:isSignifiedBy rdf:resource="&idmp-spor;SPOR-ListName-200000004983"/>
		<cmns-id:isIdentifiedBy rdf:resource="&idmp-spor;SPOR-ListIdentifier-200000004983"/>
	</owl:NamedIndividual>
	
	<owl:NamedIndividual rdf:about="&idmp-spor;SPOR-DataClassificationVocabulary-Confidential-TermName-English">
		<rdf:type rdf:resource="&idmp-spor;SPORTermName"/>
		<rdfs:label>SPOR-RMS, Data Classification Vocabulary, Confidential, Term Name, English</rdfs:label>
		<dct:source rdf:resource="https://spor.ema.europa.eu/v1/lists/200000004983/terms/200000004984"/>
		<skos:definition>SPOR term name, in English, for the RMS data classification vocabulary term, Confidential</skos:definition>
		<cmns-col:isIncludedIn rdf:resource="&idmp-spor;SPOR-DataClassificationVocabulary"/>
		<cmns-dsg:denotes rdf:resource="&idmp-spor;SPOR-DataClassification-Confidential"/>
		<cmns-txt:hasTextValue xml:lang="en">Confidential</cmns-txt:hasTextValue>
		<mvf:hasLanguage rdf:resource="&lcc-639-1;English"/>
	</owl:NamedIndividual>
	
	<owl:NamedIndividual rdf:about="&idmp-spor;SPOR-DataClassificationVocabulary-Public-TermName-English">
		<rdf:type rdf:resource="&idmp-spor;SPORTermName"/>
		<rdfs:label>SPOR-RMS, Data Classification Vocabulary, Public, Term Name, English</rdfs:label>
		<dct:source rdf:resource="https://spor.ema.europa.eu/v1/lists/200000004983/terms/200000004985"/>
		<skos:definition>SPOR term name, in English, for the RMS data classification vocabulary term, Public</skos:definition>
		<cmns-col:isIncludedIn rdf:resource="&idmp-spor;SPOR-DataClassificationVocabulary"/>
		<cmns-dsg:denotes rdf:resource="&idmp-spor;SPOR-DataClassification-Public"/>
		<cmns-txt:hasTextValue xml:lang="en">Public</cmns-txt:hasTextValue>
		<mvf:hasLanguage rdf:resource="&lcc-639-1;English"/>
	</owl:NamedIndividual>
	
	<owl:NamedIndividual rdf:about="&idmp-spor;SPOR-DataClassificationVocabulary-Restricted-TermName-English">
		<rdf:type rdf:resource="&idmp-spor;SPORTermName"/>
		<rdfs:label>SPOR-RMS, Data Classification Vocabulary, Restricted, Term Name, English</rdfs:label>
		<dct:source rdf:resource="https://spor.ema.europa.eu/v1/lists/200000004983/terms/200000004986"/>
		<skos:definition>SPOR term name, in English, for the RMS data classification vocabulary term, Restricted</skos:definition>
		<cmns-col:isIncludedIn rdf:resource="&idmp-spor;SPOR-DataClassificationVocabulary"/>
		<cmns-dsg:denotes rdf:resource="&idmp-spor;SPOR-DataClassification-Restricted"/>
		<cmns-txt:hasTextValue xml:lang="en">Restricted</cmns-txt:hasTextValue>
		<mvf:hasLanguage rdf:resource="&lcc-639-1;English"/>
	</owl:NamedIndividual>
	
	<owl:Class rdf:about="&idmp-spor;SPOR-Domain">
		<rdfs:subClassOf rdf:resource="&idmp-spor;SPORControlledVocabularyTerm"/>
		<rdfs:label>SPOR domain</rdfs:label>
		<skos:definition>classifier and code element that describes the domain in which a particular substance or product is used from a Substances Products Organisations Referentials (SPOR) perspective</skos:definition>
		<cmns-av:adaptedFrom rdf:resource="https://spor.ema.europa.eu/v1/lists/100000000004"/>
		<cmns-col:isIncludedIn rdf:resource="&idmp-spor;SPOR-DomainVocabulary"/>
	</owl:Class>
	
	<owl:NamedIndividual rdf:about="&idmp-spor;SPOR-Domain-HumanAndVeterinaryUse">
		<rdf:type rdf:resource="&idmp-spor;SPOR-Domain"/>
		<owl:sameAs rdf:resource="https://spor.ema.europa.eu/v1/lists/100000000004/terms/100000000014"/>
		<rdfs:label>SPOR domain - human and veterinary use</rdfs:label>
		<skos:definition>classifier and code element describes the domain of human and veterinary use in which a particular substance or product is used from a Substances Products Organisations Referentials (SPOR) perspective</skos:definition>
		<idmp-spor:hasSPORDomain rdf:resource="&idmp-spor;SPOR-Domain-HumanAndVeterinaryUse"/>
		<idmp-spor:hasSPOROtherName rdf:resource="&idmp-spor;SPOR-DomainVocabulary-HumanAndVeterinaryUse-OtherName-HumanVeterinär-German"/>
		<idmp-spor:hasSPORShortName rdf:resource="&idmp-spor;SPOR-DomainVocabulary-HumanAndVeterinaryUse-ShortName-Czech"/>
		<idmp-spor:hasSPORShortName rdf:resource="&idmp-spor;SPOR-DomainVocabulary-HumanAndVeterinaryUse-ShortName-English"/>
		<idmp-spor:hasSPORShortName rdf:resource="&idmp-spor;SPOR-DomainVocabulary-HumanAndVeterinaryUse-ShortName-French"/>
		<idmp-spor:hasSPORShortName rdf:resource="&idmp-spor;SPOR-DomainVocabulary-HumanAndVeterinaryUse-ShortName-German"/>
		<idmp-spor:hasSPORShortName rdf:resource="&idmp-spor;SPOR-DomainVocabulary-HumanAndVeterinaryUse-ShortName-Italian"/>
		<idmp-spor:hasSPORShortName rdf:resource="&idmp-spor;SPOR-DomainVocabulary-HumanAndVeterinaryUse-ShortName-Swedish"/>
		<idmp-spor:hasSPORStatus rdf:resource="&idmp-spor;SPOR-RecordStatus-Current"/>
		<idmp-spor:hasSPORTermName rdf:resource="&idmp-spor;SPOR-DomainVocabulary-HumanAndVeterinaryUse-TermName-Czech"/>
		<idmp-spor:hasSPORTermName rdf:resource="&idmp-spor;SPOR-DomainVocabulary-HumanAndVeterinaryUse-TermName-English"/>
		<idmp-spor:hasSPORTermName rdf:resource="&idmp-spor;SPOR-DomainVocabulary-HumanAndVeterinaryUse-TermName-French"/>
		<idmp-spor:hasSPORTermName rdf:resource="&idmp-spor;SPOR-DomainVocabulary-HumanAndVeterinaryUse-TermName-German"/>
		<idmp-spor:hasSPORTermName rdf:resource="&idmp-spor;SPOR-DomainVocabulary-HumanAndVeterinaryUse-TermName-Italian"/>
		<idmp-spor:hasSPORTermName rdf:resource="&idmp-spor;SPOR-DomainVocabulary-HumanAndVeterinaryUse-TermName-Latvian"/>
		<idmp-spor:hasSPORTermName rdf:resource="&idmp-spor;SPOR-DomainVocabulary-HumanAndVeterinaryUse-TermName-Norwegian"/>
		<idmp-spor:hasSPORTermName rdf:resource="&idmp-spor;SPOR-DomainVocabulary-HumanAndVeterinaryUse-TermName-Swedish"/>
		<idmp-spor:hasSPORVisibility rdf:resource="&idmp-spor;SPOR-DataClassification-Public"/>
		<cmns-col:isIncludedIn rdf:resource="&idmp-spor;SPOR-DomainVocabulary"/>
		<cmns-id:isIdentifiedBy rdf:resource="&idmp-spor;SPOR-TermIdentifier-100000000004-100000000014"/>
	</owl:NamedIndividual>
	
	<owl:NamedIndividual rdf:about="&idmp-spor;SPOR-Domain-HumanUse">
		<rdf:type rdf:resource="&idmp-spor;SPOR-Domain"/>
		<owl:sameAs rdf:resource="https://spor.ema.europa.eu/v1/lists/100000000004/terms/100000000012"/>
		<rdfs:label>SPOR domain - human use</rdfs:label>
		<skos:definition>classifier and code element describes the domain of human use in which a particular substance or product is used from a Substances Products Organisations Referentials (SPOR) perspective</skos:definition>
		<idmp-spor:hasSPORDomain rdf:resource="&idmp-spor;SPOR-Domain-HumanAndVeterinaryUse"/>
		<idmp-spor:hasSPOROtherName rdf:resource="&idmp-spor;SPOR-DomainVocabulary-HumanUse-OtherName-Human-German"/>
		<idmp-spor:hasSPORShortName rdf:resource="&idmp-spor;SPOR-DomainVocabulary-HumanUse-ShortName-English"/>
		<idmp-spor:hasSPORShortName rdf:resource="&idmp-spor;SPOR-DomainVocabulary-HumanUse-ShortName-French"/>
		<idmp-spor:hasSPORShortName rdf:resource="&idmp-spor;SPOR-DomainVocabulary-HumanUse-ShortName-German"/>
		<idmp-spor:hasSPORShortName rdf:resource="&idmp-spor;SPOR-DomainVocabulary-HumanUse-ShortName-Italian"/>
		<idmp-spor:hasSPORShortName rdf:resource="&idmp-spor;SPOR-DomainVocabulary-HumanUse-ShortName-Swedish"/>
		<idmp-spor:hasSPORStatus rdf:resource="&idmp-spor;SPOR-RecordStatus-Current"/>
		<idmp-spor:hasSPORTermName rdf:resource="&idmp-spor;SPOR-DomainVocabulary-HumanUse-TermName-English"/>
		<idmp-spor:hasSPORTermName rdf:resource="&idmp-spor;SPOR-DomainVocabulary-HumanUse-TermName-French"/>
		<idmp-spor:hasSPORTermName rdf:resource="&idmp-spor;SPOR-DomainVocabulary-HumanUse-TermName-German"/>
		<idmp-spor:hasSPORTermName rdf:resource="&idmp-spor;SPOR-DomainVocabulary-HumanUse-TermName-Italian"/>
		<idmp-spor:hasSPORTermName rdf:resource="&idmp-spor;SPOR-DomainVocabulary-HumanUse-TermName-Latvian"/>
		<idmp-spor:hasSPORTermName rdf:resource="&idmp-spor;SPOR-DomainVocabulary-HumanUse-TermName-Norwegian"/>
		<idmp-spor:hasSPORTermName rdf:resource="&idmp-spor;SPOR-DomainVocabulary-HumanUse-TermName-Swedish"/>
		<idmp-spor:hasSPORVisibility rdf:resource="&idmp-spor;SPOR-DataClassification-Public"/>
		<cmns-col:isIncludedIn rdf:resource="&idmp-spor;SPOR-DomainVocabulary"/>
		<cmns-id:isIdentifiedBy rdf:resource="&idmp-spor;SPOR-TermIdentifier-100000000004-100000000012"/>
	</owl:NamedIndividual>
	
	<owl:NamedIndividual rdf:about="&idmp-spor;SPOR-Domain-VeterinaryUse">
		<rdf:type rdf:resource="&idmp-spor;SPOR-Domain"/>
		<owl:sameAs rdf:resource="https://spor.ema.europa.eu/v1/lists/100000000004/terms/100000000013"/>
		<rdfs:label>SPOR domain - veterinary use</rdfs:label>
		<skos:definition>classifier and code element describes the domain of veterinary use in which a particular substance or product is used from a Substances Products Organisations Referentials (SPOR) perspective</skos:definition>
		<idmp-spor:hasSPORDomain rdf:resource="&idmp-spor;SPOR-Domain-HumanAndVeterinaryUse"/>
		<idmp-spor:hasSPOROtherName rdf:resource="&idmp-spor;SPOR-DomainVocabulary-VeterinaryUse-OtherName-Veterinär-German"/>
		<idmp-spor:hasSPORShortName rdf:resource="&idmp-spor;SPOR-DomainVocabulary-VeterinaryUse-ShortName-Czech"/>
		<idmp-spor:hasSPORShortName rdf:resource="&idmp-spor;SPOR-DomainVocabulary-VeterinaryUse-ShortName-English"/>
		<idmp-spor:hasSPORShortName rdf:resource="&idmp-spor;SPOR-DomainVocabulary-VeterinaryUse-ShortName-French"/>
		<idmp-spor:hasSPORShortName rdf:resource="&idmp-spor;SPOR-DomainVocabulary-VeterinaryUse-ShortName-German"/>
		<idmp-spor:hasSPORShortName rdf:resource="&idmp-spor;SPOR-DomainVocabulary-VeterinaryUse-ShortName-Italian"/>
		<idmp-spor:hasSPORShortName rdf:resource="&idmp-spor;SPOR-DomainVocabulary-VeterinaryUse-ShortName-Swedish"/>
		<idmp-spor:hasSPORStatus rdf:resource="&idmp-spor;SPOR-RecordStatus-Current"/>
		<idmp-spor:hasSPORTermName rdf:resource="&idmp-spor;SPOR-DomainVocabulary-VeterinaryUse-TermName-Czech"/>
		<idmp-spor:hasSPORTermName rdf:resource="&idmp-spor;SPOR-DomainVocabulary-VeterinaryUse-TermName-English"/>
		<idmp-spor:hasSPORTermName rdf:resource="&idmp-spor;SPOR-DomainVocabulary-VeterinaryUse-TermName-French"/>
		<idmp-spor:hasSPORTermName rdf:resource="&idmp-spor;SPOR-DomainVocabulary-VeterinaryUse-TermName-German"/>
		<idmp-spor:hasSPORTermName rdf:resource="&idmp-spor;SPOR-DomainVocabulary-VeterinaryUse-TermName-Italian"/>
		<idmp-spor:hasSPORTermName rdf:resource="&idmp-spor;SPOR-DomainVocabulary-VeterinaryUse-TermName-Latvian"/>
		<idmp-spor:hasSPORTermName rdf:resource="&idmp-spor;SPOR-DomainVocabulary-VeterinaryUse-TermName-Norwegian"/>
		<idmp-spor:hasSPORTermName rdf:resource="&idmp-spor;SPOR-DomainVocabulary-VeterinaryUse-TermName-Romanian"/>
		<idmp-spor:hasSPORTermName rdf:resource="&idmp-spor;SPOR-DomainVocabulary-VeterinaryUse-TermName-Swedish"/>
		<idmp-spor:hasSPORVisibility rdf:resource="&idmp-spor;SPOR-DataClassification-Public"/>
		<cmns-col:isIncludedIn rdf:resource="&idmp-spor;SPOR-DomainVocabulary"/>
		<cmns-id:isIdentifiedBy rdf:resource="&idmp-spor;SPOR-TermIdentifier-100000000004-100000000013"/>
	</owl:NamedIndividual>
	
	<owl:NamedIndividual rdf:about="&idmp-spor;SPOR-DomainVocabulary">
		<rdf:type rdf:resource="&idmp-spor;SPORControlledVocabulary"/>
		<owl:sameAs rdf:resource="https://spor.ema.europa.eu/v1/lists/100000000004"/>
		<rdfs:label>SPOR-RMS, Domain Vocabulary</rdfs:label>
		<skos:definition>controlled vocabulary used to classify the domain in which a particular substance or product is used from a Substances Products Organisations Referentials (SPOR) perspective</skos:definition>
		<cmns-av:synonym>SPOR RMS domain list</cmns-av:synonym>
		<cmns-id:isIdentifiedBy rdf:resource="&idmp-spor;SPOR-ListIdentifier-100000000004"/>
	</owl:NamedIndividual>
	
	<owl:NamedIndividual rdf:about="&idmp-spor;SPOR-DomainVocabulary-HumanAndVeterinaryUse-OtherName-HumanVeterinär-German">
		<rdf:type rdf:resource="&idmp-spor;SPORTermName"/>
		<rdfs:label>SPOR-RMS, Domain Vocabulary, Human and Veterinary Use, Other Name, Human Veterinär, German</rdfs:label>
		<dct:source rdf:resource="https://spor.ema.europa.eu/v1/lists/100000000004/terms/100000000014"/>
		<skos:definition>SPOR other term name, in German, for the RMS domain vocabulary term, Human and Veterinary use</skos:definition>
		<cmns-col:isIncludedIn rdf:resource="&idmp-spor;SPOR-DomainVocabulary"/>
		<cmns-dsg:denotes rdf:resource="&idmp-spor;SPOR-Domain-HumanAndVeterinaryUse"/>
		<cmns-txt:hasTextValue xml:lang="de">Human &amp; Veterinär</cmns-txt:hasTextValue>
		<mvf:hasLanguage rdf:resource="&lcc-639-1;German"/>
	</owl:NamedIndividual>
	
	<owl:NamedIndividual rdf:about="&idmp-spor;SPOR-DomainVocabulary-HumanAndVeterinaryUse-ShortName-Czech">
		<rdf:type rdf:resource="&idmp-spor;SPORTermName"/>
		<rdfs:label>SPOR-RMS, Domain Vocabulary, Human and Veterinary Use, Short Name, Czech</rdfs:label>
		<dct:source rdf:resource="https://spor.ema.europa.eu/v1/lists/100000000004/terms/100000000014"/>
		<skos:definition>SPOR short term name, in Czech, for the RMS domain vocabulary term, Human and Veterinary use</skos:definition>
		<cmns-col:isIncludedIn rdf:resource="&idmp-spor;SPOR-DomainVocabulary"/>
		<cmns-dsg:denotes rdf:resource="&idmp-spor;SPOR-Domain-HumanAndVeterinaryUse"/>
		<cmns-txt:hasTextValue xml:lang="cs">H+V</cmns-txt:hasTextValue>
		<mvf:hasLanguage rdf:resource="&lcc-639-1;Czech"/>
	</owl:NamedIndividual>
	
	<owl:NamedIndividual rdf:about="&idmp-spor;SPOR-DomainVocabulary-HumanAndVeterinaryUse-ShortName-English">
		<rdf:type rdf:resource="&idmp-spor;SPORTermName"/>
		<rdfs:label>SPOR-RMS, Domain Vocabulary, Human and Veterinary Use, Short Name, English</rdfs:label>
		<dct:source rdf:resource="https://spor.ema.europa.eu/v1/lists/100000000004/terms/100000000014"/>
		<skos:definition>SPOR short term name, in English, for the RMS domain vocabulary term, Human and Veterinary use</skos:definition>
		<cmns-col:isIncludedIn rdf:resource="&idmp-spor;SPOR-DomainVocabulary"/>
		<cmns-dsg:denotes rdf:resource="&idmp-spor;SPOR-Domain-HumanAndVeterinaryUse"/>
		<cmns-txt:hasTextValue xml:lang="en">H&amp;V</cmns-txt:hasTextValue>
		<mvf:hasLanguage rdf:resource="&lcc-639-1;English"/>
	</owl:NamedIndividual>
	
	<owl:NamedIndividual rdf:about="&idmp-spor;SPOR-DomainVocabulary-HumanAndVeterinaryUse-ShortName-French">
		<rdf:type rdf:resource="&idmp-spor;SPORTermName"/>
		<rdfs:label>SPOR-RMS, Domain Vocabulary, Human and Veterinary Use, Short Name, French</rdfs:label>
		<dct:source rdf:resource="https://spor.ema.europa.eu/v1/lists/100000000004/terms/100000000014"/>
		<skos:definition>SPOR short term name, in French, for the RMS domain vocabulary term, Human and Veterinary use</skos:definition>
		<cmns-col:isIncludedIn rdf:resource="&idmp-spor;SPOR-DomainVocabulary"/>
		<cmns-dsg:denotes rdf:resource="&idmp-spor;SPOR-Domain-HumanAndVeterinaryUse"/>
		<cmns-txt:hasTextValue xml:lang="fr-FR">H&amp;V</cmns-txt:hasTextValue>
		<mvf:hasLanguage rdf:resource="&lcc-639-1;French"/>
	</owl:NamedIndividual>
	
	<owl:NamedIndividual rdf:about="&idmp-spor;SPOR-DomainVocabulary-HumanAndVeterinaryUse-ShortName-German">
		<rdf:type rdf:resource="&idmp-spor;SPORTermName"/>
		<rdfs:label>SPOR-RMS, Domain Vocabulary, Human and Veterinary Use, Short Name, German</rdfs:label>
		<dct:source rdf:resource="https://spor.ema.europa.eu/v1/lists/100000000004/terms/100000000014"/>
		<skos:definition>SPOR short term name, in German, for the RMS domain vocabulary term, Human and Veterinary use</skos:definition>
		<cmns-col:isIncludedIn rdf:resource="&idmp-spor;SPOR-DomainVocabulary"/>
		<cmns-dsg:denotes rdf:resource="&idmp-spor;SPOR-Domain-HumanAndVeterinaryUse"/>
		<cmns-txt:hasTextValue xml:lang="de">H&amp;V</cmns-txt:hasTextValue>
		<mvf:hasLanguage rdf:resource="&lcc-639-1;German"/>
	</owl:NamedIndividual>
	
	<owl:NamedIndividual rdf:about="&idmp-spor;SPOR-DomainVocabulary-HumanAndVeterinaryUse-ShortName-Italian">
		<rdf:type rdf:resource="&idmp-spor;SPORTermName"/>
		<rdfs:label>SPOR-RMS, Domain Vocabulary, Human and Veterinary Use, Short Name, Italian</rdfs:label>
		<dct:source rdf:resource="https://spor.ema.europa.eu/v1/lists/100000000004/terms/100000000014"/>
		<skos:definition>SPOR short term name, in Italian, for the RMS domain vocabulary term, Human and Veterinary use</skos:definition>
		<cmns-col:isIncludedIn rdf:resource="&idmp-spor;SPOR-DomainVocabulary"/>
		<cmns-dsg:denotes rdf:resource="&idmp-spor;SPOR-Domain-HumanAndVeterinaryUse"/>
		<cmns-txt:hasTextValue xml:lang="it">H&amp;V</cmns-txt:hasTextValue>
		<mvf:hasLanguage rdf:resource="&lcc-639-1;Italian"/>
	</owl:NamedIndividual>
	
	<owl:NamedIndividual rdf:about="&idmp-spor;SPOR-DomainVocabulary-HumanAndVeterinaryUse-ShortName-Swedish">
		<rdf:type rdf:resource="&idmp-spor;SPORTermName"/>
		<rdfs:label>SPOR-RMS, Domain Vocabulary, Human and Veterinary Use, Short Name, Swedish</rdfs:label>
		<dct:source rdf:resource="https://spor.ema.europa.eu/v1/lists/100000000004/terms/100000000014"/>
		<skos:definition>SPOR short term name, in Swedish, for the RMS domain vocabulary term, Human and Veterinary use</skos:definition>
		<cmns-col:isIncludedIn rdf:resource="&idmp-spor;SPOR-DomainVocabulary"/>
		<cmns-dsg:denotes rdf:resource="&idmp-spor;SPOR-Domain-HumanAndVeterinaryUse"/>
		<cmns-txt:hasTextValue xml:lang="sv">H&amp;V</cmns-txt:hasTextValue>
		<mvf:hasLanguage rdf:resource="&lcc-639-1;Swedish"/>
	</owl:NamedIndividual>
	
	<owl:NamedIndividual rdf:about="&idmp-spor;SPOR-DomainVocabulary-HumanAndVeterinaryUse-TermName-Czech">
		<rdf:type rdf:resource="&idmp-spor;SPORTermName"/>
		<rdfs:label>SPOR-RMS, Domain Vocabulary, Human and Veterinary Use, Term Name, Czech</rdfs:label>
		<dct:source rdf:resource="https://spor.ema.europa.eu/v1/lists/100000000004/terms/100000000014"/>
		<skos:definition>SPOR term name, in Czech, for the RMS domain vocabulary term, Human and Veterinary use</skos:definition>
		<cmns-col:isIncludedIn rdf:resource="&idmp-spor;SPOR-DomainVocabulary"/>
		<cmns-dsg:denotes rdf:resource="&idmp-spor;SPOR-Domain-HumanAndVeterinaryUse"/>
		<cmns-txt:hasTextValue xml:lang="cs">Humánní a veterinární použití</cmns-txt:hasTextValue>
		<mvf:hasLanguage rdf:resource="&lcc-639-1;Czech"/>
	</owl:NamedIndividual>
	
	<owl:NamedIndividual rdf:about="&idmp-spor;SPOR-DomainVocabulary-HumanAndVeterinaryUse-TermName-English">
		<rdf:type rdf:resource="&idmp-spor;SPORTermName"/>
		<rdfs:label>SPOR-RMS, Domain Vocabulary, Human and Veterinary Use, Term Name, English</rdfs:label>
		<dct:source rdf:resource="https://spor.ema.europa.eu/v1/lists/100000000004/terms/100000000014"/>
		<skos:definition>SPOR term name, in English, for the RMS domain vocabulary term, Human and Veterinary use</skos:definition>
		<cmns-col:isIncludedIn rdf:resource="&idmp-spor;SPOR-DomainVocabulary"/>
		<cmns-dsg:denotes rdf:resource="&idmp-spor;SPOR-Domain-HumanAndVeterinaryUse"/>
		<cmns-txt:hasTextValue xml:lang="en">Human and Veterinary use</cmns-txt:hasTextValue>
		<mvf:hasLanguage rdf:resource="&lcc-639-1;English"/>
	</owl:NamedIndividual>
	
	<owl:NamedIndividual rdf:about="&idmp-spor;SPOR-DomainVocabulary-HumanAndVeterinaryUse-TermName-French">
		<rdf:type rdf:resource="&idmp-spor;SPORTermName"/>
		<rdfs:label>SPOR-RMS, Domain Vocabulary, Human and Veterinary Use, Term Name, French</rdfs:label>
		<dct:source rdf:resource="https://spor.ema.europa.eu/v1/lists/100000000004/terms/100000000014"/>
		<skos:definition>SPOR term name, in French, for the RMS domain vocabulary term, Human and Veterinary use</skos:definition>
		<cmns-col:isIncludedIn rdf:resource="&idmp-spor;SPOR-DomainVocabulary"/>
		<cmns-dsg:denotes rdf:resource="&idmp-spor;SPOR-Domain-HumanAndVeterinaryUse"/>
		<cmns-txt:hasTextValue xml:lang="fr-FR">Usage humain et vétérinaire</cmns-txt:hasTextValue>
		<mvf:hasLanguage rdf:resource="&lcc-639-1;French"/>
	</owl:NamedIndividual>
	
	<owl:NamedIndividual rdf:about="&idmp-spor;SPOR-DomainVocabulary-HumanAndVeterinaryUse-TermName-German">
		<rdf:type rdf:resource="&idmp-spor;SPORTermName"/>
		<rdfs:label>SPOR-RMS, Domain Vocabulary, Human and Veterinary Use, Term Name, German</rdfs:label>
		<dct:source rdf:resource="https://spor.ema.europa.eu/v1/lists/100000000004/terms/100000000014"/>
		<skos:definition>SPOR term name, in German, for the RMS domain vocabulary term, Human and Veterinary use</skos:definition>
		<cmns-col:isIncludedIn rdf:resource="&idmp-spor;SPOR-DomainVocabulary"/>
		<cmns-dsg:denotes rdf:resource="&idmp-spor;SPOR-Domain-HumanAndVeterinaryUse"/>
		<cmns-txt:hasTextValue xml:lang="de">Anwendung an Mensch und Tier</cmns-txt:hasTextValue>
		<mvf:hasLanguage rdf:resource="&lcc-639-1;German"/>
	</owl:NamedIndividual>
	
	<owl:NamedIndividual rdf:about="&idmp-spor;SPOR-DomainVocabulary-HumanAndVeterinaryUse-TermName-Italian">
		<rdf:type rdf:resource="&idmp-spor;SPORTermName"/>
		<rdfs:label>SPOR-RMS, Domain Vocabulary, Human and Veterinary Use, Term Name, Italian</rdfs:label>
		<dct:source rdf:resource="https://spor.ema.europa.eu/v1/lists/100000000004/terms/100000000014"/>
		<skos:definition>SPOR term name, in Italian, for the RMS domain vocabulary term, Human and Veterinary use</skos:definition>
		<cmns-col:isIncludedIn rdf:resource="&idmp-spor;SPOR-DomainVocabulary"/>
		<cmns-dsg:denotes rdf:resource="&idmp-spor;SPOR-Domain-HumanAndVeterinaryUse"/>
		<cmns-txt:hasTextValue xml:lang="it">uso umano e veterinario</cmns-txt:hasTextValue>
		<mvf:hasLanguage rdf:resource="&lcc-639-1;Italian"/>
	</owl:NamedIndividual>
	
	<owl:NamedIndividual rdf:about="&idmp-spor;SPOR-DomainVocabulary-HumanAndVeterinaryUse-TermName-Latvian">
		<rdf:type rdf:resource="&idmp-spor;SPORTermName"/>
		<rdfs:label>SPOR-RMS, Domain Vocabulary, Human and Veterinary Use, Term Name, Latvian</rdfs:label>
		<dct:source rdf:resource="https://spor.ema.europa.eu/v1/lists/100000000004/terms/100000000014"/>
		<skos:definition>SPOR term name, in Latvian, for the RMS domain vocabulary term, Human and Veterinary use</skos:definition>
		<cmns-col:isIncludedIn rdf:resource="&idmp-spor;SPOR-DomainVocabulary"/>
		<cmns-dsg:denotes rdf:resource="&idmp-spor;SPOR-Domain-HumanAndVeterinaryUse"/>
		<cmns-txt:hasTextValue xml:lang="lv">Lietošanai cilvēkiem un dzīvniekiem</cmns-txt:hasTextValue>
		<mvf:hasLanguage rdf:resource="&lcc-639-1;Latvian"/>
	</owl:NamedIndividual>
	
	<owl:NamedIndividual rdf:about="&idmp-spor;SPOR-DomainVocabulary-HumanAndVeterinaryUse-TermName-Norwegian">
		<rdf:type rdf:resource="&idmp-spor;SPORTermName"/>
		<rdfs:label>SPOR-RMS, Domain Vocabulary, Human and Veterinary Use, Term Name, Norwegian</rdfs:label>
		<dct:source rdf:resource="https://spor.ema.europa.eu/v1/lists/100000000004/terms/100000000014"/>
		<skos:definition>SPOR term name, in Norwegian, for the RMS domain vocabulary term, Human and Veterinary use</skos:definition>
		<cmns-col:isIncludedIn rdf:resource="&idmp-spor;SPOR-DomainVocabulary"/>
		<cmns-dsg:denotes rdf:resource="&idmp-spor;SPOR-Domain-HumanAndVeterinaryUse"/>
		<cmns-txt:hasTextValue xml:lang="no">Human og veterinær bruk</cmns-txt:hasTextValue>
		<mvf:hasLanguage rdf:resource="&lcc-639-1;Norwegian"/>
	</owl:NamedIndividual>
	
	<owl:NamedIndividual rdf:about="&idmp-spor;SPOR-DomainVocabulary-HumanAndVeterinaryUse-TermName-Swedish">
		<rdf:type rdf:resource="&idmp-spor;SPORTermName"/>
		<rdfs:label>SPOR-RMS, Domain Vocabulary, Human and Veterinary Use, Term Name, Swedish</rdfs:label>
		<dct:source rdf:resource="https://spor.ema.europa.eu/v1/lists/100000000004/terms/100000000014"/>
		<skos:definition>SPOR term name, in Swedish, for the RMS domain vocabulary term, Human and Veterinary use</skos:definition>
		<cmns-col:isIncludedIn rdf:resource="&idmp-spor;SPOR-DomainVocabulary"/>
		<cmns-dsg:denotes rdf:resource="&idmp-spor;SPOR-Domain-HumanAndVeterinaryUse"/>
		<cmns-txt:hasTextValue xml:lang="sv">Humant och veterinärmedicinskt bruk</cmns-txt:hasTextValue>
		<mvf:hasLanguage rdf:resource="&lcc-639-1;Swedish"/>
	</owl:NamedIndividual>
	
	<owl:NamedIndividual rdf:about="&idmp-spor;SPOR-DomainVocabulary-HumanUse-OtherName-Human-German">
		<rdf:type rdf:resource="&idmp-spor;SPORTermName"/>
		<rdfs:label>SPOR-RMS, Domain Vocabulary, Human Use, Other Name, Human, German</rdfs:label>
		<dct:source rdf:resource="https://spor.ema.europa.eu/v1/lists/100000000004/terms/100000000012"/>
		<skos:definition>SPOR other term name, in German, for the RMS domain vocabulary term, Human use</skos:definition>
		<cmns-col:isIncludedIn rdf:resource="&idmp-spor;SPOR-DomainVocabulary"/>
		<cmns-dsg:denotes rdf:resource="&idmp-spor;SPOR-Domain-HumanUse"/>
		<cmns-txt:hasTextValue xml:lang="de">Human</cmns-txt:hasTextValue>
		<mvf:hasLanguage rdf:resource="&lcc-639-1;German"/>
	</owl:NamedIndividual>
	
	<owl:NamedIndividual rdf:about="&idmp-spor;SPOR-DomainVocabulary-HumanUse-ShortName-English">
		<rdf:type rdf:resource="&idmp-spor;SPORTermName"/>
		<rdfs:label>SPOR-RMS, Domain Vocabulary, Human Use, Short Name, English</rdfs:label>
		<dct:source rdf:resource="https://spor.ema.europa.eu/v1/lists/100000000004/terms/100000000012"/>
		<skos:definition>SPOR short term name, in English, for the RMS domain vocabulary term, Human use</skos:definition>
		<cmns-col:isIncludedIn rdf:resource="&idmp-spor;SPOR-DomainVocabulary"/>
		<cmns-dsg:denotes rdf:resource="&idmp-spor;SPOR-Domain-HumanUse"/>
		<cmns-txt:hasTextValue xml:lang="en">H</cmns-txt:hasTextValue>
		<mvf:hasLanguage rdf:resource="&lcc-639-1;English"/>
	</owl:NamedIndividual>
	
	<owl:NamedIndividual rdf:about="&idmp-spor;SPOR-DomainVocabulary-HumanUse-ShortName-French">
		<rdf:type rdf:resource="&idmp-spor;SPORTermName"/>
		<rdfs:label>SPOR-RMS, Domain Vocabulary, Human Use, Short Name, French</rdfs:label>
		<dct:source rdf:resource="https://spor.ema.europa.eu/v1/lists/100000000004/terms/100000000012"/>
		<skos:definition>SPOR short term name, in French, for the RMS domain vocabulary term, Human use</skos:definition>
		<cmns-col:isIncludedIn rdf:resource="&idmp-spor;SPOR-DomainVocabulary"/>
		<cmns-dsg:denotes rdf:resource="&idmp-spor;SPOR-Domain-HumanUse"/>
		<cmns-txt:hasTextValue xml:lang="fr-FR">H</cmns-txt:hasTextValue>
		<mvf:hasLanguage rdf:resource="&lcc-639-1;French"/>
	</owl:NamedIndividual>
	
	<owl:NamedIndividual rdf:about="&idmp-spor;SPOR-DomainVocabulary-HumanUse-ShortName-German">
		<rdf:type rdf:resource="&idmp-spor;SPORTermName"/>
		<rdfs:label>SPOR-RMS, Domain Vocabulary, Human Use, Short Name, German</rdfs:label>
		<dct:source rdf:resource="https://spor.ema.europa.eu/v1/lists/100000000004/terms/100000000012"/>
		<skos:definition>SPOR short term name, in German, for the RMS domain vocabulary term, Human use</skos:definition>
		<cmns-col:isIncludedIn rdf:resource="&idmp-spor;SPOR-DomainVocabulary"/>
		<cmns-dsg:denotes rdf:resource="&idmp-spor;SPOR-Domain-HumanUse"/>
		<cmns-txt:hasTextValue xml:lang="de">H</cmns-txt:hasTextValue>
		<mvf:hasLanguage rdf:resource="&lcc-639-1;German"/>
	</owl:NamedIndividual>
	
	<owl:NamedIndividual rdf:about="&idmp-spor;SPOR-DomainVocabulary-HumanUse-ShortName-Italian">
		<rdf:type rdf:resource="&idmp-spor;SPORTermName"/>
		<rdfs:label>SPOR-RMS, Domain Vocabulary, Human Use, Short Name, Italian</rdfs:label>
		<dct:source rdf:resource="https://spor.ema.europa.eu/v1/lists/100000000004/terms/100000000012"/>
		<skos:definition>SPOR short term name, in Italian, for the RMS domain vocabulary term, Human use</skos:definition>
		<cmns-col:isIncludedIn rdf:resource="&idmp-spor;SPOR-DomainVocabulary"/>
		<cmns-dsg:denotes rdf:resource="&idmp-spor;SPOR-Domain-HumanUse"/>
		<cmns-txt:hasTextValue xml:lang="it">H</cmns-txt:hasTextValue>
		<mvf:hasLanguage rdf:resource="&lcc-639-1;Italian"/>
	</owl:NamedIndividual>
	
	<owl:NamedIndividual rdf:about="&idmp-spor;SPOR-DomainVocabulary-HumanUse-ShortName-Swedish">
		<rdf:type rdf:resource="&idmp-spor;SPORTermName"/>
		<rdfs:label>SPOR-RMS, Domain Vocabulary, Human Use, Short Name, Swedish</rdfs:label>
		<dct:source rdf:resource="https://spor.ema.europa.eu/v1/lists/100000000004/terms/100000000012"/>
		<skos:definition>SPOR short term name, in Swedish, for the RMS domain vocabulary term, Human use</skos:definition>
		<cmns-col:isIncludedIn rdf:resource="&idmp-spor;SPOR-DomainVocabulary"/>
		<cmns-dsg:denotes rdf:resource="&idmp-spor;SPOR-Domain-HumanUse"/>
		<cmns-txt:hasTextValue xml:lang="sv">H</cmns-txt:hasTextValue>
		<mvf:hasLanguage rdf:resource="&lcc-639-1;Swedish"/>
	</owl:NamedIndividual>
	
	<owl:NamedIndividual rdf:about="&idmp-spor;SPOR-DomainVocabulary-HumanUse-TermName-English">
		<rdf:type rdf:resource="&idmp-spor;SPORTermName"/>
		<rdfs:label>SPOR-RMS, Domain Vocabulary, Human Use, Term Name, English</rdfs:label>
		<dct:source rdf:resource="https://spor.ema.europa.eu/v1/lists/100000000004/terms/100000000012"/>
		<skos:definition>SPOR term name, in English, for the RMS domain vocabulary term, Human use</skos:definition>
		<cmns-col:isIncludedIn rdf:resource="&idmp-spor;SPOR-DomainVocabulary"/>
		<cmns-dsg:denotes rdf:resource="&idmp-spor;SPOR-Domain-HumanUse"/>
		<cmns-txt:hasTextValue xml:lang="en">Human use</cmns-txt:hasTextValue>
		<mvf:hasLanguage rdf:resource="&lcc-639-1;English"/>
	</owl:NamedIndividual>
	
	<owl:NamedIndividual rdf:about="&idmp-spor;SPOR-DomainVocabulary-HumanUse-TermName-French">
		<rdf:type rdf:resource="&idmp-spor;SPORTermName"/>
		<rdfs:label>SPOR-RMS, Domain Vocabulary, Human Use, Term Name, French</rdfs:label>
		<dct:source rdf:resource="https://spor.ema.europa.eu/v1/lists/100000000004/terms/100000000012"/>
		<skos:definition>SPOR term name, in French, for the RMS domain vocabulary term, Human use</skos:definition>
		<cmns-col:isIncludedIn rdf:resource="&idmp-spor;SPOR-DomainVocabulary"/>
		<cmns-dsg:denotes rdf:resource="&idmp-spor;SPOR-Domain-HumanUse"/>
		<cmns-txt:hasTextValue xml:lang="fr-FR">Usage humain</cmns-txt:hasTextValue>
		<mvf:hasLanguage rdf:resource="&lcc-639-1;French"/>
	</owl:NamedIndividual>
	
	<owl:NamedIndividual rdf:about="&idmp-spor;SPOR-DomainVocabulary-HumanUse-TermName-German">
		<rdf:type rdf:resource="&idmp-spor;SPORTermName"/>
		<rdfs:label>SPOR-RMS, Domain Vocabulary, Human Use, Term Name, German</rdfs:label>
		<dct:source rdf:resource="https://spor.ema.europa.eu/v1/lists/100000000004/terms/100000000012"/>
		<skos:definition>SPOR term name, in German, for the RMS domain vocabulary term, Human use</skos:definition>
		<cmns-col:isIncludedIn rdf:resource="&idmp-spor;SPOR-DomainVocabulary"/>
		<cmns-dsg:denotes rdf:resource="&idmp-spor;SPOR-Domain-HumanUse"/>
		<cmns-txt:hasTextValue xml:lang="de">Anwendung am Menschen</cmns-txt:hasTextValue>
		<mvf:hasLanguage rdf:resource="&lcc-639-1;German"/>
	</owl:NamedIndividual>
	
	<owl:NamedIndividual rdf:about="&idmp-spor;SPOR-DomainVocabulary-HumanUse-TermName-Italian">
		<rdf:type rdf:resource="&idmp-spor;SPORTermName"/>
		<rdfs:label>SPOR-RMS, Domain Vocabulary, Human Use, Term Name, Italian</rdfs:label>
		<dct:source rdf:resource="https://spor.ema.europa.eu/v1/lists/100000000004/terms/100000000012"/>
		<skos:definition>SPOR term name, in Italian, for the RMS domain vocabulary term, Human use</skos:definition>
		<cmns-col:isIncludedIn rdf:resource="&idmp-spor;SPOR-DomainVocabulary"/>
		<cmns-dsg:denotes rdf:resource="&idmp-spor;SPOR-Domain-HumanUse"/>
		<cmns-txt:hasTextValue xml:lang="it">uso umano</cmns-txt:hasTextValue>
		<mvf:hasLanguage rdf:resource="&lcc-639-1;Italian"/>
	</owl:NamedIndividual>
	
	<owl:NamedIndividual rdf:about="&idmp-spor;SPOR-DomainVocabulary-HumanUse-TermName-Latvian">
		<rdf:type rdf:resource="&idmp-spor;SPORTermName"/>
		<rdfs:label>SPOR-RMS, Domain Vocabulary, Human Use, Term Name, Latvian</rdfs:label>
		<dct:source rdf:resource="https://spor.ema.europa.eu/v1/lists/100000000004/terms/100000000012"/>
		<skos:definition>SPOR term name, in Latvian, for the RMS domain vocabulary term, Human use</skos:definition>
		<cmns-col:isIncludedIn rdf:resource="&idmp-spor;SPOR-DomainVocabulary"/>
		<cmns-dsg:denotes rdf:resource="&idmp-spor;SPOR-Domain-HumanUse"/>
		<cmns-txt:hasTextValue xml:lang="lv">Lietošanai cilvēkiem</cmns-txt:hasTextValue>
		<mvf:hasLanguage rdf:resource="&lcc-639-1;Latvian"/>
	</owl:NamedIndividual>
	
	<owl:NamedIndividual rdf:about="&idmp-spor;SPOR-DomainVocabulary-HumanUse-TermName-Norwegian">
		<rdf:type rdf:resource="&idmp-spor;SPORTermName"/>
		<rdfs:label>SPOR-RMS, Domain Vocabulary, Human Use, Term Name, Norwegian</rdfs:label>
		<dct:source rdf:resource="https://spor.ema.europa.eu/v1/lists/100000000004/terms/100000000012"/>
		<skos:definition>SPOR term name, in Norwegian, for the RMS domain vocabulary term, Human use</skos:definition>
		<cmns-col:isIncludedIn rdf:resource="&idmp-spor;SPOR-DomainVocabulary"/>
		<cmns-dsg:denotes rdf:resource="&idmp-spor;SPOR-Domain-HumanUse"/>
		<cmns-txt:hasTextValue xml:lang="no">Human bruk</cmns-txt:hasTextValue>
		<mvf:hasLanguage rdf:resource="&lcc-639-1;Norwegian"/>
	</owl:NamedIndividual>
	
	<owl:NamedIndividual rdf:about="&idmp-spor;SPOR-DomainVocabulary-HumanUse-TermName-Swedish">
		<rdf:type rdf:resource="&idmp-spor;SPORTermName"/>
		<rdfs:label>SPOR-RMS, Domain Vocabulary, Human Use, Term Name, Swedish</rdfs:label>
		<dct:source rdf:resource="https://spor.ema.europa.eu/v1/lists/100000000004/terms/100000000012"/>
		<skos:definition>SPOR term name, in Swedish, for the RMS domain vocabulary term, Human use</skos:definition>
		<cmns-col:isIncludedIn rdf:resource="&idmp-spor;SPOR-DomainVocabulary"/>
		<cmns-dsg:denotes rdf:resource="&idmp-spor;SPOR-Domain-HumanUse"/>
		<cmns-txt:hasTextValue xml:lang="sv">Humant bruk</cmns-txt:hasTextValue>
		<mvf:hasLanguage rdf:resource="&lcc-639-1;Swedish"/>
	</owl:NamedIndividual>
	
	<owl:NamedIndividual rdf:about="&idmp-spor;SPOR-DomainVocabulary-VeterinaryUse-OtherName-Veterinär-German">
		<rdf:type rdf:resource="&idmp-spor;SPORTermName"/>
		<rdfs:label>SPOR-RMS, Domain Vocabulary, Human Use, Other Name, Veterinär, German</rdfs:label>
		<dct:source rdf:resource="https://spor.ema.europa.eu/v1/lists/100000000004/terms/100000000013"/>
		<skos:definition>SPOR other term name, in German, for the RMS domain vocabulary term, Veterinary use</skos:definition>
		<cmns-col:isIncludedIn rdf:resource="&idmp-spor;SPOR-DomainVocabulary"/>
		<cmns-dsg:denotes rdf:resource="&idmp-spor;SPOR-Domain-VeterinaryUse"/>
		<cmns-txt:hasTextValue xml:lang="de">Veterinär</cmns-txt:hasTextValue>
		<mvf:hasLanguage rdf:resource="&lcc-639-1;German"/>
	</owl:NamedIndividual>
	
	<owl:NamedIndividual rdf:about="&idmp-spor;SPOR-DomainVocabulary-VeterinaryUse-ShortName-Czech">
		<rdf:type rdf:resource="&idmp-spor;SPORTermName"/>
		<rdfs:label>SPOR-RMS, Domain Vocabulary, Veterinary Use, Short Name, Czech</rdfs:label>
		<dct:source rdf:resource="https://spor.ema.europa.eu/v1/lists/100000000004/terms/100000000013"/>
		<skos:definition>SPOR short term name, in Czech, for the RMS domain vocabulary term, Veterinary use</skos:definition>
		<cmns-col:isIncludedIn rdf:resource="&idmp-spor;SPOR-DomainVocabulary"/>
		<cmns-dsg:denotes rdf:resource="&idmp-spor;SPOR-Domain-VeterinaryUse"/>
		<cmns-txt:hasTextValue xml:lang="cs">V</cmns-txt:hasTextValue>
		<mvf:hasLanguage rdf:resource="&lcc-639-1;Czech"/>
	</owl:NamedIndividual>
	
	<owl:NamedIndividual rdf:about="&idmp-spor;SPOR-DomainVocabulary-VeterinaryUse-ShortName-English">
		<rdf:type rdf:resource="&idmp-spor;SPORTermName"/>
		<rdfs:label>SPOR-RMS, Domain Vocabulary, Veterinary Use, Short Name, English</rdfs:label>
		<dct:source rdf:resource="https://spor.ema.europa.eu/v1/lists/100000000004/terms/100000000013"/>
		<skos:definition>SPOR short term name, in English, for the RMS domain vocabulary term, Veterinary use</skos:definition>
		<cmns-col:isIncludedIn rdf:resource="&idmp-spor;SPOR-DomainVocabulary"/>
		<cmns-dsg:denotes rdf:resource="&idmp-spor;SPOR-Domain-VeterinaryUse"/>
		<cmns-txt:hasTextValue xml:lang="en">V</cmns-txt:hasTextValue>
		<mvf:hasLanguage rdf:resource="&lcc-639-1;English"/>
	</owl:NamedIndividual>
	
	<owl:NamedIndividual rdf:about="&idmp-spor;SPOR-DomainVocabulary-VeterinaryUse-ShortName-French">
		<rdf:type rdf:resource="&idmp-spor;SPORTermName"/>
		<rdfs:label>SPOR-RMS, Domain Vocabulary, Veterinary Use, Short Name, French</rdfs:label>
		<dct:source rdf:resource="https://spor.ema.europa.eu/v1/lists/100000000004/terms/100000000013"/>
		<skos:definition>SPOR short term name, in French, for the RMS domain vocabulary term, Veterinary use</skos:definition>
		<cmns-col:isIncludedIn rdf:resource="&idmp-spor;SPOR-DomainVocabulary"/>
		<cmns-dsg:denotes rdf:resource="&idmp-spor;SPOR-Domain-VeterinaryUse"/>
		<cmns-txt:hasTextValue xml:lang="fr-FR">V</cmns-txt:hasTextValue>
		<mvf:hasLanguage rdf:resource="&lcc-639-1;French"/>
	</owl:NamedIndividual>
	
	<owl:NamedIndividual rdf:about="&idmp-spor;SPOR-DomainVocabulary-VeterinaryUse-ShortName-German">
		<rdf:type rdf:resource="&idmp-spor;SPORTermName"/>
		<rdfs:label>SPOR-RMS, Domain Vocabulary, Veterinary Use, Short Name, German</rdfs:label>
		<dct:source rdf:resource="https://spor.ema.europa.eu/v1/lists/100000000004/terms/100000000013"/>
		<skos:definition>SPOR short term name, in German, for the RMS domain vocabulary term, Veterinary use</skos:definition>
		<cmns-col:isIncludedIn rdf:resource="&idmp-spor;SPOR-DomainVocabulary"/>
		<cmns-dsg:denotes rdf:resource="&idmp-spor;SPOR-Domain-VeterinaryUse"/>
		<cmns-txt:hasTextValue xml:lang="de">V</cmns-txt:hasTextValue>
		<mvf:hasLanguage rdf:resource="&lcc-639-1;German"/>
	</owl:NamedIndividual>
	
	<owl:NamedIndividual rdf:about="&idmp-spor;SPOR-DomainVocabulary-VeterinaryUse-ShortName-Italian">
		<rdf:type rdf:resource="&idmp-spor;SPORTermName"/>
		<rdfs:label>SPOR-RMS, Domain Vocabulary, Veterinary Use, Short Name, Italian</rdfs:label>
		<dct:source rdf:resource="https://spor.ema.europa.eu/v1/lists/100000000004/terms/100000000013"/>
		<skos:definition>SPOR short term name, in Italian, for the RMS domain vocabulary term, Veterinary use</skos:definition>
		<cmns-col:isIncludedIn rdf:resource="&idmp-spor;SPOR-DomainVocabulary"/>
		<cmns-dsg:denotes rdf:resource="&idmp-spor;SPOR-Domain-VeterinaryUse"/>
		<cmns-txt:hasTextValue xml:lang="it">V</cmns-txt:hasTextValue>
		<mvf:hasLanguage rdf:resource="&lcc-639-1;Italian"/>
	</owl:NamedIndividual>
	
	<owl:NamedIndividual rdf:about="&idmp-spor;SPOR-DomainVocabulary-VeterinaryUse-ShortName-Swedish">
		<rdf:type rdf:resource="&idmp-spor;SPORTermName"/>
		<rdfs:label>SPOR-RMS, Domain Vocabulary, Veterinary Use, Short Name, Swedish</rdfs:label>
		<dct:source rdf:resource="https://spor.ema.europa.eu/v1/lists/100000000004/terms/100000000013"/>
		<skos:definition>SPOR short term name, in Swedish, for the RMS domain vocabulary term, Veterinary use</skos:definition>
		<cmns-col:isIncludedIn rdf:resource="&idmp-spor;SPOR-DomainVocabulary"/>
		<cmns-dsg:denotes rdf:resource="&idmp-spor;SPOR-Domain-VeterinaryUse"/>
		<cmns-txt:hasTextValue xml:lang="sv">V</cmns-txt:hasTextValue>
		<mvf:hasLanguage rdf:resource="&lcc-639-1;Swedish"/>
	</owl:NamedIndividual>
	
	<owl:NamedIndividual rdf:about="&idmp-spor;SPOR-DomainVocabulary-VeterinaryUse-TermName-Czech">
		<rdf:type rdf:resource="&idmp-spor;SPORTermName"/>
		<rdfs:label>SPOR-RMS, Domain Vocabulary, Veterinary Use, Term Name, Czech</rdfs:label>
		<dct:source rdf:resource="https://spor.ema.europa.eu/v1/lists/100000000004/terms/100000000013"/>
		<skos:definition>SPOR term name, in Czech, for the RMS domain vocabulary term, Veterinary use</skos:definition>
		<cmns-col:isIncludedIn rdf:resource="&idmp-spor;SPOR-DomainVocabulary"/>
		<cmns-dsg:denotes rdf:resource="&idmp-spor;SPOR-Domain-VeterinaryUse"/>
		<cmns-txt:hasTextValue xml:lang="cs">Veterinární použití</cmns-txt:hasTextValue>
		<mvf:hasLanguage rdf:resource="&lcc-639-1;Czech"/>
	</owl:NamedIndividual>
	
	<owl:NamedIndividual rdf:about="&idmp-spor;SPOR-DomainVocabulary-VeterinaryUse-TermName-English">
		<rdf:type rdf:resource="&idmp-spor;SPORTermName"/>
		<rdfs:label>SPOR-RMS, Domain Vocabulary, Veterinary Use, Term Name, English</rdfs:label>
		<dct:source rdf:resource="https://spor.ema.europa.eu/v1/lists/100000000004/terms/100000000013"/>
		<skos:definition>SPOR term name, in English, for the RMS domain vocabulary term, Veterinary use</skos:definition>
		<cmns-col:isIncludedIn rdf:resource="&idmp-spor;SPOR-DomainVocabulary"/>
		<cmns-dsg:denotes rdf:resource="&idmp-spor;SPOR-Domain-VeterinaryUse"/>
		<cmns-txt:hasTextValue xml:lang="en">Veterinary use</cmns-txt:hasTextValue>
		<mvf:hasLanguage rdf:resource="&lcc-639-1;English"/>
	</owl:NamedIndividual>
	
	<owl:NamedIndividual rdf:about="&idmp-spor;SPOR-DomainVocabulary-VeterinaryUse-TermName-French">
		<rdf:type rdf:resource="&idmp-spor;SPORTermName"/>
		<rdfs:label>SPOR-RMS, Domain Vocabulary, Veterinary Use, Term Name, French</rdfs:label>
		<dct:source rdf:resource="https://spor.ema.europa.eu/v1/lists/100000000004/terms/100000000013"/>
		<skos:definition>SPOR term name, in French, for the RMS domain vocabulary term, Veterinary use</skos:definition>
		<cmns-col:isIncludedIn rdf:resource="&idmp-spor;SPOR-DomainVocabulary"/>
		<cmns-dsg:denotes rdf:resource="&idmp-spor;SPOR-Domain-VeterinaryUse"/>
		<cmns-txt:hasTextValue xml:lang="fr-FR">Usage vétérinaire</cmns-txt:hasTextValue>
		<mvf:hasLanguage rdf:resource="&lcc-639-1;French"/>
	</owl:NamedIndividual>
	
	<owl:NamedIndividual rdf:about="&idmp-spor;SPOR-DomainVocabulary-VeterinaryUse-TermName-German">
		<rdf:type rdf:resource="&idmp-spor;SPORTermName"/>
		<rdfs:label>SPOR-RMS, Domain Vocabulary, Veterinary Use, Term Name, German</rdfs:label>
		<dct:source rdf:resource="https://spor.ema.europa.eu/v1/lists/100000000004/terms/100000000013"/>
		<skos:definition>SPOR term name, in German, for the RMS domain vocabulary term, Veterinary use</skos:definition>
		<cmns-col:isIncludedIn rdf:resource="&idmp-spor;SPOR-DomainVocabulary"/>
		<cmns-dsg:denotes rdf:resource="&idmp-spor;SPOR-Domain-VeterinaryUse"/>
		<cmns-txt:hasTextValue xml:lang="de">Anwendung am Tier</cmns-txt:hasTextValue>
		<mvf:hasLanguage rdf:resource="&lcc-639-1;German"/>
	</owl:NamedIndividual>
	
	<owl:NamedIndividual rdf:about="&idmp-spor;SPOR-DomainVocabulary-VeterinaryUse-TermName-Italian">
		<rdf:type rdf:resource="&idmp-spor;SPORTermName"/>
		<rdfs:label>SPOR-RMS, Domain Vocabulary, Veterinary Use, Term Name, Italian</rdfs:label>
		<dct:source rdf:resource="https://spor.ema.europa.eu/v1/lists/100000000004/terms/100000000013"/>
		<skos:definition>SPOR term name, in Italian, for the RMS domain vocabulary term, Veterinary use</skos:definition>
		<cmns-col:isIncludedIn rdf:resource="&idmp-spor;SPOR-DomainVocabulary"/>
		<cmns-dsg:denotes rdf:resource="&idmp-spor;SPOR-Domain-VeterinaryUse"/>
		<cmns-txt:hasTextValue xml:lang="it">uso veterinario</cmns-txt:hasTextValue>
		<mvf:hasLanguage rdf:resource="&lcc-639-1;Italian"/>
	</owl:NamedIndividual>
	
	<owl:NamedIndividual rdf:about="&idmp-spor;SPOR-DomainVocabulary-VeterinaryUse-TermName-Latvian">
		<rdf:type rdf:resource="&idmp-spor;SPORTermName"/>
		<rdfs:label>SPOR-RMS, Domain Vocabulary, Veterinary Use, Term Name, Latvian</rdfs:label>
		<dct:source rdf:resource="https://spor.ema.europa.eu/v1/lists/100000000004/terms/100000000013"/>
		<skos:definition>SPOR term name, in Latvian, for the RMS domain vocabulary term, Veterinary use</skos:definition>
		<cmns-col:isIncludedIn rdf:resource="&idmp-spor;SPOR-DomainVocabulary"/>
		<cmns-dsg:denotes rdf:resource="&idmp-spor;SPOR-Domain-VeterinaryUse"/>
		<cmns-txt:hasTextValue xml:lang="lv">Veterinārai lietošanai</cmns-txt:hasTextValue>
		<mvf:hasLanguage rdf:resource="&lcc-639-1;Latvian"/>
	</owl:NamedIndividual>
	
	<owl:NamedIndividual rdf:about="&idmp-spor;SPOR-DomainVocabulary-VeterinaryUse-TermName-Norwegian">
		<rdf:type rdf:resource="&idmp-spor;SPORTermName"/>
		<rdfs:label>SPOR-RMS, Domain Vocabulary, Veterinary Use, Term Name, Norwegian</rdfs:label>
		<dct:source rdf:resource="https://spor.ema.europa.eu/v1/lists/100000000004/terms/100000000013"/>
		<skos:definition>SPOR term name, in Norwegian, for the RMS domain vocabulary term, Veterinary use</skos:definition>
		<cmns-col:isIncludedIn rdf:resource="&idmp-spor;SPOR-DomainVocabulary"/>
		<cmns-dsg:denotes rdf:resource="&idmp-spor;SPOR-Domain-VeterinaryUse"/>
		<cmns-txt:hasTextValue xml:lang="no">Veterinær bruk</cmns-txt:hasTextValue>
		<mvf:hasLanguage rdf:resource="&lcc-639-1;Norwegian"/>
	</owl:NamedIndividual>
	
	<owl:NamedIndividual rdf:about="&idmp-spor;SPOR-DomainVocabulary-VeterinaryUse-TermName-Romanian">
		<rdf:type rdf:resource="&idmp-spor;SPORTermName"/>
		<rdfs:label>SPOR-RMS, Domain Vocabulary, Veterinary Use, Term Name, Romanian</rdfs:label>
		<dct:source rdf:resource="https://spor.ema.europa.eu/v1/lists/100000000004/terms/100000000013"/>
		<skos:definition>SPOR term name, in Romanian, for the RMS domain vocabulary term, Veterinary use</skos:definition>
		<cmns-col:isIncludedIn rdf:resource="&idmp-spor;SPOR-DomainVocabulary"/>
		<cmns-dsg:denotes rdf:resource="&idmp-spor;SPOR-Domain-VeterinaryUse"/>
		<cmns-txt:hasTextValue xml:lang="ro">Uz veterinar</cmns-txt:hasTextValue>
		<mvf:hasLanguage rdf:resource="&lcc-639-1;Romanian"/>
	</owl:NamedIndividual>
	
	<owl:NamedIndividual rdf:about="&idmp-spor;SPOR-DomainVocabulary-VeterinaryUse-TermName-Swedish">
		<rdf:type rdf:resource="&idmp-spor;SPORTermName"/>
		<rdfs:label>SPOR-RMS, Domain Vocabulary, Veterinary Use, Term Name, Swedish</rdfs:label>
		<dct:source rdf:resource="https://spor.ema.europa.eu/v1/lists/100000000004/terms/100000000013"/>
		<skos:definition>SPOR term name, in Swedish, for the RMS domain vocabulary term, Veterinary use</skos:definition>
		<cmns-col:isIncludedIn rdf:resource="&idmp-spor;SPOR-DomainVocabulary"/>
		<cmns-dsg:denotes rdf:resource="&idmp-spor;SPOR-Domain-VeterinaryUse"/>
		<cmns-txt:hasTextValue xml:lang="sv">Veterinärmedicinskt bruk</cmns-txt:hasTextValue>
		<mvf:hasLanguage rdf:resource="&lcc-639-1;Swedish"/>
	</owl:NamedIndividual>
	
	<owl:NamedIndividual rdf:about="&idmp-spor;SPOR-ListIdentifier-100000000004">
		<rdf:type rdf:resource="&idmp-spor;SPORListIdentifier"/>
		<rdfs:label>SPOR List Identifier 100000000004</rdfs:label>
		<skos:definition>SPOR list identifier for the domain vocabulary</skos:definition>
		<cmns-av:adaptedFrom rdf:resource="https://spor.ema.europa.eu/v1/lists/100000000004"/>
		<cmns-id:identifies rdf:resource="&idmp-spor;SPOR-DomainVocabulary"/>
		<cmns-ra:hasRegistrationDate>2022-12-12T05:55:17</cmns-ra:hasRegistrationDate>
		<cmns-ra:isRegisteredBy rdf:resource="&idmp-eura;EuropeanMedicinesAgencyRegistrationAuthority"/>
		<cmns-txt:hasTextValue>100000000004</cmns-txt:hasTextValue>
	</owl:NamedIndividual>
	
	<owl:NamedIndividual rdf:about="&idmp-spor;SPOR-ListIdentifier-200000004983">
		<rdf:type rdf:resource="&idmp-spor;SPORListIdentifier"/>
		<rdfs:label>SPOR List Identifier 200000004983</rdfs:label>
		<skos:definition>SPOR list identifier for the data classification vocabulary</skos:definition>
		<cmns-av:adaptedFrom rdf:resource="https://spor.ema.europa.eu/v1/lists/200000004983"/>
		<cmns-id:identifies rdf:resource="&idmp-spor;SPOR-DataClassificationVocabulary"/>
		<cmns-ra:hasRegistrationDate>2020-05-14T07:23:34</cmns-ra:hasRegistrationDate>
		<cmns-ra:isRegisteredBy rdf:resource="&idmp-eura;EuropeanMedicinesAgencyRegistrationAuthority"/>
		<cmns-txt:hasTextValue>200000004983</cmns-txt:hasTextValue>
	</owl:NamedIndividual>
	
	<owl:NamedIndividual rdf:about="&idmp-spor;SPOR-ListIdentifier-200000005003">
		<rdf:type rdf:resource="&idmp-spor;SPORListIdentifier"/>
		<rdfs:label>SPOR List Identifier 200000005003</rdfs:label>
		<skos:definition>SPOR list identifier for the record status vocabulary</skos:definition>
		<cmns-av:adaptedFrom rdf:resource="https://spor.ema.europa.eu/v1/lists/200000005003"/>
		<cmns-id:identifies rdf:resource="&idmp-spor;SPOR-RecordStatusVocabulary"/>
		<cmns-ra:hasRegistrationDate>2021-09-09T00:25:04</cmns-ra:hasRegistrationDate>
		<cmns-ra:isRegisteredBy rdf:resource="&idmp-eura;EuropeanMedicinesAgencyRegistrationAuthority"/>
		<cmns-txt:hasTextValue>200000005003</cmns-txt:hasTextValue>
	</owl:NamedIndividual>
	
	<owl:NamedIndividual rdf:about="&idmp-spor;SPOR-ListName-100000000004">
		<rdf:type rdf:resource="&idmp-spor;SPORListName"/>
		<rdfs:label>SPOR List Name 100000000004</rdfs:label>
		<dct:source rdf:resource="https://spor.ema.europa.eu/v1/lists/100000000004"/>
		<skos:definition>SPOR list name for the RMS domain vocabulary</skos:definition>
		<cmns-col:isIncludedIn rdf:resource="&idmp-spor;SPOR-DomainVocabulary"/>
		<cmns-dsg:isNameOf rdf:resource="&idmp-spor;SPOR-DomainVocabulary"/>
		<cmns-txt:hasTextValue>Domain</cmns-txt:hasTextValue>
		<mvf:hasLanguage rdf:resource="&lcc-639-1;English"/>
	</owl:NamedIndividual>
	
	<owl:NamedIndividual rdf:about="&idmp-spor;SPOR-ListName-200000004983">
		<rdf:type rdf:resource="&idmp-spor;SPORListName"/>
		<rdfs:label>SPOR List Name 200000004983</rdfs:label>
		<dct:source rdf:resource="https://spor.ema.europa.eu/v1/lists/200000004983"/>
		<skos:definition>SPOR list name for the RMS data classification vocabulary</skos:definition>
		<cmns-col:isIncludedIn rdf:resource="&idmp-spor;SPOR-DataClassificationVocabulary"/>
		<cmns-dsg:isNameOf rdf:resource="&idmp-spor;SPOR-DomainVocabulary"/>
		<cmns-txt:hasTextValue>Data Classification</cmns-txt:hasTextValue>
		<mvf:hasLanguage rdf:resource="&lcc-639-1;English"/>
	</owl:NamedIndividual>
	
	<owl:NamedIndividual rdf:about="&idmp-spor;SPOR-ListName-200000005003">
		<rdf:type rdf:resource="&idmp-spor;SPORListName"/>
		<rdfs:label>SPOR List Name 200000005003</rdfs:label>
		<dct:source rdf:resource="https://spor.ema.europa.eu/v1/lists/200000005003"/>
		<skos:definition>SPOR list name for the record status vocabulary</skos:definition>
		<cmns-col:isIncludedIn rdf:resource="&idmp-spor;SPOR-RecordStatusVocabulary"/>
		<cmns-dsg:isNameOf rdf:resource="&idmp-spor;SPOR-RecordStatusVocabulary"/>
		<cmns-txt:hasTextValue>Record Status</cmns-txt:hasTextValue>
		<mvf:hasLanguage rdf:resource="&lcc-639-1;English"/>
	</owl:NamedIndividual>
	
	<owl:Class rdf:about="&idmp-spor;SPOR-RecordStatus">
		<rdfs:subClassOf rdf:resource="&idmp-spor;SPORControlledVocabularyTerm"/>
		<rdfs:subClassOf rdf:resource="&mvf;TermStatus"/>
		<rdfs:label>SPOR record status</rdfs:label>
		<skos:definition>classifier and code element that describes the state of something in a Substances Products Organisations Referentials (SPOR) registry as of some point in time</skos:definition>
		<cmns-av:adaptedFrom rdf:resource="https://spor.ema.europa.eu/v1/lists/200000005003"/>
	</owl:Class>
	
	<owl:NamedIndividual rdf:about="&idmp-spor;SPOR-RecordStatus-Current">
		<rdf:type rdf:resource="&idmp-spor;SPOR-RecordStatus"/>
		<owl:sameAs rdf:resource="https://spor.ema.europa.eu/v1/lists/200000005003/terms/200000005004"/>
		<rdfs:label>SPOR record status - current</rdfs:label>
		<skos:definition>classifier and code element that describes the state of something in a Substances Products Organisations Referentials (SPOR) registry as being current as of some point in time</skos:definition>
		<idmp-spor:hasSPORDomain rdf:resource="&idmp-spor;SPOR-Domain-HumanAndVeterinaryUse"/>
		<idmp-spor:hasSPORStatus rdf:resource="&idmp-spor;SPOR-RecordStatus-Current"/>
		<idmp-spor:hasSPORTermName rdf:resource="&idmp-spor;SPOR-RecordStatusVocabulary-Current-TermName-English"/>
		<idmp-spor:hasSPORTermName rdf:resource="&idmp-spor;SPOR-RecordStatusVocabulary-Current-TermName-French"/>
		<idmp-spor:hasSPORTermName rdf:resource="&idmp-spor;SPOR-RecordStatusVocabulary-Current-TermName-Italian"/>
		<idmp-spor:hasSPORTermName rdf:resource="&idmp-spor;SPOR-RecordStatusVocabulary-Current-TermName-Latvian"/>
		<idmp-spor:hasSPORVisibility rdf:resource="&idmp-spor;SPOR-DataClassification-Public"/>
		<cmns-col:isIncludedIn rdf:resource="&idmp-spor;SPOR-RecordStatusVocabulary"/>
		<cmns-id:isIdentifiedBy rdf:resource="&idmp-spor;SPOR-TermIdentifier-200000005003-200000005004"/>
	</owl:NamedIndividual>
	
	<owl:NamedIndividual rdf:about="&idmp-spor;SPOR-RecordStatus-NonCurrent">
		<rdf:type rdf:resource="&idmp-spor;SPOR-RecordStatus"/>
		<owl:sameAs rdf:resource="https://spor.ema.europa.eu/v1/lists/200000005003/terms/200000005006"/>
		<rdfs:label>SPOR record status - non-current</rdfs:label>
		<skos:definition>classifier and code element that describes the state of something in a Substances Products Organisations Referentials (SPOR) registry as being non-current as of some point in time</skos:definition>
		<idmp-spor:hasSPORDomain rdf:resource="&idmp-spor;SPOR-Domain-HumanAndVeterinaryUse"/>
		<idmp-spor:hasSPORStatus rdf:resource="&idmp-spor;SPOR-RecordStatus-Current"/>
		<idmp-spor:hasSPORTermName rdf:resource="&idmp-spor;SPOR-RecordStatusVocabulary-NonCurrent-TermName-English"/>
		<idmp-spor:hasSPORTermName rdf:resource="&idmp-spor;SPOR-RecordStatusVocabulary-NonCurrent-TermName-French"/>
		<idmp-spor:hasSPORTermName rdf:resource="&idmp-spor;SPOR-RecordStatusVocabulary-NonCurrent-TermName-Italian"/>
		<idmp-spor:hasSPORTermName rdf:resource="&idmp-spor;SPOR-RecordStatusVocabulary-NonCurrent-TermName-Latvian"/>
		<idmp-spor:hasSPORVisibility rdf:resource="&idmp-spor;SPOR-DataClassification-Public"/>
		<cmns-col:isIncludedIn rdf:resource="&idmp-spor;SPOR-RecordStatusVocabulary"/>
		<cmns-id:isIdentifiedBy rdf:resource="&idmp-spor;SPOR-TermIdentifier-200000005003-200000005006"/>
	</owl:NamedIndividual>
	
	<owl:NamedIndividual rdf:about="&idmp-spor;SPOR-RecordStatus-Nullified">
		<rdf:type rdf:resource="&idmp-spor;SPOR-RecordStatus"/>
		<owl:sameAs rdf:resource="https://spor.ema.europa.eu/v1/lists/200000005003/terms/200000005007"/>
		<rdfs:label>SPOR record status - nullified</rdfs:label>
		<skos:definition>classifier and code element that describes the state of something in a Substances Products Organisations Referentials (SPOR) registry as being nullified as of some point in time</skos:definition>
		<idmp-spor:hasSPORDomain rdf:resource="&idmp-spor;SPOR-Domain-HumanAndVeterinaryUse"/>
		<idmp-spor:hasSPORStatus rdf:resource="&idmp-spor;SPOR-RecordStatus-Current"/>
		<idmp-spor:hasSPORTermName rdf:resource="&idmp-spor;SPOR-RecordStatusVocabulary-Nullified-TermName-English"/>
		<idmp-spor:hasSPORTermName rdf:resource="&idmp-spor;SPOR-RecordStatusVocabulary-Nullified-TermName-French"/>
		<idmp-spor:hasSPORTermName rdf:resource="&idmp-spor;SPOR-RecordStatusVocabulary-Nullified-TermName-Italian"/>
		<idmp-spor:hasSPORTermName rdf:resource="&idmp-spor;SPOR-RecordStatusVocabulary-Nullified-TermName-Latvian"/>
		<idmp-spor:hasSPORVisibility rdf:resource="&idmp-spor;SPOR-DataClassification-Public"/>
		<cmns-col:isIncludedIn rdf:resource="&idmp-spor;SPOR-RecordStatusVocabulary"/>
		<cmns-id:isIdentifiedBy rdf:resource="&idmp-spor;SPOR-TermIdentifier-200000005003-200000005007"/>
	</owl:NamedIndividual>
	
	<owl:NamedIndividual rdf:about="&idmp-spor;SPOR-RecordStatus-Provisional">
		<rdf:type rdf:resource="&idmp-spor;SPOR-RecordStatus"/>
		<rdfs:label>SPOR record status - provisional</rdfs:label>
		<dct:source rdf:resource="https://spor.ema.europa.eu/v1/lists/200000005003/terms/200000005005"/>
		<skos:definition>classifier and code element that describes the state of something in a Substances Products Organisations Referentials (SPOR) registry as being provisional as of some point in time</skos:definition>
		<idmp-spor:hasSPORDomain rdf:resource="&idmp-spor;SPOR-Domain-HumanAndVeterinaryUse"/>
		<idmp-spor:hasSPORStatus rdf:resource="&idmp-spor;SPOR-RecordStatus-Current"/>
		<idmp-spor:hasSPORTermName rdf:resource="&idmp-spor;SPOR-RecordStatusVocabulary-Provisional-TermName-English"/>
		<idmp-spor:hasSPORTermName rdf:resource="&idmp-spor;SPOR-RecordStatusVocabulary-Provisional-TermName-French"/>
		<idmp-spor:hasSPORTermName rdf:resource="&idmp-spor;SPOR-RecordStatusVocabulary-Provisional-TermName-Italian"/>
		<idmp-spor:hasSPORTermName rdf:resource="&idmp-spor;SPOR-RecordStatusVocabulary-Provisional-TermName-Latvian"/>
		<idmp-spor:hasSPORVisibility rdf:resource="&idmp-spor;SPOR-DataClassification-Public"/>
		<cmns-col:isIncludedIn rdf:resource="&idmp-spor;SPOR-RecordStatusVocabulary"/>
		<cmns-id:isIdentifiedBy rdf:resource="&idmp-spor;SPOR-TermIdentifier-200000005003-200000005005"/>
	</owl:NamedIndividual>
	
	<owl:NamedIndividual rdf:about="&idmp-spor;SPOR-RecordStatusVocabulary">
		<rdf:type rdf:resource="&idmp-spor;SPORControlledVocabulary"/>
		<owl:sameAs rdf:resource="https://spor.ema.europa.eu/v1/lists/200000005003"/>
		<rdfs:label>SPOR-RMS, Record Status Vocabulary</rdfs:label>
		<skos:definition>controlled vocabulary used to provide an indication of the status of any vocabulary (list) or term in Substances Products Organisations Referentials (SPOR)</skos:definition>
		<cmns-av:synonym>SPOR RMS record status list</cmns-av:synonym>
		<cmns-dsg:isSignifiedBy rdf:resource="&idmp-spor;SPOR-ListName-200000005003"/>
		<cmns-id:isIdentifiedBy rdf:resource="&idmp-spor;SPOR-ListIdentifier-200000005003"/>
	</owl:NamedIndividual>
	
	<owl:NamedIndividual rdf:about="&idmp-spor;SPOR-RecordStatusVocabulary-Current-TermName-English">
		<rdf:type rdf:resource="&idmp-spor;SPORTermName"/>
		<rdfs:label>SPOR-RMS, Record Status Vocabulary, Current, Term Name, English</rdfs:label>
		<dct:source rdf:resource="https://spor.ema.europa.eu/v1/lists/200000005003/terms/200000005004"/>
		<skos:definition>SPOR term name, in English, for the RMS record status vocabulary term, Current</skos:definition>
		<cmns-col:isIncludedIn rdf:resource="&idmp-spor;SPOR-DomainVocabulary"/>
		<cmns-dsg:denotes rdf:resource="&idmp-spor;SPOR-RecordStatus-Current"/>
		<cmns-txt:hasTextValue xml:lang="en">Current</cmns-txt:hasTextValue>
		<mvf:hasLanguage rdf:resource="&lcc-639-1;English"/>
	</owl:NamedIndividual>
	
	<owl:NamedIndividual rdf:about="&idmp-spor;SPOR-RecordStatusVocabulary-Current-TermName-French">
		<rdf:type rdf:resource="&idmp-spor;SPORTermName"/>
		<rdfs:label>SPOR-RMS, Record Status Vocabulary, Current, Term Name, French</rdfs:label>
		<dct:source rdf:resource="https://spor.ema.europa.eu/v1/lists/200000005003/terms/200000005004"/>
		<skos:definition>SPOR term name, in French, for the RMS record status vocabulary term, Current</skos:definition>
		<cmns-col:isIncludedIn rdf:resource="&idmp-spor;SPOR-DomainVocabulary"/>
		<cmns-dsg:denotes rdf:resource="&idmp-spor;SPOR-RecordStatus-Current"/>
		<cmns-txt:hasTextValue xml:lang="fr-FR">Valide</cmns-txt:hasTextValue>
		<mvf:hasLanguage rdf:resource="&lcc-639-1;French"/>
	</owl:NamedIndividual>
	
	<owl:NamedIndividual rdf:about="&idmp-spor;SPOR-RecordStatusVocabulary-Current-TermName-Italian">
		<rdf:type rdf:resource="&idmp-spor;SPORTermName"/>
		<rdfs:label>SPOR-RMS, Record Status Vocabulary, Current, Term Name, Italian</rdfs:label>
		<dct:source rdf:resource="https://spor.ema.europa.eu/v1/lists/200000005003/terms/200000005004"/>
		<skos:definition>SPOR term name, in Italian, for the RMS record status vocabulary term, Current</skos:definition>
		<cmns-col:isIncludedIn rdf:resource="&idmp-spor;SPOR-DomainVocabulary"/>
		<cmns-dsg:denotes rdf:resource="&idmp-spor;SPOR-RecordStatus-Current"/>
		<cmns-txt:hasTextValue xml:lang="it">Attuale</cmns-txt:hasTextValue>
		<mvf:hasLanguage rdf:resource="&lcc-639-1;Italian"/>
	</owl:NamedIndividual>
	
	<owl:NamedIndividual rdf:about="&idmp-spor;SPOR-RecordStatusVocabulary-Current-TermName-Latvian">
		<rdf:type rdf:resource="&idmp-spor;SPORTermName"/>
		<rdfs:label>SPOR-RMS, Record Status Vocabulary, Current, Term Name, Latvian</rdfs:label>
		<dct:source rdf:resource="https://spor.ema.europa.eu/v1/lists/200000005003/terms/200000005004"/>
		<skos:definition>SPOR term name, in Latvian, for the RMS record status vocabulary term, Current</skos:definition>
		<cmns-col:isIncludedIn rdf:resource="&idmp-spor;SPOR-DomainVocabulary"/>
		<cmns-dsg:denotes rdf:resource="&idmp-spor;SPOR-RecordStatus-Current"/>
		<cmns-txt:hasTextValue xml:lang="lv">Aktuāls</cmns-txt:hasTextValue>
		<mvf:hasLanguage rdf:resource="&lcc-639-1;Latvian"/>
	</owl:NamedIndividual>
	
	<owl:NamedIndividual rdf:about="&idmp-spor;SPOR-RecordStatusVocabulary-NonCurrent-TermName-English">
		<rdf:type rdf:resource="&idmp-spor;SPORTermName"/>
		<rdfs:label>SPOR-RMS, Record Status Vocabulary, Non-Current, Term Name, English</rdfs:label>
		<dct:source rdf:resource="https://spor.ema.europa.eu/v1/lists/200000005003/terms/200000005006"/>
		<skos:definition>SPOR term name, in English, for the RMS record status vocabulary term, Non-current</skos:definition>
		<cmns-col:isIncludedIn rdf:resource="&idmp-spor;SPOR-DomainVocabulary"/>
		<cmns-dsg:denotes rdf:resource="&idmp-spor;SPOR-RecordStatus-NonCurrent"/>
		<cmns-txt:hasTextValue xml:lang="en">Non-current</cmns-txt:hasTextValue>
		<mvf:hasLanguage rdf:resource="&lcc-639-1;English"/>
	</owl:NamedIndividual>
	
	<owl:NamedIndividual rdf:about="&idmp-spor;SPOR-RecordStatusVocabulary-NonCurrent-TermName-French">
		<rdf:type rdf:resource="&idmp-spor;SPORTermName"/>
		<rdfs:label>SPOR-RMS, Record Status Vocabulary, Non-Current, Term Name, French</rdfs:label>
		<dct:source rdf:resource="https://spor.ema.europa.eu/v1/lists/200000005003/terms/200000005006"/>
		<skos:definition>SPOR term name, in French, for the RMS record status vocabulary term, Non-current</skos:definition>
		<cmns-col:isIncludedIn rdf:resource="&idmp-spor;SPOR-DomainVocabulary"/>
		<cmns-dsg:denotes rdf:resource="&idmp-spor;SPOR-RecordStatus-NonCurrent"/>
		<cmns-txt:hasTextValue xml:lang="fr-FR">Non valide</cmns-txt:hasTextValue>
		<mvf:hasLanguage rdf:resource="&lcc-639-1;French"/>
	</owl:NamedIndividual>
	
	<owl:NamedIndividual rdf:about="&idmp-spor;SPOR-RecordStatusVocabulary-NonCurrent-TermName-Italian">
		<rdf:type rdf:resource="&idmp-spor;SPORTermName"/>
		<rdfs:label>SPOR-RMS, Record Status Vocabulary, Non-Current, Term Name, Italian</rdfs:label>
		<dct:source rdf:resource="https://spor.ema.europa.eu/v1/lists/200000005003/terms/200000005006"/>
		<skos:definition>SPOR term name, in Italian, for the RMS record status vocabulary term, Non-current</skos:definition>
		<cmns-col:isIncludedIn rdf:resource="&idmp-spor;SPOR-DomainVocabulary"/>
		<cmns-dsg:denotes rdf:resource="&idmp-spor;SPOR-RecordStatus-NonCurrent"/>
		<cmns-txt:hasTextValue xml:lang="it">Non attuale</cmns-txt:hasTextValue>
		<mvf:hasLanguage rdf:resource="&lcc-639-1;Italian"/>
	</owl:NamedIndividual>
	
	<owl:NamedIndividual rdf:about="&idmp-spor;SPOR-RecordStatusVocabulary-NonCurrent-TermName-Latvian">
		<rdf:type rdf:resource="&idmp-spor;SPORTermName"/>
		<rdfs:label>SPOR-RMS, Record Status Vocabulary, Non-Current, Term Name, Latvian</rdfs:label>
		<dct:source rdf:resource="https://spor.ema.europa.eu/v1/lists/200000005003/terms/200000005006"/>
		<skos:definition>SPOR term name, in Latvian, for the RMS record status vocabulary term, Non-current</skos:definition>
		<cmns-col:isIncludedIn rdf:resource="&idmp-spor;SPOR-DomainVocabulary"/>
		<cmns-dsg:denotes rdf:resource="&idmp-spor;SPOR-RecordStatus-NonCurrent"/>
		<cmns-txt:hasTextValue xml:lang="lv">Neaktuāls</cmns-txt:hasTextValue>
		<mvf:hasLanguage rdf:resource="&lcc-639-1;Latvian"/>
	</owl:NamedIndividual>
	
	<owl:NamedIndividual rdf:about="&idmp-spor;SPOR-RecordStatusVocabulary-Nullified-TermName-English">
		<rdf:type rdf:resource="&idmp-spor;SPORTermName"/>
		<rdfs:label>SPOR-RMS, Record Status Vocabulary, Nullified, Term Name, English</rdfs:label>
		<dct:source rdf:resource="https://spor.ema.europa.eu/v1/lists/200000005003/terms/200000005007"/>
		<skos:definition>SPOR term name, in English, for the RMS record status vocabulary term, Nullified</skos:definition>
		<cmns-col:isIncludedIn rdf:resource="&idmp-spor;SPOR-DomainVocabulary"/>
		<cmns-dsg:denotes rdf:resource="&idmp-spor;SPOR-RecordStatus-Nullified"/>
		<cmns-txt:hasTextValue xml:lang="en">Nullified</cmns-txt:hasTextValue>
		<mvf:hasLanguage rdf:resource="&lcc-639-1;English"/>
	</owl:NamedIndividual>
	
	<owl:NamedIndividual rdf:about="&idmp-spor;SPOR-RecordStatusVocabulary-Nullified-TermName-French">
		<rdf:type rdf:resource="&idmp-spor;SPORTermName"/>
		<rdfs:label>SPOR-RMS, Record Status Vocabulary, Nullified, Term Name, French</rdfs:label>
		<dct:source rdf:resource="https://spor.ema.europa.eu/v1/lists/200000005003/terms/200000005007"/>
		<skos:definition>SPOR term name, in French, for the RMS record status vocabulary term, Nullified</skos:definition>
		<cmns-col:isIncludedIn rdf:resource="&idmp-spor;SPOR-DomainVocabulary"/>
		<cmns-dsg:denotes rdf:resource="&idmp-spor;SPOR-RecordStatus-Nullified"/>
		<cmns-txt:hasTextValue xml:lang="fr-FR">Annulé</cmns-txt:hasTextValue>
		<mvf:hasLanguage rdf:resource="&lcc-639-1;French"/>
	</owl:NamedIndividual>
	
	<owl:NamedIndividual rdf:about="&idmp-spor;SPOR-RecordStatusVocabulary-Nullified-TermName-Italian">
		<rdf:type rdf:resource="&idmp-spor;SPORTermName"/>
		<rdfs:label>SPOR-RMS, Record Status Vocabulary, Nullified, Term Name, Italian</rdfs:label>
		<dct:source rdf:resource="https://spor.ema.europa.eu/v1/lists/200000005003/terms/200000005007"/>
		<skos:definition>SPOR term name, in Italian, for the RMS record status vocabulary term, Nullified</skos:definition>
		<cmns-col:isIncludedIn rdf:resource="&idmp-spor;SPOR-DomainVocabulary"/>
		<cmns-dsg:denotes rdf:resource="&idmp-spor;SPOR-RecordStatus-Nullified"/>
		<cmns-txt:hasTextValue xml:lang="it">Annullato</cmns-txt:hasTextValue>
		<mvf:hasLanguage rdf:resource="&lcc-639-1;Italian"/>
	</owl:NamedIndividual>
	
	<owl:NamedIndividual rdf:about="&idmp-spor;SPOR-RecordStatusVocabulary-Nullified-TermName-Latvian">
		<rdf:type rdf:resource="&idmp-spor;SPORTermName"/>
		<rdfs:label>SPOR-RMS, Record Status Vocabulary, Nullified, Term Name, Latvian</rdfs:label>
		<dct:source rdf:resource="https://spor.ema.europa.eu/v1/lists/200000005003/terms/200000005007"/>
		<skos:definition>SPOR term name, in Latvian, for the RMS record status vocabulary term, Nullified</skos:definition>
		<cmns-col:isIncludedIn rdf:resource="&idmp-spor;SPOR-DomainVocabulary"/>
		<cmns-dsg:denotes rdf:resource="&idmp-spor;SPOR-RecordStatus-Nullified"/>
		<cmns-txt:hasTextValue xml:lang="lv">Atcelts</cmns-txt:hasTextValue>
		<mvf:hasLanguage rdf:resource="&lcc-639-1;Latvian"/>
	</owl:NamedIndividual>
	
	<owl:NamedIndividual rdf:about="&idmp-spor;SPOR-RecordStatusVocabulary-Provisional-TermName-English">
		<rdf:type rdf:resource="&idmp-spor;SPORTermName"/>
		<rdfs:label>SPOR-RMS, Record Status Vocabulary, Provisional, Term Name, English</rdfs:label>
		<dct:source rdf:resource="https://spor.ema.europa.eu/v1/lists/200000005003/terms/200000005005"/>
		<skos:definition>SPOR term name, in English, for the RMS record status vocabulary term, Provisional</skos:definition>
		<cmns-col:isIncludedIn rdf:resource="&idmp-spor;SPOR-DomainVocabulary"/>
		<cmns-dsg:denotes rdf:resource="&idmp-spor;SPOR-RecordStatus-Provisional"/>
		<cmns-txt:hasTextValue xml:lang="en">Provisional</cmns-txt:hasTextValue>
		<mvf:hasLanguage rdf:resource="&lcc-639-1;English"/>
	</owl:NamedIndividual>
	
	<owl:NamedIndividual rdf:about="&idmp-spor;SPOR-RecordStatusVocabulary-Provisional-TermName-French">
		<rdf:type rdf:resource="&idmp-spor;SPORTermName"/>
		<rdfs:label>SPOR-RMS, Record Status Vocabulary, Provisional, Term Name, French</rdfs:label>
		<dct:source rdf:resource="https://spor.ema.europa.eu/v1/lists/200000005003/terms/200000005005"/>
		<skos:definition>SPOR term name, in French, for the RMS record status vocabulary term, Provisional</skos:definition>
		<cmns-col:isIncludedIn rdf:resource="&idmp-spor;SPOR-DomainVocabulary"/>
		<cmns-dsg:denotes rdf:resource="&idmp-spor;SPOR-RecordStatus-Provisional"/>
		<cmns-txt:hasTextValue xml:lang="fr-FR">Provisoire</cmns-txt:hasTextValue>
		<mvf:hasLanguage rdf:resource="&lcc-639-1;French"/>
	</owl:NamedIndividual>
	
	<owl:NamedIndividual rdf:about="&idmp-spor;SPOR-RecordStatusVocabulary-Provisional-TermName-Italian">
		<rdf:type rdf:resource="&idmp-spor;SPORTermName"/>
		<rdfs:label>SPOR-RMS, Record Status Vocabulary, Provisional, Term Name, Italian</rdfs:label>
		<dct:source rdf:resource="https://spor.ema.europa.eu/v1/lists/200000005003/terms/200000005005"/>
		<skos:definition>SPOR term name, in Italian, for the RMS record status vocabulary term, Provisional</skos:definition>
		<cmns-col:isIncludedIn rdf:resource="&idmp-spor;SPOR-DomainVocabulary"/>
		<cmns-dsg:denotes rdf:resource="&idmp-spor;SPOR-RecordStatus-Provisional"/>
		<cmns-txt:hasTextValue xml:lang="it">Provvisorio</cmns-txt:hasTextValue>
		<mvf:hasLanguage rdf:resource="&lcc-639-1;Italian"/>
	</owl:NamedIndividual>
	
	<owl:NamedIndividual rdf:about="&idmp-spor;SPOR-RecordStatusVocabulary-Provisional-TermName-Latvian">
		<rdf:type rdf:resource="&idmp-spor;SPORTermName"/>
		<rdfs:label>SPOR-RMS, Record Status Vocabulary, Provisional, Term Name, Latvian</rdfs:label>
		<dct:source rdf:resource="https://spor.ema.europa.eu/v1/lists/200000005003/terms/200000005005"/>
		<skos:definition>SPOR term name, in Latvian, for the RMS record status vocabulary term, Provisional</skos:definition>
		<cmns-col:isIncludedIn rdf:resource="&idmp-spor;SPOR-DomainVocabulary"/>
		<cmns-dsg:denotes rdf:resource="&idmp-spor;SPOR-RecordStatus-Provisional"/>
		<cmns-txt:hasTextValue xml:lang="lv">Provizorisks</cmns-txt:hasTextValue>
		<mvf:hasLanguage rdf:resource="&lcc-639-1;Latvian"/>
	</owl:NamedIndividual>
	
	<owl:NamedIndividual rdf:about="&idmp-spor;SPOR-TermIdentifier-100000000004-100000000012">
		<rdf:type rdf:resource="&idmp-spor;SPORTermIdentifier"/>
		<rdfs:label>SPOR Term Identifier 100000000004-100000000012</rdfs:label>
		<dct:source rdf:resource="https://spor.ema.europa.eu/v1/lists/100000000004/terms/100000000012"/>
		<skos:definition>SPOR term identifier for the domain term, Human use</skos:definition>
		<cmns-id:identifies rdf:resource="&idmp-spor;SPOR-Domain-HumanUse"/>
		<cmns-txt:hasTextValue>100000000012</cmns-txt:hasTextValue>
	</owl:NamedIndividual>
	
	<owl:NamedIndividual rdf:about="&idmp-spor;SPOR-TermIdentifier-100000000004-100000000013">
		<rdf:type rdf:resource="&idmp-spor;SPORTermIdentifier"/>
		<rdfs:label>SPOR Term Identifier 100000000004-100000000013</rdfs:label>
		<dct:source rdf:resource="https://spor.ema.europa.eu/v1/lists/100000000004/terms/100000000013"/>
		<skos:definition>SPOR term identifier for the domain term, Veterinary use</skos:definition>
		<cmns-id:identifies rdf:resource="&idmp-spor;SPOR-Domain-VeterinaryUse"/>
		<cmns-txt:hasTextValue>100000000013</cmns-txt:hasTextValue>
	</owl:NamedIndividual>
	
	<owl:NamedIndividual rdf:about="&idmp-spor;SPOR-TermIdentifier-100000000004-100000000014">
		<rdf:type rdf:resource="&idmp-spor;SPORTermIdentifier"/>
		<rdfs:label>SPOR Term Identifier 100000000004-00000000014</rdfs:label>
		<dct:source rdf:resource="https://spor.ema.europa.eu/v1/lists/100000000004/terms/100000000014"/>
		<skos:definition>SPOR term identifier for the domain term, Human and Veterinary use</skos:definition>
		<cmns-id:identifies rdf:resource="&idmp-spor;SPOR-Domain-HumanAndVeterinaryUse"/>
		<cmns-txt:hasTextValue>100000000014</cmns-txt:hasTextValue>
	</owl:NamedIndividual>
	
	<owl:NamedIndividual rdf:about="&idmp-spor;SPOR-TermIdentifier-200000004983-200000004984">
		<rdf:type rdf:resource="&idmp-spor;SPORTermIdentifier"/>
		<rdfs:label>SPOR Term Identifier 200000004983-200000004984</rdfs:label>
		<dct:source rdf:resource="https://spor.ema.europa.eu/v1/lists/200000004983/terms/200000004984"/>
		<skos:definition>SPOR term identifier for the data classification vocabulary term, Confidential</skos:definition>
		<cmns-id:identifies rdf:resource="&idmp-spor;SPOR-DataClassification-Confidential"/>
		<cmns-txt:hasTextValue>200000004984</cmns-txt:hasTextValue>
	</owl:NamedIndividual>
	
	<owl:NamedIndividual rdf:about="&idmp-spor;SPOR-TermIdentifier-200000004983-200000004985">
		<rdf:type rdf:resource="&idmp-spor;SPORTermIdentifier"/>
		<rdfs:label>SPOR Term Identifier 200000004983-200000004985</rdfs:label>
		<dct:source rdf:resource="https://spor.ema.europa.eu/v1/lists/200000004983/terms/200000004985"/>
		<skos:definition>SPOR term identifier for the data classification vocabulary term, Public</skos:definition>
		<cmns-id:identifies rdf:resource="&idmp-spor;SPOR-DataClassification-Public"/>
		<cmns-txt:hasTextValue>200000004985</cmns-txt:hasTextValue>
	</owl:NamedIndividual>
	
	<owl:NamedIndividual rdf:about="&idmp-spor;SPOR-TermIdentifier-200000004983-200000004986">
		<rdf:type rdf:resource="&idmp-spor;SPORTermIdentifier"/>
		<rdfs:label>SPOR Term Identifier 200000004983-200000004986</rdfs:label>
		<dct:source rdf:resource="https://spor.ema.europa.eu/v1/lists/200000004983/terms/200000004986"/>
		<skos:definition>SPOR term identifier for the data classification vocabulary term, Restricted</skos:definition>
		<cmns-id:identifies rdf:resource="&idmp-spor;SPOR-DataClassification-Restricted"/>
		<cmns-txt:hasTextValue>200000004986</cmns-txt:hasTextValue>
	</owl:NamedIndividual>
	
	<owl:NamedIndividual rdf:about="&idmp-spor;SPOR-TermIdentifier-200000005003-200000005004">
		<rdf:type rdf:resource="&idmp-spor;SPORTermIdentifier"/>
		<rdfs:label>SPOR Term Identifier 200000005003-200000005004</rdfs:label>
		<dct:source rdf:resource="https://spor.ema.europa.eu/v1/lists/200000005003/terms/200000005004"/>
		<skos:definition>SPOR term identifier for the record status term, Current</skos:definition>
		<cmns-id:identifies rdf:resource="&idmp-spor;SPOR-RecordStatus-Current"/>
		<cmns-txt:hasTextValue>200000005004</cmns-txt:hasTextValue>
	</owl:NamedIndividual>
	
	<owl:NamedIndividual rdf:about="&idmp-spor;SPOR-TermIdentifier-200000005003-200000005005">
		<rdf:type rdf:resource="&idmp-spor;SPORTermIdentifier"/>
		<rdfs:label>SPOR Term Identifier 200000005003-200000005005</rdfs:label>
		<dct:source rdf:resource="https://spor.ema.europa.eu/v1/lists/200000005003/terms/200000005005"/>
		<skos:definition>SPOR term identifier for the record status term, Provisional</skos:definition>
		<cmns-id:identifies rdf:resource="&idmp-spor;SPOR-RecordStatus-Provisional"/>
		<cmns-txt:hasTextValue>200000005005</cmns-txt:hasTextValue>
	</owl:NamedIndividual>
	
	<owl:NamedIndividual rdf:about="&idmp-spor;SPOR-TermIdentifier-200000005003-200000005006">
		<rdf:type rdf:resource="&idmp-spor;SPORTermIdentifier"/>
		<rdfs:label>SPOR Term Identifier 200000005003-200000005006</rdfs:label>
		<dct:source rdf:resource="https://spor.ema.europa.eu/v1/lists/200000005003/terms/200000005006"/>
		<skos:definition>SPOR term identifier for the record status term, Non-current</skos:definition>
		<cmns-id:identifies rdf:resource="&idmp-spor;SPOR-RecordStatus-NonCurrent"/>
		<cmns-txt:hasTextValue>200000005006</cmns-txt:hasTextValue>
	</owl:NamedIndividual>
	
	<owl:NamedIndividual rdf:about="&idmp-spor;SPOR-TermIdentifier-200000005003-200000005007">
		<rdf:type rdf:resource="&idmp-spor;SPORTermIdentifier"/>
		<rdfs:label>SPOR Term Identifier 200000005003-200000005007</rdfs:label>
		<dct:source rdf:resource="https://spor.ema.europa.eu/v1/lists/200000005003/terms/200000005007"/>
		<skos:definition>SPOR term identifier for the record status term, Nullified</skos:definition>
		<cmns-id:identifies rdf:resource="&idmp-spor;SPOR-RecordStatus-Nullified"/>
		<cmns-txt:hasTextValue>200000005007</cmns-txt:hasTextValue>
	</owl:NamedIndividual>
	
	<owl:Class rdf:about="&idmp-spor;SPORControlledVocabulary">
		<rdfs:subClassOf rdf:resource="&idmp-dtp;ControlledVocabulary"/>
		<rdfs:subClassOf rdf:resource="&cmns-cls;ClassificationScheme"/>
		<rdfs:subClassOf rdf:resource="&cmns-cds;CodeSet"/>
		<rdfs:subClassOf>
			<owl:Restriction>
				<owl:onProperty rdf:resource="&cmns-col;isIncludedIn"/>
				<owl:hasValue rdf:resource="&idmp-spor;ReferentialsManagementServicesRegistry"/>
			</owl:Restriction>
		</rdfs:subClassOf>
		<rdfs:subClassOf>
			<owl:Restriction>
				<owl:onProperty rdf:resource="&cmns-dsg;isSignifiedBy"/>
				<owl:onClass rdf:resource="&idmp-spor;SPORListName"/>
				<owl:minQualifiedCardinality rdf:datatype="&xsd;nonNegativeInteger">0</owl:minQualifiedCardinality>
			</owl:Restriction>
		</rdfs:subClassOf>
		<rdfs:subClassOf>
			<owl:Restriction>
				<owl:onProperty rdf:resource="&cmns-id;isIdentifiedBy"/>
				<owl:onClass rdf:resource="&idmp-spor;SPORListIdentifier"/>
				<owl:qualifiedCardinality rdf:datatype="&xsd;nonNegativeInteger">1</owl:qualifiedCardinality>
			</owl:Restriction>
		</rdfs:subClassOf>
		<rdfs:label>SPOR controlled vocabulary</rdfs:label>
		<skos:definition>controlled vocabulary used to classify entities included in the Substances Products Organisations Referentials (SPOR) Referentials Management Services (RMS) related services and repositories</skos:definition>
		<cmns-av:synonym>SPOR List</cmns-av:synonym>
	</owl:Class>
	
	<owl:Class rdf:about="&idmp-spor;SPORControlledVocabularyTerm">
		<rdfs:subClassOf rdf:resource="&cmns-cls;Classifier"/>
		<rdfs:subClassOf rdf:resource="&cmns-cds;CodeElement"/>
		<rdfs:subClassOf rdf:resource="&mvf-trm;Term"/>
		<rdfs:subClassOf>
			<owl:Restriction>
				<owl:onProperty rdf:resource="&cmns-col;isIncludedIn"/>
				<owl:onClass rdf:resource="&idmp-spor;SPORControlledVocabulary"/>
				<owl:minQualifiedCardinality rdf:datatype="&xsd;nonNegativeInteger">0</owl:minQualifiedCardinality>
			</owl:Restriction>
		</rdfs:subClassOf>
		<rdfs:subClassOf>
			<owl:Restriction>
				<owl:onProperty rdf:resource="&idmp-spor;hasSPORTermDescription"/>
				<owl:onClass rdf:resource="&idmp-spor;SPORTermDescription"/>
				<owl:minQualifiedCardinality rdf:datatype="&xsd;nonNegativeInteger">0</owl:minQualifiedCardinality>
			</owl:Restriction>
		</rdfs:subClassOf>
		<rdfs:subClassOf>
			<owl:Restriction>
				<owl:onProperty rdf:resource="&idmp-spor;hasSPOROtherName"/>
				<owl:onClass rdf:resource="&idmp-spor;SPORTermName"/>
				<owl:minQualifiedCardinality rdf:datatype="&xsd;nonNegativeInteger">0</owl:minQualifiedCardinality>
			</owl:Restriction>
		</rdfs:subClassOf>
		<rdfs:subClassOf>
			<owl:Restriction>
				<owl:onProperty rdf:resource="&idmp-spor;hasSPORShortName"/>
				<owl:onClass rdf:resource="&idmp-spor;SPORTermName"/>
				<owl:minQualifiedCardinality rdf:datatype="&xsd;nonNegativeInteger">0</owl:minQualifiedCardinality>
			</owl:Restriction>
		</rdfs:subClassOf>
		<rdfs:subClassOf>
			<owl:Restriction>
				<owl:onProperty rdf:resource="&cmns-dsg;denotes"/>
				<owl:onClass>
					<owl:Class>
						<owl:unionOf rdf:parseType="Collection">
							<rdf:Description rdf:about="&idmp-sub;Substance">
							</rdf:Description>
							<rdf:Description rdf:about="&cmns-prd;Product">
							</rdf:Description>
						</owl:unionOf>
					</owl:Class>
				</owl:onClass>
				<owl:minQualifiedCardinality rdf:datatype="&xsd;nonNegativeInteger">0</owl:minQualifiedCardinality>
			</owl:Restriction>
		</rdfs:subClassOf>
		<rdfs:subClassOf>
			<owl:Restriction>
				<owl:onProperty rdf:resource="&cmns-cls;classifies"/>
				<owl:onClass>
					<owl:Class>
						<owl:unionOf rdf:parseType="Collection">
							<rdf:Description rdf:about="&idmp-sub;Substance">
							</rdf:Description>
							<rdf:Description rdf:about="&cmns-prd;Product">
							</rdf:Description>
						</owl:unionOf>
					</owl:Class>
				</owl:onClass>
				<owl:minQualifiedCardinality rdf:datatype="&xsd;nonNegativeInteger">0</owl:minQualifiedCardinality>
			</owl:Restriction>
		</rdfs:subClassOf>
		<rdfs:subClassOf>
			<owl:Restriction>
				<owl:onProperty rdf:resource="&idmp-spor;hasSPORVisibility"/>
				<owl:onClass rdf:resource="&idmp-spor;SPOR-DataClassification"/>
				<owl:qualifiedCardinality rdf:datatype="&xsd;nonNegativeInteger">1</owl:qualifiedCardinality>
			</owl:Restriction>
		</rdfs:subClassOf>
		<rdfs:subClassOf>
			<owl:Restriction>
				<owl:onProperty rdf:resource="&idmp-spor;hasSPORStatus"/>
				<owl:onClass rdf:resource="&idmp-spor;SPOR-RecordStatus"/>
				<owl:qualifiedCardinality rdf:datatype="&xsd;nonNegativeInteger">1</owl:qualifiedCardinality>
			</owl:Restriction>
		</rdfs:subClassOf>
		<rdfs:subClassOf>
			<owl:Restriction>
				<owl:onProperty rdf:resource="&cmns-id;isIdentifiedBy"/>
				<owl:onClass rdf:resource="&idmp-spor;SPORTermIdentifier"/>
				<owl:qualifiedCardinality rdf:datatype="&xsd;nonNegativeInteger">1</owl:qualifiedCardinality>
			</owl:Restriction>
		</rdfs:subClassOf>
		<rdfs:subClassOf>
			<owl:Restriction>
				<owl:onProperty rdf:resource="&idmp-spor;hasSPORTermName"/>
				<owl:someValuesFrom rdf:resource="&idmp-spor;SPORTermName"/>
			</owl:Restriction>
		</rdfs:subClassOf>
		<rdfs:label>SPOR controlled vocabulary term</rdfs:label>
		<skos:definition>term in a controlled vocabulary whose values describe some substance or product from a Substances Products Organisations Referentials (SPOR) perspective</skos:definition>
		<cmns-av:synonym>SPOR term</cmns-av:synonym>
	</owl:Class>
	
	<owl:Class rdf:about="&idmp-spor;SPORListIdentifier">
		<rdfs:subClassOf rdf:resource="&cmns-ra;RegisteredIdentifier"/>
		<rdfs:subClassOf>
			<owl:Restriction>
				<owl:onProperty rdf:resource="&cmns-col;compliesWith"/>
				<owl:hasValue rdf:resource="&idmp-spor;ReferentialsManagementServicesRegistrationScheme"/>
			</owl:Restriction>
		</rdfs:subClassOf>
		<rdfs:subClassOf>
			<owl:Restriction>
				<owl:onProperty rdf:resource="&cmns-ra;isRegisteredIn"/>
				<owl:hasValue rdf:resource="&idmp-spor;ReferentialsManagementServicesRegistry"/>
			</owl:Restriction>
		</rdfs:subClassOf>
		<rdfs:label>SPOR list identifier</rdfs:label>
		<skos:definition>contextual identifier for a controlled vocabulary (list) that is registered in the Substances Products Organisations Referentials (SPOR) Referentials Management Services (RMS) registry</skos:definition>
	</owl:Class>
	
	<owl:Class rdf:about="&idmp-spor;SPORListName">
		<rdfs:subClassOf rdf:resource="&cmns-cxtdsg;ContextualName"/>
		<rdfs:subClassOf rdf:resource="&mvf-trm;Term"/>
		<rdfs:subClassOf>
			<owl:Restriction>
				<owl:onProperty rdf:resource="&cmns-cxtdsg;isApplicableIn"/>
				<owl:hasValue rdf:resource="&idmp-spor;SubstancesProductsOrganisationsReferentialsDataManagementServices"/>
			</owl:Restriction>
		</rdfs:subClassOf>
		<rdfs:subClassOf>
			<owl:Restriction>
				<owl:onProperty rdf:resource="&mvf;hasLanguage"/>
				<owl:onClass rdf:resource="&lcc-lr;Language"/>
				<owl:minQualifiedCardinality rdf:datatype="&xsd;nonNegativeInteger">0</owl:minQualifiedCardinality>
			</owl:Restriction>
		</rdfs:subClassOf>
		<rdfs:subClassOf>
			<owl:Restriction>
				<owl:onProperty rdf:resource="&cmns-dsg;isNameOf"/>
				<owl:someValuesFrom rdf:resource="&idmp-spor;SPORControlledVocabulary"/>
			</owl:Restriction>
		</rdfs:subClassOf>
		<rdfs:label>SPOR list name</rdfs:label>
		<skos:definition>name for a controlled vocabulary (list) managed in the Substances Products Organisations Referentials (SPOR) Referentials Management Services (RMS) registry</skos:definition>
	</owl:Class>
	
	<owl:Class rdf:about="&idmp-spor;SPORTermDescription">
		<rdfs:subClassOf rdf:resource="&cmns-cls;Aspect"/>
		<rdfs:subClassOf>
			<owl:Restriction>
				<owl:onProperty rdf:resource="&cmns-cxtdsg;isApplicableIn"/>
				<owl:hasValue rdf:resource="&idmp-spor;SubstancesProductsOrganisationsReferentialsDataManagementServices"/>
			</owl:Restriction>
		</rdfs:subClassOf>
		<rdfs:subClassOf>
			<owl:Restriction>
				<owl:onProperty rdf:resource="&mvf;hasLanguage"/>
				<owl:onClass rdf:resource="&lcc-lr;Language"/>
				<owl:minQualifiedCardinality rdf:datatype="&xsd;nonNegativeInteger">0</owl:minQualifiedCardinality>
			</owl:Restriction>
		</rdfs:subClassOf>
		<rdfs:subClassOf>
			<owl:Restriction>
				<owl:onProperty rdf:resource="&cmns-dsg;describes"/>
				<owl:someValuesFrom rdf:resource="&idmp-spor;SPORControlledVocabularyTerm"/>
			</owl:Restriction>
		</rdfs:subClassOf>
		<rdfs:label>SPOR term description</rdfs:label>
		<skos:definition>description of a term in a controlled vocabulary (list) that is registered in the Substances Products Organisations Referentials (SPOR) Referentials Management Services (RMS) registry</skos:definition>
	</owl:Class>
	
	<owl:Class rdf:about="&idmp-spor;SPORTermIdentifier">
		<rdfs:subClassOf rdf:resource="&cmns-ra;RegisteredIdentifier"/>
		<rdfs:subClassOf>
			<owl:Restriction>
				<owl:onProperty rdf:resource="&cmns-col;compliesWith"/>
				<owl:hasValue rdf:resource="&idmp-spor;ReferentialsManagementServicesRegistrationScheme"/>
			</owl:Restriction>
		</rdfs:subClassOf>
		<rdfs:subClassOf>
			<owl:Restriction>
				<owl:onProperty rdf:resource="&cmns-ra;isRegisteredIn"/>
				<owl:hasValue rdf:resource="&idmp-spor;ReferentialsManagementServicesRegistry"/>
			</owl:Restriction>
		</rdfs:subClassOf>
		<rdfs:label>SPOR term identifier</rdfs:label>
		<skos:definition>contextual identifier for a term in a controlled vocabulary (list) that is registered in the Substances Products Organisations Referentials (SPOR) Referentials Management Services (RMS) registry</skos:definition>
	</owl:Class>
	
	<owl:Class rdf:about="&idmp-spor;SPORTermName">
		<rdfs:subClassOf rdf:resource="&cmns-cxtdsg;ContextualName"/>
		<rdfs:subClassOf rdf:resource="&mvf-trm;Term"/>
		<rdfs:subClassOf>
			<owl:Restriction>
				<owl:onProperty rdf:resource="&cmns-cxtdsg;isApplicableIn"/>
				<owl:hasValue rdf:resource="&idmp-spor;SubstancesProductsOrganisationsReferentialsDataManagementServices"/>
			</owl:Restriction>
		</rdfs:subClassOf>
		<rdfs:subClassOf>
			<owl:Restriction>
				<owl:onProperty rdf:resource="&mvf;hasLanguage"/>
				<owl:onClass rdf:resource="&lcc-lr;Language"/>
				<owl:minQualifiedCardinality rdf:datatype="&xsd;nonNegativeInteger">0</owl:minQualifiedCardinality>
			</owl:Restriction>
		</rdfs:subClassOf>
		<rdfs:subClassOf>
			<owl:Restriction>
				<owl:onProperty rdf:resource="&cmns-dsg;isNameOf"/>
				<owl:someValuesFrom rdf:resource="&idmp-spor;SPORControlledVocabularyTerm"/>
			</owl:Restriction>
		</rdfs:subClassOf>
		<rdfs:label>SPOR term name</rdfs:label>
		<skos:definition>name for a term in a controlled vocabulary in Substances Products Organisations Referentials (SPOR)</skos:definition>
	</owl:Class>
	
	<owl:NamedIndividual rdf:about="&idmp-spor;SubstanceManagementServices">
		<rdf:type rdf:resource="&cmns-ra;RegistrationService"/>
		<rdfs:label>Substance Management Services (SMS)</rdfs:label>
		<skos:definition>services supporting a central dictionary of substance data in multiple languages</skos:definition>
		<cmns-av:abbreviation>SMS service</cmns-av:abbreviation>
		<cmns-av:directSource rdf:resource="https://spor.ema.europa.eu/"/>
		<cmns-col:isPartOf rdf:resource="&idmp-spor;SubstancesProductsOrganisationsReferentialsDataManagementServices"/>
		<cmns-prd:isProvidedBy rdf:resource="&idmp-eura;EuropeanMedicinesAgencyRegistrationAuthority"/>
	</owl:NamedIndividual>
	
	<owl:NamedIndividual rdf:about="&idmp-spor;SubstancesManagementServicesRegistry">
		<rdf:type rdf:resource="&cmns-ra;Registry"/>
		<rdfs:label>Substances Management Services registry</rdfs:label>
		<skos:definition>central dictionary of substance data in multiple languages available through the Substances Products Organisations Referentials (SPOR) Substances Management Services (SMS)</skos:definition>
		<cmns-av:abbreviation>SPOR SMS</cmns-av:abbreviation>
		<cmns-av:abbreviation>SPOR-SMS</cmns-av:abbreviation>
		<cmns-av:directSource rdf:resource="https://spor.ema.europa.eu/"/>
		<cmns-av:explanatoryNote>SMS is currently live as an EMA internal system. Until it is onboarded in the SPOR portal, external users should use the following systems: view and search substance data in EUTCT or IRIS; submit substance change requests in the EMA Service Desk portal; Export of substance data are available at https://spor.ema.europa.eu/web-ui-data-backend/download/csv.</cmns-av:explanatoryNote>
		<cmns-ra:isManagedBy rdf:resource="&idmp-eura;EuropeanMedicinesAgencyRegistrationAuthority"/>
	</owl:NamedIndividual>
	
	<owl:NamedIndividual rdf:about="&idmp-spor;SubstancesProductsOrganisationsReferentialsDataManagementServices">
		<rdf:type rdf:resource="&cmns-ra;RegistrationService"/>
		<rdfs:label>Substances Products Organisations Referentials (SPOR) data management services</rdfs:label>
		<skos:definition>data management services for substances, products, organisations and referentials (SPOR) designed to support regulatory activities in the European Union</skos:definition>
		<cmns-av:abbreviation>SPOR data management services</cmns-av:abbreviation>
		<cmns-av:directSource rdf:resource="https://spor.ema.europa.eu/"/>
		<cmns-col:hasPart rdf:resource="&idmp-spor;OrganisationManagementServices"/>
		<cmns-col:hasPart rdf:resource="&idmp-spor;ProductManagementServices"/>
		<cmns-col:hasPart rdf:resource="&idmp-spor;ReferentialsManagementServices"/>
		<cmns-col:hasPart rdf:resource="&idmp-spor;SubstanceManagementServices"/>
		<cmns-prd:isProvidedBy rdf:resource="&idmp-eura;EuropeanMedicinesAgencyRegistrationAuthority"/>
	</owl:NamedIndividual>
	
	<owl:ObjectProperty rdf:about="&idmp-spor;hasSPORDomain">
		<rdfs:subPropertyOf rdf:resource="&cmns-cls;isClassifiedBy"/>
		<rdfs:subPropertyOf rdf:resource="&cmns-cxtdsg;isApplicableIn"/>
		<rdfs:label>has SPOR domain</rdfs:label>
		<rdfs:range rdf:resource="&idmp-spor;SPOR-Domain"/>
		<skos:definition>indicates the domain in which a particular substance or product is used from a Substances Products Organisations Referentials (SPOR) perspective</skos:definition>
	</owl:ObjectProperty>
	
	<owl:ObjectProperty rdf:about="&idmp-spor;hasSPOROtherName">
		<rdfs:subPropertyOf rdf:resource="&cmns-dsg;hasName"/>
		<rdfs:label>has SPOR other name</rdfs:label>
		<rdfs:range rdf:resource="&idmp-spor;SPORTermName"/>
		<skos:definition>provides an alternate name of a given term</skos:definition>
	</owl:ObjectProperty>
	
	<owl:ObjectProperty rdf:about="&idmp-spor;hasSPORShortName">
		<rdfs:subPropertyOf rdf:resource="&cmns-dsg;hasName"/>
		<rdfs:label>has SPOR short name</rdfs:label>
		<rdfs:range rdf:resource="&idmp-spor;SPORTermName"/>
		<skos:definition>provides an abbreviated name of a given term</skos:definition>
	</owl:ObjectProperty>
	
	<owl:ObjectProperty rdf:about="&idmp-spor;hasSPORStatus">
		<rdfs:subPropertyOf rdf:resource="&cmns-cls;isClassifiedBy"/>
		<rdfs:label>has SPOR status</rdfs:label>
		<rdfs:range rdf:resource="&idmp-spor;SPOR-RecordStatus"/>
		<skos:definition>indicates the status of the vocabulary term in Substances Products Organisations Referentials (SPOR)</skos:definition>
	</owl:ObjectProperty>
	
	<owl:ObjectProperty rdf:about="&idmp-spor;hasSPORTermDescription">
		<rdfs:subPropertyOf rdf:resource="&cmns-dsg;isDescribedBy"/>
		<rdfs:label>has SPOR term description</rdfs:label>
		<rdfs:range rdf:resource="&idmp-spor;SPORTermDescription"/>
		<skos:definition>provides a language-specific statement describing the term</skos:definition>
	</owl:ObjectProperty>
	
	<owl:ObjectProperty rdf:about="&idmp-spor;hasSPORTermName">
		<rdfs:subPropertyOf rdf:resource="&cmns-dsg;hasName"/>
		<rdfs:label>has SPOR term name</rdfs:label>
		<rdfs:range rdf:resource="&idmp-spor;SPORTermName"/>
		<skos:definition>provides the name of a given term</skos:definition>
	</owl:ObjectProperty>
	
	<owl:ObjectProperty rdf:about="&idmp-spor;hasSPORVisibility">
		<rdfs:subPropertyOf rdf:resource="&cmns-cls;isCharacterizedBy"/>
		<rdfs:label>has SPOR visibility</rdfs:label>
		<rdfs:range rdf:resource="&idmp-spor;SPOR-DataClassification"/>
		<skos:definition>characterizes the vocabulary term with respect to whether or not it is public, has restricted access, or other visibility in Substances Products Organisations Referentials (SPOR)</skos:definition>
	</owl:ObjectProperty>

</rdf:RDF>