<?xml version="1.0" encoding="UTF-8"?>
<!DOCTYPE rdf:RDF [
	<!ENTITY cmns-av "https://www.omg.org/spec/Commons/AnnotationVocabulary/">
	<!ENTITY cmns-cds "https://www.omg.org/spec/Commons/CodesAndCodeSets/">
	<!ENTITY cmns-cls "https://www.omg.org/spec/Commons/Classifiers/">
	<!ENTITY cmns-col "https://www.omg.org/spec/Commons/Collections/">
	<!ENTITY cmns-dsg "https://www.omg.org/spec/Commons/Designators/">
	<!ENTITY cmns-prd "https://www.omg.org/spec/Commons/ProductsAndServices/">
	<!ENTITY cmns-ra "https://www.omg.org/spec/Commons/RegistrationAuthorities/">
	<!ENTITY cmns-txt "https://www.omg.org/spec/Commons/TextDatatype/">
	<!ENTITY dct "http://purl.org/dc/terms/">
	<!ENTITY idmp-chg "https://spec.pistoiaalliance.org/idmp/ontology/META/ChangeManagement/">
	<!ENTITY idmp-eura "https://spec.pistoiaalliance.org/idmp/ontology/ISO/EuropeanJurisdiction/EuropeanRegistrationAuthorities/">
	<!ENTITY idmp-eurga "https://spec.pistoiaalliance.org/idmp/ontology/ISO/EuropeanJurisdiction/EuropeanRegulatoryAgencies/">
	<!ENTITY idmp-mprd "https://spec.pistoiaalliance.org/idmp/ontology/ISO/ISO11615-MedicinalProducts/">
	<!ENTITY idmp-spor "https://spec.pistoiaalliance.org/idmp/ontology/ISO/EuropeanJurisdiction/SubstancesProductsOrganisationsReferentials/">
	<!ENTITY idmp-sub "https://spec.pistoiaalliance.org/idmp/ontology/ISO/ISO11238-Substances/">
	<!ENTITY lcc-lr "https://www.omg.org/spec/LCC/Languages/LanguageRepresentation/">
	<!ENTITY owl "http://www.w3.org/2002/07/owl#">
	<!ENTITY rdf "http://www.w3.org/1999/02/22-rdf-syntax-ns#">
	<!ENTITY rdfs "http://www.w3.org/2000/01/rdf-schema#">
	<!ENTITY skos "http://www.w3.org/2004/02/skos/core#">
	<!ENTITY xsd "http://www.w3.org/2001/XMLSchema#">
]>
<rdf:RDF xml:base="https://spec.pistoiaalliance.org/idmp/ontology/ISO/EuropeanJurisdiction/SubstancesProductsOrganisationsReferentials/"
	xmlns:cmns-av="https://www.omg.org/spec/Commons/AnnotationVocabulary/"
	xmlns:cmns-cds="https://www.omg.org/spec/Commons/CodesAndCodeSets/"
	xmlns:cmns-cls="https://www.omg.org/spec/Commons/Classifiers/"
	xmlns:cmns-col="https://www.omg.org/spec/Commons/Collections/"
	xmlns:cmns-dsg="https://www.omg.org/spec/Commons/Designators/"
	xmlns:cmns-prd="https://www.omg.org/spec/Commons/ProductsAndServices/"
	xmlns:cmns-ra="https://www.omg.org/spec/Commons/RegistrationAuthorities/"
	xmlns:cmns-txt="https://www.omg.org/spec/Commons/TextDatatype/"
	xmlns:dct="http://purl.org/dc/terms/"
	xmlns:idmp-chg="https://spec.pistoiaalliance.org/idmp/ontology/META/ChangeManagement/"
	xmlns:idmp-eura="https://spec.pistoiaalliance.org/idmp/ontology/ISO/EuropeanJurisdiction/EuropeanRegistrationAuthorities/"
	xmlns:idmp-eurga="https://spec.pistoiaalliance.org/idmp/ontology/ISO/EuropeanJurisdiction/EuropeanRegulatoryAgencies/"
	xmlns:idmp-mprd="https://spec.pistoiaalliance.org/idmp/ontology/ISO/ISO11615-MedicinalProducts/"
	xmlns:idmp-spor="https://spec.pistoiaalliance.org/idmp/ontology/ISO/EuropeanJurisdiction/SubstancesProductsOrganisationsReferentials/"
	xmlns:idmp-sub="https://spec.pistoiaalliance.org/idmp/ontology/ISO/ISO11238-Substances/"
	xmlns:lcc-lr="https://www.omg.org/spec/LCC/Languages/LanguageRepresentation/"
	xmlns:owl="http://www.w3.org/2002/07/owl#"
	xmlns:rdf="http://www.w3.org/1999/02/22-rdf-syntax-ns#"
	xmlns:rdfs="http://www.w3.org/2000/01/rdf-schema#"
	xmlns:skos="http://www.w3.org/2004/02/skos/core#"
	xmlns:xsd="http://www.w3.org/2001/XMLSchema#">
	
	<owl:Ontology rdf:about="https://spec.pistoiaalliance.org/idmp/ontology/ISO/EuropeanJurisdiction/SubstancesProductsOrganisationsReferentials/">
		<rdfs:label>Substances, Products, Organisations and Referentials (SPOR) Ontology</rdfs:label>
		<dct:abstract>The Substances, Products, Organisations and Referentials (SPOR) ontology extends the core IDMP ontologies to define additional content required to support alignment with the European Medicines Agency data management services for substances, products, organisations and referentials.</dct:abstract>
		<dct:license rdf:datatype="&xsd;anyURI">https://opensource.org/licenses/MIT</dct:license>
		<owl:imports rdf:resource="https://spec.pistoiaalliance.org/idmp/ontology/ISO/EuropeanJurisdiction/EuropeanRegistrationAuthorities/"/>
		<owl:imports rdf:resource="https://spec.pistoiaalliance.org/idmp/ontology/ISO/EuropeanJurisdiction/EuropeanRegulatoryAgencies/"/>
		<owl:imports rdf:resource="https://spec.pistoiaalliance.org/idmp/ontology/ISO/ISO11238-Substances/"/>
		<owl:imports rdf:resource="https://spec.pistoiaalliance.org/idmp/ontology/ISO/ISO11615-MedicinalProducts/"/>
		<owl:imports rdf:resource="https://spec.pistoiaalliance.org/idmp/ontology/META/ChangeManagement/"/>
		<owl:imports rdf:resource="https://www.omg.org/spec/Commons/AnnotationVocabulary/"/>
		<owl:imports rdf:resource="https://www.omg.org/spec/Commons/Classifiers/"/>
		<owl:imports rdf:resource="https://www.omg.org/spec/Commons/CodesAndCodeSets/"/>
		<owl:imports rdf:resource="https://www.omg.org/spec/Commons/Collections/"/>
		<owl:imports rdf:resource="https://www.omg.org/spec/Commons/Designators/"/>
		<owl:imports rdf:resource="https://www.omg.org/spec/Commons/ProductsAndServices/"/>
		<owl:imports rdf:resource="https://www.omg.org/spec/Commons/RegistrationAuthorities/"/>
		<owl:imports rdf:resource="https://www.omg.org/spec/Commons/TextDatatype/"/>
		<owl:imports rdf:resource="https://www.omg.org/spec/LCC/Languages/LanguageRepresentation/"/>
		<owl:versionIRI rdf:resource="https://spec.pistoiaalliance.org/idmp/ontology/ISO/20230601/EuropeanJurisdiction/SubstancesProductsOrganisationsReferentials/"/>
		<idmp-chg:hasMaturityLevel rdf:resource="&idmp-chg;Provisional"/>
		<cmns-av:copyright>Copyright (c) 2022-2023 EDM Council, Inc.</cmns-av:copyright>
		<cmns-av:copyright>Copyright (c) 2022-2023 Pistoia Alliance, Inc.</cmns-av:copyright>
	</owl:Ontology>
	
	<owl:NamedIndividual rdf:about="&idmp-eura;EuropeanMedicinesAgencyRegistrationAuthority">
		<cmns-ra:manages rdf:resource="&idmp-spor;ReferentialsManagementServicesRegistry"/>
		<cmns-ra:manages rdf:resource="&idmp-spor;SubstancesManagementServicesRegistry"/>
	</owl:NamedIndividual>
	
	<owl:NamedIndividual rdf:about="&idmp-spor;OrganisationManagementServices">
		<rdf:type rdf:resource="&cmns-ra;RegistrationService"/>
		<rdfs:label>Organisation Management Services (OMS)</rdfs:label>
		<skos:definition>services supporting a central dictionary of organisation data in multiple languages</skos:definition>
		<cmns-av:abbreviation>OMS service</cmns-av:abbreviation>
		<cmns-av:directSource rdf:resource="https://spor.ema.europa.eu/"/>
		<cmns-col:isPartOf rdf:resource="&idmp-spor;SubstancesProductsOrganisationsReferentialsDataManagementServices"/>
		<cmns-prd:isProvidedBy rdf:resource="&idmp-eura;EuropeanMedicinesAgencyRegistrationAuthority"/>
	</owl:NamedIndividual>
	
	<owl:NamedIndividual rdf:about="&idmp-spor;ProductManagementServices">
		<rdf:type rdf:resource="&cmns-ra;RegistrationService"/>
		<rdfs:label>Product Management Services (PMS)</rdfs:label>
		<skos:definition>services supporting a central dictionary of product data in multiple languages</skos:definition>
		<cmns-av:abbreviation>PMS service</cmns-av:abbreviation>
		<cmns-av:adaptedFrom>https://spor.ema.europa.eu/sporwi/</cmns-av:adaptedFrom>
		<cmns-col:isPartOf rdf:resource="&idmp-spor;SubstancesProductsOrganisationsReferentialsDataManagementServices"/>
		<cmns-prd:isProvidedBy rdf:resource="&idmp-eura;EuropeanMedicinesAgencyRegistrationAuthority"/>
	</owl:NamedIndividual>
	
	<owl:NamedIndividual rdf:about="&idmp-spor;ReferentialsManagementServices">
		<rdf:type rdf:resource="&cmns-ra;RegistrationService"/>
		<rdfs:label>Referentials Management Services (RMS)</rdfs:label>
		<skos:definition>services supporting a central dictionary of referentials data in multiple languages</skos:definition>
		<cmns-av:abbreviation>RMS service</cmns-av:abbreviation>
		<cmns-av:directSource rdf:resource="https://spor.ema.europa.eu/"/>
		<cmns-col:isPartOf rdf:resource="&idmp-spor;SubstancesProductsOrganisationsReferentialsDataManagementServices"/>
		<cmns-prd:isProvidedBy rdf:resource="&idmp-eura;EuropeanMedicinesAgencyRegistrationAuthority"/>
	</owl:NamedIndividual>
	
	<owl:NamedIndividual rdf:about="&idmp-spor;ReferentialsManagementServicesClassificationScheme">
		<rdf:type rdf:resource="&cmns-cls;ClassificationScheme"/>
		<rdf:type rdf:resource="&cmns-cds;CodeSet"/>
		<rdfs:label>Referentials Management Services (RMS) classification scheme</rdfs:label>
		<skos:definition>classification scheme that includes the controlled vocabularies used to classify entities included in the Substances Products Organisations Referentials (SPOR) Referentials Management Services (RMS) related services and repositories</skos:definition>
	</owl:NamedIndividual>
	
	<owl:Class rdf:about="&idmp-spor;ReferentialsManagementServicesControlledVocabularyTerm">
		<rdfs:subClassOf rdf:resource="&cmns-cls;Classifier"/>
		<rdfs:subClassOf rdf:resource="&cmns-cds;CodeElement"/>
		<rdfs:subClassOf>
			<owl:Restriction>
				<owl:onProperty rdf:resource="&cmns-dsg;denotes"/>
				<owl:onClass>
					<owl:Class>
						<owl:unionOf rdf:parseType="Collection">
							<rdf:Description rdf:about="&idmp-sub;Substance">
							</rdf:Description>
							<rdf:Description rdf:about="&cmns-prd;Product">
							</rdf:Description>
						</owl:unionOf>
					</owl:Class>
				</owl:onClass>
				<owl:minQualifiedCardinality rdf:datatype="&xsd;nonNegativeInteger">0</owl:minQualifiedCardinality>
			</owl:Restriction>
		</rdfs:subClassOf>
		<rdfs:subClassOf>
			<owl:Restriction>
				<owl:onProperty rdf:resource="&cmns-cls;classifies"/>
				<owl:onClass>
					<owl:Class>
						<owl:unionOf rdf:parseType="Collection">
							<rdf:Description rdf:about="&idmp-sub;Substance">
							</rdf:Description>
							<rdf:Description rdf:about="&cmns-prd;Product">
							</rdf:Description>
						</owl:unionOf>
					</owl:Class>
				</owl:onClass>
				<owl:minQualifiedCardinality rdf:datatype="&xsd;nonNegativeInteger">0</owl:minQualifiedCardinality>
			</owl:Restriction>
		</rdfs:subClassOf>
		<rdfs:label>Referentials Management Services (RMS) controlled vocabulary term</rdfs:label>
		<skos:definition>term in a controlled vocabulary whose values describe some substance or product from a Substances Products Organisations Referentials (SPOR) Referentials Management Services (RMS) perspective</skos:definition>
		<cmns-av:abbreviation>RMS controlled vocabulary term</cmns-av:abbreviation>
	</owl:Class>
	
	<owl:NamedIndividual rdf:about="&idmp-spor;ReferentialsManagementServicesRegistry">
		<rdf:type rdf:resource="&cmns-ra;Registry"/>
		<rdfs:label>Referentials Management Services (RMS) registry</rdfs:label>
		<skos:definition>central dictionary of referentials data in multiple languages available through the Substances Products Organisations Referentials (SPOR) Referentials Management Services (RMS)</skos:definition>
		<cmns-av:abbreviation>SPOR RMS</cmns-av:abbreviation>
		<cmns-av:abbreviation>SPOR-RMS</cmns-av:abbreviation>
		<cmns-av:directSource rdf:resource="https://spor.ema.europa.eu/"/>
		<cmns-ra:isManagedBy rdf:resource="&idmp-eura;EuropeanMedicinesAgencyRegistrationAuthority"/>
	</owl:NamedIndividual>
	
	<owl:Class rdf:about="&idmp-spor;SPOR-DataClassification">
		<rdfs:subClassOf rdf:resource="&idmp-spor;ReferentialsManagementServicesControlledVocabularyTerm"/>
		<rdfs:label>SPOR data classification</rdfs:label>
		<skos:definition>classifier and code element that describes the nature of any data element in terms of accessibility from a Substances Products Organisations Referentials (SPOR) Referentials Management Services (RMS) perspective</skos:definition>
		<cmns-av:directSource rdf:resource="https://spor.ema.europa.eu/rmswi/#/lists/200000004983/terms"/>
	</owl:Class>
	
	<owl:Class rdf:about="&idmp-spor;SPOR-Domain">
		<rdfs:subClassOf rdf:resource="&idmp-spor;ReferentialsManagementServicesControlledVocabularyTerm"/>
		<rdfs:label>SPOR domain</rdfs:label>
		<skos:definition>classifier and code element that describes the domain in which a particular substance or product is used from a Substances Products Organisations Referentials (SPOR) Referentials Management Services (RMS) perspective</skos:definition>
		<cmns-av:adaptedFrom rdf:resource="https://spor.ema.europa.eu/rmswi/#/lists/100000000004/terms"/>
	</owl:Class>
	
	<owl:Class rdf:about="&idmp-spor;SPOR-MarketingStatusClassifier">
		<rdfs:subClassOf rdf:resource="&idmp-spor;ReferentialsManagementServicesControlledVocabularyTerm"/>
		<rdfs:label>SPOR marketing status classifier</rdfs:label>
		<skos:definition>classifier and code element that describes the current status of some substance with respect to whether or not it has been placed on the market from a Substances Products Organisations Referentials (SPOR) Referentials Management Services (RMS) perspective</skos:definition>
		<cmns-av:directSource rdf:resource="https://spor.ema.europa.eu/rmswi/#/lists/100000072052/terms"/>
	</owl:Class>
	
	<owl:Class rdf:about="&idmp-spor;SPOR-ShelfLifeType">
		<rdfs:subClassOf rdf:resource="&idmp-spor;ReferentialsManagementServicesControlledVocabularyTerm"/>
		<rdfs:subClassOf rdf:resource="&idmp-mprd;ShelfLifeType"/>
		<rdfs:label>SPOR shelf life type</rdfs:label>
		<skos:definition>classifier and code element that describes the point in the life cycle from manufacturing to administration to a patient that a value for shelf life applies to, including potentially with respect to a specific packaging item, from a Substances Products Organisations Referentials (SPOR) Referentials Management Services (RMS) perspective</skos:definition>
		<cmns-av:directSource rdf:resource="https://spor.ema.europa.eu/rmswi/#/lists/100000073343/terms"/>
	</owl:Class>
	
	<owl:Class rdf:about="&idmp-spor;SPOR-SpecialPrecautionsForStorage">
		<rdfs:subClassOf rdf:resource="&idmp-spor;ReferentialsManagementServicesControlledVocabularyTerm"/>
		<rdfs:subClassOf rdf:resource="&idmp-mprd;SpecialPrecautionsForStorage"/>
		<rdfs:label>SPOR special precautions for storage</rdfs:label>
		<skos:definition>classifier and code element that provides precise instructions for storage of a substance or product, such as the kind of container, temperature restrictions, container management, and other restrictions on the way something must be handled from a Substances Products Organisations Referentials (SPOR) Referentials Management Services (RMS) perspective</skos:definition>
		<cmns-av:directSource rdf:resource="https://spor.ema.europa.eu/rmswi/#/lists/100000073344/terms"/>
	</owl:Class>
	
	<owl:NamedIndividual rdf:about="&idmp-spor;SubstanceManagementServices">
		<rdf:type rdf:resource="&cmns-ra;RegistrationService"/>
		<rdfs:label>Substance Management Services (SMS)</rdfs:label>
		<skos:definition>services supporting a central dictionary of substance data in multiple languages</skos:definition>
		<cmns-av:abbreviation>SMS service</cmns-av:abbreviation>
		<cmns-av:directSource rdf:resource="https://spor.ema.europa.eu/"/>
		<cmns-col:isPartOf rdf:resource="&idmp-spor;SubstancesProductsOrganisationsReferentialsDataManagementServices"/>
		<cmns-prd:isProvidedBy rdf:resource="&idmp-eura;EuropeanMedicinesAgencyRegistrationAuthority"/>
	</owl:NamedIndividual>
	
	<owl:NamedIndividual rdf:about="&idmp-spor;SubstancesManagementServicesRegistry">
		<rdf:type rdf:resource="&cmns-ra;Registry"/>
		<rdfs:label>Substances Management Services registry</rdfs:label>
		<skos:definition>central dictionary of substance data in multiple languages available through the Substances Products Organisations Referentials (SPOR) Substances Management Services (SMS)</skos:definition>
		<cmns-av:abbreviation>SPOR SMS</cmns-av:abbreviation>
		<cmns-av:abbreviation>SPOR-SMS</cmns-av:abbreviation>
		<cmns-av:directSource rdf:resource="https://spor.ema.europa.eu/"/>
		<cmns-av:explanatoryNote>SMS is currently live as an EMA internal system. Until it is onboarded in the SPOR portal, external users should use the following systems: view and search substance data in EUTCT or IRIS; submit substance change requests in the EMA Service Desk portal; Export of substance data are available at https://spor.ema.europa.eu/web-ui-data-backend/download/csv.</cmns-av:explanatoryNote>
		<cmns-ra:isManagedBy rdf:resource="&idmp-eura;EuropeanMedicinesAgencyRegistrationAuthority"/>
	</owl:NamedIndividual>
	
	<owl:NamedIndividual rdf:about="&idmp-spor;SubstancesProductsOrganisationsReferentialsDataManagementServices">
		<rdf:type rdf:resource="&cmns-ra;RegistrationService"/>
		<rdfs:label>Substances Products Organisations Referentials (SPOR) data management services</rdfs:label>
		<skos:definition>data management services for substances, products, organisations and referentials (SPOR) designed to support regulatory activities in the European Union</skos:definition>
		<cmns-av:abbreviation>SPOR data management services</cmns-av:abbreviation>
		<cmns-av:directSource rdf:resource="https://spor.ema.europa.eu/"/>
		<cmns-col:hasPart rdf:resource="&idmp-spor;OrganisationManagementServices"/>
		<cmns-col:hasPart rdf:resource="&idmp-spor;ProductManagementServices"/>
		<cmns-col:hasPart rdf:resource="&idmp-spor;ReferentialsManagementServices"/>
		<cmns-col:hasPart rdf:resource="&idmp-spor;SubstanceManagementServices"/>
		<cmns-prd:isProvidedBy rdf:resource="&idmp-eura;EuropeanMedicinesAgencyRegistrationAuthority"/>
	</owl:NamedIndividual>
	
	<owl:DatatypeProperty rdf:about="&idmp-spor;hasSPOROtherName">
		<rdfs:subPropertyOf rdf:resource="&lcc-lr;hasTextualName"/>
		<rdfs:label>has SPOR other name</rdfs:label>
		<skos:definition>provides a language-tagged string value indicating an alternate name of a given term</skos:definition>
	</owl:DatatypeProperty>
	
	<owl:DatatypeProperty rdf:about="&idmp-spor;hasSPORShortName">
		<rdfs:subPropertyOf rdf:resource="&lcc-lr;hasTextualName"/>
		<rdfs:label>has SPOR short name</rdfs:label>
		<skos:definition>provides a language-tagged string value indicating an abbreviated name of a given term</skos:definition>
	</owl:DatatypeProperty>
	
	<owl:DatatypeProperty rdf:about="&idmp-spor;hasSPORTermDescription">
		<rdfs:subPropertyOf rdf:resource="&cmns-dsg;hasDescription"/>
		<rdfs:label>has SPOR term description</rdfs:label>
		<skos:definition>provides a language-tagged string value that is a textual statement describing the term</skos:definition>
	</owl:DatatypeProperty>
	
	<owl:DatatypeProperty rdf:about="&idmp-spor;hasSPORTermName">
		<rdfs:subPropertyOf rdf:resource="&lcc-lr;hasTextualName"/>
		<rdfs:label>has SPOR term name</rdfs:label>
		<skos:definition>provides a language-tagged string value indicating the preferred name of a given term</skos:definition>
	</owl:DatatypeProperty>
	
	<owl:DatatypeProperty rdf:about="&idmp-spor;hasSPORTermStatus">
		<rdfs:subPropertyOf rdf:resource="&cmns-dsg;hasDescription"/>
		<rdfs:label>has SPOR term status</rdfs:label>
		<skos:definition>provides a language-tagged string value that is a textual indicator of the status of the vocabulary term in SPOR</skos:definition>
		<skos:example>Valid values for status include CURRENT, PROVISIONAL, NULLIFIED and the like.</skos:example>
	</owl:DatatypeProperty>

</rdf:RDF>